{"@context":{"rdf":"http://www.w3.org/1999/02/22-rdf-syntax-ns#","owl":"http://www.w3.org/2002/07/owl#","rdfs":"http://www.w3.org/2000/01/rdf-schema#","schema":"https://schema.org/","unece":"https://vocabulary.uncefact.org/"},"@graph":[{"rdfs:label":"AccessRightsTypeCodeList","@type":"rdfs:Class","@id":"unece:AccessRightsTypeCodeList","rdfs:comment":"A character string used to represent the type of access rights."},{"@id":"unece:AccessRightsTypeCodeList#P","@type":"unece:AccessRightsTypeCodeList","rdf:value":"P","rdfs:comment":"Prohibited"},{"@id":"unece:AccessRightsTypeCodeList#R","@type":"unece:AccessRightsTypeCodeList","rdf:value":"R","rdfs:comment":"Restricted"},{"@id":"unece:AccessRightsTypeCodeList#U","@type":"unece:AccessRightsTypeCodeList","rdf:value":"U","rdfs:comment":"Unlimited"},{"rdfs:label":"AccountingAccountTypeCodeList","@type":"rdfs:Class","@id":"unece:AccountingAccountTypeCodeList","rdfs:comment":"A character string used to represent the type of an accounting account."},{"@id":"unece:AccountingAccountTypeCodeList#1","@type":"unece:AccountingAccountTypeCodeList","rdf:value":"1","rdfs:comment":"Financial"},{"@id":"unece:AccountingAccountTypeCodeList#2","@type":"unece:AccountingAccountTypeCodeList","rdf:value":"2","rdfs:comment":"Subsidiary"},{"@id":"unece:AccountingAccountTypeCodeList#3","@type":"unece:AccountingAccountTypeCodeList","rdf:value":"3","rdfs:comment":"Budget"},{"@id":"unece:AccountingAccountTypeCodeList#4","@type":"unece:AccountingAccountTypeCodeList","rdf:value":"4","rdfs:comment":"Cost Accounting"},{"@id":"unece:AccountingAccountTypeCodeList#5","@type":"unece:AccountingAccountTypeCodeList","rdf:value":"5","rdfs:comment":"Receivable"},{"@id":"unece:AccountingAccountTypeCodeList#6","@type":"unece:AccountingAccountTypeCodeList","rdf:value":"6","rdfs:comment":"Payable"},{"@id":"unece:AccountingAccountTypeCodeList#7","@type":"unece:AccountingAccountTypeCodeList","rdf:value":"7","rdfs:comment":"Job Cost Accounting"},{"rdfs:label":"AccountingAmountTypeCodeList","@type":"rdfs:Class","@id":"unece:AccountingAmountTypeCodeList","rdfs:comment":"A character string used to represent the type of accounting amount."},{"@id":"unece:AccountingAmountTypeCodeList#1","@type":"unece:AccountingAmountTypeCodeList","rdf:value":"1","rdfs:comment":"Allowance Charge Amount"},{"@id":"unece:AccountingAmountTypeCodeList#2","@type":"unece:AccountingAmountTypeCodeList","rdf:value":"2","rdfs:comment":"Insurance Charge Amount"},{"@id":"unece:AccountingAmountTypeCodeList#3","@type":"unece:AccountingAmountTypeCodeList","rdf:value":"3","rdfs:comment":"Taxable Transport Charge Amount"},{"@id":"unece:AccountingAmountTypeCodeList#4","@type":"unece:AccountingAmountTypeCodeList","rdf:value":"4","rdfs:comment":"Adjustment Amount"},{"@id":"unece:AccountingAmountTypeCodeList#5","@type":"unece:AccountingAmountTypeCodeList","rdf:value":"5","rdfs:comment":"Taxable Amount"},{"@id":"unece:AccountingAmountTypeCodeList#6","@type":"unece:AccountingAmountTypeCodeList","rdf:value":"6","rdfs:comment":"Tax Amount"},{"rdfs:label":"AccountingDebitCreditStatusCodeList","@type":"rdfs:Class","@id":"unece:AccountingDebitCreditStatusCodeList","rdfs:comment":"A character string used to represent the accounting debit or credit sign."},{"@id":"unece:AccountingDebitCreditStatusCodeList#29","@type":"unece:AccountingDebitCreditStatusCodeList","rdf:value":"29","rdfs:comment":"Debit"},{"@id":"unece:AccountingDebitCreditStatusCodeList#30","@type":"unece:AccountingDebitCreditStatusCodeList","rdf:value":"30","rdfs:comment":"Credit"},{"@id":"unece:AccountingDebitCreditStatusCodeList#31","@type":"unece:AccountingDebitCreditStatusCodeList","rdf:value":"31","rdfs:comment":"Positive debit"},{"@id":"unece:AccountingDebitCreditStatusCodeList#32","@type":"unece:AccountingDebitCreditStatusCodeList","rdf:value":"32","rdfs:comment":"Negative debit"},{"@id":"unece:AccountingDebitCreditStatusCodeList#33","@type":"unece:AccountingDebitCreditStatusCodeList","rdf:value":"33","rdfs:comment":"Positive credit"},{"@id":"unece:AccountingDebitCreditStatusCodeList#34","@type":"unece:AccountingDebitCreditStatusCodeList","rdf:value":"34","rdfs:comment":"Negative credit"},{"@id":"unece:AccountingDebitCreditStatusCodeList#66","@type":"unece:AccountingDebitCreditStatusCodeList","rdf:value":"66","rdfs:comment":"Unsigned amount"},{"rdfs:label":"AccountingDocumentCodeList","@type":"rdfs:Class","@id":"unece:AccountingDocumentCodeList","rdfs:comment":"A character string used to represent the type of an accounting document."},{"@id":"unece:AccountingDocumentCodeList#105","@type":"unece:AccountingDocumentCodeList","rdf:value":"105","rdfs:comment":"Purchase order"},{"@id":"unece:AccountingDocumentCodeList#220","@type":"unece:AccountingDocumentCodeList","rdf:value":"220","rdfs:comment":"Order"},{"@id":"unece:AccountingDocumentCodeList#223","@type":"unece:AccountingDocumentCodeList","rdf:value":"223","rdfs:comment":"Lease order"},{"@id":"unece:AccountingDocumentCodeList#224","@type":"unece:AccountingDocumentCodeList","rdf:value":"224","rdfs:comment":"Rush order"},{"@id":"unece:AccountingDocumentCodeList#245","@type":"unece:AccountingDocumentCodeList","rdf:value":"245","rdfs:comment":"Delivery release"},{"@id":"unece:AccountingDocumentCodeList#315","@type":"unece:AccountingDocumentCodeList","rdf:value":"315","rdfs:comment":"Contract"},{"@id":"unece:AccountingDocumentCodeList#320","@type":"unece:AccountingDocumentCodeList","rdf:value":"320","rdfs:comment":"Acknowledgement of order"},{"@id":"unece:AccountingDocumentCodeList#325","@type":"unece:AccountingDocumentCodeList","rdf:value":"325","rdfs:comment":"Proforma invoice"},{"@id":"unece:AccountingDocumentCodeList#326","@type":"unece:AccountingDocumentCodeList","rdf:value":"326","rdfs:comment":"Partial invoice"},{"@id":"unece:AccountingDocumentCodeList#380","@type":"unece:AccountingDocumentCodeList","rdf:value":"380","rdfs:comment":"Commercial invoice"},{"@id":"unece:AccountingDocumentCodeList#389","@type":"unece:AccountingDocumentCodeList","rdf:value":"389","rdfs:comment":"Self-billed invoice"},{"@id":"unece:AccountingDocumentCodeList#393","@type":"unece:AccountingDocumentCodeList","rdf:value":"393","rdfs:comment":"Factored invoice"},{"@id":"unece:AccountingDocumentCodeList#394","@type":"unece:AccountingDocumentCodeList","rdf:value":"394","rdfs:comment":"Lease invoice"},{"@id":"unece:AccountingDocumentCodeList#395","@type":"unece:AccountingDocumentCodeList","rdf:value":"395","rdfs:comment":"Consignment invoice"},{"@id":"unece:AccountingDocumentCodeList#398","@type":"unece:AccountingDocumentCodeList","rdf:value":"398","rdfs:comment":"Cross docking despatch advice"},{"@id":"unece:AccountingDocumentCodeList#399","@type":"unece:AccountingDocumentCodeList","rdf:value":"399","rdfs:comment":"Transshipment despatch advice"},{"@id":"unece:AccountingDocumentCodeList#455","@type":"unece:AccountingDocumentCodeList","rdf:value":"455","rdfs:comment":"Extended credit advice"},{"@id":"unece:AccountingDocumentCodeList#481","@type":"unece:AccountingDocumentCodeList","rdf:value":"481","rdfs:comment":"Remittance advice"},{"@id":"unece:AccountingDocumentCodeList#533","@type":"unece:AccountingDocumentCodeList","rdf:value":"533","rdfs:comment":"Original accounting voucher"},{"@id":"unece:AccountingDocumentCodeList#534","@type":"unece:AccountingDocumentCodeList","rdf:value":"534","rdfs:comment":"Copy accounting voucher"},{"@id":"unece:AccountingDocumentCodeList#640","@type":"unece:AccountingDocumentCodeList","rdf:value":"640","rdfs:comment":"Delivery order"},{"@id":"unece:AccountingDocumentCodeList#719","@type":"unece:AccountingDocumentCodeList","rdf:value":"719","rdfs:comment":"General message"},{"@id":"unece:AccountingDocumentCodeList#731","@type":"unece:AccountingDocumentCodeList","rdf:value":"731","rdfs:comment":"Commercial account summary"},{"@id":"unece:AccountingDocumentCodeList#747","@type":"unece:AccountingDocumentCodeList","rdf:value":"747","rdfs:comment":"Payroll deductions advice"},{"rdfs:label":"AllowanceChargeIdCodeList","@type":"rdfs:Class","@id":"unece:AllowanceChargeIdCodeList","rdfs:comment":"A character string used to identify a type of allowance or charge."},{"@id":"unece:AllowanceChargeIdCodeList#1","@type":"unece:AllowanceChargeIdCodeList","rdf:value":"1","rdfs:comment":"Handling commission"},{"@id":"unece:AllowanceChargeIdCodeList#2","@type":"unece:AllowanceChargeIdCodeList","rdf:value":"2","rdfs:comment":"Amendment commission"},{"@id":"unece:AllowanceChargeIdCodeList#3","@type":"unece:AllowanceChargeIdCodeList","rdf:value":"3","rdfs:comment":"Acceptance commission"},{"@id":"unece:AllowanceChargeIdCodeList#4","@type":"unece:AllowanceChargeIdCodeList","rdf:value":"4","rdfs:comment":"Commission for obtaining acceptance"},{"@id":"unece:AllowanceChargeIdCodeList#5","@type":"unece:AllowanceChargeIdCodeList","rdf:value":"5","rdfs:comment":"Commission on delivery"},{"@id":"unece:AllowanceChargeIdCodeList#6","@type":"unece:AllowanceChargeIdCodeList","rdf:value":"6","rdfs:comment":"Advising commission"},{"@id":"unece:AllowanceChargeIdCodeList#7","@type":"unece:AllowanceChargeIdCodeList","rdf:value":"7","rdfs:comment":"Confirmation commission"},{"@id":"unece:AllowanceChargeIdCodeList#8","@type":"unece:AllowanceChargeIdCodeList","rdf:value":"8","rdfs:comment":"Deferred payment commission"},{"@id":"unece:AllowanceChargeIdCodeList#9","@type":"unece:AllowanceChargeIdCodeList","rdf:value":"9","rdfs:comment":"Commission for taking up documents"},{"@id":"unece:AllowanceChargeIdCodeList#10","@type":"unece:AllowanceChargeIdCodeList","rdf:value":"10","rdfs:comment":"Opening commission"},{"@id":"unece:AllowanceChargeIdCodeList#11","@type":"unece:AllowanceChargeIdCodeList","rdf:value":"11","rdfs:comment":"Fee for payment under reserve"},{"@id":"unece:AllowanceChargeIdCodeList#12","@type":"unece:AllowanceChargeIdCodeList","rdf:value":"12","rdfs:comment":"Discrepancy fee"},{"@id":"unece:AllowanceChargeIdCodeList#13","@type":"unece:AllowanceChargeIdCodeList","rdf:value":"13","rdfs:comment":"Domicilation commission"},{"@id":"unece:AllowanceChargeIdCodeList#14","@type":"unece:AllowanceChargeIdCodeList","rdf:value":"14","rdfs:comment":"Commission for release of goods"},{"@id":"unece:AllowanceChargeIdCodeList#15","@type":"unece:AllowanceChargeIdCodeList","rdf:value":"15","rdfs:comment":"Collection commission"},{"@id":"unece:AllowanceChargeIdCodeList#16","@type":"unece:AllowanceChargeIdCodeList","rdf:value":"16","rdfs:comment":"Negotiation commission"},{"@id":"unece:AllowanceChargeIdCodeList#17","@type":"unece:AllowanceChargeIdCodeList","rdf:value":"17","rdfs:comment":"Return commission"},{"@id":"unece:AllowanceChargeIdCodeList#18","@type":"unece:AllowanceChargeIdCodeList","rdf:value":"18","rdfs:comment":"B/L splitting charges"},{"@id":"unece:AllowanceChargeIdCodeList#19","@type":"unece:AllowanceChargeIdCodeList","rdf:value":"19","rdfs:comment":"Trust commission"},{"@id":"unece:AllowanceChargeIdCodeList#20","@type":"unece:AllowanceChargeIdCodeList","rdf:value":"20","rdfs:comment":"Transfer commission"},{"@id":"unece:AllowanceChargeIdCodeList#21","@type":"unece:AllowanceChargeIdCodeList","rdf:value":"21","rdfs:comment":"Commission for opening irrevocable documentary credits"},{"@id":"unece:AllowanceChargeIdCodeList#22","@type":"unece:AllowanceChargeIdCodeList","rdf:value":"22","rdfs:comment":"Pre-advice commission"},{"@id":"unece:AllowanceChargeIdCodeList#23","@type":"unece:AllowanceChargeIdCodeList","rdf:value":"23","rdfs:comment":"Supervisory commission"},{"@id":"unece:AllowanceChargeIdCodeList#24","@type":"unece:AllowanceChargeIdCodeList","rdf:value":"24","rdfs:comment":"Model charges"},{"@id":"unece:AllowanceChargeIdCodeList#25","@type":"unece:AllowanceChargeIdCodeList","rdf:value":"25","rdfs:comment":"Risk commission"},{"@id":"unece:AllowanceChargeIdCodeList#26","@type":"unece:AllowanceChargeIdCodeList","rdf:value":"26","rdfs:comment":"Guarantee commission"},{"@id":"unece:AllowanceChargeIdCodeList#27","@type":"unece:AllowanceChargeIdCodeList","rdf:value":"27","rdfs:comment":"Reimbursement commission"},{"@id":"unece:AllowanceChargeIdCodeList#28","@type":"unece:AllowanceChargeIdCodeList","rdf:value":"28","rdfs:comment":"Stamp duty"},{"@id":"unece:AllowanceChargeIdCodeList#29","@type":"unece:AllowanceChargeIdCodeList","rdf:value":"29","rdfs:comment":"Brokerage"},{"@id":"unece:AllowanceChargeIdCodeList#30","@type":"unece:AllowanceChargeIdCodeList","rdf:value":"30","rdfs:comment":"Bank charges"},{"@id":"unece:AllowanceChargeIdCodeList#31","@type":"unece:AllowanceChargeIdCodeList","rdf:value":"31","rdfs:comment":"Bank charges information"},{"@id":"unece:AllowanceChargeIdCodeList#32","@type":"unece:AllowanceChargeIdCodeList","rdf:value":"32","rdfs:comment":"Courier fee"},{"@id":"unece:AllowanceChargeIdCodeList#33","@type":"unece:AllowanceChargeIdCodeList","rdf:value":"33","rdfs:comment":"Phone fee"},{"@id":"unece:AllowanceChargeIdCodeList#34","@type":"unece:AllowanceChargeIdCodeList","rdf:value":"34","rdfs:comment":"Postage fee"},{"@id":"unece:AllowanceChargeIdCodeList#35","@type":"unece:AllowanceChargeIdCodeList","rdf:value":"35","rdfs:comment":"S.W.I.F.T. fee"},{"@id":"unece:AllowanceChargeIdCodeList#36","@type":"unece:AllowanceChargeIdCodeList","rdf:value":"36","rdfs:comment":"Telex fee"},{"@id":"unece:AllowanceChargeIdCodeList#37","@type":"unece:AllowanceChargeIdCodeList","rdf:value":"37","rdfs:comment":"Penalty for late delivery of documents"},{"@id":"unece:AllowanceChargeIdCodeList#38","@type":"unece:AllowanceChargeIdCodeList","rdf:value":"38","rdfs:comment":"Penalty for late delivery of valuation of works"},{"@id":"unece:AllowanceChargeIdCodeList#39","@type":"unece:AllowanceChargeIdCodeList","rdf:value":"39","rdfs:comment":"Penalty for execution of works behind schedule"},{"@id":"unece:AllowanceChargeIdCodeList#40","@type":"unece:AllowanceChargeIdCodeList","rdf:value":"40","rdfs:comment":"Other penalties"},{"@id":"unece:AllowanceChargeIdCodeList#41","@type":"unece:AllowanceChargeIdCodeList","rdf:value":"41","rdfs:comment":"Bonus for works ahead of schedule"},{"@id":"unece:AllowanceChargeIdCodeList#42","@type":"unece:AllowanceChargeIdCodeList","rdf:value":"42","rdfs:comment":"Other bonus"},{"@id":"unece:AllowanceChargeIdCodeList#44","@type":"unece:AllowanceChargeIdCodeList","rdf:value":"44","rdfs:comment":"Project management cost"},{"@id":"unece:AllowanceChargeIdCodeList#45","@type":"unece:AllowanceChargeIdCodeList","rdf:value":"45","rdfs:comment":"Pro rata retention"},{"@id":"unece:AllowanceChargeIdCodeList#46","@type":"unece:AllowanceChargeIdCodeList","rdf:value":"46","rdfs:comment":"Contractual retention"},{"@id":"unece:AllowanceChargeIdCodeList#47","@type":"unece:AllowanceChargeIdCodeList","rdf:value":"47","rdfs:comment":"Other retentions"},{"@id":"unece:AllowanceChargeIdCodeList#48","@type":"unece:AllowanceChargeIdCodeList","rdf:value":"48","rdfs:comment":"Interest on arrears"},{"@id":"unece:AllowanceChargeIdCodeList#49","@type":"unece:AllowanceChargeIdCodeList","rdf:value":"49","rdfs:comment":"Interest"},{"@id":"unece:AllowanceChargeIdCodeList#50","@type":"unece:AllowanceChargeIdCodeList","rdf:value":"50","rdfs:comment":"Charge per credit cover"},{"@id":"unece:AllowanceChargeIdCodeList#51","@type":"unece:AllowanceChargeIdCodeList","rdf:value":"51","rdfs:comment":"Charge per unused credit cover"},{"@id":"unece:AllowanceChargeIdCodeList#52","@type":"unece:AllowanceChargeIdCodeList","rdf:value":"52","rdfs:comment":"Minimum commission"},{"@id":"unece:AllowanceChargeIdCodeList#53","@type":"unece:AllowanceChargeIdCodeList","rdf:value":"53","rdfs:comment":"Factoring commission"},{"@id":"unece:AllowanceChargeIdCodeList#54","@type":"unece:AllowanceChargeIdCodeList","rdf:value":"54","rdfs:comment":"Chamber of commerce charge"},{"@id":"unece:AllowanceChargeIdCodeList#55","@type":"unece:AllowanceChargeIdCodeList","rdf:value":"55","rdfs:comment":"Transfer charges"},{"@id":"unece:AllowanceChargeIdCodeList#56","@type":"unece:AllowanceChargeIdCodeList","rdf:value":"56","rdfs:comment":"Repatriation charges"},{"@id":"unece:AllowanceChargeIdCodeList#57","@type":"unece:AllowanceChargeIdCodeList","rdf:value":"57","rdfs:comment":"Miscellaneous charges"},{"@id":"unece:AllowanceChargeIdCodeList#58","@type":"unece:AllowanceChargeIdCodeList","rdf:value":"58","rdfs:comment":"Foreign exchange charges"},{"@id":"unece:AllowanceChargeIdCodeList#59","@type":"unece:AllowanceChargeIdCodeList","rdf:value":"59","rdfs:comment":"Agreed debit interest charge"},{"@id":"unece:AllowanceChargeIdCodeList#60","@type":"unece:AllowanceChargeIdCodeList","rdf:value":"60","rdfs:comment":"Manufacturer's consumer discount"},{"@id":"unece:AllowanceChargeIdCodeList#61","@type":"unece:AllowanceChargeIdCodeList","rdf:value":"61","rdfs:comment":"Fax advice charge"},{"@id":"unece:AllowanceChargeIdCodeList#62","@type":"unece:AllowanceChargeIdCodeList","rdf:value":"62","rdfs:comment":"Due to military status"},{"@id":"unece:AllowanceChargeIdCodeList#63","@type":"unece:AllowanceChargeIdCodeList","rdf:value":"63","rdfs:comment":"Due to work accident"},{"@id":"unece:AllowanceChargeIdCodeList#64","@type":"unece:AllowanceChargeIdCodeList","rdf:value":"64","rdfs:comment":"Special agreement"},{"@id":"unece:AllowanceChargeIdCodeList#65","@type":"unece:AllowanceChargeIdCodeList","rdf:value":"65","rdfs:comment":"Production error discount"},{"@id":"unece:AllowanceChargeIdCodeList#66","@type":"unece:AllowanceChargeIdCodeList","rdf:value":"66","rdfs:comment":"New outlet discount"},{"@id":"unece:AllowanceChargeIdCodeList#67","@type":"unece:AllowanceChargeIdCodeList","rdf:value":"67","rdfs:comment":"Sample discount"},{"@id":"unece:AllowanceChargeIdCodeList#68","@type":"unece:AllowanceChargeIdCodeList","rdf:value":"68","rdfs:comment":"End-of-range discount"},{"@id":"unece:AllowanceChargeIdCodeList#69","@type":"unece:AllowanceChargeIdCodeList","rdf:value":"69","rdfs:comment":"Charge for a customer specific finish"},{"@id":"unece:AllowanceChargeIdCodeList#70","@type":"unece:AllowanceChargeIdCodeList","rdf:value":"70","rdfs:comment":"Incoterm discount"},{"@id":"unece:AllowanceChargeIdCodeList#71","@type":"unece:AllowanceChargeIdCodeList","rdf:value":"71","rdfs:comment":"Point of sales threshold allowance"},{"@id":"unece:AllowanceChargeIdCodeList#72","@type":"unece:AllowanceChargeIdCodeList","rdf:value":"72","rdfs:comment":"Technical modification costs"},{"@id":"unece:AllowanceChargeIdCodeList#73","@type":"unece:AllowanceChargeIdCodeList","rdf:value":"73","rdfs:comment":"Job-order production costs"},{"@id":"unece:AllowanceChargeIdCodeList#74","@type":"unece:AllowanceChargeIdCodeList","rdf:value":"74","rdfs:comment":"Off-premises costs"},{"@id":"unece:AllowanceChargeIdCodeList#75","@type":"unece:AllowanceChargeIdCodeList","rdf:value":"75","rdfs:comment":"Additional processing costs"},{"@id":"unece:AllowanceChargeIdCodeList#76","@type":"unece:AllowanceChargeIdCodeList","rdf:value":"76","rdfs:comment":"Attesting charge"},{"@id":"unece:AllowanceChargeIdCodeList#77","@type":"unece:AllowanceChargeIdCodeList","rdf:value":"77","rdfs:comment":"Rush delivery surcharge"},{"@id":"unece:AllowanceChargeIdCodeList#78","@type":"unece:AllowanceChargeIdCodeList","rdf:value":"78","rdfs:comment":"Special construction costs"},{"@id":"unece:AllowanceChargeIdCodeList#79","@type":"unece:AllowanceChargeIdCodeList","rdf:value":"79","rdfs:comment":"Freight charges"},{"@id":"unece:AllowanceChargeIdCodeList#80","@type":"unece:AllowanceChargeIdCodeList","rdf:value":"80","rdfs:comment":"Packing charge"},{"@id":"unece:AllowanceChargeIdCodeList#81","@type":"unece:AllowanceChargeIdCodeList","rdf:value":"81","rdfs:comment":"Repair charge"},{"@id":"unece:AllowanceChargeIdCodeList#82","@type":"unece:AllowanceChargeIdCodeList","rdf:value":"82","rdfs:comment":"Loading charge"},{"@id":"unece:AllowanceChargeIdCodeList#83","@type":"unece:AllowanceChargeIdCodeList","rdf:value":"83","rdfs:comment":"Setup charge"},{"@id":"unece:AllowanceChargeIdCodeList#84","@type":"unece:AllowanceChargeIdCodeList","rdf:value":"84","rdfs:comment":"Testing charge"},{"@id":"unece:AllowanceChargeIdCodeList#85","@type":"unece:AllowanceChargeIdCodeList","rdf:value":"85","rdfs:comment":"Warehousing charge"},{"@id":"unece:AllowanceChargeIdCodeList#86","@type":"unece:AllowanceChargeIdCodeList","rdf:value":"86","rdfs:comment":"Gold surcharge"},{"@id":"unece:AllowanceChargeIdCodeList#87","@type":"unece:AllowanceChargeIdCodeList","rdf:value":"87","rdfs:comment":"Copper surcharge"},{"@id":"unece:AllowanceChargeIdCodeList#88","@type":"unece:AllowanceChargeIdCodeList","rdf:value":"88","rdfs:comment":"Material surcharge/deduction"},{"@id":"unece:AllowanceChargeIdCodeList#89","@type":"unece:AllowanceChargeIdCodeList","rdf:value":"89","rdfs:comment":"Lead surcharge"},{"@id":"unece:AllowanceChargeIdCodeList#90","@type":"unece:AllowanceChargeIdCodeList","rdf:value":"90","rdfs:comment":"Price index surcharge"},{"@id":"unece:AllowanceChargeIdCodeList#91","@type":"unece:AllowanceChargeIdCodeList","rdf:value":"91","rdfs:comment":"Platinum surcharge"},{"@id":"unece:AllowanceChargeIdCodeList#92","@type":"unece:AllowanceChargeIdCodeList","rdf:value":"92","rdfs:comment":"Silver surcharge"},{"@id":"unece:AllowanceChargeIdCodeList#93","@type":"unece:AllowanceChargeIdCodeList","rdf:value":"93","rdfs:comment":"Wolfram surcharge"},{"@id":"unece:AllowanceChargeIdCodeList#94","@type":"unece:AllowanceChargeIdCodeList","rdf:value":"94","rdfs:comment":"Aluminum surcharge"},{"@id":"unece:AllowanceChargeIdCodeList#95","@type":"unece:AllowanceChargeIdCodeList","rdf:value":"95","rdfs:comment":"Discount"},{"@id":"unece:AllowanceChargeIdCodeList#96","@type":"unece:AllowanceChargeIdCodeList","rdf:value":"96","rdfs:comment":"Insurance"},{"@id":"unece:AllowanceChargeIdCodeList#97","@type":"unece:AllowanceChargeIdCodeList","rdf:value":"97","rdfs:comment":"Minimum order / minimum billing charge"},{"@id":"unece:AllowanceChargeIdCodeList#98","@type":"unece:AllowanceChargeIdCodeList","rdf:value":"98","rdfs:comment":"Material surcharge (special materials)"},{"@id":"unece:AllowanceChargeIdCodeList#99","@type":"unece:AllowanceChargeIdCodeList","rdf:value":"99","rdfs:comment":"Surcharge"},{"@id":"unece:AllowanceChargeIdCodeList#100","@type":"unece:AllowanceChargeIdCodeList","rdf:value":"100","rdfs:comment":"Special rebate"},{"@id":"unece:AllowanceChargeIdCodeList#101","@type":"unece:AllowanceChargeIdCodeList","rdf:value":"101","rdfs:comment":"Carbon footprint charge"},{"@id":"unece:AllowanceChargeIdCodeList#102","@type":"unece:AllowanceChargeIdCodeList","rdf:value":"102","rdfs:comment":"Fixed long term"},{"@id":"unece:AllowanceChargeIdCodeList#103","@type":"unece:AllowanceChargeIdCodeList","rdf:value":"103","rdfs:comment":"Temporary"},{"@id":"unece:AllowanceChargeIdCodeList#104","@type":"unece:AllowanceChargeIdCodeList","rdf:value":"104","rdfs:comment":"Standard"},{"@id":"unece:AllowanceChargeIdCodeList#105","@type":"unece:AllowanceChargeIdCodeList","rdf:value":"105","rdfs:comment":"Yearly turnover"},{"@id":"unece:AllowanceChargeIdCodeList#106","@type":"unece:AllowanceChargeIdCodeList","rdf:value":"106","rdfs:comment":"Withheld taxes and social security contributions"},{"rdfs:label":"AllowanceChargeReasonCodeList","@type":"rdfs:Class","@id":"unece:AllowanceChargeReasonCodeList","rdfs:comment":"A character string used to represent an allowance charge reason."},{"@id":"unece:AllowanceChargeReasonCodeList#1","@type":"unece:AllowanceChargeReasonCodeList","rdf:value":"1","rdfs:comment":"Agreed settlement"},{"@id":"unece:AllowanceChargeReasonCodeList#2","@type":"unece:AllowanceChargeReasonCodeList","rdf:value":"2","rdfs:comment":"Below specification goods"},{"@id":"unece:AllowanceChargeReasonCodeList#3","@type":"unece:AllowanceChargeReasonCodeList","rdf:value":"3","rdfs:comment":"Damaged goods"},{"@id":"unece:AllowanceChargeReasonCodeList#4","@type":"unece:AllowanceChargeReasonCodeList","rdf:value":"4","rdfs:comment":"Short delivery"},{"@id":"unece:AllowanceChargeReasonCodeList#5","@type":"unece:AllowanceChargeReasonCodeList","rdf:value":"5","rdfs:comment":"Price query"},{"@id":"unece:AllowanceChargeReasonCodeList#6","@type":"unece:AllowanceChargeReasonCodeList","rdf:value":"6","rdfs:comment":"Proof of delivery required"},{"@id":"unece:AllowanceChargeReasonCodeList#7","@type":"unece:AllowanceChargeReasonCodeList","rdf:value":"7","rdfs:comment":"Payment on account"},{"@id":"unece:AllowanceChargeReasonCodeList#8","@type":"unece:AllowanceChargeReasonCodeList","rdf:value":"8","rdfs:comment":"Returnable container charge included"},{"@id":"unece:AllowanceChargeReasonCodeList#9","@type":"unece:AllowanceChargeReasonCodeList","rdf:value":"9","rdfs:comment":"Invoice error"},{"@id":"unece:AllowanceChargeReasonCodeList#10","@type":"unece:AllowanceChargeReasonCodeList","rdf:value":"10","rdfs:comment":"Costs for draft"},{"@id":"unece:AllowanceChargeReasonCodeList#11","@type":"unece:AllowanceChargeReasonCodeList","rdf:value":"11","rdfs:comment":"Bank charges"},{"@id":"unece:AllowanceChargeReasonCodeList#12","@type":"unece:AllowanceChargeReasonCodeList","rdf:value":"12","rdfs:comment":"Agent commission"},{"@id":"unece:AllowanceChargeReasonCodeList#13","@type":"unece:AllowanceChargeReasonCodeList","rdf:value":"13","rdfs:comment":"Counter claim"},{"@id":"unece:AllowanceChargeReasonCodeList#14","@type":"unece:AllowanceChargeReasonCodeList","rdf:value":"14","rdfs:comment":"Wrong delivery"},{"@id":"unece:AllowanceChargeReasonCodeList#15","@type":"unece:AllowanceChargeReasonCodeList","rdf:value":"15","rdfs:comment":"Goods returned to agent"},{"@id":"unece:AllowanceChargeReasonCodeList#16","@type":"unece:AllowanceChargeReasonCodeList","rdf:value":"16","rdfs:comment":"Goods partly returned"},{"@id":"unece:AllowanceChargeReasonCodeList#17","@type":"unece:AllowanceChargeReasonCodeList","rdf:value":"17","rdfs:comment":"Transport damage"},{"@id":"unece:AllowanceChargeReasonCodeList#18","@type":"unece:AllowanceChargeReasonCodeList","rdf:value":"18","rdfs:comment":"Goods on consignment"},{"@id":"unece:AllowanceChargeReasonCodeList#19","@type":"unece:AllowanceChargeReasonCodeList","rdf:value":"19","rdfs:comment":"Trade discount"},{"@id":"unece:AllowanceChargeReasonCodeList#20","@type":"unece:AllowanceChargeReasonCodeList","rdf:value":"20","rdfs:comment":"Deduction for late delivery"},{"@id":"unece:AllowanceChargeReasonCodeList#21","@type":"unece:AllowanceChargeReasonCodeList","rdf:value":"21","rdfs:comment":"Advertising costs"},{"@id":"unece:AllowanceChargeReasonCodeList#22","@type":"unece:AllowanceChargeReasonCodeList","rdf:value":"22","rdfs:comment":"Customs duties"},{"@id":"unece:AllowanceChargeReasonCodeList#23","@type":"unece:AllowanceChargeReasonCodeList","rdf:value":"23","rdfs:comment":"Telephone and postal costs"},{"@id":"unece:AllowanceChargeReasonCodeList#24","@type":"unece:AllowanceChargeReasonCodeList","rdf:value":"24","rdfs:comment":"Repair costs"},{"@id":"unece:AllowanceChargeReasonCodeList#25","@type":"unece:AllowanceChargeReasonCodeList","rdf:value":"25","rdfs:comment":"Attorney fees"},{"@id":"unece:AllowanceChargeReasonCodeList#26","@type":"unece:AllowanceChargeReasonCodeList","rdf:value":"26","rdfs:comment":"Taxes"},{"@id":"unece:AllowanceChargeReasonCodeList#27","@type":"unece:AllowanceChargeReasonCodeList","rdf:value":"27","rdfs:comment":"Reclaimed deduction"},{"@id":"unece:AllowanceChargeReasonCodeList#28","@type":"unece:AllowanceChargeReasonCodeList","rdf:value":"28","rdfs:comment":"See separate advice"},{"@id":"unece:AllowanceChargeReasonCodeList#29","@type":"unece:AllowanceChargeReasonCodeList","rdf:value":"29","rdfs:comment":"Buyer refused to take delivery"},{"@id":"unece:AllowanceChargeReasonCodeList#30","@type":"unece:AllowanceChargeReasonCodeList","rdf:value":"30","rdfs:comment":"Direct payment to seller"},{"@id":"unece:AllowanceChargeReasonCodeList#31","@type":"unece:AllowanceChargeReasonCodeList","rdf:value":"31","rdfs:comment":"Buyer disagrees with due date"},{"@id":"unece:AllowanceChargeReasonCodeList#32","@type":"unece:AllowanceChargeReasonCodeList","rdf:value":"32","rdfs:comment":"Goods not delivered"},{"@id":"unece:AllowanceChargeReasonCodeList#33","@type":"unece:AllowanceChargeReasonCodeList","rdf:value":"33","rdfs:comment":"Late delivery"},{"@id":"unece:AllowanceChargeReasonCodeList#34","@type":"unece:AllowanceChargeReasonCodeList","rdf:value":"34","rdfs:comment":"Quoted as paid to you"},{"@id":"unece:AllowanceChargeReasonCodeList#35","@type":"unece:AllowanceChargeReasonCodeList","rdf:value":"35","rdfs:comment":"Goods returned"},{"@id":"unece:AllowanceChargeReasonCodeList#36","@type":"unece:AllowanceChargeReasonCodeList","rdf:value":"36","rdfs:comment":"Invoice not received"},{"@id":"unece:AllowanceChargeReasonCodeList#37","@type":"unece:AllowanceChargeReasonCodeList","rdf:value":"37","rdfs:comment":"Credit note to debtor/not to us"},{"@id":"unece:AllowanceChargeReasonCodeList#38","@type":"unece:AllowanceChargeReasonCodeList","rdf:value":"38","rdfs:comment":"Deducted bonus"},{"@id":"unece:AllowanceChargeReasonCodeList#39","@type":"unece:AllowanceChargeReasonCodeList","rdf:value":"39","rdfs:comment":"Deducted discount"},{"@id":"unece:AllowanceChargeReasonCodeList#40","@type":"unece:AllowanceChargeReasonCodeList","rdf:value":"40","rdfs:comment":"Deducted freight costs"},{"@id":"unece:AllowanceChargeReasonCodeList#41","@type":"unece:AllowanceChargeReasonCodeList","rdf:value":"41","rdfs:comment":"Deduction against other invoices"},{"@id":"unece:AllowanceChargeReasonCodeList#42","@type":"unece:AllowanceChargeReasonCodeList","rdf:value":"42","rdfs:comment":"Credit balance(s)"},{"@id":"unece:AllowanceChargeReasonCodeList#43","@type":"unece:AllowanceChargeReasonCodeList","rdf:value":"43","rdfs:comment":"Reason unknown"},{"@id":"unece:AllowanceChargeReasonCodeList#44","@type":"unece:AllowanceChargeReasonCodeList","rdf:value":"44","rdfs:comment":"Awaiting message from seller"},{"@id":"unece:AllowanceChargeReasonCodeList#45","@type":"unece:AllowanceChargeReasonCodeList","rdf:value":"45","rdfs:comment":"Debit note to seller"},{"@id":"unece:AllowanceChargeReasonCodeList#46","@type":"unece:AllowanceChargeReasonCodeList","rdf:value":"46","rdfs:comment":"Discount beyond terms"},{"@id":"unece:AllowanceChargeReasonCodeList#47","@type":"unece:AllowanceChargeReasonCodeList","rdf:value":"47","rdfs:comment":"See buyer's letter"},{"@id":"unece:AllowanceChargeReasonCodeList#48","@type":"unece:AllowanceChargeReasonCodeList","rdf:value":"48","rdfs:comment":"Allowance/charge error"},{"@id":"unece:AllowanceChargeReasonCodeList#49","@type":"unece:AllowanceChargeReasonCodeList","rdf:value":"49","rdfs:comment":"Substitute product"},{"@id":"unece:AllowanceChargeReasonCodeList#50","@type":"unece:AllowanceChargeReasonCodeList","rdf:value":"50","rdfs:comment":"Terms of sale error"},{"@id":"unece:AllowanceChargeReasonCodeList#51","@type":"unece:AllowanceChargeReasonCodeList","rdf:value":"51","rdfs:comment":"Required data missing"},{"@id":"unece:AllowanceChargeReasonCodeList#52","@type":"unece:AllowanceChargeReasonCodeList","rdf:value":"52","rdfs:comment":"Wrong invoice"},{"@id":"unece:AllowanceChargeReasonCodeList#53","@type":"unece:AllowanceChargeReasonCodeList","rdf:value":"53","rdfs:comment":"Duplicate invoice"},{"@id":"unece:AllowanceChargeReasonCodeList#54","@type":"unece:AllowanceChargeReasonCodeList","rdf:value":"54","rdfs:comment":"Weight error"},{"@id":"unece:AllowanceChargeReasonCodeList#55","@type":"unece:AllowanceChargeReasonCodeList","rdf:value":"55","rdfs:comment":"Additional charge not authorized"},{"@id":"unece:AllowanceChargeReasonCodeList#56","@type":"unece:AllowanceChargeReasonCodeList","rdf:value":"56","rdfs:comment":"Incorrect discount"},{"@id":"unece:AllowanceChargeReasonCodeList#57","@type":"unece:AllowanceChargeReasonCodeList","rdf:value":"57","rdfs:comment":"Price change"},{"@id":"unece:AllowanceChargeReasonCodeList#58","@type":"unece:AllowanceChargeReasonCodeList","rdf:value":"58","rdfs:comment":"Variation"},{"@id":"unece:AllowanceChargeReasonCodeList#59","@type":"unece:AllowanceChargeReasonCodeList","rdf:value":"59","rdfs:comment":"Chargeback"},{"@id":"unece:AllowanceChargeReasonCodeList#60","@type":"unece:AllowanceChargeReasonCodeList","rdf:value":"60","rdfs:comment":"Offset"},{"@id":"unece:AllowanceChargeReasonCodeList#61","@type":"unece:AllowanceChargeReasonCodeList","rdf:value":"61","rdfs:comment":"Indirect payment"},{"@id":"unece:AllowanceChargeReasonCodeList#62","@type":"unece:AllowanceChargeReasonCodeList","rdf:value":"62","rdfs:comment":"Financial reassignment"},{"@id":"unece:AllowanceChargeReasonCodeList#63","@type":"unece:AllowanceChargeReasonCodeList","rdf:value":"63","rdfs:comment":"Reinstatement of chargeback/offset"},{"@id":"unece:AllowanceChargeReasonCodeList#64","@type":"unece:AllowanceChargeReasonCodeList","rdf:value":"64","rdfs:comment":"Expecting new terms"},{"@id":"unece:AllowanceChargeReasonCodeList#65","@type":"unece:AllowanceChargeReasonCodeList","rdf:value":"65","rdfs:comment":"Settlement to agent"},{"@id":"unece:AllowanceChargeReasonCodeList#66","@type":"unece:AllowanceChargeReasonCodeList","rdf:value":"66","rdfs:comment":"Cash discount"},{"@id":"unece:AllowanceChargeReasonCodeList#67","@type":"unece:AllowanceChargeReasonCodeList","rdf:value":"67","rdfs:comment":"Delcredere costs"},{"@id":"unece:AllowanceChargeReasonCodeList#68","@type":"unece:AllowanceChargeReasonCodeList","rdf:value":"68","rdfs:comment":"Early payment allowance adjustment"},{"@id":"unece:AllowanceChargeReasonCodeList#69","@type":"unece:AllowanceChargeReasonCodeList","rdf:value":"69","rdfs:comment":"Incorrect due date for monetary amount"},{"@id":"unece:AllowanceChargeReasonCodeList#70","@type":"unece:AllowanceChargeReasonCodeList","rdf:value":"70","rdfs:comment":"Wrong monetary amount resulting from incorrect free goods quantity"},{"@id":"unece:AllowanceChargeReasonCodeList#71","@type":"unece:AllowanceChargeReasonCodeList","rdf:value":"71","rdfs:comment":"Rack or shelf replenishment service by a supplier"},{"@id":"unece:AllowanceChargeReasonCodeList#72","@type":"unece:AllowanceChargeReasonCodeList","rdf:value":"72","rdfs:comment":"Temporary special promotion"},{"@id":"unece:AllowanceChargeReasonCodeList#73","@type":"unece:AllowanceChargeReasonCodeList","rdf:value":"73","rdfs:comment":"Difference in tax rate"},{"@id":"unece:AllowanceChargeReasonCodeList#74","@type":"unece:AllowanceChargeReasonCodeList","rdf:value":"74","rdfs:comment":"Quantity discount"},{"@id":"unece:AllowanceChargeReasonCodeList#75","@type":"unece:AllowanceChargeReasonCodeList","rdf:value":"75","rdfs:comment":"Promotion discount"},{"@id":"unece:AllowanceChargeReasonCodeList#76","@type":"unece:AllowanceChargeReasonCodeList","rdf:value":"76","rdfs:comment":"Cancellation deadline passed"},{"@id":"unece:AllowanceChargeReasonCodeList#77","@type":"unece:AllowanceChargeReasonCodeList","rdf:value":"77","rdfs:comment":"Pricing discount"},{"@id":"unece:AllowanceChargeReasonCodeList#78","@type":"unece:AllowanceChargeReasonCodeList","rdf:value":"78","rdfs:comment":"Volume discount"},{"@id":"unece:AllowanceChargeReasonCodeList#79","@type":"unece:AllowanceChargeReasonCodeList","rdf:value":"79","rdfs:comment":"Sundry discount"},{"@id":"unece:AllowanceChargeReasonCodeList#80","@type":"unece:AllowanceChargeReasonCodeList","rdf:value":"80","rdfs:comment":"Card holder signature missing"},{"@id":"unece:AllowanceChargeReasonCodeList#81","@type":"unece:AllowanceChargeReasonCodeList","rdf:value":"81","rdfs:comment":"Card expiry date missing"},{"@id":"unece:AllowanceChargeReasonCodeList#82","@type":"unece:AllowanceChargeReasonCodeList","rdf:value":"82","rdfs:comment":"Card number error"},{"@id":"unece:AllowanceChargeReasonCodeList#83","@type":"unece:AllowanceChargeReasonCodeList","rdf:value":"83","rdfs:comment":"Card expired"},{"@id":"unece:AllowanceChargeReasonCodeList#84","@type":"unece:AllowanceChargeReasonCodeList","rdf:value":"84","rdfs:comment":"Test card transaction"},{"@id":"unece:AllowanceChargeReasonCodeList#85","@type":"unece:AllowanceChargeReasonCodeList","rdf:value":"85","rdfs:comment":"Permission limit exceeded"},{"@id":"unece:AllowanceChargeReasonCodeList#86","@type":"unece:AllowanceChargeReasonCodeList","rdf:value":"86","rdfs:comment":"Wrong authorisation code"},{"@id":"unece:AllowanceChargeReasonCodeList#87","@type":"unece:AllowanceChargeReasonCodeList","rdf:value":"87","rdfs:comment":"Wrong authorised amount"},{"@id":"unece:AllowanceChargeReasonCodeList#88","@type":"unece:AllowanceChargeReasonCodeList","rdf:value":"88","rdfs:comment":"Authorisation failed"},{"@id":"unece:AllowanceChargeReasonCodeList#89","@type":"unece:AllowanceChargeReasonCodeList","rdf:value":"89","rdfs:comment":"Card acceptor data error"},{"@id":"unece:AllowanceChargeReasonCodeList#90","@type":"unece:AllowanceChargeReasonCodeList","rdf:value":"90","rdfs:comment":"Treasury management service charge"},{"@id":"unece:AllowanceChargeReasonCodeList#91","@type":"unece:AllowanceChargeReasonCodeList","rdf:value":"91","rdfs:comment":"Agreed discount"},{"@id":"unece:AllowanceChargeReasonCodeList#92","@type":"unece:AllowanceChargeReasonCodeList","rdf:value":"92","rdfs:comment":"Expediting fee"},{"@id":"unece:AllowanceChargeReasonCodeList#93","@type":"unece:AllowanceChargeReasonCodeList","rdf:value":"93","rdfs:comment":"Invoicing fee"},{"@id":"unece:AllowanceChargeReasonCodeList#94","@type":"unece:AllowanceChargeReasonCodeList","rdf:value":"94","rdfs:comment":"Freight charge"},{"@id":"unece:AllowanceChargeReasonCodeList#95","@type":"unece:AllowanceChargeReasonCodeList","rdf:value":"95","rdfs:comment":"Small order processing service charge"},{"@id":"unece:AllowanceChargeReasonCodeList#96","@type":"unece:AllowanceChargeReasonCodeList","rdf:value":"96","rdfs:comment":"Currency exchange differences"},{"@id":"unece:AllowanceChargeReasonCodeList#97","@type":"unece:AllowanceChargeReasonCodeList","rdf:value":"97","rdfs:comment":"Insolvency"},{"@id":"unece:AllowanceChargeReasonCodeList#98","@type":"unece:AllowanceChargeReasonCodeList","rdf:value":"98","rdfs:comment":"Incorrect references"},{"@id":"unece:AllowanceChargeReasonCodeList#99","@type":"unece:AllowanceChargeReasonCodeList","rdf:value":"99","rdfs:comment":"Incorrect identification of the buyer"},{"@id":"unece:AllowanceChargeReasonCodeList#100","@type":"unece:AllowanceChargeReasonCodeList","rdf:value":"100","rdfs:comment":"Incorrect product identification"},{"@id":"unece:AllowanceChargeReasonCodeList#101","@type":"unece:AllowanceChargeReasonCodeList","rdf:value":"101","rdfs:comment":"New employee"},{"@id":"unece:AllowanceChargeReasonCodeList#102","@type":"unece:AllowanceChargeReasonCodeList","rdf:value":"102","rdfs:comment":"Employee retirement"},{"@id":"unece:AllowanceChargeReasonCodeList#103","@type":"unece:AllowanceChargeReasonCodeList","rdf:value":"103","rdfs:comment":"Salary change"},{"@id":"unece:AllowanceChargeReasonCodeList#104","@type":"unece:AllowanceChargeReasonCodeList","rdf:value":"104","rdfs:comment":"Parental leave"},{"@id":"unece:AllowanceChargeReasonCodeList#ZZZ","@type":"unece:AllowanceChargeReasonCodeList","rdf:value":"ZZZ","rdfs:comment":"Mutually defined"},{"rdfs:label":"CashAccountTypeCodeList","@type":"rdfs:Class","@id":"unece:CashAccountTypeCodeList","rdfs:comment":""},{"rdfs:label":"CurrencyCodeList","@type":"rdfs:Class","@id":"unece:CurrencyCodeList","rdfs:comment":"A character string used to represent a currency."},{"@id":"unece:CurrencyCodeList#AED","@type":"unece:CurrencyCodeList","rdf:value":"AED","rdfs:comment":"Dirham"},{"@id":"unece:CurrencyCodeList#AFN","@type":"unece:CurrencyCodeList","rdf:value":"AFN","rdfs:comment":"Afghani"},{"@id":"unece:CurrencyCodeList#ALL","@type":"unece:CurrencyCodeList","rdf:value":"ALL","rdfs:comment":"Lek"},{"@id":"unece:CurrencyCodeList#AMD","@type":"unece:CurrencyCodeList","rdf:value":"AMD","rdfs:comment":"Dram"},{"@id":"unece:CurrencyCodeList#ANG","@type":"unece:CurrencyCodeList","rdf:value":"ANG","rdfs:comment":"Netherlands Antillian Guilder"},{"@id":"unece:CurrencyCodeList#AOA","@type":"unece:CurrencyCodeList","rdf:value":"AOA","rdfs:comment":"Kwanza"},{"@id":"unece:CurrencyCodeList#ARS","@type":"unece:CurrencyCodeList","rdf:value":"ARS","rdfs:comment":"Argentine Peso"},{"@id":"unece:CurrencyCodeList#AUD","@type":"unece:CurrencyCodeList","rdf:value":"AUD","rdfs:comment":"Australian Dollar"},{"@id":"unece:CurrencyCodeList#AWG","@type":"unece:CurrencyCodeList","rdf:value":"AWG","rdfs:comment":"Aruban Florin"},{"@id":"unece:CurrencyCodeList#AZN","@type":"unece:CurrencyCodeList","rdf:value":"AZN","rdfs:comment":"Azerbaijan Manat"},{"@id":"unece:CurrencyCodeList#BAM","@type":"unece:CurrencyCodeList","rdf:value":"BAM","rdfs:comment":"Convertible Mark"},{"@id":"unece:CurrencyCodeList#BBD","@type":"unece:CurrencyCodeList","rdf:value":"BBD","rdfs:comment":"Barbados Dollar"},{"@id":"unece:CurrencyCodeList#BDT","@type":"unece:CurrencyCodeList","rdf:value":"BDT","rdfs:comment":"Taka"},{"@id":"unece:CurrencyCodeList#BGN","@type":"unece:CurrencyCodeList","rdf:value":"BGN","rdfs:comment":"Bulgarian Lev"},{"@id":"unece:CurrencyCodeList#BHD","@type":"unece:CurrencyCodeList","rdf:value":"BHD","rdfs:comment":"Bahraini Dinar"},{"@id":"unece:CurrencyCodeList#BIF","@type":"unece:CurrencyCodeList","rdf:value":"BIF","rdfs:comment":"Burundi Franc"},{"@id":"unece:CurrencyCodeList#BMD","@type":"unece:CurrencyCodeList","rdf:value":"BMD","rdfs:comment":"Bermudian Dollar (customarily: Bermuda Dollar)"},{"@id":"unece:CurrencyCodeList#BND","@type":"unece:CurrencyCodeList","rdf:value":"BND","rdfs:comment":"Brunei Dollar"},{"@id":"unece:CurrencyCodeList#BOB","@type":"unece:CurrencyCodeList","rdf:value":"BOB","rdfs:comment":"Boliviano"},{"@id":"unece:CurrencyCodeList#BOV","@type":"unece:CurrencyCodeList","rdf:value":"BOV","rdfs:comment":"Mvdol"},{"@id":"unece:CurrencyCodeList#BRL","@type":"unece:CurrencyCodeList","rdf:value":"BRL","rdfs:comment":"Brazilian Real"},{"@id":"unece:CurrencyCodeList#BSD","@type":"unece:CurrencyCodeList","rdf:value":"BSD","rdfs:comment":"Bahamian Dollar"},{"@id":"unece:CurrencyCodeList#BTN","@type":"unece:CurrencyCodeList","rdf:value":"BTN","rdfs:comment":"Ngultrum"},{"@id":"unece:CurrencyCodeList#BWP","@type":"unece:CurrencyCodeList","rdf:value":"BWP","rdfs:comment":"Pula"},{"@id":"unece:CurrencyCodeList#BYN","@type":"unece:CurrencyCodeList","rdf:value":"BYN","rdfs:comment":"Belarussian Ruble"},{"@id":"unece:CurrencyCodeList#BZD","@type":"unece:CurrencyCodeList","rdf:value":"BZD","rdfs:comment":"Belize Dollar"},{"@id":"unece:CurrencyCodeList#CAD","@type":"unece:CurrencyCodeList","rdf:value":"CAD","rdfs:comment":"Canadian Dollar"},{"@id":"unece:CurrencyCodeList#CDF","@type":"unece:CurrencyCodeList","rdf:value":"CDF","rdfs:comment":"Franc Congolais"},{"@id":"unece:CurrencyCodeList#CHE","@type":"unece:CurrencyCodeList","rdf:value":"CHE","rdfs:comment":"WIR Euro"},{"@id":"unece:CurrencyCodeList#CHF","@type":"unece:CurrencyCodeList","rdf:value":"CHF","rdfs:comment":"Swiss Franc"},{"@id":"unece:CurrencyCodeList#CHW","@type":"unece:CurrencyCodeList","rdf:value":"CHW","rdfs:comment":"WIR Franc"},{"@id":"unece:CurrencyCodeList#CLF","@type":"unece:CurrencyCodeList","rdf:value":"CLF","rdfs:comment":"Unidad de Fomento"},{"@id":"unece:CurrencyCodeList#CLP","@type":"unece:CurrencyCodeList","rdf:value":"CLP","rdfs:comment":"Chilean Peso"},{"@id":"unece:CurrencyCodeList#CNY","@type":"unece:CurrencyCodeList","rdf:value":"CNY","rdfs:comment":"Yuan Renminbi"},{"@id":"unece:CurrencyCodeList#COP","@type":"unece:CurrencyCodeList","rdf:value":"COP","rdfs:comment":"Colombian Peso"},{"@id":"unece:CurrencyCodeList#COU","@type":"unece:CurrencyCodeList","rdf:value":"COU","rdfs:comment":"Unidad de Valor Real"},{"@id":"unece:CurrencyCodeList#CRC","@type":"unece:CurrencyCodeList","rdf:value":"CRC","rdfs:comment":"Costa Rican Colon"},{"@id":"unece:CurrencyCodeList#CUC","@type":"unece:CurrencyCodeList","rdf:value":"CUC","rdfs:comment":"Peso Convertible"},{"@id":"unece:CurrencyCodeList#CUP","@type":"unece:CurrencyCodeList","rdf:value":"CUP","rdfs:comment":"Cuban Peso"},{"@id":"unece:CurrencyCodeList#CVE","@type":"unece:CurrencyCodeList","rdf:value":"CVE","rdfs:comment":"Cabo Verde Escudo"},{"@id":"unece:CurrencyCodeList#CZK","@type":"unece:CurrencyCodeList","rdf:value":"CZK","rdfs:comment":"Czech Koruna"},{"@id":"unece:CurrencyCodeList#DJF","@type":"unece:CurrencyCodeList","rdf:value":"DJF","rdfs:comment":"Djibouti Franc"},{"@id":"unece:CurrencyCodeList#DKK","@type":"unece:CurrencyCodeList","rdf:value":"DKK","rdfs:comment":"Danish Krone"},{"@id":"unece:CurrencyCodeList#DOP","@type":"unece:CurrencyCodeList","rdf:value":"DOP","rdfs:comment":"Dominican Peso"},{"@id":"unece:CurrencyCodeList#DZD","@type":"unece:CurrencyCodeList","rdf:value":"DZD","rdfs:comment":"Algerian Dinar"},{"@id":"unece:CurrencyCodeList#EGP","@type":"unece:CurrencyCodeList","rdf:value":"EGP","rdfs:comment":"Egyptian Pound"},{"@id":"unece:CurrencyCodeList#ERN","@type":"unece:CurrencyCodeList","rdf:value":"ERN","rdfs:comment":"Nakfa"},{"@id":"unece:CurrencyCodeList#ETB","@type":"unece:CurrencyCodeList","rdf:value":"ETB","rdfs:comment":"Ethopian Birr"},{"@id":"unece:CurrencyCodeList#EUR","@type":"unece:CurrencyCodeList","rdf:value":"EUR","rdfs:comment":"Euro"},{"@id":"unece:CurrencyCodeList#FJD","@type":"unece:CurrencyCodeList","rdf:value":"FJD","rdfs:comment":"Fiji Dollar"},{"@id":"unece:CurrencyCodeList#FKP","@type":"unece:CurrencyCodeList","rdf:value":"FKP","rdfs:comment":"Falkland Islands Pound"},{"@id":"unece:CurrencyCodeList#GBP","@type":"unece:CurrencyCodeList","rdf:value":"GBP","rdfs:comment":"Pound Sterling"},{"@id":"unece:CurrencyCodeList#GEL","@type":"unece:CurrencyCodeList","rdf:value":"GEL","rdfs:comment":"Lari"},{"@id":"unece:CurrencyCodeList#GHS","@type":"unece:CurrencyCodeList","rdf:value":"GHS","rdfs:comment":"Ghana Cedi"},{"@id":"unece:CurrencyCodeList#GIP","@type":"unece:CurrencyCodeList","rdf:value":"GIP","rdfs:comment":"Gibraltar Pound"},{"@id":"unece:CurrencyCodeList#GMD","@type":"unece:CurrencyCodeList","rdf:value":"GMD","rdfs:comment":"Dalasi"},{"@id":"unece:CurrencyCodeList#GNF","@type":"unece:CurrencyCodeList","rdf:value":"GNF","rdfs:comment":"Guinean Franc"},{"@id":"unece:CurrencyCodeList#GTQ","@type":"unece:CurrencyCodeList","rdf:value":"GTQ","rdfs:comment":"Quetzal"},{"@id":"unece:CurrencyCodeList#GYD","@type":"unece:CurrencyCodeList","rdf:value":"GYD","rdfs:comment":"Guyana Dollar"},{"@id":"unece:CurrencyCodeList#HKD","@type":"unece:CurrencyCodeList","rdf:value":"HKD","rdfs:comment":"Honk Kong Dollar"},{"@id":"unece:CurrencyCodeList#HNL","@type":"unece:CurrencyCodeList","rdf:value":"HNL","rdfs:comment":"Lempira"},{"@id":"unece:CurrencyCodeList#HRK","@type":"unece:CurrencyCodeList","rdf:value":"HRK","rdfs:comment":"Kuna"},{"@id":"unece:CurrencyCodeList#HTG","@type":"unece:CurrencyCodeList","rdf:value":"HTG","rdfs:comment":"Gourde"},{"@id":"unece:CurrencyCodeList#HUF","@type":"unece:CurrencyCodeList","rdf:value":"HUF","rdfs:comment":"Forint"},{"@id":"unece:CurrencyCodeList#IDR","@type":"unece:CurrencyCodeList","rdf:value":"IDR","rdfs:comment":"Rupiah"},{"@id":"unece:CurrencyCodeList#ILS","@type":"unece:CurrencyCodeList","rdf:value":"ILS","rdfs:comment":"New Israeli Sheqel"},{"@id":"unece:CurrencyCodeList#INR","@type":"unece:CurrencyCodeList","rdf:value":"INR","rdfs:comment":"Indian Rupee"},{"@id":"unece:CurrencyCodeList#IQD","@type":"unece:CurrencyCodeList","rdf:value":"IQD","rdfs:comment":"Iraqi Dinar"},{"@id":"unece:CurrencyCodeList#IRR","@type":"unece:CurrencyCodeList","rdf:value":"IRR","rdfs:comment":"Iranian Rial"},{"@id":"unece:CurrencyCodeList#ISK","@type":"unece:CurrencyCodeList","rdf:value":"ISK","rdfs:comment":"Iceland Krona"},{"@id":"unece:CurrencyCodeList#JMD","@type":"unece:CurrencyCodeList","rdf:value":"JMD","rdfs:comment":"Jamaican Dollar"},{"@id":"unece:CurrencyCodeList#JOD","@type":"unece:CurrencyCodeList","rdf:value":"JOD","rdfs:comment":"Jordanian Dinar"},{"@id":"unece:CurrencyCodeList#JPY","@type":"unece:CurrencyCodeList","rdf:value":"JPY","rdfs:comment":"Yen"},{"@id":"unece:CurrencyCodeList#KES","@type":"unece:CurrencyCodeList","rdf:value":"KES","rdfs:comment":"Kenyan Shilling"},{"@id":"unece:CurrencyCodeList#KGS","@type":"unece:CurrencyCodeList","rdf:value":"KGS","rdfs:comment":"Som"},{"@id":"unece:CurrencyCodeList#KHR","@type":"unece:CurrencyCodeList","rdf:value":"KHR","rdfs:comment":"Riel"},{"@id":"unece:CurrencyCodeList#KMF","@type":"unece:CurrencyCodeList","rdf:value":"KMF","rdfs:comment":"Comorian Franc"},{"@id":"unece:CurrencyCodeList#KPW","@type":"unece:CurrencyCodeList","rdf:value":"KPW","rdfs:comment":"North Korean Won"},{"@id":"unece:CurrencyCodeList#KRW","@type":"unece:CurrencyCodeList","rdf:value":"KRW","rdfs:comment":"Won"},{"@id":"unece:CurrencyCodeList#KWD","@type":"unece:CurrencyCodeList","rdf:value":"KWD","rdfs:comment":"Kuwaiti Dinar"},{"@id":"unece:CurrencyCodeList#KYD","@type":"unece:CurrencyCodeList","rdf:value":"KYD","rdfs:comment":"Cayman Islands Dollar"},{"@id":"unece:CurrencyCodeList#KZT","@type":"unece:CurrencyCodeList","rdf:value":"KZT","rdfs:comment":"Tenge"},{"@id":"unece:CurrencyCodeList#LAK","@type":"unece:CurrencyCodeList","rdf:value":"LAK","rdfs:comment":"Lao Kip"},{"@id":"unece:CurrencyCodeList#LBP","@type":"unece:CurrencyCodeList","rdf:value":"LBP","rdfs:comment":"Lebanese Pound"},{"@id":"unece:CurrencyCodeList#LKR","@type":"unece:CurrencyCodeList","rdf:value":"LKR","rdfs:comment":"Sri Lanka Rupee"},{"@id":"unece:CurrencyCodeList#LRD","@type":"unece:CurrencyCodeList","rdf:value":"LRD","rdfs:comment":"Liberian Dollar"},{"@id":"unece:CurrencyCodeList#LSL","@type":"unece:CurrencyCodeList","rdf:value":"LSL","rdfs:comment":"Loti"},{"@id":"unece:CurrencyCodeList#LYD","@type":"unece:CurrencyCodeList","rdf:value":"LYD","rdfs:comment":"Libyan Dinar"},{"@id":"unece:CurrencyCodeList#MAD","@type":"unece:CurrencyCodeList","rdf:value":"MAD","rdfs:comment":"Morrocan Dirham"},{"@id":"unece:CurrencyCodeList#MDL","@type":"unece:CurrencyCodeList","rdf:value":"MDL","rdfs:comment":"Moldovan Leu"},{"@id":"unece:CurrencyCodeList#MGA","@type":"unece:CurrencyCodeList","rdf:value":"MGA","rdfs:comment":"Ariary"},{"@id":"unece:CurrencyCodeList#MKD","@type":"unece:CurrencyCodeList","rdf:value":"MKD","rdfs:comment":"Denar"},{"@id":"unece:CurrencyCodeList#MMK","@type":"unece:CurrencyCodeList","rdf:value":"MMK","rdfs:comment":"Kyat"},{"@id":"unece:CurrencyCodeList#MNT","@type":"unece:CurrencyCodeList","rdf:value":"MNT","rdfs:comment":"Tugrik"},{"@id":"unece:CurrencyCodeList#MOP","@type":"unece:CurrencyCodeList","rdf:value":"MOP","rdfs:comment":"Pataca"},{"@id":"unece:CurrencyCodeList#MRU","@type":"unece:CurrencyCodeList","rdf:value":"MRU","rdfs:comment":"Ouguiya"},{"@id":"unece:CurrencyCodeList#MUR","@type":"unece:CurrencyCodeList","rdf:value":"MUR","rdfs:comment":"Mauritius Rupee"},{"@id":"unece:CurrencyCodeList#MVR","@type":"unece:CurrencyCodeList","rdf:value":"MVR","rdfs:comment":"Rufiyaa"},{"@id":"unece:CurrencyCodeList#MWK","@type":"unece:CurrencyCodeList","rdf:value":"MWK","rdfs:comment":"Malawi Kwacha"},{"@id":"unece:CurrencyCodeList#MXN","@type":"unece:CurrencyCodeList","rdf:value":"MXN","rdfs:comment":"Mexican Peso"},{"@id":"unece:CurrencyCodeList#MXV","@type":"unece:CurrencyCodeList","rdf:value":"MXV","rdfs:comment":"Mexican Unidad de Inversion (UDI)"},{"@id":"unece:CurrencyCodeList#MYR","@type":"unece:CurrencyCodeList","rdf:value":"MYR","rdfs:comment":"Malaysian Ringgit"},{"@id":"unece:CurrencyCodeList#MZN","@type":"unece:CurrencyCodeList","rdf:value":"MZN","rdfs:comment":"Mozambique Metical"},{"@id":"unece:CurrencyCodeList#NAD","@type":"unece:CurrencyCodeList","rdf:value":"NAD","rdfs:comment":"Namibia Dollar"},{"@id":"unece:CurrencyCodeList#NGN","@type":"unece:CurrencyCodeList","rdf:value":"NGN","rdfs:comment":"Naira"},{"@id":"unece:CurrencyCodeList#NIO","@type":"unece:CurrencyCodeList","rdf:value":"NIO","rdfs:comment":"Cordoba Oro"},{"@id":"unece:CurrencyCodeList#NOK","@type":"unece:CurrencyCodeList","rdf:value":"NOK","rdfs:comment":"Norwegian Krone"},{"@id":"unece:CurrencyCodeList#NPR","@type":"unece:CurrencyCodeList","rdf:value":"NPR","rdfs:comment":"Nepalese Rupee"},{"@id":"unece:CurrencyCodeList#NZD","@type":"unece:CurrencyCodeList","rdf:value":"NZD","rdfs:comment":"New Zealand Dollar"},{"@id":"unece:CurrencyCodeList#OMR","@type":"unece:CurrencyCodeList","rdf:value":"OMR","rdfs:comment":"Rial Omani"},{"@id":"unece:CurrencyCodeList#PAB","@type":"unece:CurrencyCodeList","rdf:value":"PAB","rdfs:comment":"Balboa"},{"@id":"unece:CurrencyCodeList#PEN","@type":"unece:CurrencyCodeList","rdf:value":"PEN","rdfs:comment":"Sol"},{"@id":"unece:CurrencyCodeList#PGK","@type":"unece:CurrencyCodeList","rdf:value":"PGK","rdfs:comment":"Kina"},{"@id":"unece:CurrencyCodeList#PHP","@type":"unece:CurrencyCodeList","rdf:value":"PHP","rdfs:comment":"Philippine Piso"},{"@id":"unece:CurrencyCodeList#PKR","@type":"unece:CurrencyCodeList","rdf:value":"PKR","rdfs:comment":"Pakistan Rupee"},{"@id":"unece:CurrencyCodeList#PLN","@type":"unece:CurrencyCodeList","rdf:value":"PLN","rdfs:comment":"Zloty"},{"@id":"unece:CurrencyCodeList#PYG","@type":"unece:CurrencyCodeList","rdf:value":"PYG","rdfs:comment":"Guarani"},{"@id":"unece:CurrencyCodeList#QAR","@type":"unece:CurrencyCodeList","rdf:value":"QAR","rdfs:comment":"Qatari Rial"},{"@id":"unece:CurrencyCodeList#RON","@type":"unece:CurrencyCodeList","rdf:value":"RON","rdfs:comment":"Romanian Leu"},{"@id":"unece:CurrencyCodeList#RSD","@type":"unece:CurrencyCodeList","rdf:value":"RSD","rdfs:comment":"Serbian Dinar"},{"@id":"unece:CurrencyCodeList#RUB","@type":"unece:CurrencyCodeList","rdf:value":"RUB","rdfs:comment":"Russian Ruble"},{"@id":"unece:CurrencyCodeList#RWF","@type":"unece:CurrencyCodeList","rdf:value":"RWF","rdfs:comment":"Rwanda Franc"},{"@id":"unece:CurrencyCodeList#SAR","@type":"unece:CurrencyCodeList","rdf:value":"SAR","rdfs:comment":"Saudi Riyal"},{"@id":"unece:CurrencyCodeList#SBD","@type":"unece:CurrencyCodeList","rdf:value":"SBD","rdfs:comment":"Solomon Islands Dollar"},{"@id":"unece:CurrencyCodeList#SCR","@type":"unece:CurrencyCodeList","rdf:value":"SCR","rdfs:comment":"Seychelles Rupee"},{"@id":"unece:CurrencyCodeList#SDG","@type":"unece:CurrencyCodeList","rdf:value":"SDG","rdfs:comment":"Sudanese Pound"},{"@id":"unece:CurrencyCodeList#SEK","@type":"unece:CurrencyCodeList","rdf:value":"SEK","rdfs:comment":"Swedish Krona"},{"@id":"unece:CurrencyCodeList#SGD","@type":"unece:CurrencyCodeList","rdf:value":"SGD","rdfs:comment":"Singapore Dollar"},{"@id":"unece:CurrencyCodeList#SHP","@type":"unece:CurrencyCodeList","rdf:value":"SHP","rdfs:comment":"St. Helena Pound"},{"@id":"unece:CurrencyCodeList#SLL","@type":"unece:CurrencyCodeList","rdf:value":"SLL","rdfs:comment":"Leone"},{"@id":"unece:CurrencyCodeList#SOS","@type":"unece:CurrencyCodeList","rdf:value":"SOS","rdfs:comment":"Somali Shilling"},{"@id":"unece:CurrencyCodeList#SRD","@type":"unece:CurrencyCodeList","rdf:value":"SRD","rdfs:comment":"Suriname Dollar"},{"@id":"unece:CurrencyCodeList#SSP","@type":"unece:CurrencyCodeList","rdf:value":"SSP","rdfs:comment":"South Sudanese Pound"},{"@id":"unece:CurrencyCodeList#STN","@type":"unece:CurrencyCodeList","rdf:value":"STN","rdfs:comment":"Dobra"},{"@id":"unece:CurrencyCodeList#SVC","@type":"unece:CurrencyCodeList","rdf:value":"SVC","rdfs:comment":"El Salvador Colon"},{"@id":"unece:CurrencyCodeList#SYP","@type":"unece:CurrencyCodeList","rdf:value":"SYP","rdfs:comment":"Syrian Pound"},{"@id":"unece:CurrencyCodeList#SZL","@type":"unece:CurrencyCodeList","rdf:value":"SZL","rdfs:comment":"Lilangeni"},{"@id":"unece:CurrencyCodeList#THB","@type":"unece:CurrencyCodeList","rdf:value":"THB","rdfs:comment":"Baht"},{"@id":"unece:CurrencyCodeList#TJS","@type":"unece:CurrencyCodeList","rdf:value":"TJS","rdfs:comment":"Somoni"},{"@id":"unece:CurrencyCodeList#TMT","@type":"unece:CurrencyCodeList","rdf:value":"TMT","rdfs:comment":"Turkmenistan New Manat"},{"@id":"unece:CurrencyCodeList#TND","@type":"unece:CurrencyCodeList","rdf:value":"TND","rdfs:comment":"Tunisian Dinar"},{"@id":"unece:CurrencyCodeList#TOP","@type":"unece:CurrencyCodeList","rdf:value":"TOP","rdfs:comment":"Pa'anga"},{"@id":"unece:CurrencyCodeList#TRY","@type":"unece:CurrencyCodeList","rdf:value":"TRY","rdfs:comment":"Turkish Lira"},{"@id":"unece:CurrencyCodeList#TTD","@type":"unece:CurrencyCodeList","rdf:value":"TTD","rdfs:comment":"Trinidad and Tobago Dollar"},{"@id":"unece:CurrencyCodeList#TWD","@type":"unece:CurrencyCodeList","rdf:value":"TWD","rdfs:comment":"New Taiwan Dollar"},{"@id":"unece:CurrencyCodeList#TZS","@type":"unece:CurrencyCodeList","rdf:value":"TZS","rdfs:comment":"Tanzanian Shilling"},{"@id":"unece:CurrencyCodeList#UAH","@type":"unece:CurrencyCodeList","rdf:value":"UAH","rdfs:comment":"Hryvnia"},{"@id":"unece:CurrencyCodeList#UGX","@type":"unece:CurrencyCodeList","rdf:value":"UGX","rdfs:comment":"Uganda Shilling"},{"@id":"unece:CurrencyCodeList#USD","@type":"unece:CurrencyCodeList","rdf:value":"USD","rdfs:comment":"US Dollar"},{"@id":"unece:CurrencyCodeList#USN","@type":"unece:CurrencyCodeList","rdf:value":"USN","rdfs:comment":"US Dollar (Next day)"},{"@id":"unece:CurrencyCodeList#UYI","@type":"unece:CurrencyCodeList","rdf:value":"UYI","rdfs:comment":"Uruguayo Peso en Unidades"},{"@id":"unece:CurrencyCodeList#UYU","@type":"unece:CurrencyCodeList","rdf:value":"UYU","rdfs:comment":"Peso Uruguayo"},{"@id":"unece:CurrencyCodeList#UYW","@type":"unece:CurrencyCodeList","rdf:value":"UYW","rdfs:comment":"Unidad Previsional"},{"@id":"unece:CurrencyCodeList#UZS","@type":"unece:CurrencyCodeList","rdf:value":"UZS","rdfs:comment":"Uzbekistan Sum"},{"@id":"unece:CurrencyCodeList#VED","@type":"unece:CurrencyCodeList","rdf:value":"VED","rdfs:comment":"Bolvar Soberano"},{"@id":"unece:CurrencyCodeList#VES","@type":"unece:CurrencyCodeList","rdf:value":"VES","rdfs:comment":"Bolvar Soberano"},{"@id":"unece:CurrencyCodeList#VND","@type":"unece:CurrencyCodeList","rdf:value":"VND","rdfs:comment":"Dong"},{"@id":"unece:CurrencyCodeList#VUV","@type":"unece:CurrencyCodeList","rdf:value":"VUV","rdfs:comment":"Vatu"},{"@id":"unece:CurrencyCodeList#WST","@type":"unece:CurrencyCodeList","rdf:value":"WST","rdfs:comment":"Tala"},{"@id":"unece:CurrencyCodeList#XAF","@type":"unece:CurrencyCodeList","rdf:value":"XAF","rdfs:comment":"CFA Franc"},{"@id":"unece:CurrencyCodeList#XAG","@type":"unece:CurrencyCodeList","rdf:value":"XAG","rdfs:comment":"Silver"},{"@id":"unece:CurrencyCodeList#XAU","@type":"unece:CurrencyCodeList","rdf:value":"XAU","rdfs:comment":"Gold"},{"@id":"unece:CurrencyCodeList#XBA","@type":"unece:CurrencyCodeList","rdf:value":"XBA","rdfs:comment":"Bond Markets Units European Composite Unit (EURCO)"},{"@id":"unece:CurrencyCodeList#XBB","@type":"unece:CurrencyCodeList","rdf:value":"XBB","rdfs:comment":"European Monetary Unit (E.M.U.-6)"},{"@id":"unece:CurrencyCodeList#XBC","@type":"unece:CurrencyCodeList","rdf:value":"XBC","rdfs:comment":"European Unit of Account 9 (E.U.A.-9)"},{"@id":"unece:CurrencyCodeList#XBD","@type":"unece:CurrencyCodeList","rdf:value":"XBD","rdfs:comment":"European Unit of Account 17 (E.U.A.-17)"},{"@id":"unece:CurrencyCodeList#XCD","@type":"unece:CurrencyCodeList","rdf:value":"XCD","rdfs:comment":"East Carribean Dollar"},{"@id":"unece:CurrencyCodeList#XDR","@type":"unece:CurrencyCodeList","rdf:value":"XDR","rdfs:comment":"SDR"},{"@id":"unece:CurrencyCodeList#XOF","@type":"unece:CurrencyCodeList","rdf:value":"XOF","rdfs:comment":"CFA Franc"},{"@id":"unece:CurrencyCodeList#XPD","@type":"unece:CurrencyCodeList","rdf:value":"XPD","rdfs:comment":"Palladium"},{"@id":"unece:CurrencyCodeList#XPF","@type":"unece:CurrencyCodeList","rdf:value":"XPF","rdfs:comment":"CFP Franc"},{"@id":"unece:CurrencyCodeList#XPT","@type":"unece:CurrencyCodeList","rdf:value":"XPT","rdfs:comment":"Platinum"},{"@id":"unece:CurrencyCodeList#XSU","@type":"unece:CurrencyCodeList","rdf:value":"XSU","rdfs:comment":"Sucre"},{"@id":"unece:CurrencyCodeList#XTS","@type":"unece:CurrencyCodeList","rdf:value":"XTS","rdfs:comment":"Codes specifically reserved for testing purposes"},{"@id":"unece:CurrencyCodeList#XUA","@type":"unece:CurrencyCodeList","rdf:value":"XUA","rdfs:comment":"ADB Unit of Account"},{"@id":"unece:CurrencyCodeList#XXX","@type":"unece:CurrencyCodeList","rdf:value":"XXX","rdfs:comment":"The codes assigned for transactions where no currency is involved"},{"@id":"unece:CurrencyCodeList#YER","@type":"unece:CurrencyCodeList","rdf:value":"YER","rdfs:comment":"Yemeni Rial"},{"@id":"unece:CurrencyCodeList#ZAR","@type":"unece:CurrencyCodeList","rdf:value":"ZAR","rdfs:comment":"Rand"},{"@id":"unece:CurrencyCodeList#ZMW","@type":"unece:CurrencyCodeList","rdf:value":"ZMW","rdfs:comment":"Zambian Kwacha"},{"@id":"unece:CurrencyCodeList#ZWL","@type":"unece:CurrencyCodeList","rdf:value":"ZWL","rdfs:comment":"Zimbabwe Dollar"},{"rdfs:label":"CustomsDutyRegimeTypeCodeList","@type":"rdfs:Class","@id":"unece:CustomsDutyRegimeTypeCodeList","rdfs:comment":"A character string used to represent the type of customs duty regime."},{"@id":"unece:CustomsDutyRegimeTypeCodeList#1","@type":"unece:CustomsDutyRegimeTypeCodeList","rdf:value":"1","rdfs:comment":"Origin subject to EC/EFTA preference"},{"@id":"unece:CustomsDutyRegimeTypeCodeList#2","@type":"unece:CustomsDutyRegimeTypeCodeList","rdf:value":"2","rdfs:comment":"Origin subject to other preference agreement"},{"@id":"unece:CustomsDutyRegimeTypeCodeList#3","@type":"unece:CustomsDutyRegimeTypeCodeList","rdf:value":"3","rdfs:comment":"No preference origin"},{"@id":"unece:CustomsDutyRegimeTypeCodeList#8","@type":"unece:CustomsDutyRegimeTypeCodeList","rdf:value":"8","rdfs:comment":"Excluded origin"},{"@id":"unece:CustomsDutyRegimeTypeCodeList#9","@type":"unece:CustomsDutyRegimeTypeCodeList","rdf:value":"9","rdfs:comment":"Imposed origin"},{"rdfs:label":"CustomsProcedureGuaranteeCodeList","@type":"rdfs:Class","@id":"unece:CustomsProcedureGuaranteeCodeList","rdfs:comment":"A character string used to represent a customs procedure guarantee."},{"@id":"unece:CustomsProcedureGuaranteeCodeList#ZZZ","@type":"unece:CustomsProcedureGuaranteeCodeList","rdf:value":"ZZZ","rdfs:comment":"Mutually defined"},{"rdfs:label":"FinancialAdjustmentReasonCodeList","@type":"rdfs:Class","@id":"unece:FinancialAdjustmentReasonCodeList","rdfs:comment":"A character string used to represent a financial adjustment reason."},{"@id":"unece:FinancialAdjustmentReasonCodeList#1","@type":"unece:FinancialAdjustmentReasonCodeList","rdf:value":"1","rdfs:comment":"Agreed settlement"},{"@id":"unece:FinancialAdjustmentReasonCodeList#5","@type":"unece:FinancialAdjustmentReasonCodeList","rdf:value":"5","rdfs:comment":"Price query"},{"@id":"unece:FinancialAdjustmentReasonCodeList#7","@type":"unece:FinancialAdjustmentReasonCodeList","rdf:value":"7","rdfs:comment":"Payment on account"},{"@id":"unece:FinancialAdjustmentReasonCodeList#8","@type":"unece:FinancialAdjustmentReasonCodeList","rdf:value":"8","rdfs:comment":"Returnable container charge included"},{"@id":"unece:FinancialAdjustmentReasonCodeList#9","@type":"unece:FinancialAdjustmentReasonCodeList","rdf:value":"9","rdfs:comment":"Invoice error"},{"@id":"unece:FinancialAdjustmentReasonCodeList#10","@type":"unece:FinancialAdjustmentReasonCodeList","rdf:value":"10","rdfs:comment":"Costs for draft"},{"@id":"unece:FinancialAdjustmentReasonCodeList#11","@type":"unece:FinancialAdjustmentReasonCodeList","rdf:value":"11","rdfs:comment":"Bank charges"},{"@id":"unece:FinancialAdjustmentReasonCodeList#12","@type":"unece:FinancialAdjustmentReasonCodeList","rdf:value":"12","rdfs:comment":"Agent commission"},{"@id":"unece:FinancialAdjustmentReasonCodeList#13","@type":"unece:FinancialAdjustmentReasonCodeList","rdf:value":"13","rdfs:comment":"Counter claim"},{"@id":"unece:FinancialAdjustmentReasonCodeList#19","@type":"unece:FinancialAdjustmentReasonCodeList","rdf:value":"19","rdfs:comment":"Trade discount"},{"@id":"unece:FinancialAdjustmentReasonCodeList#20","@type":"unece:FinancialAdjustmentReasonCodeList","rdf:value":"20","rdfs:comment":"Deduction for late delivery"},{"@id":"unece:FinancialAdjustmentReasonCodeList#21","@type":"unece:FinancialAdjustmentReasonCodeList","rdf:value":"21","rdfs:comment":"Advertising costs"},{"@id":"unece:FinancialAdjustmentReasonCodeList#22","@type":"unece:FinancialAdjustmentReasonCodeList","rdf:value":"22","rdfs:comment":"Customs duties"},{"@id":"unece:FinancialAdjustmentReasonCodeList#23","@type":"unece:FinancialAdjustmentReasonCodeList","rdf:value":"23","rdfs:comment":"Telephone and postal costs"},{"@id":"unece:FinancialAdjustmentReasonCodeList#24","@type":"unece:FinancialAdjustmentReasonCodeList","rdf:value":"24","rdfs:comment":"Repair costs"},{"@id":"unece:FinancialAdjustmentReasonCodeList#25","@type":"unece:FinancialAdjustmentReasonCodeList","rdf:value":"25","rdfs:comment":"Attorney fees"},{"@id":"unece:FinancialAdjustmentReasonCodeList#26","@type":"unece:FinancialAdjustmentReasonCodeList","rdf:value":"26","rdfs:comment":"Taxes"},{"@id":"unece:FinancialAdjustmentReasonCodeList#27","@type":"unece:FinancialAdjustmentReasonCodeList","rdf:value":"27","rdfs:comment":"Reclaimed deduction"},{"@id":"unece:FinancialAdjustmentReasonCodeList#30","@type":"unece:FinancialAdjustmentReasonCodeList","rdf:value":"30","rdfs:comment":"Direct payment to seller"},{"@id":"unece:FinancialAdjustmentReasonCodeList#34","@type":"unece:FinancialAdjustmentReasonCodeList","rdf:value":"34","rdfs:comment":"Quoted as paid to you"},{"@id":"unece:FinancialAdjustmentReasonCodeList#36","@type":"unece:FinancialAdjustmentReasonCodeList","rdf:value":"36","rdfs:comment":"Invoice not received"},{"@id":"unece:FinancialAdjustmentReasonCodeList#37","@type":"unece:FinancialAdjustmentReasonCodeList","rdf:value":"37","rdfs:comment":"Credit note to debtor/not to us"},{"@id":"unece:FinancialAdjustmentReasonCodeList#38","@type":"unece:FinancialAdjustmentReasonCodeList","rdf:value":"38","rdfs:comment":"Deducted bonus"},{"@id":"unece:FinancialAdjustmentReasonCodeList#39","@type":"unece:FinancialAdjustmentReasonCodeList","rdf:value":"39","rdfs:comment":"Deducted discount"},{"@id":"unece:FinancialAdjustmentReasonCodeList#40","@type":"unece:FinancialAdjustmentReasonCodeList","rdf:value":"40","rdfs:comment":"Deducted freight costs"},{"@id":"unece:FinancialAdjustmentReasonCodeList#41","@type":"unece:FinancialAdjustmentReasonCodeList","rdf:value":"41","rdfs:comment":"Deduction against other invoices"},{"@id":"unece:FinancialAdjustmentReasonCodeList#42","@type":"unece:FinancialAdjustmentReasonCodeList","rdf:value":"42","rdfs:comment":"Credit balance(s)"},{"@id":"unece:FinancialAdjustmentReasonCodeList#43","@type":"unece:FinancialAdjustmentReasonCodeList","rdf:value":"43","rdfs:comment":"Reason unknown"},{"@id":"unece:FinancialAdjustmentReasonCodeList#44","@type":"unece:FinancialAdjustmentReasonCodeList","rdf:value":"44","rdfs:comment":"Awaiting message from seller"},{"@id":"unece:FinancialAdjustmentReasonCodeList#45","@type":"unece:FinancialAdjustmentReasonCodeList","rdf:value":"45","rdfs:comment":"Debit note to seller"},{"@id":"unece:FinancialAdjustmentReasonCodeList#46","@type":"unece:FinancialAdjustmentReasonCodeList","rdf:value":"46","rdfs:comment":"Discount beyond terms"},{"@id":"unece:FinancialAdjustmentReasonCodeList#47","@type":"unece:FinancialAdjustmentReasonCodeList","rdf:value":"47","rdfs:comment":"See buyer's letter"},{"@id":"unece:FinancialAdjustmentReasonCodeList#48","@type":"unece:FinancialAdjustmentReasonCodeList","rdf:value":"48","rdfs:comment":"Allowance/charge error"},{"@id":"unece:FinancialAdjustmentReasonCodeList#50","@type":"unece:FinancialAdjustmentReasonCodeList","rdf:value":"50","rdfs:comment":"Terms of sale error"},{"@id":"unece:FinancialAdjustmentReasonCodeList#52","@type":"unece:FinancialAdjustmentReasonCodeList","rdf:value":"52","rdfs:comment":"Wrong invoice"},{"@id":"unece:FinancialAdjustmentReasonCodeList#53","@type":"unece:FinancialAdjustmentReasonCodeList","rdf:value":"53","rdfs:comment":"Duplicate invoice"},{"@id":"unece:FinancialAdjustmentReasonCodeList#54","@type":"unece:FinancialAdjustmentReasonCodeList","rdf:value":"54","rdfs:comment":"Weight error"},{"@id":"unece:FinancialAdjustmentReasonCodeList#55","@type":"unece:FinancialAdjustmentReasonCodeList","rdf:value":"55","rdfs:comment":"Additional charge not authorized"},{"@id":"unece:FinancialAdjustmentReasonCodeList#56","@type":"unece:FinancialAdjustmentReasonCodeList","rdf:value":"56","rdfs:comment":"Incorrect discount"},{"@id":"unece:FinancialAdjustmentReasonCodeList#57","@type":"unece:FinancialAdjustmentReasonCodeList","rdf:value":"57","rdfs:comment":"Price change"},{"@id":"unece:FinancialAdjustmentReasonCodeList#58","@type":"unece:FinancialAdjustmentReasonCodeList","rdf:value":"58","rdfs:comment":"Variation"},{"@id":"unece:FinancialAdjustmentReasonCodeList#59","@type":"unece:FinancialAdjustmentReasonCodeList","rdf:value":"59","rdfs:comment":"Chargeback"},{"@id":"unece:FinancialAdjustmentReasonCodeList#60","@type":"unece:FinancialAdjustmentReasonCodeList","rdf:value":"60","rdfs:comment":"Offset"},{"@id":"unece:FinancialAdjustmentReasonCodeList#61","@type":"unece:FinancialAdjustmentReasonCodeList","rdf:value":"61","rdfs:comment":"Indirect payment"},{"@id":"unece:FinancialAdjustmentReasonCodeList#62","@type":"unece:FinancialAdjustmentReasonCodeList","rdf:value":"62","rdfs:comment":"Financial reassignment"},{"@id":"unece:FinancialAdjustmentReasonCodeList#63","@type":"unece:FinancialAdjustmentReasonCodeList","rdf:value":"63","rdfs:comment":"Reinstatement of chargeback/offset"},{"@id":"unece:FinancialAdjustmentReasonCodeList#64","@type":"unece:FinancialAdjustmentReasonCodeList","rdf:value":"64","rdfs:comment":"Expecting new terms"},{"@id":"unece:FinancialAdjustmentReasonCodeList#65","@type":"unece:FinancialAdjustmentReasonCodeList","rdf:value":"65","rdfs:comment":"Settlement to agent"},{"@id":"unece:FinancialAdjustmentReasonCodeList#66","@type":"unece:FinancialAdjustmentReasonCodeList","rdf:value":"66","rdfs:comment":"Cash discount"},{"@id":"unece:FinancialAdjustmentReasonCodeList#67","@type":"unece:FinancialAdjustmentReasonCodeList","rdf:value":"67","rdfs:comment":"Delcredere costs"},{"@id":"unece:FinancialAdjustmentReasonCodeList#68","@type":"unece:FinancialAdjustmentReasonCodeList","rdf:value":"68","rdfs:comment":"Early payment allowance adjustment"},{"@id":"unece:FinancialAdjustmentReasonCodeList#69","@type":"unece:FinancialAdjustmentReasonCodeList","rdf:value":"69","rdfs:comment":"Incorrect due date for monetary amount"},{"@id":"unece:FinancialAdjustmentReasonCodeList#70","@type":"unece:FinancialAdjustmentReasonCodeList","rdf:value":"70","rdfs:comment":"Wrong monetary amount resulting from incorrect free goods quantity"},{"@id":"unece:FinancialAdjustmentReasonCodeList#73","@type":"unece:FinancialAdjustmentReasonCodeList","rdf:value":"73","rdfs:comment":"Difference in tax rate"},{"@id":"unece:FinancialAdjustmentReasonCodeList#74","@type":"unece:FinancialAdjustmentReasonCodeList","rdf:value":"74","rdfs:comment":"Quantity discount"},{"@id":"unece:FinancialAdjustmentReasonCodeList#75","@type":"unece:FinancialAdjustmentReasonCodeList","rdf:value":"75","rdfs:comment":"Promotion discount"},{"@id":"unece:FinancialAdjustmentReasonCodeList#77","@type":"unece:FinancialAdjustmentReasonCodeList","rdf:value":"77","rdfs:comment":"Pricing discount"},{"@id":"unece:FinancialAdjustmentReasonCodeList#78","@type":"unece:FinancialAdjustmentReasonCodeList","rdf:value":"78","rdfs:comment":"Volume discount"},{"@id":"unece:FinancialAdjustmentReasonCodeList#79","@type":"unece:FinancialAdjustmentReasonCodeList","rdf:value":"79","rdfs:comment":"Sundry discount"},{"@id":"unece:FinancialAdjustmentReasonCodeList#80","@type":"unece:FinancialAdjustmentReasonCodeList","rdf:value":"80","rdfs:comment":"Card holder signature missing"},{"@id":"unece:FinancialAdjustmentReasonCodeList#81","@type":"unece:FinancialAdjustmentReasonCodeList","rdf:value":"81","rdfs:comment":"Card expiry date missing"},{"@id":"unece:FinancialAdjustmentReasonCodeList#82","@type":"unece:FinancialAdjustmentReasonCodeList","rdf:value":"82","rdfs:comment":"Card number error"},{"@id":"unece:FinancialAdjustmentReasonCodeList#83","@type":"unece:FinancialAdjustmentReasonCodeList","rdf:value":"83","rdfs:comment":"Card expired"},{"@id":"unece:FinancialAdjustmentReasonCodeList#84","@type":"unece:FinancialAdjustmentReasonCodeList","rdf:value":"84","rdfs:comment":"Test card transaction"},{"@id":"unece:FinancialAdjustmentReasonCodeList#85","@type":"unece:FinancialAdjustmentReasonCodeList","rdf:value":"85","rdfs:comment":"Permission limit exceeded"},{"@id":"unece:FinancialAdjustmentReasonCodeList#86","@type":"unece:FinancialAdjustmentReasonCodeList","rdf:value":"86","rdfs:comment":"Wrong authorisation code"},{"@id":"unece:FinancialAdjustmentReasonCodeList#87","@type":"unece:FinancialAdjustmentReasonCodeList","rdf:value":"87","rdfs:comment":"Wrong authorised amount"},{"@id":"unece:FinancialAdjustmentReasonCodeList#88","@type":"unece:FinancialAdjustmentReasonCodeList","rdf:value":"88","rdfs:comment":"Authorisation failed"},{"@id":"unece:FinancialAdjustmentReasonCodeList#89","@type":"unece:FinancialAdjustmentReasonCodeList","rdf:value":"89","rdfs:comment":"Card acceptor data error"},{"@id":"unece:FinancialAdjustmentReasonCodeList#90","@type":"unece:FinancialAdjustmentReasonCodeList","rdf:value":"90","rdfs:comment":"Treasury management service charge"},{"@id":"unece:FinancialAdjustmentReasonCodeList#91","@type":"unece:FinancialAdjustmentReasonCodeList","rdf:value":"91","rdfs:comment":"Agreed discount"},{"@id":"unece:FinancialAdjustmentReasonCodeList#92","@type":"unece:FinancialAdjustmentReasonCodeList","rdf:value":"92","rdfs:comment":"Expediting fee"},{"@id":"unece:FinancialAdjustmentReasonCodeList#93","@type":"unece:FinancialAdjustmentReasonCodeList","rdf:value":"93","rdfs:comment":"Invoicing fee"},{"@id":"unece:FinancialAdjustmentReasonCodeList#94","@type":"unece:FinancialAdjustmentReasonCodeList","rdf:value":"94","rdfs:comment":"Freight charge"},{"@id":"unece:FinancialAdjustmentReasonCodeList#95","@type":"unece:FinancialAdjustmentReasonCodeList","rdf:value":"95","rdfs:comment":"Small order processing service charge"},{"@id":"unece:FinancialAdjustmentReasonCodeList#96","@type":"unece:FinancialAdjustmentReasonCodeList","rdf:value":"96","rdfs:comment":"Currency exchange differences"},{"@id":"unece:FinancialAdjustmentReasonCodeList#97","@type":"unece:FinancialAdjustmentReasonCodeList","rdf:value":"97","rdfs:comment":"Insolvency"},{"@id":"unece:FinancialAdjustmentReasonCodeList#98","@type":"unece:FinancialAdjustmentReasonCodeList","rdf:value":"98","rdfs:comment":"Incorrect references"},{"@id":"unece:FinancialAdjustmentReasonCodeList#99","@type":"unece:FinancialAdjustmentReasonCodeList","rdf:value":"99","rdfs:comment":"Incorrect identification of the buyer"},{"@id":"unece:FinancialAdjustmentReasonCodeList#100","@type":"unece:FinancialAdjustmentReasonCodeList","rdf:value":"100","rdfs:comment":"Incorrect product identification"},{"@id":"unece:FinancialAdjustmentReasonCodeList#ZZZ","@type":"unece:FinancialAdjustmentReasonCodeList","rdf:value":"ZZZ","rdfs:comment":"Mutually defined"},{"rdfs:label":"FinancingStatusCodeList","@type":"rdfs:Class","@id":"unece:FinancingStatusCodeList","rdfs:comment":""},{"rdfs:label":"FinancingStatusReasonCodeList","@type":"rdfs:Class","@id":"unece:FinancingStatusReasonCodeList","rdfs:comment":""},{"rdfs:label":"PartyTypeCodeList","@type":"rdfs:Class","@id":"unece:PartyTypeCodeList","rdfs:comment":"A character string used to represent the type of a party."},{"@id":"unece:PartyTypeCodeList#BRA","@type":"unece:PartyTypeCodeList","rdf:value":"BRA","rdfs:comment":"Branch"},{"@id":"unece:PartyTypeCodeList#DEP","@type":"unece:PartyTypeCodeList","rdf:value":"DEP","rdfs:comment":"Department"},{"@id":"unece:PartyTypeCodeList#DIR","@type":"unece:PartyTypeCodeList","rdf:value":"DIR","rdfs:comment":"Direction"},{"@id":"unece:PartyTypeCodeList#SEC","@type":"unece:PartyTypeCodeList","rdf:value":"SEC","rdfs:comment":"Section"},{"@id":"unece:PartyTypeCodeList#SER","@type":"unece:PartyTypeCodeList","rdf:value":"SER","rdfs:comment":"Service"},{"rdfs:label":"PaymentGuaranteeMeansCodeList","@type":"rdfs:Class","@id":"unece:PaymentGuaranteeMeansCodeList","rdfs:comment":"A character string used to represent a payment guarantee means."},{"@id":"unece:PaymentGuaranteeMeansCodeList#1","@type":"unece:PaymentGuaranteeMeansCodeList","rdf:value":"1","rdfs:comment":"Factor guarantee"},{"@id":"unece:PaymentGuaranteeMeansCodeList#10","@type":"unece:PaymentGuaranteeMeansCodeList","rdf:value":"10","rdfs:comment":"Bank guarantee"},{"@id":"unece:PaymentGuaranteeMeansCodeList#11","@type":"unece:PaymentGuaranteeMeansCodeList","rdf:value":"11","rdfs:comment":"Public authority guarantee"},{"@id":"unece:PaymentGuaranteeMeansCodeList#12","@type":"unece:PaymentGuaranteeMeansCodeList","rdf:value":"12","rdfs:comment":"Third party guarantee"},{"@id":"unece:PaymentGuaranteeMeansCodeList#13","@type":"unece:PaymentGuaranteeMeansCodeList","rdf:value":"13","rdfs:comment":"Standby letter of credit"},{"@id":"unece:PaymentGuaranteeMeansCodeList#14","@type":"unece:PaymentGuaranteeMeansCodeList","rdf:value":"14","rdfs:comment":"No guarantee"},{"@id":"unece:PaymentGuaranteeMeansCodeList#20","@type":"unece:PaymentGuaranteeMeansCodeList","rdf:value":"20","rdfs:comment":"Goods as security"},{"@id":"unece:PaymentGuaranteeMeansCodeList#21","@type":"unece:PaymentGuaranteeMeansCodeList","rdf:value":"21","rdfs:comment":"Business as security"},{"@id":"unece:PaymentGuaranteeMeansCodeList#23","@type":"unece:PaymentGuaranteeMeansCodeList","rdf:value":"23","rdfs:comment":"Warrant or similar (warehouse receipts)"},{"@id":"unece:PaymentGuaranteeMeansCodeList#24","@type":"unece:PaymentGuaranteeMeansCodeList","rdf:value":"24","rdfs:comment":"Mortgage"},{"@id":"unece:PaymentGuaranteeMeansCodeList#45","@type":"unece:PaymentGuaranteeMeansCodeList","rdf:value":"45","rdfs:comment":"Insurance certificate"},{"@id":"unece:PaymentGuaranteeMeansCodeList#ZZZ","@type":"unece:PaymentGuaranteeMeansCodeList","rdf:value":"ZZZ","rdfs:comment":"Mutually defined"},{"rdfs:label":"PaymentMeansChannelCodeList","@type":"rdfs:Class","@id":"unece:PaymentMeansChannelCodeList","rdfs:comment":"A character string used to represent the payment means channel."},{"@id":"unece:PaymentMeansChannelCodeList#1","@type":"unece:PaymentMeansChannelCodeList","rdf:value":"1","rdfs:comment":"Ordinary post"},{"@id":"unece:PaymentMeansChannelCodeList#2","@type":"unece:PaymentMeansChannelCodeList","rdf:value":"2","rdfs:comment":"Air mail"},{"@id":"unece:PaymentMeansChannelCodeList#3","@type":"unece:PaymentMeansChannelCodeList","rdf:value":"3","rdfs:comment":"Telegraph"},{"@id":"unece:PaymentMeansChannelCodeList#4","@type":"unece:PaymentMeansChannelCodeList","rdf:value":"4","rdfs:comment":"Telex"},{"@id":"unece:PaymentMeansChannelCodeList#5","@type":"unece:PaymentMeansChannelCodeList","rdf:value":"5","rdfs:comment":"S.W.I.F.T."},{"@id":"unece:PaymentMeansChannelCodeList#6","@type":"unece:PaymentMeansChannelCodeList","rdf:value":"6","rdfs:comment":"Other transmission networks"},{"@id":"unece:PaymentMeansChannelCodeList#7","@type":"unece:PaymentMeansChannelCodeList","rdf:value":"7","rdfs:comment":"Networks not defined"},{"@id":"unece:PaymentMeansChannelCodeList#8","@type":"unece:PaymentMeansChannelCodeList","rdf:value":"8","rdfs:comment":"Fedwire"},{"@id":"unece:PaymentMeansChannelCodeList#9","@type":"unece:PaymentMeansChannelCodeList","rdf:value":"9","rdfs:comment":"Personal (face-to-face)"},{"@id":"unece:PaymentMeansChannelCodeList#10","@type":"unece:PaymentMeansChannelCodeList","rdf:value":"10","rdfs:comment":"Registered air mail"},{"@id":"unece:PaymentMeansChannelCodeList#11","@type":"unece:PaymentMeansChannelCodeList","rdf:value":"11","rdfs:comment":"Registered mail"},{"@id":"unece:PaymentMeansChannelCodeList#12","@type":"unece:PaymentMeansChannelCodeList","rdf:value":"12","rdfs:comment":"Courier"},{"@id":"unece:PaymentMeansChannelCodeList#13","@type":"unece:PaymentMeansChannelCodeList","rdf:value":"13","rdfs:comment":"Messenger"},{"@id":"unece:PaymentMeansChannelCodeList#14","@type":"unece:PaymentMeansChannelCodeList","rdf:value":"14","rdfs:comment":"National ACH"},{"@id":"unece:PaymentMeansChannelCodeList#15","@type":"unece:PaymentMeansChannelCodeList","rdf:value":"15","rdfs:comment":"Other ACH"},{"@id":"unece:PaymentMeansChannelCodeList#ZZZ","@type":"unece:PaymentMeansChannelCodeList","rdf:value":"ZZZ","rdfs:comment":"Mutually defined"},{"rdfs:label":"PaymentMeansCodeList","@type":"rdfs:Class","@id":"unece:PaymentMeansCodeList","rdfs:comment":"A character string used to represent a payment means."},{"@id":"unece:PaymentMeansCodeList#1","@type":"unece:PaymentMeansCodeList","rdf:value":"1","rdfs:comment":"Instrument not defined"},{"@id":"unece:PaymentMeansCodeList#2","@type":"unece:PaymentMeansCodeList","rdf:value":"2","rdfs:comment":"Automated clearing house credit"},{"@id":"unece:PaymentMeansCodeList#3","@type":"unece:PaymentMeansCodeList","rdf:value":"3","rdfs:comment":"Automated clearing house debit"},{"@id":"unece:PaymentMeansCodeList#4","@type":"unece:PaymentMeansCodeList","rdf:value":"4","rdfs:comment":"ACH demand debit reversal"},{"@id":"unece:PaymentMeansCodeList#5","@type":"unece:PaymentMeansCodeList","rdf:value":"5","rdfs:comment":"ACH demand credit reversal"},{"@id":"unece:PaymentMeansCodeList#6","@type":"unece:PaymentMeansCodeList","rdf:value":"6","rdfs:comment":"ACH demand credit"},{"@id":"unece:PaymentMeansCodeList#7","@type":"unece:PaymentMeansCodeList","rdf:value":"7","rdfs:comment":"ACH demand debit"},{"@id":"unece:PaymentMeansCodeList#8","@type":"unece:PaymentMeansCodeList","rdf:value":"8","rdfs:comment":"Hold"},{"@id":"unece:PaymentMeansCodeList#9","@type":"unece:PaymentMeansCodeList","rdf:value":"9","rdfs:comment":"National or regional clearing"},{"@id":"unece:PaymentMeansCodeList#10","@type":"unece:PaymentMeansCodeList","rdf:value":"10","rdfs:comment":"In cash"},{"@id":"unece:PaymentMeansCodeList#11","@type":"unece:PaymentMeansCodeList","rdf:value":"11","rdfs:comment":"ACH savings credit reversal"},{"@id":"unece:PaymentMeansCodeList#12","@type":"unece:PaymentMeansCodeList","rdf:value":"12","rdfs:comment":"ACH savings debit reversal"},{"@id":"unece:PaymentMeansCodeList#13","@type":"unece:PaymentMeansCodeList","rdf:value":"13","rdfs:comment":"ACH savings credit"},{"@id":"unece:PaymentMeansCodeList#14","@type":"unece:PaymentMeansCodeList","rdf:value":"14","rdfs:comment":"ACH savings debit"},{"@id":"unece:PaymentMeansCodeList#15","@type":"unece:PaymentMeansCodeList","rdf:value":"15","rdfs:comment":"Bookentry credit"},{"@id":"unece:PaymentMeansCodeList#16","@type":"unece:PaymentMeansCodeList","rdf:value":"16","rdfs:comment":"Bookentry debit"},{"@id":"unece:PaymentMeansCodeList#17","@type":"unece:PaymentMeansCodeList","rdf:value":"17","rdfs:comment":"ACH demand cash concentration/disbursement (CCD) credit"},{"@id":"unece:PaymentMeansCodeList#18","@type":"unece:PaymentMeansCodeList","rdf:value":"18","rdfs:comment":"ACH demand cash concentration/disbursement (CCD) debit"},{"@id":"unece:PaymentMeansCodeList#19","@type":"unece:PaymentMeansCodeList","rdf:value":"19","rdfs:comment":"ACH demand corporate trade payment (CTP) credit"},{"@id":"unece:PaymentMeansCodeList#20","@type":"unece:PaymentMeansCodeList","rdf:value":"20","rdfs:comment":"Cheque"},{"@id":"unece:PaymentMeansCodeList#21","@type":"unece:PaymentMeansCodeList","rdf:value":"21","rdfs:comment":"Banker's draft"},{"@id":"unece:PaymentMeansCodeList#22","@type":"unece:PaymentMeansCodeList","rdf:value":"22","rdfs:comment":"Certified banker's draft"},{"@id":"unece:PaymentMeansCodeList#23","@type":"unece:PaymentMeansCodeList","rdf:value":"23","rdfs:comment":"Bank cheque (issued by a banking or similar establishment)"},{"@id":"unece:PaymentMeansCodeList#24","@type":"unece:PaymentMeansCodeList","rdf:value":"24","rdfs:comment":"Bill of exchange awaiting acceptance"},{"@id":"unece:PaymentMeansCodeList#25","@type":"unece:PaymentMeansCodeList","rdf:value":"25","rdfs:comment":"Certified cheque"},{"@id":"unece:PaymentMeansCodeList#26","@type":"unece:PaymentMeansCodeList","rdf:value":"26","rdfs:comment":"Local cheque"},{"@id":"unece:PaymentMeansCodeList#27","@type":"unece:PaymentMeansCodeList","rdf:value":"27","rdfs:comment":"ACH demand corporate trade payment (CTP) debit"},{"@id":"unece:PaymentMeansCodeList#28","@type":"unece:PaymentMeansCodeList","rdf:value":"28","rdfs:comment":"ACH demand corporate trade exchange (CTX) credit"},{"@id":"unece:PaymentMeansCodeList#29","@type":"unece:PaymentMeansCodeList","rdf:value":"29","rdfs:comment":"ACH demand corporate trade exchange (CTX) debit"},{"@id":"unece:PaymentMeansCodeList#30","@type":"unece:PaymentMeansCodeList","rdf:value":"30","rdfs:comment":"Credit transfer"},{"@id":"unece:PaymentMeansCodeList#31","@type":"unece:PaymentMeansCodeList","rdf:value":"31","rdfs:comment":"Debit transfer"},{"@id":"unece:PaymentMeansCodeList#32","@type":"unece:PaymentMeansCodeList","rdf:value":"32","rdfs:comment":"ACH demand cash concentration/disbursement plus (CCD+) credit"},{"@id":"unece:PaymentMeansCodeList#33","@type":"unece:PaymentMeansCodeList","rdf:value":"33","rdfs:comment":"ACH demand cash concentration/disbursement plus (CCD+) debit"},{"@id":"unece:PaymentMeansCodeList#34","@type":"unece:PaymentMeansCodeList","rdf:value":"34","rdfs:comment":"ACH prearranged payment and deposit (PPD)"},{"@id":"unece:PaymentMeansCodeList#35","@type":"unece:PaymentMeansCodeList","rdf:value":"35","rdfs:comment":"ACH savings cash concentration/disbursement (CCD) credit"},{"@id":"unece:PaymentMeansCodeList#36","@type":"unece:PaymentMeansCodeList","rdf:value":"36","rdfs:comment":"ACH savings cash concentration/disbursement (CCD) debit"},{"@id":"unece:PaymentMeansCodeList#37","@type":"unece:PaymentMeansCodeList","rdf:value":"37","rdfs:comment":"ACH savings corporate trade payment (CTP) credit"},{"@id":"unece:PaymentMeansCodeList#38","@type":"unece:PaymentMeansCodeList","rdf:value":"38","rdfs:comment":"ACH savings corporate trade payment (CTP) debit"},{"@id":"unece:PaymentMeansCodeList#39","@type":"unece:PaymentMeansCodeList","rdf:value":"39","rdfs:comment":"ACH savings corporate trade exchange (CTX) credit"},{"@id":"unece:PaymentMeansCodeList#40","@type":"unece:PaymentMeansCodeList","rdf:value":"40","rdfs:comment":"ACH savings corporate trade exchange (CTX) debit"},{"@id":"unece:PaymentMeansCodeList#41","@type":"unece:PaymentMeansCodeList","rdf:value":"41","rdfs:comment":"ACH savings cash concentration/disbursement plus (CCD+) credit"},{"@id":"unece:PaymentMeansCodeList#42","@type":"unece:PaymentMeansCodeList","rdf:value":"42","rdfs:comment":"Payment to bank account"},{"@id":"unece:PaymentMeansCodeList#43","@type":"unece:PaymentMeansCodeList","rdf:value":"43","rdfs:comment":"ACH savings cash concentration/disbursement plus (CCD+) debit"},{"@id":"unece:PaymentMeansCodeList#44","@type":"unece:PaymentMeansCodeList","rdf:value":"44","rdfs:comment":"Accepted bill of exchange"},{"@id":"unece:PaymentMeansCodeList#45","@type":"unece:PaymentMeansCodeList","rdf:value":"45","rdfs:comment":"Referenced home-banking credit transfer"},{"@id":"unece:PaymentMeansCodeList#46","@type":"unece:PaymentMeansCodeList","rdf:value":"46","rdfs:comment":"Interbank debit transfer"},{"@id":"unece:PaymentMeansCodeList#47","@type":"unece:PaymentMeansCodeList","rdf:value":"47","rdfs:comment":"Home-banking debit transfer"},{"@id":"unece:PaymentMeansCodeList#48","@type":"unece:PaymentMeansCodeList","rdf:value":"48","rdfs:comment":"Bank card"},{"@id":"unece:PaymentMeansCodeList#49","@type":"unece:PaymentMeansCodeList","rdf:value":"49","rdfs:comment":"Direct debit"},{"@id":"unece:PaymentMeansCodeList#50","@type":"unece:PaymentMeansCodeList","rdf:value":"50","rdfs:comment":"Payment by postgiro"},{"@id":"unece:PaymentMeansCodeList#51","@type":"unece:PaymentMeansCodeList","rdf:value":"51","rdfs:comment":"FR, norme 6 97-Telereglement CFONB (French Organisation for Banking Standards)  - Option A"},{"@id":"unece:PaymentMeansCodeList#52","@type":"unece:PaymentMeansCodeList","rdf:value":"52","rdfs:comment":"Urgent commercial payment"},{"@id":"unece:PaymentMeansCodeList#53","@type":"unece:PaymentMeansCodeList","rdf:value":"53","rdfs:comment":"Urgent Treasury Payment"},{"@id":"unece:PaymentMeansCodeList#54","@type":"unece:PaymentMeansCodeList","rdf:value":"54","rdfs:comment":"Credit card"},{"@id":"unece:PaymentMeansCodeList#55","@type":"unece:PaymentMeansCodeList","rdf:value":"55","rdfs:comment":"Debit card"},{"@id":"unece:PaymentMeansCodeList#56","@type":"unece:PaymentMeansCodeList","rdf:value":"56","rdfs:comment":"Bankgiro"},{"@id":"unece:PaymentMeansCodeList#57","@type":"unece:PaymentMeansCodeList","rdf:value":"57","rdfs:comment":"Standing agreement"},{"@id":"unece:PaymentMeansCodeList#58","@type":"unece:PaymentMeansCodeList","rdf:value":"58","rdfs:comment":"SEPA credit transfer"},{"@id":"unece:PaymentMeansCodeList#59","@type":"unece:PaymentMeansCodeList","rdf:value":"59","rdfs:comment":"SEPA direct debit"},{"@id":"unece:PaymentMeansCodeList#60","@type":"unece:PaymentMeansCodeList","rdf:value":"60","rdfs:comment":"Promissory note"},{"@id":"unece:PaymentMeansCodeList#61","@type":"unece:PaymentMeansCodeList","rdf:value":"61","rdfs:comment":"Promissory note signed by the debtor"},{"@id":"unece:PaymentMeansCodeList#62","@type":"unece:PaymentMeansCodeList","rdf:value":"62","rdfs:comment":"Promissory note signed by the debtor and endorsed by a bank"},{"@id":"unece:PaymentMeansCodeList#63","@type":"unece:PaymentMeansCodeList","rdf:value":"63","rdfs:comment":"Promissory note signed by the debtor and endorsed by a third party"},{"@id":"unece:PaymentMeansCodeList#64","@type":"unece:PaymentMeansCodeList","rdf:value":"64","rdfs:comment":"Promissory note signed by a bank"},{"@id":"unece:PaymentMeansCodeList#65","@type":"unece:PaymentMeansCodeList","rdf:value":"65","rdfs:comment":"Promissory note signed by a bank and endorsed by another bank"},{"@id":"unece:PaymentMeansCodeList#66","@type":"unece:PaymentMeansCodeList","rdf:value":"66","rdfs:comment":"Promissory note signed by a third party"},{"@id":"unece:PaymentMeansCodeList#67","@type":"unece:PaymentMeansCodeList","rdf:value":"67","rdfs:comment":"Promissory note signed by a third party and endorsed by a bank"},{"@id":"unece:PaymentMeansCodeList#68","@type":"unece:PaymentMeansCodeList","rdf:value":"68","rdfs:comment":"Online payment service"},{"@id":"unece:PaymentMeansCodeList#69","@type":"unece:PaymentMeansCodeList","rdf:value":"69","rdfs:comment":"Transfer Advice"},{"@id":"unece:PaymentMeansCodeList#70","@type":"unece:PaymentMeansCodeList","rdf:value":"70","rdfs:comment":"Bill drawn by the creditor on the debtor"},{"@id":"unece:PaymentMeansCodeList#74","@type":"unece:PaymentMeansCodeList","rdf:value":"74","rdfs:comment":"Bill drawn by the creditor on a bank"},{"@id":"unece:PaymentMeansCodeList#75","@type":"unece:PaymentMeansCodeList","rdf:value":"75","rdfs:comment":"Bill drawn by the creditor, endorsed by another bank"},{"@id":"unece:PaymentMeansCodeList#76","@type":"unece:PaymentMeansCodeList","rdf:value":"76","rdfs:comment":"Bill drawn by the creditor on a bank and endorsed by a third party"},{"@id":"unece:PaymentMeansCodeList#77","@type":"unece:PaymentMeansCodeList","rdf:value":"77","rdfs:comment":"Bill drawn by the creditor on a third party"},{"@id":"unece:PaymentMeansCodeList#78","@type":"unece:PaymentMeansCodeList","rdf:value":"78","rdfs:comment":"Bill drawn by creditor on third party, accepted and endorsed by bank"},{"@id":"unece:PaymentMeansCodeList#91","@type":"unece:PaymentMeansCodeList","rdf:value":"91","rdfs:comment":"Not transferable banker's draft"},{"@id":"unece:PaymentMeansCodeList#92","@type":"unece:PaymentMeansCodeList","rdf:value":"92","rdfs:comment":"Not transferable local cheque"},{"@id":"unece:PaymentMeansCodeList#93","@type":"unece:PaymentMeansCodeList","rdf:value":"93","rdfs:comment":"Reference giro"},{"@id":"unece:PaymentMeansCodeList#94","@type":"unece:PaymentMeansCodeList","rdf:value":"94","rdfs:comment":"Urgent giro"},{"@id":"unece:PaymentMeansCodeList#95","@type":"unece:PaymentMeansCodeList","rdf:value":"95","rdfs:comment":"Free format giro"},{"@id":"unece:PaymentMeansCodeList#96","@type":"unece:PaymentMeansCodeList","rdf:value":"96","rdfs:comment":"Requested method for payment was not used"},{"@id":"unece:PaymentMeansCodeList#97","@type":"unece:PaymentMeansCodeList","rdf:value":"97","rdfs:comment":"Clearing between partners"},{"@id":"unece:PaymentMeansCodeList#ZZZ","@type":"unece:PaymentMeansCodeList","rdf:value":"ZZZ","rdfs:comment":"Mutually defined"},{"rdfs:label":"PaymentMethodCodeList","@type":"rdfs:Class","@id":"unece:PaymentMethodCodeList","rdfs:comment":"A character string used to represent a payment method."},{"@id":"unece:PaymentMethodCodeList#1","@type":"unece:PaymentMethodCodeList","rdf:value":"1","rdfs:comment":"Direct payment"},{"@id":"unece:PaymentMethodCodeList#2","@type":"unece:PaymentMethodCodeList","rdf:value":"2","rdfs:comment":"Automatic clearing house credit"},{"@id":"unece:PaymentMethodCodeList#3","@type":"unece:PaymentMethodCodeList","rdf:value":"3","rdfs:comment":"Automatic clearing house debit"},{"@id":"unece:PaymentMethodCodeList#4","@type":"unece:PaymentMethodCodeList","rdf:value":"4","rdfs:comment":"Automatic clearing house credit-savings account"},{"@id":"unece:PaymentMethodCodeList#5","@type":"unece:PaymentMethodCodeList","rdf:value":"5","rdfs:comment":"Automatic clearing house debit-demand account"},{"@id":"unece:PaymentMethodCodeList#6","@type":"unece:PaymentMethodCodeList","rdf:value":"6","rdfs:comment":"Bank book transfer (credit)"},{"@id":"unece:PaymentMethodCodeList#7","@type":"unece:PaymentMethodCodeList","rdf:value":"7","rdfs:comment":"Bank book transfer (debit)"},{"@id":"unece:PaymentMethodCodeList#8","@type":"unece:PaymentMethodCodeList","rdf:value":"8","rdfs:comment":"Doc collection via 3rd party with bill of EX"},{"@id":"unece:PaymentMethodCodeList#9","@type":"unece:PaymentMethodCodeList","rdf:value":"9","rdfs:comment":"Doc collection via 3rd party no bill of EX"},{"@id":"unece:PaymentMethodCodeList#10","@type":"unece:PaymentMethodCodeList","rdf:value":"10","rdfs:comment":"Irrevocable documentary credit"},{"@id":"unece:PaymentMethodCodeList#11","@type":"unece:PaymentMethodCodeList","rdf:value":"11","rdfs:comment":"Transferable irrevocable documentary credit"},{"@id":"unece:PaymentMethodCodeList#12","@type":"unece:PaymentMethodCodeList","rdf:value":"12","rdfs:comment":"Confirmed irrevocable documentary credit"},{"@id":"unece:PaymentMethodCodeList#13","@type":"unece:PaymentMethodCodeList","rdf:value":"13","rdfs:comment":"Transferable confirmed irrevocable documentary credit"},{"@id":"unece:PaymentMethodCodeList#14","@type":"unece:PaymentMethodCodeList","rdf:value":"14","rdfs:comment":"Revocable documentary credit"},{"@id":"unece:PaymentMethodCodeList#15","@type":"unece:PaymentMethodCodeList","rdf:value":"15","rdfs:comment":"Irrevocable letter of credit-confirmed"},{"@id":"unece:PaymentMethodCodeList#16","@type":"unece:PaymentMethodCodeList","rdf:value":"16","rdfs:comment":"Letter of guarantee"},{"@id":"unece:PaymentMethodCodeList#17","@type":"unece:PaymentMethodCodeList","rdf:value":"17","rdfs:comment":"Revocable letter of credit"},{"@id":"unece:PaymentMethodCodeList#18","@type":"unece:PaymentMethodCodeList","rdf:value":"18","rdfs:comment":"Standby letter of credit"},{"@id":"unece:PaymentMethodCodeList#19","@type":"unece:PaymentMethodCodeList","rdf:value":"19","rdfs:comment":"Irrevocable letter of credit unconfirmed"},{"@id":"unece:PaymentMethodCodeList#20","@type":"unece:PaymentMethodCodeList","rdf:value":"20","rdfs:comment":"Clean collection (ICC)"},{"@id":"unece:PaymentMethodCodeList#21","@type":"unece:PaymentMethodCodeList","rdf:value":"21","rdfs:comment":"Documentary collection (ICC)"},{"@id":"unece:PaymentMethodCodeList#22","@type":"unece:PaymentMethodCodeList","rdf:value":"22","rdfs:comment":"Documentary sight collection (ICC)"},{"@id":"unece:PaymentMethodCodeList#23","@type":"unece:PaymentMethodCodeList","rdf:value":"23","rdfs:comment":"Documentary collection with date of expiry (ICC)"},{"@id":"unece:PaymentMethodCodeList#24","@type":"unece:PaymentMethodCodeList","rdf:value":"24","rdfs:comment":"Documentary collection: bill of exchange against acceptance"},{"@id":"unece:PaymentMethodCodeList#25","@type":"unece:PaymentMethodCodeList","rdf:value":"25","rdfs:comment":"Documentary collection: bill of exchange against payment"},{"@id":"unece:PaymentMethodCodeList#26","@type":"unece:PaymentMethodCodeList","rdf:value":"26","rdfs:comment":"Collection subject to buyer's approval (ICC)"},{"@id":"unece:PaymentMethodCodeList#27","@type":"unece:PaymentMethodCodeList","rdf:value":"27","rdfs:comment":"Collection by a bank consignee for the goods (ICC)"},{"@id":"unece:PaymentMethodCodeList#34","@type":"unece:PaymentMethodCodeList","rdf:value":"34","rdfs:comment":"Seller to advise buyer"},{"@id":"unece:PaymentMethodCodeList#35","@type":"unece:PaymentMethodCodeList","rdf:value":"35","rdfs:comment":"Documents through banks"},{"@id":"unece:PaymentMethodCodeList#36","@type":"unece:PaymentMethodCodeList","rdf:value":"36","rdfs:comment":"Charging (to account)"},{"@id":"unece:PaymentMethodCodeList#37","@type":"unece:PaymentMethodCodeList","rdf:value":"37","rdfs:comment":"Available with issuing bank"},{"@id":"unece:PaymentMethodCodeList#38","@type":"unece:PaymentMethodCodeList","rdf:value":"38","rdfs:comment":"Available with advising bank"},{"@id":"unece:PaymentMethodCodeList#39","@type":"unece:PaymentMethodCodeList","rdf:value":"39","rdfs:comment":"Available with named bank"},{"@id":"unece:PaymentMethodCodeList#40","@type":"unece:PaymentMethodCodeList","rdf:value":"40","rdfs:comment":"Available with any bank"},{"@id":"unece:PaymentMethodCodeList#41","@type":"unece:PaymentMethodCodeList","rdf:value":"41","rdfs:comment":"Available with any bank in ..."},{"@id":"unece:PaymentMethodCodeList#42","@type":"unece:PaymentMethodCodeList","rdf:value":"42","rdfs:comment":"Indirect payment"},{"@id":"unece:PaymentMethodCodeList#43","@type":"unece:PaymentMethodCodeList","rdf:value":"43","rdfs:comment":"Reassignment"},{"@id":"unece:PaymentMethodCodeList#44","@type":"unece:PaymentMethodCodeList","rdf:value":"44","rdfs:comment":"Offset"},{"@id":"unece:PaymentMethodCodeList#45","@type":"unece:PaymentMethodCodeList","rdf:value":"45","rdfs:comment":"Special entries"},{"@id":"unece:PaymentMethodCodeList#46","@type":"unece:PaymentMethodCodeList","rdf:value":"46","rdfs:comment":"Instalment payment"},{"@id":"unece:PaymentMethodCodeList#47","@type":"unece:PaymentMethodCodeList","rdf:value":"47","rdfs:comment":"Instalment payment with draft"},{"@id":"unece:PaymentMethodCodeList#48","@type":"unece:PaymentMethodCodeList","rdf:value":"48","rdfs:comment":"Available with advise through bank"},{"@id":"unece:PaymentMethodCodeList#49","@type":"unece:PaymentMethodCodeList","rdf:value":"49","rdfs:comment":"General conditions of sale"},{"@id":"unece:PaymentMethodCodeList#50","@type":"unece:PaymentMethodCodeList","rdf:value":"50","rdfs:comment":"Special payment"},{"@id":"unece:PaymentMethodCodeList#61","@type":"unece:PaymentMethodCodeList","rdf:value":"61","rdfs:comment":"Set-off by exchange of documents"},{"@id":"unece:PaymentMethodCodeList#62","@type":"unece:PaymentMethodCodeList","rdf:value":"62","rdfs:comment":"Set-off by reciprocal credits"},{"@id":"unece:PaymentMethodCodeList#64","@type":"unece:PaymentMethodCodeList","rdf:value":"64","rdfs:comment":"Set-off by exchange of goods"},{"@id":"unece:PaymentMethodCodeList#65","@type":"unece:PaymentMethodCodeList","rdf:value":"65","rdfs:comment":"Reverse factoring"},{"@id":"unece:PaymentMethodCodeList#69","@type":"unece:PaymentMethodCodeList","rdf:value":"69","rdfs:comment":"Other set-off"},{"@id":"unece:PaymentMethodCodeList#70","@type":"unece:PaymentMethodCodeList","rdf:value":"70","rdfs:comment":"Supplier to invoice"},{"@id":"unece:PaymentMethodCodeList#71","@type":"unece:PaymentMethodCodeList","rdf:value":"71","rdfs:comment":"Recipient to self bill"},{"@id":"unece:PaymentMethodCodeList#ZZZ","@type":"unece:PaymentMethodCodeList","rdf:value":"ZZZ","rdfs:comment":"Mutually defined"},{"rdfs:label":"PaymentTermsEventTimeReferenceCodeList","@type":"rdfs:Class","@id":"unece:PaymentTermsEventTimeReferenceCodeList","rdfs:comment":"A character string used to represent a time reference for a payment terms event."},{"@id":"unece:PaymentTermsEventTimeReferenceCodeList#5","@type":"unece:PaymentTermsEventTimeReferenceCodeList","rdf:value":"5","rdfs:comment":"Date of invoice"},{"@id":"unece:PaymentTermsEventTimeReferenceCodeList#24","@type":"unece:PaymentTermsEventTimeReferenceCodeList","rdf:value":"24","rdfs:comment":"Date ex-works"},{"@id":"unece:PaymentTermsEventTimeReferenceCodeList#29","@type":"unece:PaymentTermsEventTimeReferenceCodeList","rdf:value":"29","rdfs:comment":"Date of delivery of goods to establishments/domicile/site"},{"@id":"unece:PaymentTermsEventTimeReferenceCodeList#45","@type":"unece:PaymentTermsEventTimeReferenceCodeList","rdf:value":"45","rdfs:comment":"Date of bill of lading, consignment note or other transport document"},{"@id":"unece:PaymentTermsEventTimeReferenceCodeList#71","@type":"unece:PaymentTermsEventTimeReferenceCodeList","rdf:value":"71","rdfs:comment":"Date of presentation of documents"},{"rdfs:label":"PaymentTermsId","@type":"rdfs:Class","@id":"unece:PaymentTermsId","rdfs:comment":"A character string used to represent a payment terms."},{"@id":"unece:PaymentTermsId#1","@type":"unece:PaymentTermsId","rdf:value":"1","rdfs:comment":"Draft(s) drawn on issuing bank"},{"@id":"unece:PaymentTermsId#2","@type":"unece:PaymentTermsId","rdf:value":"2","rdfs:comment":"Draft(s) drawn on advising bank"},{"@id":"unece:PaymentTermsId#3","@type":"unece:PaymentTermsId","rdf:value":"3","rdfs:comment":"Draft(s) drawn on reimbursing bank"},{"@id":"unece:PaymentTermsId#4","@type":"unece:PaymentTermsId","rdf:value":"4","rdfs:comment":"Draft(s) drawn on applicant"},{"@id":"unece:PaymentTermsId#5","@type":"unece:PaymentTermsId","rdf:value":"5","rdfs:comment":"Draft(s) drawn on any other drawee"},{"@id":"unece:PaymentTermsId#6","@type":"unece:PaymentTermsId","rdf:value":"6","rdfs:comment":"No drafts"},{"@id":"unece:PaymentTermsId#7","@type":"unece:PaymentTermsId","rdf:value":"7","rdfs:comment":"Payment means specified in commercial account summary"},{"rdfs:label":"PaymentTermsTypeCodeList","@type":"rdfs:Class","@id":"unece:PaymentTermsTypeCodeList","rdfs:comment":"A character string used to represent the payment terms type."},{"@id":"unece:PaymentTermsTypeCodeList#1","@type":"unece:PaymentTermsTypeCodeList","rdf:value":"1","rdfs:comment":"Basic"},{"@id":"unece:PaymentTermsTypeCodeList#2","@type":"unece:PaymentTermsTypeCodeList","rdf:value":"2","rdfs:comment":"End of month"},{"@id":"unece:PaymentTermsTypeCodeList#3","@type":"unece:PaymentTermsTypeCodeList","rdf:value":"3","rdfs:comment":"Fixed date"},{"@id":"unece:PaymentTermsTypeCodeList#4","@type":"unece:PaymentTermsTypeCodeList","rdf:value":"4","rdfs:comment":"Deferred"},{"@id":"unece:PaymentTermsTypeCodeList#5","@type":"unece:PaymentTermsTypeCodeList","rdf:value":"5","rdfs:comment":"Discount not applicable"},{"@id":"unece:PaymentTermsTypeCodeList#6","@type":"unece:PaymentTermsTypeCodeList","rdf:value":"6","rdfs:comment":"Mixed"},{"@id":"unece:PaymentTermsTypeCodeList#7","@type":"unece:PaymentTermsTypeCodeList","rdf:value":"7","rdfs:comment":"Extended"},{"@id":"unece:PaymentTermsTypeCodeList#8","@type":"unece:PaymentTermsTypeCodeList","rdf:value":"8","rdfs:comment":"Basic discount offered"},{"@id":"unece:PaymentTermsTypeCodeList#9","@type":"unece:PaymentTermsTypeCodeList","rdf:value":"9","rdfs:comment":"Proximo"},{"@id":"unece:PaymentTermsTypeCodeList#10","@type":"unece:PaymentTermsTypeCodeList","rdf:value":"10","rdfs:comment":"Instant"},{"@id":"unece:PaymentTermsTypeCodeList#11","@type":"unece:PaymentTermsTypeCodeList","rdf:value":"11","rdfs:comment":"Elective"},{"@id":"unece:PaymentTermsTypeCodeList#12","@type":"unece:PaymentTermsTypeCodeList","rdf:value":"12","rdfs:comment":"10 days after end of month"},{"@id":"unece:PaymentTermsTypeCodeList#13","@type":"unece:PaymentTermsTypeCodeList","rdf:value":"13","rdfs:comment":"Seller to advise buyer"},{"@id":"unece:PaymentTermsTypeCodeList#14","@type":"unece:PaymentTermsTypeCodeList","rdf:value":"14","rdfs:comment":"Paid against statement"},{"@id":"unece:PaymentTermsTypeCodeList#15","@type":"unece:PaymentTermsTypeCodeList","rdf:value":"15","rdfs:comment":"No charge"},{"@id":"unece:PaymentTermsTypeCodeList#16","@type":"unece:PaymentTermsTypeCodeList","rdf:value":"16","rdfs:comment":"Not yet defined"},{"@id":"unece:PaymentTermsTypeCodeList#17","@type":"unece:PaymentTermsTypeCodeList","rdf:value":"17","rdfs:comment":"Ultimo"},{"@id":"unece:PaymentTermsTypeCodeList#18","@type":"unece:PaymentTermsTypeCodeList","rdf:value":"18","rdfs:comment":"Previously agreed upon"},{"@id":"unece:PaymentTermsTypeCodeList#19","@type":"unece:PaymentTermsTypeCodeList","rdf:value":"19","rdfs:comment":"United States funds"},{"@id":"unece:PaymentTermsTypeCodeList#20","@type":"unece:PaymentTermsTypeCodeList","rdf:value":"20","rdfs:comment":"Penalty terms"},{"@id":"unece:PaymentTermsTypeCodeList#21","@type":"unece:PaymentTermsTypeCodeList","rdf:value":"21","rdfs:comment":"Payment by instalment"},{"@id":"unece:PaymentTermsTypeCodeList#22","@type":"unece:PaymentTermsTypeCodeList","rdf:value":"22","rdfs:comment":"Discount"},{"@id":"unece:PaymentTermsTypeCodeList#23","@type":"unece:PaymentTermsTypeCodeList","rdf:value":"23","rdfs:comment":"Available by sight payment"},{"@id":"unece:PaymentTermsTypeCodeList#24","@type":"unece:PaymentTermsTypeCodeList","rdf:value":"24","rdfs:comment":"Available by deferred payment"},{"@id":"unece:PaymentTermsTypeCodeList#25","@type":"unece:PaymentTermsTypeCodeList","rdf:value":"25","rdfs:comment":"Available by acceptance"},{"@id":"unece:PaymentTermsTypeCodeList#26","@type":"unece:PaymentTermsTypeCodeList","rdf:value":"26","rdfs:comment":"Available by negotiation with any bank"},{"@id":"unece:PaymentTermsTypeCodeList#27","@type":"unece:PaymentTermsTypeCodeList","rdf:value":"27","rdfs:comment":"Available by negotiation with any bank in ..."},{"@id":"unece:PaymentTermsTypeCodeList#28","@type":"unece:PaymentTermsTypeCodeList","rdf:value":"28","rdfs:comment":"Available by negotiation by named bank"},{"@id":"unece:PaymentTermsTypeCodeList#29","@type":"unece:PaymentTermsTypeCodeList","rdf:value":"29","rdfs:comment":"Available by negotiation"},{"@id":"unece:PaymentTermsTypeCodeList#30","@type":"unece:PaymentTermsTypeCodeList","rdf:value":"30","rdfs:comment":"Adjustment payment"},{"@id":"unece:PaymentTermsTypeCodeList#31","@type":"unece:PaymentTermsTypeCodeList","rdf:value":"31","rdfs:comment":"Late payment"},{"@id":"unece:PaymentTermsTypeCodeList#32","@type":"unece:PaymentTermsTypeCodeList","rdf:value":"32","rdfs:comment":"Advanced payment"},{"@id":"unece:PaymentTermsTypeCodeList#33","@type":"unece:PaymentTermsTypeCodeList","rdf:value":"33","rdfs:comment":"Payment by instalments according to progress (as agreed)"},{"@id":"unece:PaymentTermsTypeCodeList#34","@type":"unece:PaymentTermsTypeCodeList","rdf:value":"34","rdfs:comment":"Payment by instalments according to progress (to be agreed)"},{"@id":"unece:PaymentTermsTypeCodeList#35","@type":"unece:PaymentTermsTypeCodeList","rdf:value":"35","rdfs:comment":"Nonstandard"},{"@id":"unece:PaymentTermsTypeCodeList#36","@type":"unece:PaymentTermsTypeCodeList","rdf:value":"36","rdfs:comment":"Tenor payment terms"},{"@id":"unece:PaymentTermsTypeCodeList#37","@type":"unece:PaymentTermsTypeCodeList","rdf:value":"37","rdfs:comment":"Complete payment"},{"@id":"unece:PaymentTermsTypeCodeList#38","@type":"unece:PaymentTermsTypeCodeList","rdf:value":"38","rdfs:comment":"Payment terms defined in consolidated invoice"},{"@id":"unece:PaymentTermsTypeCodeList#39","@type":"unece:PaymentTermsTypeCodeList","rdf:value":"39","rdfs:comment":"Payment upon completion"},{"@id":"unece:PaymentTermsTypeCodeList#40","@type":"unece:PaymentTermsTypeCodeList","rdf:value":"40","rdfs:comment":"Partial advance"},{"@id":"unece:PaymentTermsTypeCodeList#41","@type":"unece:PaymentTermsTypeCodeList","rdf:value":"41","rdfs:comment":"Consignment"},{"@id":"unece:PaymentTermsTypeCodeList#42","@type":"unece:PaymentTermsTypeCodeList","rdf:value":"42","rdfs:comment":"Inter-company account"},{"@id":"unece:PaymentTermsTypeCodeList#43","@type":"unece:PaymentTermsTypeCodeList","rdf:value":"43","rdfs:comment":"Sell by note"},{"@id":"unece:PaymentTermsTypeCodeList#44","@type":"unece:PaymentTermsTypeCodeList","rdf:value":"44","rdfs:comment":"Supplier floor plan"},{"@id":"unece:PaymentTermsTypeCodeList#45","@type":"unece:PaymentTermsTypeCodeList","rdf:value":"45","rdfs:comment":"Contract basis"},{"@id":"unece:PaymentTermsTypeCodeList#46","@type":"unece:PaymentTermsTypeCodeList","rdf:value":"46","rdfs:comment":"Credit controlled"},{"@id":"unece:PaymentTermsTypeCodeList#47","@type":"unece:PaymentTermsTypeCodeList","rdf:value":"47","rdfs:comment":"Dating given"},{"@id":"unece:PaymentTermsTypeCodeList#48","@type":"unece:PaymentTermsTypeCodeList","rdf:value":"48","rdfs:comment":"Trade acceptance"},{"@id":"unece:PaymentTermsTypeCodeList#49","@type":"unece:PaymentTermsTypeCodeList","rdf:value":"49","rdfs:comment":"Cost plus"},{"@id":"unece:PaymentTermsTypeCodeList#50","@type":"unece:PaymentTermsTypeCodeList","rdf:value":"50","rdfs:comment":"Letter of credit"},{"@id":"unece:PaymentTermsTypeCodeList#51","@type":"unece:PaymentTermsTypeCodeList","rdf:value":"51","rdfs:comment":"Lease agreement"},{"@id":"unece:PaymentTermsTypeCodeList#52","@type":"unece:PaymentTermsTypeCodeList","rdf:value":"52","rdfs:comment":"Cash On Delivery (COD)"},{"@id":"unece:PaymentTermsTypeCodeList#53","@type":"unece:PaymentTermsTypeCodeList","rdf:value":"53","rdfs:comment":"Cash by state law"},{"@id":"unece:PaymentTermsTypeCodeList#54","@type":"unece:PaymentTermsTypeCodeList","rdf:value":"54","rdfs:comment":"Bank transfer"},{"@id":"unece:PaymentTermsTypeCodeList#55","@type":"unece:PaymentTermsTypeCodeList","rdf:value":"55","rdfs:comment":"Cash on arrival"},{"@id":"unece:PaymentTermsTypeCodeList#56","@type":"unece:PaymentTermsTypeCodeList","rdf:value":"56","rdfs:comment":"Cash"},{"@id":"unece:PaymentTermsTypeCodeList#57","@type":"unece:PaymentTermsTypeCodeList","rdf:value":"57","rdfs:comment":"Cash discount terms apply"},{"@id":"unece:PaymentTermsTypeCodeList#58","@type":"unece:PaymentTermsTypeCodeList","rdf:value":"58","rdfs:comment":"Cash with order"},{"@id":"unece:PaymentTermsTypeCodeList#59","@type":"unece:PaymentTermsTypeCodeList","rdf:value":"59","rdfs:comment":"Cash per vendor request"},{"@id":"unece:PaymentTermsTypeCodeList#60","@type":"unece:PaymentTermsTypeCodeList","rdf:value":"60","rdfs:comment":"Irrevocable letter of credit"},{"@id":"unece:PaymentTermsTypeCodeList#61","@type":"unece:PaymentTermsTypeCodeList","rdf:value":"61","rdfs:comment":"Documents against acceptance"},{"@id":"unece:PaymentTermsTypeCodeList#62","@type":"unece:PaymentTermsTypeCodeList","rdf:value":"62","rdfs:comment":"Charge card"},{"@id":"unece:PaymentTermsTypeCodeList#63","@type":"unece:PaymentTermsTypeCodeList","rdf:value":"63","rdfs:comment":"Documents against payment"},{"@id":"unece:PaymentTermsTypeCodeList#64","@type":"unece:PaymentTermsTypeCodeList","rdf:value":"64","rdfs:comment":"Usance bill"},{"@id":"unece:PaymentTermsTypeCodeList#65","@type":"unece:PaymentTermsTypeCodeList","rdf:value":"65","rdfs:comment":"Letter of credit at sight"},{"@id":"unece:PaymentTermsTypeCodeList#66","@type":"unece:PaymentTermsTypeCodeList","rdf:value":"66","rdfs:comment":"Secured account"},{"@id":"unece:PaymentTermsTypeCodeList#67","@type":"unece:PaymentTermsTypeCodeList","rdf:value":"67","rdfs:comment":"Basic commission terms"},{"@id":"unece:PaymentTermsTypeCodeList#68","@type":"unece:PaymentTermsTypeCodeList","rdf:value":"68","rdfs:comment":"Deposit required"},{"@id":"unece:PaymentTermsTypeCodeList#69","@type":"unece:PaymentTermsTypeCodeList","rdf:value":"69","rdfs:comment":"Discount with prompt pay"},{"@id":"unece:PaymentTermsTypeCodeList#70","@type":"unece:PaymentTermsTypeCodeList","rdf:value":"70","rdfs:comment":"Discount with advance payment"},{"@id":"unece:PaymentTermsTypeCodeList#71","@type":"unece:PaymentTermsTypeCodeList","rdf:value":"71","rdfs:comment":"Certified cheque"},{"@id":"unece:PaymentTermsTypeCodeList#72","@type":"unece:PaymentTermsTypeCodeList","rdf:value":"72","rdfs:comment":"Cash against documents"},{"@id":"unece:PaymentTermsTypeCodeList#73","@type":"unece:PaymentTermsTypeCodeList","rdf:value":"73","rdfs:comment":"Bill of exchange"},{"@id":"unece:PaymentTermsTypeCodeList#74","@type":"unece:PaymentTermsTypeCodeList","rdf:value":"74","rdfs:comment":"Progressive discount"},{"@id":"unece:PaymentTermsTypeCodeList#75","@type":"unece:PaymentTermsTypeCodeList","rdf:value":"75","rdfs:comment":"Lump sum"},{"@id":"unece:PaymentTermsTypeCodeList#76","@type":"unece:PaymentTermsTypeCodeList","rdf:value":"76","rdfs:comment":"Fixed fee"},{"@id":"unece:PaymentTermsTypeCodeList#77","@type":"unece:PaymentTermsTypeCodeList","rdf:value":"77","rdfs:comment":"Promissory note"},{"@id":"unece:PaymentTermsTypeCodeList#78","@type":"unece:PaymentTermsTypeCodeList","rdf:value":"78","rdfs:comment":"Factoring"},{"@id":"unece:PaymentTermsTypeCodeList#ZZZ","@type":"unece:PaymentTermsTypeCodeList","rdf:value":"ZZZ","rdfs:comment":"Mutually defined"},{"rdfs:label":"PriceTypeCodeList","@type":"rdfs:Class","@id":"unece:PriceTypeCodeList","rdfs:comment":"A character string used to represent or replace a type of price."},{"@id":"unece:PriceTypeCodeList#AA","@type":"unece:PriceTypeCodeList","rdf:value":"AA","rdfs:comment":"Cancellation price"},{"@id":"unece:PriceTypeCodeList#AB","@type":"unece:PriceTypeCodeList","rdf:value":"AB","rdfs:comment":"Per ton"},{"@id":"unece:PriceTypeCodeList#AC","@type":"unece:PriceTypeCodeList","rdf:value":"AC","rdfs:comment":"Minimum order price"},{"@id":"unece:PriceTypeCodeList#AD","@type":"unece:PriceTypeCodeList","rdf:value":"AD","rdfs:comment":"Export price"},{"@id":"unece:PriceTypeCodeList#AE","@type":"unece:PriceTypeCodeList","rdf:value":"AE","rdfs:comment":"Range dependent price"},{"@id":"unece:PriceTypeCodeList#AF","@type":"unece:PriceTypeCodeList","rdf:value":"AF","rdfs:comment":"Competitor price"},{"@id":"unece:PriceTypeCodeList#AI","@type":"unece:PriceTypeCodeList","rdf:value":"AI","rdfs:comment":"Active ingredient"},{"@id":"unece:PriceTypeCodeList#AQ","@type":"unece:PriceTypeCodeList","rdf:value":"AQ","rdfs:comment":"As is quantity"},{"@id":"unece:PriceTypeCodeList#CA","@type":"unece:PriceTypeCodeList","rdf:value":"CA","rdfs:comment":"Catalogue"},{"@id":"unece:PriceTypeCodeList#CT","@type":"unece:PriceTypeCodeList","rdf:value":"CT","rdfs:comment":"Contract"},{"@id":"unece:PriceTypeCodeList#CU","@type":"unece:PriceTypeCodeList","rdf:value":"CU","rdfs:comment":"Consumer unit"},{"@id":"unece:PriceTypeCodeList#DI","@type":"unece:PriceTypeCodeList","rdf:value":"DI","rdfs:comment":"Distributor"},{"@id":"unece:PriceTypeCodeList#EC","@type":"unece:PriceTypeCodeList","rdf:value":"EC","rdfs:comment":"ECSC price"},{"@id":"unece:PriceTypeCodeList#NW","@type":"unece:PriceTypeCodeList","rdf:value":"NW","rdfs:comment":"Net weight"},{"@id":"unece:PriceTypeCodeList#PC","@type":"unece:PriceTypeCodeList","rdf:value":"PC","rdfs:comment":"Price catalogue"},{"@id":"unece:PriceTypeCodeList#PE","@type":"unece:PriceTypeCodeList","rdf:value":"PE","rdfs:comment":"Per each"},{"@id":"unece:PriceTypeCodeList#PK","@type":"unece:PriceTypeCodeList","rdf:value":"PK","rdfs:comment":"Per kilogram"},{"@id":"unece:PriceTypeCodeList#PL","@type":"unece:PriceTypeCodeList","rdf:value":"PL","rdfs:comment":"Per litre"},{"@id":"unece:PriceTypeCodeList#PT","@type":"unece:PriceTypeCodeList","rdf:value":"PT","rdfs:comment":"Per tonne"},{"@id":"unece:PriceTypeCodeList#PU","@type":"unece:PriceTypeCodeList","rdf:value":"PU","rdfs:comment":"Specified unit"},{"@id":"unece:PriceTypeCodeList#PV","@type":"unece:PriceTypeCodeList","rdf:value":"PV","rdfs:comment":"Provisional price"},{"@id":"unece:PriceTypeCodeList#PW","@type":"unece:PriceTypeCodeList","rdf:value":"PW","rdfs:comment":"Gross weight"},{"@id":"unece:PriceTypeCodeList#QT","@type":"unece:PriceTypeCodeList","rdf:value":"QT","rdfs:comment":"Quoted"},{"@id":"unece:PriceTypeCodeList#SR","@type":"unece:PriceTypeCodeList","rdf:value":"SR","rdfs:comment":"Suggested retail"},{"@id":"unece:PriceTypeCodeList#TB","@type":"unece:PriceTypeCodeList","rdf:value":"TB","rdfs:comment":"To be negotiated"},{"@id":"unece:PriceTypeCodeList#TU","@type":"unece:PriceTypeCodeList","rdf:value":"TU","rdfs:comment":"Traded unit"},{"@id":"unece:PriceTypeCodeList#TW","@type":"unece:PriceTypeCodeList","rdf:value":"TW","rdfs:comment":"Theoretical weight"},{"@id":"unece:PriceTypeCodeList#WH","@type":"unece:PriceTypeCodeList","rdf:value":"WH","rdfs:comment":"Wholesale"},{"@id":"unece:PriceTypeCodeList#WI","@type":"unece:PriceTypeCodeList","rdf:value":"WI","rdfs:comment":"Gross volume"},{"rdfs:label":"TaxCategoryCodeList","@type":"rdfs:Class","@id":"unece:TaxCategoryCodeList","rdfs:comment":"A character string used to represent a duty or tax category."},{"@id":"unece:TaxCategoryCodeList#A","@type":"unece:TaxCategoryCodeList","rdf:value":"A","rdfs:comment":"Mixed tax rate"},{"@id":"unece:TaxCategoryCodeList#AA","@type":"unece:TaxCategoryCodeList","rdf:value":"AA","rdfs:comment":"Lower rate"},{"@id":"unece:TaxCategoryCodeList#AB","@type":"unece:TaxCategoryCodeList","rdf:value":"AB","rdfs:comment":"Exempt for resale"},{"@id":"unece:TaxCategoryCodeList#AC","@type":"unece:TaxCategoryCodeList","rdf:value":"AC","rdfs:comment":"Value Added Tax (VAT) not now due for payment"},{"@id":"unece:TaxCategoryCodeList#AD","@type":"unece:TaxCategoryCodeList","rdf:value":"AD","rdfs:comment":"Value Added Tax (VAT) due from a previous invoice"},{"@id":"unece:TaxCategoryCodeList#AE","@type":"unece:TaxCategoryCodeList","rdf:value":"AE","rdfs:comment":"VAT Reverse Charge"},{"@id":"unece:TaxCategoryCodeList#B","@type":"unece:TaxCategoryCodeList","rdf:value":"B","rdfs:comment":"Transferred (VAT)"},{"@id":"unece:TaxCategoryCodeList#C","@type":"unece:TaxCategoryCodeList","rdf:value":"C","rdfs:comment":"Duty paid by supplier"},{"@id":"unece:TaxCategoryCodeList#D","@type":"unece:TaxCategoryCodeList","rdf:value":"D","rdfs:comment":"Value Added Tax (VAT) margin scheme - travel agents"},{"@id":"unece:TaxCategoryCodeList#E","@type":"unece:TaxCategoryCodeList","rdf:value":"E","rdfs:comment":"Exempt from tax"},{"@id":"unece:TaxCategoryCodeList#F","@type":"unece:TaxCategoryCodeList","rdf:value":"F","rdfs:comment":"Value Added Tax (VAT) margin scheme - second-hand goods"},{"@id":"unece:TaxCategoryCodeList#G","@type":"unece:TaxCategoryCodeList","rdf:value":"G","rdfs:comment":"Free export item, tax not charged"},{"@id":"unece:TaxCategoryCodeList#H","@type":"unece:TaxCategoryCodeList","rdf:value":"H","rdfs:comment":"Higher rate"},{"@id":"unece:TaxCategoryCodeList#I","@type":"unece:TaxCategoryCodeList","rdf:value":"I","rdfs:comment":"Value Added Tax (VAT) margin scheme - works of art Margin scheme  Works of art"},{"@id":"unece:TaxCategoryCodeList#J","@type":"unece:TaxCategoryCodeList","rdf:value":"J","rdfs:comment":"Value Added Tax (VAT) margin scheme - collectors items and antiques"},{"@id":"unece:TaxCategoryCodeList#K","@type":"unece:TaxCategoryCodeList","rdf:value":"K","rdfs:comment":"VAT exempt for EEA intra-community supply of goods and services"},{"@id":"unece:TaxCategoryCodeList#L","@type":"unece:TaxCategoryCodeList","rdf:value":"L","rdfs:comment":"Canary Islands general indirect tax"},{"@id":"unece:TaxCategoryCodeList#M","@type":"unece:TaxCategoryCodeList","rdf:value":"M","rdfs:comment":"Tax for production, services and importation in Ceuta and Melilla"},{"@id":"unece:TaxCategoryCodeList#N","@type":"unece:TaxCategoryCodeList","rdf:value":"N","rdfs:comment":"standard rate additional VAT"},{"@id":"unece:TaxCategoryCodeList#O","@type":"unece:TaxCategoryCodeList","rdf:value":"O","rdfs:comment":"Services outside scope of tax"},{"@id":"unece:TaxCategoryCodeList#S","@type":"unece:TaxCategoryCodeList","rdf:value":"S","rdfs:comment":"Standard rate"},{"@id":"unece:TaxCategoryCodeList#Z","@type":"unece:TaxCategoryCodeList","rdf:value":"Z","rdfs:comment":"Zero rated goods"},{"rdfs:label":"TaxExemptionReasonCodeList","@type":"rdfs:Class","@id":"unece:TaxExemptionReasonCodeList","rdfs:comment":"A character string used to represent or replace a reason for tax exemption."},{"@id":"unece:TaxExemptionReasonCodeList#1","@type":"unece:TaxExemptionReasonCodeList","rdf:value":"1","rdfs:comment":"Exports and Related Operations"},{"@id":"unece:TaxExemptionReasonCodeList#2","@type":"unece:TaxExemptionReasonCodeList","rdf:value":"2","rdfs:comment":"Manufacturing intraCommunity"},{"@id":"unece:TaxExemptionReasonCodeList#3","@type":"unece:TaxExemptionReasonCodeList","rdf:value":"3","rdfs:comment":"Import Exemption"},{"@id":"unece:TaxExemptionReasonCodeList#4","@type":"unece:TaxExemptionReasonCodeList","rdf:value":"4","rdfs:comment":"Acquisition intraCommunity exempt"},{"@id":"unece:TaxExemptionReasonCodeList#5","@type":"unece:TaxExemptionReasonCodeList","rdf:value":"5","rdfs:comment":"International Transport"},{"@id":"unece:TaxExemptionReasonCodeList#6","@type":"unece:TaxExemptionReasonCodeList","rdf:value":"6","rdfs:comment":"FR DOM (special exemptions)"},{"@id":"unece:TaxExemptionReasonCodeList#7","@type":"unece:TaxExemptionReasonCodeList","rdf:value":"7","rdfs:comment":"Medical professions and allied"},{"@id":"unece:TaxExemptionReasonCodeList#8","@type":"unece:TaxExemptionReasonCodeList","rdf:value":"8","rdfs:comment":"Health institutions"},{"@id":"unece:TaxExemptionReasonCodeList#9","@type":"unece:TaxExemptionReasonCodeList","rdf:value":"9","rdfs:comment":"Education and professional training provided by recognized institutions"},{"@id":"unece:TaxExemptionReasonCodeList#10","@type":"unece:TaxExemptionReasonCodeList","rdf:value":"10","rdfs:comment":"Exemption on particular bank and financial transactions"},{"@id":"unece:TaxExemptionReasonCodeList#11","@type":"unece:TaxExemptionReasonCodeList","rdf:value":"11","rdfs:comment":"Gold investment transactions"},{"@id":"unece:TaxExemptionReasonCodeList#12","@type":"unece:TaxExemptionReasonCodeList","rdf:value":"12","rdfs:comment":"Insurance and reinsurance transactions"},{"@id":"unece:TaxExemptionReasonCodeList#13","@type":"unece:TaxExemptionReasonCodeList","rdf:value":"13","rdfs:comment":"Particular real estate rental (farm land and buildings; unmanaged soil; unequipped business premises)"},{"@id":"unece:TaxExemptionReasonCodeList#14","@type":"unece:TaxExemptionReasonCodeList","rdf:value":"14","rdfs:comment":"Particular rentals of furnished dwelling"},{"@id":"unece:TaxExemptionReasonCodeList#15","@type":"unece:TaxExemptionReasonCodeList","rdf:value":"15","rdfs:comment":"Real estate transactions"},{"@id":"unece:TaxExemptionReasonCodeList#16","@type":"unece:TaxExemptionReasonCodeList","rdf:value":"16","rdfs:comment":"Cost reimbursement of equipment by members of grouping"},{"@id":"unece:TaxExemptionReasonCodeList#17","@type":"unece:TaxExemptionReasonCodeList","rdf:value":"17","rdfs:comment":"Pluri property Entities"},{"@id":"unece:TaxExemptionReasonCodeList#18","@type":"unece:TaxExemptionReasonCodeList","rdf:value":"18","rdfs:comment":"Not for profit organizations (including groupings of blind or disabled workers, philosophical, religious, political, civic organizations or unions)"},{"@id":"unece:TaxExemptionReasonCodeList#19","@type":"unece:TaxExemptionReasonCodeList","rdf:value":"19","rdfs:comment":"War memorial"},{"@id":"unece:TaxExemptionReasonCodeList#20","@type":"unece:TaxExemptionReasonCodeList","rdf:value":"20","rdfs:comment":"Second hand objects sold by their users"},{"@id":"unece:TaxExemptionReasonCodeList#21","@type":"unece:TaxExemptionReasonCodeList","rdf:value":"21","rdfs:comment":"Agricultural mutual aid"},{"@id":"unece:TaxExemptionReasonCodeList#22","@type":"unece:TaxExemptionReasonCodeList","rdf:value":"22","rdfs:comment":"Fishing"},{"@id":"unece:TaxExemptionReasonCodeList#23","@type":"unece:TaxExemptionReasonCodeList","rdf:value":"23","rdfs:comment":"Clubs and gambling houses"},{"@id":"unece:TaxExemptionReasonCodeList#24","@type":"unece:TaxExemptionReasonCodeList","rdf:value":"24","rdfs:comment":"Gamings and bets (casinos; races; lotto)"},{"@id":"unece:TaxExemptionReasonCodeList#25","@type":"unece:TaxExemptionReasonCodeList","rdf:value":"25","rdfs:comment":"Health Transport"},{"@id":"unece:TaxExemptionReasonCodeList#26","@type":"unece:TaxExemptionReasonCodeList","rdf:value":"26","rdfs:comment":"Medicinal biology analysis"},{"@id":"unece:TaxExemptionReasonCodeList#27","@type":"unece:TaxExemptionReasonCodeList","rdf:value":"27","rdfs:comment":"Prosthesis supply by prosthodontist"},{"@id":"unece:TaxExemptionReasonCodeList#28","@type":"unece:TaxExemptionReasonCodeList","rdf:value":"28","rdfs:comment":"Organs, blood and human milk"},{"@id":"unece:TaxExemptionReasonCodeList#29","@type":"unece:TaxExemptionReasonCodeList","rdf:value":"29","rdfs:comment":"Sport meetings"},{"@id":"unece:TaxExemptionReasonCodeList#30","@type":"unece:TaxExemptionReasonCodeList","rdf:value":"30","rdfs:comment":"Goods future markets"},{"@id":"unece:TaxExemptionReasonCodeList#31","@type":"unece:TaxExemptionReasonCodeList","rdf:value":"31","rdfs:comment":"Industry brand-new wastes and recycling/recovering materials"},{"@id":"unece:TaxExemptionReasonCodeList#32","@type":"unece:TaxExemptionReasonCodeList","rdf:value":"32","rdfs:comment":"Fiscal and postage stamps"},{"rdfs:label":"TaxTypeCodeList","@type":"rdfs:Class","@id":"unece:TaxTypeCodeList","rdfs:comment":"A character string used to represent or replace a tax type."},{"@id":"unece:TaxTypeCodeList#AAA","@type":"unece:TaxTypeCodeList","rdf:value":"AAA","rdfs:comment":"Petroleum tax"},{"@id":"unece:TaxTypeCodeList#AAB","@type":"unece:TaxTypeCodeList","rdf:value":"AAB","rdfs:comment":"Provisional countervailing duty cash"},{"@id":"unece:TaxTypeCodeList#AAC","@type":"unece:TaxTypeCodeList","rdf:value":"AAC","rdfs:comment":"Provisional countervailing duty bond"},{"@id":"unece:TaxTypeCodeList#AAD","@type":"unece:TaxTypeCodeList","rdf:value":"AAD","rdfs:comment":"Tobacco tax"},{"@id":"unece:TaxTypeCodeList#AAE","@type":"unece:TaxTypeCodeList","rdf:value":"AAE","rdfs:comment":"Energy fee"},{"@id":"unece:TaxTypeCodeList#AAF","@type":"unece:TaxTypeCodeList","rdf:value":"AAF","rdfs:comment":"Coffee tax"},{"@id":"unece:TaxTypeCodeList#AAG","@type":"unece:TaxTypeCodeList","rdf:value":"AAG","rdfs:comment":"Harmonised sales tax, Canadian"},{"@id":"unece:TaxTypeCodeList#AAH","@type":"unece:TaxTypeCodeList","rdf:value":"AAH","rdfs:comment":"Quebec sales tax"},{"@id":"unece:TaxTypeCodeList#AAI","@type":"unece:TaxTypeCodeList","rdf:value":"AAI","rdfs:comment":"Canadian provincial sales tax"},{"@id":"unece:TaxTypeCodeList#AAJ","@type":"unece:TaxTypeCodeList","rdf:value":"AAJ","rdfs:comment":"Tax on replacement part"},{"@id":"unece:TaxTypeCodeList#AAK","@type":"unece:TaxTypeCodeList","rdf:value":"AAK","rdfs:comment":"Mineral oil tax"},{"@id":"unece:TaxTypeCodeList#AAL","@type":"unece:TaxTypeCodeList","rdf:value":"AAL","rdfs:comment":"Special tax"},{"@id":"unece:TaxTypeCodeList#AAM","@type":"unece:TaxTypeCodeList","rdf:value":"AAM","rdfs:comment":"Insurance tax"},{"@id":"unece:TaxTypeCodeList#AAO","@type":"unece:TaxTypeCodeList","rdf:value":"AAO","rdfs:comment":"Provincial Cannabis Tax"},{"@id":"unece:TaxTypeCodeList#AAP","@type":"unece:TaxTypeCodeList","rdf:value":"AAP","rdfs:comment":"Outstanding duty interest"},{"@id":"unece:TaxTypeCodeList#ADD","@type":"unece:TaxTypeCodeList","rdf:value":"ADD","rdfs:comment":"Anti-dumping duty"},{"@id":"unece:TaxTypeCodeList#BOL","@type":"unece:TaxTypeCodeList","rdf:value":"BOL","rdfs:comment":"Stamp duty (Imposta di Bollo)"},{"@id":"unece:TaxTypeCodeList#CAP","@type":"unece:TaxTypeCodeList","rdf:value":"CAP","rdfs:comment":"Agricultural levy"},{"@id":"unece:TaxTypeCodeList#CAR","@type":"unece:TaxTypeCodeList","rdf:value":"CAR","rdfs:comment":"Car tax"},{"@id":"unece:TaxTypeCodeList#COC","@type":"unece:TaxTypeCodeList","rdf:value":"COC","rdfs:comment":"Paper consortium tax (Italy)"},{"@id":"unece:TaxTypeCodeList#CST","@type":"unece:TaxTypeCodeList","rdf:value":"CST","rdfs:comment":"Commodity specific tax"},{"@id":"unece:TaxTypeCodeList#CUD","@type":"unece:TaxTypeCodeList","rdf:value":"CUD","rdfs:comment":"Customs duty"},{"@id":"unece:TaxTypeCodeList#CVD","@type":"unece:TaxTypeCodeList","rdf:value":"CVD","rdfs:comment":"Countervailing duty"},{"@id":"unece:TaxTypeCodeList#ENV","@type":"unece:TaxTypeCodeList","rdf:value":"ENV","rdfs:comment":"Environmental tax"},{"@id":"unece:TaxTypeCodeList#EXC","@type":"unece:TaxTypeCodeList","rdf:value":"EXC","rdfs:comment":"Excise duty"},{"@id":"unece:TaxTypeCodeList#EXP","@type":"unece:TaxTypeCodeList","rdf:value":"EXP","rdfs:comment":"Agricultural export rebate"},{"@id":"unece:TaxTypeCodeList#FET","@type":"unece:TaxTypeCodeList","rdf:value":"FET","rdfs:comment":"Federal excise tax"},{"@id":"unece:TaxTypeCodeList#FRE","@type":"unece:TaxTypeCodeList","rdf:value":"FRE","rdfs:comment":"Free"},{"@id":"unece:TaxTypeCodeList#GCN","@type":"unece:TaxTypeCodeList","rdf:value":"GCN","rdfs:comment":"General construction tax"},{"@id":"unece:TaxTypeCodeList#GST","@type":"unece:TaxTypeCodeList","rdf:value":"GST","rdfs:comment":"Goods and services tax"},{"@id":"unece:TaxTypeCodeList#ILL","@type":"unece:TaxTypeCodeList","rdf:value":"ILL","rdfs:comment":"Illuminants tax"},{"@id":"unece:TaxTypeCodeList#IMP","@type":"unece:TaxTypeCodeList","rdf:value":"IMP","rdfs:comment":"Import tax"},{"@id":"unece:TaxTypeCodeList#IND","@type":"unece:TaxTypeCodeList","rdf:value":"IND","rdfs:comment":"Individual tax"},{"@id":"unece:TaxTypeCodeList#LAC","@type":"unece:TaxTypeCodeList","rdf:value":"LAC","rdfs:comment":"Business license fee"},{"@id":"unece:TaxTypeCodeList#LCN","@type":"unece:TaxTypeCodeList","rdf:value":"LCN","rdfs:comment":"Local construction tax"},{"@id":"unece:TaxTypeCodeList#LDP","@type":"unece:TaxTypeCodeList","rdf:value":"LDP","rdfs:comment":"Light dues payable"},{"@id":"unece:TaxTypeCodeList#LOC","@type":"unece:TaxTypeCodeList","rdf:value":"LOC","rdfs:comment":"Local sales tax"},{"@id":"unece:TaxTypeCodeList#LST","@type":"unece:TaxTypeCodeList","rdf:value":"LST","rdfs:comment":"Lust tax"},{"@id":"unece:TaxTypeCodeList#MCA","@type":"unece:TaxTypeCodeList","rdf:value":"MCA","rdfs:comment":"Monetary compensatory amount"},{"@id":"unece:TaxTypeCodeList#MCD","@type":"unece:TaxTypeCodeList","rdf:value":"MCD","rdfs:comment":"Miscellaneous cash deposit"},{"@id":"unece:TaxTypeCodeList#OTH","@type":"unece:TaxTypeCodeList","rdf:value":"OTH","rdfs:comment":"Other taxes"},{"@id":"unece:TaxTypeCodeList#PDB","@type":"unece:TaxTypeCodeList","rdf:value":"PDB","rdfs:comment":"Provisional duty bond"},{"@id":"unece:TaxTypeCodeList#PDC","@type":"unece:TaxTypeCodeList","rdf:value":"PDC","rdfs:comment":"Provisional duty cash"},{"@id":"unece:TaxTypeCodeList#PRF","@type":"unece:TaxTypeCodeList","rdf:value":"PRF","rdfs:comment":"Preference duty"},{"@id":"unece:TaxTypeCodeList#SCN","@type":"unece:TaxTypeCodeList","rdf:value":"SCN","rdfs:comment":"Special construction tax"},{"@id":"unece:TaxTypeCodeList#SSS","@type":"unece:TaxTypeCodeList","rdf:value":"SSS","rdfs:comment":"Shifted social securities"},{"@id":"unece:TaxTypeCodeList#STT","@type":"unece:TaxTypeCodeList","rdf:value":"STT","rdfs:comment":"State/provincial sales tax"},{"@id":"unece:TaxTypeCodeList#SUP","@type":"unece:TaxTypeCodeList","rdf:value":"SUP","rdfs:comment":"Suspended duty"},{"@id":"unece:TaxTypeCodeList#SUR","@type":"unece:TaxTypeCodeList","rdf:value":"SUR","rdfs:comment":"Surtax"},{"@id":"unece:TaxTypeCodeList#SWT","@type":"unece:TaxTypeCodeList","rdf:value":"SWT","rdfs:comment":"Shifted wage tax"},{"@id":"unece:TaxTypeCodeList#TAC","@type":"unece:TaxTypeCodeList","rdf:value":"TAC","rdfs:comment":"Alcohol mark tax"},{"@id":"unece:TaxTypeCodeList#TOT","@type":"unece:TaxTypeCodeList","rdf:value":"TOT","rdfs:comment":"Total"},{"@id":"unece:TaxTypeCodeList#TOX","@type":"unece:TaxTypeCodeList","rdf:value":"TOX","rdfs:comment":"Turnover tax"},{"@id":"unece:TaxTypeCodeList#TTA","@type":"unece:TaxTypeCodeList","rdf:value":"TTA","rdfs:comment":"Tonnage taxes"},{"@id":"unece:TaxTypeCodeList#VAD","@type":"unece:TaxTypeCodeList","rdf:value":"VAD","rdfs:comment":"Valuation deposit"},{"@id":"unece:TaxTypeCodeList#VAT","@type":"unece:TaxTypeCodeList","rdf:value":"VAT","rdfs:comment":"Value added tax"},{"rdfs:label":"TimeReferenceCodeList","@type":"rdfs:Class","@id":"unece:TimeReferenceCodeList","rdfs:comment":"A character string used to represent a time reference."},{"@id":"unece:TimeReferenceCodeList#1","@type":"unece:TimeReferenceCodeList","rdf:value":"1","rdfs:comment":"Date of order"},{"@id":"unece:TimeReferenceCodeList#2","@type":"unece:TimeReferenceCodeList","rdf:value":"2","rdfs:comment":"Date of confirmation"},{"@id":"unece:TimeReferenceCodeList#3","@type":"unece:TimeReferenceCodeList","rdf:value":"3","rdfs:comment":"Date of contract"},{"@id":"unece:TimeReferenceCodeList#4","@type":"unece:TimeReferenceCodeList","rdf:value":"4","rdfs:comment":"Date of signature of contract"},{"@id":"unece:TimeReferenceCodeList#5","@type":"unece:TimeReferenceCodeList","rdf:value":"5","rdfs:comment":"Date of invoice"},{"@id":"unece:TimeReferenceCodeList#6","@type":"unece:TimeReferenceCodeList","rdf:value":"6","rdfs:comment":"Date of credit note"},{"@id":"unece:TimeReferenceCodeList#7","@type":"unece:TimeReferenceCodeList","rdf:value":"7","rdfs:comment":"Date of present document"},{"@id":"unece:TimeReferenceCodeList#8","@type":"unece:TimeReferenceCodeList","rdf:value":"8","rdfs:comment":"Date of confirmation of order received"},{"@id":"unece:TimeReferenceCodeList#9","@type":"unece:TimeReferenceCodeList","rdf:value":"9","rdfs:comment":"Date invoice received"},{"@id":"unece:TimeReferenceCodeList#10","@type":"unece:TimeReferenceCodeList","rdf:value":"10","rdfs:comment":"Latest date/time for bid reception"},{"@id":"unece:TimeReferenceCodeList#11","@type":"unece:TimeReferenceCodeList","rdf:value":"11","rdfs:comment":"Date credit note received"},{"@id":"unece:TimeReferenceCodeList#12","@type":"unece:TimeReferenceCodeList","rdf:value":"12","rdfs:comment":"Date present document received"},{"@id":"unece:TimeReferenceCodeList#13","@type":"unece:TimeReferenceCodeList","rdf:value":"13","rdfs:comment":"Date of resale by buyer"},{"@id":"unece:TimeReferenceCodeList#14","@type":"unece:TimeReferenceCodeList","rdf:value":"14","rdfs:comment":"Date proceeds of resale collected by buyer"},{"@id":"unece:TimeReferenceCodeList#21","@type":"unece:TimeReferenceCodeList","rdf:value":"21","rdfs:comment":"Date goods received by buyer"},{"@id":"unece:TimeReferenceCodeList#22","@type":"unece:TimeReferenceCodeList","rdf:value":"22","rdfs:comment":"Date goods received by buyer's agent"},{"@id":"unece:TimeReferenceCodeList#23","@type":"unece:TimeReferenceCodeList","rdf:value":"23","rdfs:comment":"Date goods received by carrier"},{"@id":"unece:TimeReferenceCodeList#24","@type":"unece:TimeReferenceCodeList","rdf:value":"24","rdfs:comment":"Date ex-works"},{"@id":"unece:TimeReferenceCodeList#25","@type":"unece:TimeReferenceCodeList","rdf:value":"25","rdfs:comment":"Date goods handed over for shipment by seller or agent"},{"@id":"unece:TimeReferenceCodeList#26","@type":"unece:TimeReferenceCodeList","rdf:value":"26","rdfs:comment":"Date of arrival of transport"},{"@id":"unece:TimeReferenceCodeList#27","@type":"unece:TimeReferenceCodeList","rdf:value":"27","rdfs:comment":"Date of outward frontier crossing"},{"@id":"unece:TimeReferenceCodeList#28","@type":"unece:TimeReferenceCodeList","rdf:value":"28","rdfs:comment":"Date of inward frontier crossing"},{"@id":"unece:TimeReferenceCodeList#29","@type":"unece:TimeReferenceCodeList","rdf:value":"29","rdfs:comment":"Date of delivery of goods to establishments/domicile/site"},{"@id":"unece:TimeReferenceCodeList#31","@type":"unece:TimeReferenceCodeList","rdf:value":"31","rdfs:comment":"Stipulated date for payment of documentary credit"},{"@id":"unece:TimeReferenceCodeList#32","@type":"unece:TimeReferenceCodeList","rdf:value":"32","rdfs:comment":"Stipulated date for acceptance of documentary credit"},{"@id":"unece:TimeReferenceCodeList#33","@type":"unece:TimeReferenceCodeList","rdf:value":"33","rdfs:comment":"Stipulated date for negotiation of documentary credit"},{"@id":"unece:TimeReferenceCodeList#41","@type":"unece:TimeReferenceCodeList","rdf:value":"41","rdfs:comment":"Date of delivery to buyer of documents representing goods"},{"@id":"unece:TimeReferenceCodeList#42","@type":"unece:TimeReferenceCodeList","rdf:value":"42","rdfs:comment":"Date of delivery to buyer's agent of documents representing goods"},{"@id":"unece:TimeReferenceCodeList#43","@type":"unece:TimeReferenceCodeList","rdf:value":"43","rdfs:comment":"Date of delivery to carrier of documents representing goods"},{"@id":"unece:TimeReferenceCodeList#44","@type":"unece:TimeReferenceCodeList","rdf:value":"44","rdfs:comment":"Date of delivery to intermediary bank of documents representing good"},{"@id":"unece:TimeReferenceCodeList#45","@type":"unece:TimeReferenceCodeList","rdf:value":"45","rdfs:comment":"Date of bill of lading, consignment note or other transport document"},{"@id":"unece:TimeReferenceCodeList#46","@type":"unece:TimeReferenceCodeList","rdf:value":"46","rdfs:comment":"Date of receipt for loading (mate's receipt)"},{"@id":"unece:TimeReferenceCodeList#47","@type":"unece:TimeReferenceCodeList","rdf:value":"47","rdfs:comment":"Date of negotiable instrument (draft, promissory note, bank)"},{"@id":"unece:TimeReferenceCodeList#48","@type":"unece:TimeReferenceCodeList","rdf:value":"48","rdfs:comment":"Date of receipt of tool dependent initial samples plus unlimited absolute bank guarantee plus value added tax"},{"@id":"unece:TimeReferenceCodeList#52","@type":"unece:TimeReferenceCodeList","rdf:value":"52","rdfs:comment":"Due date of negotiable instrument"},{"@id":"unece:TimeReferenceCodeList#53","@type":"unece:TimeReferenceCodeList","rdf:value":"53","rdfs:comment":"Date of presentation of negotiable instrument"},{"@id":"unece:TimeReferenceCodeList#54","@type":"unece:TimeReferenceCodeList","rdf:value":"54","rdfs:comment":"Date of acceptance of negotiable instrument"},{"@id":"unece:TimeReferenceCodeList#55","@type":"unece:TimeReferenceCodeList","rdf:value":"55","rdfs:comment":"Date of acceptance of tooling"},{"@id":"unece:TimeReferenceCodeList#56","@type":"unece:TimeReferenceCodeList","rdf:value":"56","rdfs:comment":"Date of receipt of tooling"},{"@id":"unece:TimeReferenceCodeList#57","@type":"unece:TimeReferenceCodeList","rdf:value":"57","rdfs:comment":"Date of acceptance of first samples produced under production conditions"},{"@id":"unece:TimeReferenceCodeList#60","@type":"unece:TimeReferenceCodeList","rdf:value":"60","rdfs:comment":"Date of start of work"},{"@id":"unece:TimeReferenceCodeList#61","@type":"unece:TimeReferenceCodeList","rdf:value":"61","rdfs:comment":"Date of end of work"},{"@id":"unece:TimeReferenceCodeList#62","@type":"unece:TimeReferenceCodeList","rdf:value":"62","rdfs:comment":"Date of provisional reception of work"},{"@id":"unece:TimeReferenceCodeList#63","@type":"unece:TimeReferenceCodeList","rdf:value":"63","rdfs:comment":"Date of final acceptance of work"},{"@id":"unece:TimeReferenceCodeList#64","@type":"unece:TimeReferenceCodeList","rdf:value":"64","rdfs:comment":"Date of certificate of preliminary acceptance"},{"@id":"unece:TimeReferenceCodeList#65","@type":"unece:TimeReferenceCodeList","rdf:value":"65","rdfs:comment":"Date of certificate of final acceptance"},{"@id":"unece:TimeReferenceCodeList#66","@type":"unece:TimeReferenceCodeList","rdf:value":"66","rdfs:comment":"Specified date"},{"@id":"unece:TimeReferenceCodeList#67","@type":"unece:TimeReferenceCodeList","rdf:value":"67","rdfs:comment":"Anticipated delivery date"},{"@id":"unece:TimeReferenceCodeList#68","@type":"unece:TimeReferenceCodeList","rdf:value":"68","rdfs:comment":"Effective date"},{"@id":"unece:TimeReferenceCodeList#69","@type":"unece:TimeReferenceCodeList","rdf:value":"69","rdfs:comment":"Invoice transmission date"},{"@id":"unece:TimeReferenceCodeList#70","@type":"unece:TimeReferenceCodeList","rdf:value":"70","rdfs:comment":"Date of issue of transport document(s)"},{"@id":"unece:TimeReferenceCodeList#71","@type":"unece:TimeReferenceCodeList","rdf:value":"71","rdfs:comment":"Date of presentation of documents"},{"@id":"unece:TimeReferenceCodeList#72","@type":"unece:TimeReferenceCodeList","rdf:value":"72","rdfs:comment":"Payment date"},{"@id":"unece:TimeReferenceCodeList#73","@type":"unece:TimeReferenceCodeList","rdf:value":"73","rdfs:comment":"Draft(s) at ... days sight"},{"@id":"unece:TimeReferenceCodeList#74","@type":"unece:TimeReferenceCodeList","rdf:value":"74","rdfs:comment":"Draft(s) at ... days date"},{"@id":"unece:TimeReferenceCodeList#75","@type":"unece:TimeReferenceCodeList","rdf:value":"75","rdfs:comment":"Draft(s) at ... days after date of issuance of transport document(s)"},{"@id":"unece:TimeReferenceCodeList#76","@type":"unece:TimeReferenceCodeList","rdf:value":"76","rdfs:comment":"Draft(s) at ... days after date of presentation of documents"},{"@id":"unece:TimeReferenceCodeList#77","@type":"unece:TimeReferenceCodeList","rdf:value":"77","rdfs:comment":"Specified draft date"},{"@id":"unece:TimeReferenceCodeList#78","@type":"unece:TimeReferenceCodeList","rdf:value":"78","rdfs:comment":"Customs clearance date (import)"},{"@id":"unece:TimeReferenceCodeList#79","@type":"unece:TimeReferenceCodeList","rdf:value":"79","rdfs:comment":"Customs clearance date (export)"},{"@id":"unece:TimeReferenceCodeList#80","@type":"unece:TimeReferenceCodeList","rdf:value":"80","rdfs:comment":"Date of salary payment"},{"@id":"unece:TimeReferenceCodeList#81","@type":"unece:TimeReferenceCodeList","rdf:value":"81","rdfs:comment":"Date of shipment as evidenced by the transport document(s)"},{"@id":"unece:TimeReferenceCodeList#82","@type":"unece:TimeReferenceCodeList","rdf:value":"82","rdfs:comment":"Payment due date"},{"@id":"unece:TimeReferenceCodeList#83","@type":"unece:TimeReferenceCodeList","rdf:value":"83","rdfs:comment":"Requested date of delivery"},{"@id":"unece:TimeReferenceCodeList#ZZZ","@type":"unece:TimeReferenceCodeList","rdf:value":"ZZZ","rdfs:comment":"Other reference date agreed upon between the parties"},{"@id":"unece:PaymentTradeSettlement","@type":"rdfs:Class","rdfs:label":"PaymentTradeSettlement","schema:source":{"@id":"https://vocabulary.uncefact.org/PaymentTradeSettlement"},"rdfs:comment":"The information that enables the reconciliation of a payment with the item(s) that the payment is intended to settle, for example a commercial invoice."},{"@id":"unece:FinancingSummaryDocument","@type":"rdfs:Class","rdfs:label":"FinancingSummaryDocument","schema:source":{"@id":"https://vocabulary.uncefact.org/FinancingSummaryDocument"},"rdfs:comment":"A collection of financing related data that provides an overview of key points."},{"@id":"unece:CreditorFinancialAccount","@type":"rdfs:Class","rdfs:label":"CreditorFinancialAccount","schema:source":{"@id":"https://vocabulary.uncefact.org/CreditorFinancialAccount"},"rdfs:comment":"A specific business arrangement whereby credits arising from transactions are recorded."},{"@id":"unece:DebtorFinancialAccount","@type":"rdfs:Class","rdfs:label":"DebtorFinancialAccount","schema:source":{"@id":"https://vocabulary.uncefact.org/DebtorFinancialAccount"},"rdfs:comment":"A specific business arrangement whereby debits arising from transactions are recorded."},{"@id":"unece:FinancingFinancialAccount","@type":"rdfs:Class","rdfs:label":"FinancingFinancialAccount","schema:source":{"@id":"https://vocabulary.uncefact.org/FinancingFinancialAccount"},"rdfs:comment":"A financial account used internally by a bank to manage the line of credit granted to financing requesting party."},{"@id":"unece:PaymentFinancialAccount","@type":"rdfs:Class","rdfs:label":"PaymentFinancialAccount","schema:source":{"@id":"https://vocabulary.uncefact.org/PaymentFinancialAccount"},"rdfs:comment":"A specific business arrangement whereby monetary values pertaining to payment, collected or paid, are recorded."},{"@id":"unece:AccountingAccount","@type":"rdfs:Class","rdfs:label":"AccountingAccount","schema:source":{"@id":"https://vocabulary.uncefact.org/AccountingAccount"},"rdfs:comment":"A specific trade account for recording debits and credits to general accounting, cost accounting or budget accounting."},{"@id":"unece:FinancialAdjustment","@type":"rdfs:Class","rdfs:label":"FinancialAdjustment","schema:source":{"@id":"https://vocabulary.uncefact.org/FinancialAdjustment"},"rdfs:comment":"A correction or modification to reflect actual financial conditions."},{"@id":"unece:AppliedAllowanceCharge","@type":"rdfs:Class","rdfs:label":"AppliedAllowanceCharge","schema:source":{"@id":"https://vocabulary.uncefact.org/AppliedAllowanceCharge"},"rdfs:comment":"The applied allowance or charge component of pricing."},{"@id":"unece:Booking","@type":"rdfs:Class","rdfs:label":"Booking","schema:source":{"@id":"https://vocabulary.uncefact.org/Booking"},"rdfs:comment":"A result of a financial transaction recorded within a financial account."},{"@id":"unece:PaymentDiscountTerms","@type":"rdfs:Class","rdfs:label":"PaymentDiscountTerms","schema:source":{"@id":"https://vocabulary.uncefact.org/PaymentDiscountTerms"},"rdfs:comment":"Trade terms and conditions by which a discount is or can be applied to a payable amount."},{"@id":"unece:PaymentPenaltyTerms","@type":"rdfs:Class","rdfs:label":"PaymentPenaltyTerms","schema:source":{"@id":"https://vocabulary.uncefact.org/PaymentPenaltyTerms"},"rdfs:comment":"Trade terms and conditions by which a penalty is or can be applied to a payable amount."},{"@id":"unece:CreditorFinancialInstitution","@type":"rdfs:Class","rdfs:label":"CreditorFinancialInstitution","schema:source":{"@id":"https://vocabulary.uncefact.org/CreditorFinancialInstitution"},"rdfs:comment":"A bank, building society, credit union, stock brokerage, or similar business of the party that receives money."},{"@id":"unece:FinancingRequestDocument","@type":"rdfs:Class","rdfs:label":"FinancingRequestDocument","schema:source":{"@id":"https://vocabulary.uncefact.org/FinancingRequestDocument"},"rdfs:comment":"The set of characteristics shared by all individual transactions grouped for this financing request document."},{"@id":"unece:FinancialIdentity","@type":"rdfs:Class","rdfs:label":"FinancialIdentity","schema:source":{"@id":"https://vocabulary.uncefact.org/FinancialIdentity"},"rdfs:comment":"A financial identification for an organization."},{"@id":"unece:PaymentMeans","@type":"rdfs:Class","rdfs:label":"PaymentMeans","schema:source":{"@id":"https://vocabulary.uncefact.org/PaymentMeans"},"rdfs:comment":"The means by which a payment will be or has been made for trade settlement purposes."},{"@id":"unece:Cash","@type":"rdfs:Class","rdfs:label":"Cash","schema:source":{"@id":"https://vocabulary.uncefact.org/Cash"},"rdfs:comment":"Coins, banknotes paid by the recipient of goods or services to the provider."},{"@id":"unece:Cheque","@type":"rdfs:Class","rdfs:label":"Cheque","schema:source":{"@id":"https://vocabulary.uncefact.org/Cheque"},"rdfs:comment":"A written payment order to a bank to pay the stated sum from the drawer's account."},{"@id":"unece:DigitalMethod","@type":"rdfs:Class","rdfs:label":"DigitalMethod","schema:source":{"@id":"https://vocabulary.uncefact.org/DigitalMethod"},"rdfs:comment":"The use of online and digital technologies to collect monetary payment amounts."},{"@id":"unece:FinancialCard","@type":"rdfs:Class","rdfs:label":"FinancialCard","schema:source":{"@id":"https://vocabulary.uncefact.org/FinancialCard"},"rdfs:comment":"A card used to represent a financial account for a trade settlement."},{"@id":"unece:PaymentTerms","@type":"rdfs:Class","rdfs:label":"PaymentTerms","schema:source":{"@id":"https://vocabulary.uncefact.org/PaymentTerms"},"rdfs:comment":"Terms and conditions by which payment has been or will be made for trade purposes."},{"@id":"unece:AppliedTax","@type":"rdfs:Class","rdfs:label":"AppliedTax","schema:source":{"@id":"https://vocabulary.uncefact.org/AppliedTax"},"rdfs:comment":"A total levy or payment for the support of a government that is required of persons, groups, or businesses within the domain of that government."},{"@id":"unece:DebtorFinancialInstitution","@type":"rdfs:Class","rdfs:label":"DebtorFinancialInstitution","schema:source":{"@id":"https://vocabulary.uncefact.org/DebtorFinancialInstitution"},"rdfs:comment":"A bank, building society, credit union, stock brokerage, or similar business of the party that owes money."},{"@id":"unece:PaymentFinancialInstitution","@type":"rdfs:Class","rdfs:label":"PaymentFinancialInstitution","schema:source":{"@id":"https://vocabulary.uncefact.org/PaymentFinancialInstitution"},"rdfs:comment":"An institution that provides financial services and financial transactions for payment."},{"@id":"unece:BreakdownStatement","@type":"rdfs:Class","rdfs:label":"BreakdownStatement","schema:source":{"@id":"https://vocabulary.uncefact.org/BreakdownStatement"},"rdfs:comment":"A detailed statement of work, prices, and dimensions for this valuation."},{"@id":"unece:HeaderBalanceOut","@type":"rdfs:Class","rdfs:label":"HeaderBalanceOut","schema:source":{"@id":"https://vocabulary.uncefact.org/HeaderBalanceOut"},"rdfs:comment":"Offset header information to ensure that debits and credits are equal for a transaction."},{"@id":"unece:FinancialInstitutionAddress","@type":"rdfs:Class","rdfs:label":"FinancialInstitutionAddress","schema:source":{"@id":"https://vocabulary.uncefact.org/FinancialInstitutionAddress"},"rdfs:comment":"The location at which a financial institution may be found or reached."},{"@id":"unece:PaymentBalanceOut","@type":"rdfs:Class","rdfs:label":"PaymentBalanceOut","schema:source":{"@id":"https://vocabulary.uncefact.org/PaymentBalanceOut"},"rdfs:comment":"Offset information to ensure that debits and credits are equal for a transaction."},{"@id":"unece:Guarantee","@type":"rdfs:Class","rdfs:label":"Guarantee","schema:source":{"@id":"https://vocabulary.uncefact.org/Guarantee"},"rdfs:comment":"An official promise or assurance to fulfil a financial obligation."},{"@id":"unece:RegisteredTax","@type":"rdfs:Class","rdfs:label":"RegisteredTax","schema:source":{"@id":"https://vocabulary.uncefact.org/RegisteredTax"},"rdfs:comment":"A registered tax or duty system pertaining to an authority."},{"@id":"unece:InstalmentPayment","@type":"rdfs:Class","rdfs:label":"InstalmentPayment","schema:source":{"@id":"https://vocabulary.uncefact.org/InstalmentPayment"},"rdfs:comment":"A discharge of obligations in respect of funds or securities, transferred through one of several payments, between two or more parties."},{"@id":"unece:FinancingRequestResultDocument","@type":"rdfs:Class","rdfs:label":"FinancingRequestResultDocument","schema:source":{"@id":"https://vocabulary.uncefact.org/FinancingRequestResultDocument"},"rdfs:comment":"A collection of data that reports the result of a financing request."},{"@id":"unece:FinancingStatus","@type":"rdfs:Class","rdfs:label":"FinancingStatus","schema:source":{"@id":"https://vocabulary.uncefact.org/FinancingStatus"},"rdfs:comment":"Information relevant to a condition of financing."},{"@id":"unece:BranchFinancialInstitution","@type":"rdfs:Class","rdfs:label":"BranchFinancialInstitution","schema:source":{"@id":"https://vocabulary.uncefact.org/BranchFinancialInstitution"},"rdfs:comment":"A sub-division of a bank, building society, credit union, stock brokerage, or similar business; established primarily to provide financial services and financial transactions."},{"@id":"unece:AdvancePayment","@type":"rdfs:Class","rdfs:label":"AdvancePayment","schema:source":{"@id":"https://vocabulary.uncefact.org/AdvancePayment"},"rdfs:comment":"A prepaid discharge of obligations in respect of funds or securities transferred between two or more parties."},{"@id":"unece:InstalmentPlan","@type":"rdfs:Class","rdfs:label":"InstalmentPlan","schema:source":{"@id":"https://vocabulary.uncefact.org/InstalmentPlan"},"rdfs:comment":"A plan for paying a total sum of money by several payments made over a period of time."},{"@id":"unece:RequestingParty","@type":"rdfs:Class","rdfs:label":"RequestingParty","schema:source":{"@id":"https://vocabulary.uncefact.org/RequestingParty"},"rdfs:comment":"An individual, a group, or a body having a role as a requestor."},{"@id":"unece:BasicWorkItem","@type":"rdfs:Class","rdfs:label":"BasicWorkItem","schema:source":{"@id":"https://vocabulary.uncefact.org/BasicWorkItem"},"rdfs:comment":"A basic item of work."},{"@id":"unece:GroupedWorkItem","@type":"rdfs:Class","rdfs:label":"GroupedWorkItem","schema:source":{"@id":"https://vocabulary.uncefact.org/GroupedWorkItem"},"rdfs:comment":"A grouping of related work items."},{"@id":"unece:CalculatedPrice","@type":"rdfs:Class","rdfs:label":"CalculatedPrice","schema:source":{"@id":"https://vocabulary.uncefact.org/CalculatedPrice"},"rdfs:comment":"Information related to a calculated price."},{"@id":"unece:Tax","@type":"rdfs:Class","rdfs:label":"Tax","schema:source":{"@id":"https://vocabulary.uncefact.org/Tax"},"rdfs:comment":"A trade related fiscal levy or duty."},{"@id":"unece:CurrencyExchange","@type":"rdfs:Class","rdfs:label":"CurrencyExchange","schema:source":{"@id":"https://vocabulary.uncefact.org/CurrencyExchange"},"rdfs:comment":"The conversion of one currency to another for trade purposes."},{"@id":"unece:Voucher","@type":"rdfs:Class","rdfs:label":"Voucher","schema:source":{"@id":"https://vocabulary.uncefact.org/Voucher"},"rdfs:comment":"A printed piece of paper or an electronic document that can be used instead of money to pay for an experience, such as a tour, a trip or a meal in a restaurant."},{"@id":"unece:TradeSettlementPaymentMonetarySummation","@type":"rdfs:Class","rdfs:label":"TradeSettlementPaymentMonetarySummation","schema:source":{"@id":"https://vocabulary.uncefact.org/TradeSettlementPaymentMonetarySummation"},"rdfs:comment":"A collection of monetary amount totals specified for a trade settlement payment."},{"@id":"unece:TradeAllowanceCharge","@type":"rdfs:Class","rdfs:label":"TradeAllowanceCharge","schema:source":{"@id":"https://vocabulary.uncefact.org/TradeAllowanceCharge"},"rdfs:comment":"A component of pricing, such as an allowance or charge for trade purposes."},{"@id":"unece:TradePrice","@type":"rdfs:Class","rdfs:label":"TradePrice","schema:source":{"@id":"https://vocabulary.uncefact.org/TradePrice"},"rdfs:comment":"A sum of money for which something is or may be bought or sold for trade purposes."},{"@id":"unece:ReferencePrice","@type":"rdfs:Class","rdfs:label":"ReferencePrice","schema:source":{"@id":"https://vocabulary.uncefact.org/ReferencePrice"},"rdfs:comment":"A reference to a sum of money for which something is or may be bought or sold."},{"@id":"unece:CustomsValuation","@type":"rdfs:Class","rdfs:label":"CustomsValuation","schema:source":{"@id":"https://vocabulary.uncefact.org/CustomsValuation"},"rdfs:comment":"A cross-border trade related assessment of the worth of an object, such as its monetary value, for customs purposes."},{"@id":"unece:acceptedAmount","@type":["rdf:Property","owl:ObjectProperty"],"rdfs:label":"acceptedAmount","schema:rangeIncludes":{"@id":"unece:AmountType"},"schema:domainIncludes":{"@id":"unece:PaymentTradeSettlement"},"rdfs:comment":""},{"@id":"unece:additionalDescription","@type":["rdf:Property","owl:DatatypeProperty"],"rdfs:label":"additionalDescription","schema:rangeIncludes":{"@id":"schema:Text"},"schema:domainIncludes":[{"@id":"unece:PaymentTradeSettlement"},{"@id":"unece:Picture"}],"rdfs:comment":"An additional textual description for this trade product."},{"@id":"unece:applicableTax","@type":["rdf:Property","owl:ObjectProperty"],"rdfs:label":"applicableTax","schema:rangeIncludes":{"@id":"unece:Tax"},"schema:domainIncludes":{"@id":"unece:PaymentTradeSettlement"},"rdfs:comment":"A tax applicable to this header trade settlement."},{"@id":"unece:creationDateTime","@type":["rdf:Property","owl:DatatypeProperty"],"rdfs:label":"creationDateTime","schema:rangeIncludes":{"@id":"schema:Text"},"schema:domainIncludes":[{"@id":"unece:PaymentTradeSettlement"},{"@id":"unece:FinancingRequestDocument"},{"@id":"unece:BreakdownStatement"},{"@id":"unece:ExchangedDocument"},{"@id":"unece:SpecifiedNote"}],"rdfs:comment":"The creation date, time, date time, or other date time value for this payment trade settlement."},{"@id":"unece:dueDateTime","@type":["rdf:Property","owl:DatatypeProperty"],"rdfs:label":"dueDateTime","schema:rangeIncludes":{"@id":"schema:Text"},"schema:domainIncludes":[{"@id":"unece:PaymentTradeSettlement"},{"@id":"unece:PaymentTerms"},{"@id":"unece:InstalmentPayment"}],"rdfs:comment":"The date, time, date time, or other date time value of the due date specified by these trade payment terms."},{"@id":"unece:identifiedGuarantee","@type":["rdf:Property","owl:ObjectProperty"],"rdfs:label":"identifiedGuarantee","schema:rangeIncludes":{"@id":"unece:Guarantee"},"schema:domainIncludes":{"@id":"unece:PaymentTradeSettlement"},"rdfs:comment":"The financial guarantee identified for this payment trade settlement."},{"@id":"unece:instruction","@type":["rdf:Property","owl:DatatypeProperty"],"rdfs:label":"instruction","schema:rangeIncludes":{"@id":"schema:Text"},"schema:domainIncludes":{"@id":"unece:PaymentTradeSettlement"},"rdfs:comment":"An instruction, expressed as text, for this experience event."},{"@id":"unece:invoicePayerAssignedReferenceId","@type":["rdf:Property","owl:DatatypeProperty"],"rdfs:label":"invoicePayerAssignedReferenceId","schema:rangeIncludes":{"@id":"schema:Text"},"schema:domainIncludes":{"@id":"unece:PaymentTradeSettlement"},"rdfs:comment":"The identifier of the invoice payer assigned reference of this payment trade settlement."},{"@id":"unece:payeeParty","@type":["rdf:Property","owl:ObjectProperty"],"rdfs:label":"payeeParty","schema:rangeIncludes":{"@id":"unece:Party"},"schema:domainIncludes":[{"@id":"unece:PaymentTradeSettlement"},{"@id":"unece:PaymentTerms"}],"rdfs:comment":""},{"@id":"unece:payerParty","@type":["rdf:Property","owl:ObjectProperty"],"rdfs:label":"payerParty","schema:rangeIncludes":{"@id":"unece:Party"},"schema:domainIncludes":{"@id":"unece:PaymentTradeSettlement"},"rdfs:comment":""},{"@id":"unece:paymentAmount","@type":["rdf:Property","owl:ObjectProperty"],"rdfs:label":"paymentAmount","schema:rangeIncludes":{"@id":"unece:AmountType"},"schema:domainIncludes":{"@id":"unece:PaymentTradeSettlement"},"rdfs:comment":""},{"@id":"unece:paymentApplicableCurrencyExchange","@type":["rdf:Property","owl:ObjectProperty"],"rdfs:label":"paymentApplicableCurrencyExchange","schema:rangeIncludes":{"@id":"unece:CurrencyExchange"},"schema:domainIncludes":{"@id":"unece:PaymentTradeSettlement"},"rdfs:comment":"The currency exchange applicable to the payment in this header trade settlement."},{"@id":"unece:paymentCurrencyCode","@type":["rdf:Property","owl:DatatypeProperty"],"rdfs:label":"paymentCurrencyCode","schema:rangeIncludes":{"@id":"unece:CurrencyCodeList"},"schema:domainIncludes":{"@id":"unece:PaymentTradeSettlement"},"rdfs:comment":"The code specifying the currency for this payment trade settlement."},{"@id":"unece:penaltyPercent","@type":["rdf:Property","owl:DatatypeProperty"],"rdfs:label":"penaltyPercent","schema:rangeIncludes":{"@id":"schema:Text"},"schema:domainIncludes":{"@id":"unece:PaymentTradeSettlement"},"rdfs:comment":"The penalty percentage related to this payment trade settlement."},{"@id":"unece:priorityCode","@type":["rdf:Property","owl:DatatypeProperty"],"rdfs:label":"priorityCode","schema:rangeIncludes":{"@id":"schema:Text"},"schema:domainIncludes":{"@id":"unece:PaymentTradeSettlement"},"rdfs:comment":"The code specifying the priority for this header trade agreement."},{"@id":"unece:receiptDateTime","@type":["rdf:Property","owl:DatatypeProperty"],"rdfs:label":"receiptDateTime","schema:rangeIncludes":{"@id":"schema:Text"},"schema:domainIncludes":[{"@id":"unece:PaymentTradeSettlement"},{"@id":"unece:Document"}],"rdfs:comment":"The date, time, date time, or other date time value for the formal receipt of this referenced document."},{"@id":"unece:refundAmount","@type":["rdf:Property","owl:ObjectProperty"],"rdfs:label":"refundAmount","schema:rangeIncludes":{"@id":"unece:AmountType"},"schema:domainIncludes":[{"@id":"unece:PaymentTradeSettlement"},{"@id":"unece:Tax"}],"rdfs:comment":""},{"@id":"unece:requestedAmount","@type":["rdf:Property","owl:ObjectProperty"],"rdfs:label":"requestedAmount","schema:rangeIncludes":{"@id":"unece:AmountType"},"schema:domainIncludes":{"@id":"unece:PaymentTradeSettlement"},"rdfs:comment":""},{"@id":"unece:specifiedPaymentMeans","@type":["rdf:Property","owl:ObjectProperty"],"rdfs:label":"specifiedPaymentMeans","schema:rangeIncludes":{"@id":"unece:PaymentMeans"},"schema:domainIncludes":{"@id":"unece:PaymentTradeSettlement"},"rdfs:comment":"A payment means specified for this header trade settlement."},{"@id":"unece:specifiedTradeSettlementPaymentMonetarySummation","@type":["rdf:Property","owl:ObjectProperty"],"rdfs:label":"specifiedTradeSettlementPaymentMonetarySummation","schema:rangeIncludes":{"@id":"unece:TradeSettlementPaymentMonetarySummation"},"schema:domainIncludes":{"@id":"unece:PaymentTradeSettlement"},"rdfs:comment":"The monetary summation totals specified for this payment trade settlement."},{"@id":"unece:statusCode","@type":["rdf:Property","owl:DatatypeProperty"],"rdfs:label":"statusCode","schema:rangeIncludes":{"@id":"schema:Text"},"schema:domainIncludes":[{"@id":"unece:PaymentTradeSettlement"},{"@id":"unece:Schedule"},{"@id":"unece:SpecifiedParameter"}],"rdfs:comment":"A code specifying a status for this trade product."},{"@id":"unece:taxAmount","@type":["rdf:Property","owl:ObjectProperty"],"rdfs:label":"taxAmount","schema:rangeIncludes":{"@id":"unece:AmountType"},"schema:domainIncludes":{"@id":"unece:PaymentTradeSettlement"},"rdfs:comment":""},{"@id":"unece:transferFeeInclusiveIndicator","@type":["rdf:Property","owl:DatatypeProperty"],"rdfs:label":"transferFeeInclusiveIndicator","schema:rangeIncludes":{"@id":"schema:Boolean"},"schema:domainIncludes":{"@id":"unece:PaymentTradeSettlement"},"rdfs:comment":"The indication of whether or not this payment trade settlement includes a transfer fee."},{"@id":"unece:typeCode","@type":["rdf:Property","owl:DatatypeProperty"],"rdfs:label":"typeCode","schema:rangeIncludes":{"@id":"schema:Text"},"schema:domainIncludes":[{"@id":"unece:PaymentTradeSettlement"},{"@id":"unece:PaymentFinancialAccount"},{"@id":"unece:Cash"},{"@id":"unece:Cheque"},{"@id":"unece:DigitalMethod"},{"@id":"unece:FinancialCard"},{"@id":"unece:PaymentFinancialInstitution"},{"@id":"unece:BreakdownStatement"},{"@id":"unece:BasicWorkItem"},{"@id":"unece:GroupedWorkItem"},{"@id":"unece:Voucher"},{"@id":"unece:CustomsValuation"},{"@id":"unece:SpecifiedAction"},{"@id":"unece:CountrySubDivision"},{"@id":"unece:Measurement"},{"@id":"unece:QuantityAnalysis"},{"@id":"unece:SpecifiedFault"},{"@id":"unece:RadioactiveMaterial"},{"@id":"unece:CommunicationEvent"},{"@id":"unece:LegalOrganization"},{"@id":"unece:Object"},{"@id":"unece:SpecifiedPeriod"},{"@id":"unece:Project"},{"@id":"unece:MetricCharacteristic"},{"@id":"unece:LegalRegistration"},{"@id":"unece:DocumentCharacteristic"},{"@id":"unece:Schedule"},{"@id":"unece:SpecifiedFeature"},{"@id":"unece:SpecifiedParameter"},{"@id":"unece:Range"},{"@id":"unece:GeopoliticalRegion"},{"@id":"unece:Issue"},{"@id":"unece:Segment"},{"@id":"unece:SecurityTag"},{"@id":"unece:SpecificationQuery"}],"rdfs:comment":"A code specifying a type of MDH health indication."},{"@id":"unece:acceptedTransactionOriginalTotalAmount","@type":["rdf:Property","owl:ObjectProperty"],"rdfs:label":"acceptedTransactionOriginalTotalAmount","schema:rangeIncludes":{"@id":"unece:AmountType"},"schema:domainIncludes":{"@id":"unece:FinancingSummaryDocument"},"rdfs:comment":""},{"@id":"unece:financedAppliedRatePercent","@type":["rdf:Property","owl:DatatypeProperty"],"rdfs:label":"financedAppliedRatePercent","schema:rangeIncludes":{"@id":"schema:Text"},"schema:domainIncludes":{"@id":"unece:FinancingSummaryDocument"},"rdfs:comment":"The financed applied rate, expressed as a percentage, in this financing summary document."},{"@id":"unece:financedTotalAmount","@type":["rdf:Property","owl:ObjectProperty"],"rdfs:label":"financedTotalAmount","schema:rangeIncludes":{"@id":"unece:AmountType"},"schema:domainIncludes":[{"@id":"unece:FinancingSummaryDocument"},{"@id":"unece:FinancingRequestResultDocument"}],"rdfs:comment":""},{"@id":"unece:financedTransactionSpecifiedQuantity","@type":["rdf:Property","owl:ObjectProperty"],"rdfs:label":"financedTransactionSpecifiedQuantity","schema:rangeIncludes":{"@id":"unece:QuantityType"},"schema:domainIncludes":{"@id":"unece:FinancingSummaryDocument"},"rdfs:comment":""},{"@id":"unece:lineOfCreditSpecifiedFinancialAccount","@type":["rdf:Property","owl:ObjectProperty"],"rdfs:label":"lineOfCreditSpecifiedFinancialAccount","schema:rangeIncludes":{"@id":"unece:FinancingFinancialAccount"},"schema:domainIncludes":[{"@id":"unece:FinancingSummaryDocument"},{"@id":"unece:RequestingParty"}],"rdfs:comment":"The financing financial account, used for managing the line of credit, specified for this financing summary document."},{"@id":"unece:relatedBooking","@type":["rdf:Property","owl:ObjectProperty"],"rdfs:label":"relatedBooking","schema:rangeIncludes":{"@id":"unece:Booking"},"schema:domainIncludes":{"@id":"unece:FinancingSummaryDocument"},"rdfs:comment":"The financial booking related to this financing summary document."},{"@id":"unece:specifiedCreditorFinancialAccount","@type":["rdf:Property","owl:ObjectProperty"],"rdfs:label":"specifiedCreditorFinancialAccount","schema:rangeIncludes":{"@id":"unece:CreditorFinancialAccount"},"schema:domainIncludes":[{"@id":"unece:FinancingSummaryDocument"},{"@id":"unece:PaymentMeans"},{"@id":"unece:RequestingParty"}],"rdfs:comment":"A creditor financial account specified for this trade settlement payment means."},{"@id":"unece:accountName","@type":["rdf:Property","owl:DatatypeProperty"],"rdfs:label":"accountName","schema:rangeIncludes":{"@id":"schema:Text"},"schema:domainIncludes":[{"@id":"unece:CreditorFinancialAccount"},{"@id":"unece:DebtorFinancialAccount"},{"@id":"unece:FinancingFinancialAccount"},{"@id":"unece:PaymentFinancialAccount"}],"rdfs:comment":"An account name, expressed as text, of this payment financial account."},{"@id":"unece:bBANId","@type":["rdf:Property","owl:DatatypeProperty"],"rdfs:label":"bBANId","schema:rangeIncludes":{"@id":"schema:Text"},"schema:domainIncludes":[{"@id":"unece:CreditorFinancialAccount"},{"@id":"unece:DebtorFinancialAccount"},{"@id":"unece:FinancingFinancialAccount"}],"rdfs:comment":"The unique Basic Bank Account Number (BBAN) identifier used as part of a National Account Numbering Scheme for this financing financial account."},{"@id":"unece:creditorFinancialAccountTypeCode","@type":["rdf:Property","owl:DatatypeProperty"],"rdfs:label":"creditorFinancialAccountTypeCode","schema:rangeIncludes":{"@id":"schema:Text"},"schema:domainIncludes":{"@id":"unece:CreditorFinancialAccount"},"rdfs:comment":"The code specifying the type of creditor financial account."},{"@id":"unece:currencyCode","@type":["rdf:Property","owl:DatatypeProperty"],"rdfs:label":"currencyCode","schema:rangeIncludes":{"@id":"schema:Text"},"schema:domainIncludes":[{"@id":"unece:CreditorFinancialAccount"},{"@id":"unece:DebtorFinancialAccount"},{"@id":"unece:Cash"},{"@id":"unece:RegisteredTax"}],"rdfs:comment":"The code specifying a currency of this cash used for payment."},{"@id":"unece:iBANId","@type":["rdf:Property","owl:DatatypeProperty"],"rdfs:label":"iBANId","schema:rangeIncludes":{"@id":"schema:Text"},"schema:domainIncludes":[{"@id":"unece:CreditorFinancialAccount"},{"@id":"unece:DebtorFinancialAccount"},{"@id":"unece:FinancingFinancialAccount"},{"@id":"unece:PaymentFinancialAccount"}],"rdfs:comment":"The unique International Bank Account Number (IBAN) identifier for this creditor financial account."},{"@id":"unece:proprietaryId","@type":["rdf:Property","owl:DatatypeProperty"],"rdfs:label":"proprietaryId","schema:rangeIncludes":{"@id":"schema:Text"},"schema:domainIncludes":[{"@id":"unece:CreditorFinancialAccount"},{"@id":"unece:DebtorFinancialAccount"},{"@id":"unece:FinancingFinancialAccount"}],"rdfs:comment":"The proprietary identifier for this financing financial account."},{"@id":"unece:proprietaryType","@type":["rdf:Property","owl:DatatypeProperty"],"rdfs:label":"proprietaryType","schema:rangeIncludes":{"@id":"schema:Text"},"schema:domainIncludes":[{"@id":"unece:CreditorFinancialAccount"},{"@id":"unece:DebtorFinancialAccount"},{"@id":"unece:FinancingFinancialAccount"},{"@id":"unece:Document"}],"rdfs:comment":"A proprietary type, expressed as text, for this referenced document."},{"@id":"unece:uPICId","@type":["rdf:Property","owl:DatatypeProperty"],"rdfs:label":"uPICId","schema:rangeIncludes":{"@id":"schema:Text"},"schema:domainIncludes":[{"@id":"unece:CreditorFinancialAccount"},{"@id":"unece:DebtorFinancialAccount"},{"@id":"unece:FinancingFinancialAccount"}],"rdfs:comment":"The unique Universal Payment Identification Code (UPIC) identifier used by the New York Clearing House for this creditor financial account."},{"@id":"unece:debtorFinancialAccountTypeCode","@type":["rdf:Property","owl:DatatypeProperty"],"rdfs:label":"debtorFinancialAccountTypeCode","schema:rangeIncludes":{"@id":"schema:Text"},"schema:domainIncludes":{"@id":"unece:DebtorFinancialAccount"},"rdfs:comment":"The code specifying the type of debtor financial account."},{"@id":"unece:cashAccountTypeCode","@type":["rdf:Property","owl:DatatypeProperty"],"rdfs:label":"cashAccountTypeCode","schema:rangeIncludes":{"@id":"unece:CashAccountTypeCodeList"},"schema:domainIncludes":{"@id":"unece:FinancingFinancialAccount"},"rdfs:comment":"The code specifying the type of financing financial account."},{"@id":"unece:financingFinancialAccountCurrencyCode","@type":["rdf:Property","owl:DatatypeProperty"],"rdfs:label":"financingFinancialAccountCurrencyCode","schema:rangeIncludes":{"@id":"unece:CurrencyCodeList"},"schema:domainIncludes":{"@id":"unece:FinancingFinancialAccount"},"rdfs:comment":"The code specifying the currency of this financing financial account."},{"@id":"unece:identifier","@type":["rdf:Property","owl:DatatypeProperty"],"rdfs:label":"identifier","schema:rangeIncludes":{"@id":"schema:Text"},"schema:domainIncludes":[{"@id":"unece:PaymentFinancialAccount"},{"@id":"unece:AccountingAccount"},{"@id":"unece:Cheque"},{"@id":"unece:DigitalMethod"},{"@id":"unece:FinancialCard"},{"@id":"unece:PaymentFinancialInstitution"},{"@id":"unece:BreakdownStatement"},{"@id":"unece:HeaderBalanceOut"},{"@id":"unece:PaymentBalanceOut"},{"@id":"unece:BranchFinancialInstitution"},{"@id":"unece:RequestingParty"},{"@id":"unece:BasicWorkItem"},{"@id":"unece:GroupedWorkItem"},{"@id":"unece:Tax"},{"@id":"unece:Voucher"},{"@id":"unece:TradeAllowanceCharge"},{"@id":"unece:Document"},{"@id":"unece:ExchangedDocument"},{"@id":"unece:BinaryFile"},{"@id":"unece:GeographicalCoordinate"},{"@id":"unece:CountrySubDivision"},{"@id":"unece:QuantityAnalysis"},{"@id":"unece:Picture"},{"@id":"unece:SpecifiedMethod"},{"@id":"unece:Location"},{"@id":"unece:CommunicationEvent"},{"@id":"unece:GeographicalGrid"},{"@id":"unece:LegalOrganization"},{"@id":"unece:Object"},{"@id":"unece:GeographicalFeature"},{"@id":"unece:SpecifiedPeriod"},{"@id":"unece:WorkItemDimension"},{"@id":"unece:Project"},{"@id":"unece:Note"},{"@id":"unece:Response"},{"@id":"unece:SpecialQuery"},{"@id":"unece:SpecifiedNote"},{"@id":"unece:MetricCharacteristic"},{"@id":"unece:LegalRegistration"},{"@id":"unece:DocumentCharacteristic"},{"@id":"unece:GeographicalObjectCharacteristic"},{"@id":"unece:Membership"},{"@id":"unece:Schedule"},{"@id":"unece:SpatialDimension"},{"@id":"unece:SpecifiedParameter"},{"@id":"unece:ProprietaryIdentity"},{"@id":"unece:CoordinateReferenceSystem"},{"@id":"unece:CoordinateSourceSystem"},{"@id":"unece:DocumentContextParameter"},{"@id":"unece:EmployerIdentity"},{"@id":"unece:GeopoliticalRegion"},{"@id":"unece:Issue"},{"@id":"unece:Radionuclide"},{"@id":"unece:Section"},{"@id":"unece:Segment"},{"@id":"unece:SubordinateLocation"},{"@id":"unece:SubordinateSubordinateLocation"},{"@id":"unece:Version"},{"@id":"unece:WorkflowObject"},{"@id":"unece:Party"},{"@id":"unece:Authentication"},{"@id":"unece:Clause"},{"@id":"unece:Address"},{"@id":"unece:Event"},{"@id":"unece:SpecificationQuery"},{"@id":"unece:Person"}],"rdfs:comment":"A proprietary identifier."},{"@id":"unece:paymentFinancialAccountCurrencyCode","@type":["rdf:Property","owl:DatatypeProperty"],"rdfs:label":"paymentFinancialAccountCurrencyCode","schema:rangeIncludes":{"@id":"unece:CurrencyCodeList"},"schema:domainIncludes":{"@id":"unece:PaymentFinancialAccount"},"rdfs:comment":"The code specifying the currency of this payment financial account."},{"@id":"unece:accountingAccountTypeCode","@type":["rdf:Property","owl:DatatypeProperty"],"rdfs:label":"accountingAccountTypeCode","schema:rangeIncludes":{"@id":"unece:AccountingAccountTypeCodeList"},"schema:domainIncludes":{"@id":"unece:AccountingAccount"},"rdfs:comment":"The code specifying the type of trade accounting account, such as general (main), secondary, cost accounting or budget account."},{"@id":"unece:accountingAmountTypeAmountTypeCode","@type":["rdf:Property","owl:DatatypeProperty"],"rdfs:label":"accountingAmountTypeAmountTypeCode","schema:rangeIncludes":{"@id":"unece:AccountingAmountTypeCodeList"},"schema:domainIncludes":{"@id":"unece:AccountingAccount"},"rdfs:comment":"The code specifying the amount type for this trade accounting account."},{"@id":"unece:accountingDocumentSetTriggerCode","@type":["rdf:Property","owl:DatatypeProperty"],"rdfs:label":"accountingDocumentSetTriggerCode","schema:rangeIncludes":{"@id":"unece:AccountingDocumentCodeList"},"schema:domainIncludes":{"@id":"unece:AccountingAccount"},"rdfs:comment":"A code specifying a set trigger for this trade accounting account to be used in response to a specific event or a set of events."},{"@id":"unece:costReferenceDimensionPattern","@type":["rdf:Property","owl:DatatypeProperty"],"rdfs:label":"costReferenceDimensionPattern","schema:rangeIncludes":{"@id":"schema:Text"},"schema:domainIncludes":{"@id":"unece:AccountingAccount"},"rdfs:comment":"The cost reference dimension pattern, expressed as text, for this trade accounting account."},{"@id":"unece:name","@type":["rdf:Property","owl:DatatypeProperty"],"rdfs:label":"name","schema:rangeIncludes":{"@id":"schema:Text"},"schema:domainIncludes":[{"@id":"unece:AccountingAccount"},{"@id":"unece:CreditorFinancialInstitution"},{"@id":"unece:DebtorFinancialInstitution"},{"@id":"unece:PaymentFinancialInstitution"},{"@id":"unece:BreakdownStatement"},{"@id":"unece:BranchFinancialInstitution"},{"@id":"unece:RequestingParty"},{"@id":"unece:Document"},{"@id":"unece:ExchangedDocument"},{"@id":"unece:CountrySubDivision"},{"@id":"unece:RadioactiveIsotope"},{"@id":"unece:SpecifiedMethod"},{"@id":"unece:Location"},{"@id":"unece:LegalOrganization"},{"@id":"unece:DirectPosition"},{"@id":"unece:DirectPositionList"},{"@id":"unece:InformationSource"},{"@id":"unece:GeographicalFeature"},{"@id":"unece:SpecifiedPeriod"},{"@id":"unece:Project"},{"@id":"unece:SpecifiedNote"},{"@id":"unece:Country"},{"@id":"unece:DocumentCharacteristic"},{"@id":"unece:GeographicalObjectCharacteristic"},{"@id":"unece:Membership"},{"@id":"unece:SpecifiedLocation"},{"@id":"unece:SpecifiedParameter"},{"@id":"unece:CoordinateReferenceSystem"},{"@id":"unece:GeopoliticalRegion"},{"@id":"unece:Radionuclide"},{"@id":"unece:SubordinateLocation"},{"@id":"unece:SubordinateSubordinateLocation"},{"@id":"unece:Version"},{"@id":"unece:CooperatingOrganization"},{"@id":"unece:Keyword"}],"rdfs:comment":"A name or symbol, expressed as text, of a radioactive radionuclide."},{"@id":"unece:accountingDebitCreditStatusDirectionCode","@type":["rdf:Property","owl:DatatypeProperty"],"rdfs:label":"accountingDebitCreditStatusDirectionCode","schema:rangeIncludes":{"@id":"unece:AccountingDebitCreditStatusCodeList"},"schema:domainIncludes":{"@id":"unece:FinancialAdjustment"},"rdfs:comment":"The code specifying whether the financial adjustment must be subtracted or added."},{"@id":"unece:actualAmount","@type":["rdf:Property","owl:ObjectProperty"],"rdfs:label":"actualAmount","schema:rangeIncludes":{"@id":"unece:AmountType"},"schema:domainIncludes":[{"@id":"unece:FinancialAdjustment"},{"@id":"unece:AppliedAllowanceCharge"},{"@id":"unece:TradeAllowanceCharge"}],"rdfs:comment":""},{"@id":"unece:actualDateTime","@type":["rdf:Property","owl:DatatypeProperty"],"rdfs:label":"actualDateTime","schema:rangeIncludes":{"@id":"schema:Text"},"schema:domainIncludes":[{"@id":"unece:FinancialAdjustment"},{"@id":"unece:Booking"},{"@id":"unece:Authentication"}],"rdfs:comment":"An actual date, time, date time, or other date time value of this financial booking."},{"@id":"unece:actualQuantity","@type":["rdf:Property","owl:ObjectProperty"],"rdfs:label":"actualQuantity","schema:rangeIncludes":{"@id":"unece:QuantityType"},"schema:domainIncludes":[{"@id":"unece:FinancialAdjustment"},{"@id":"unece:QuantityAnalysis"}],"rdfs:comment":""},{"@id":"unece:claimRelatedParty","@type":["rdf:Property","owl:ObjectProperty"],"rdfs:label":"claimRelatedParty","schema:rangeIncludes":{"@id":"unece:Party"},"schema:domainIncludes":{"@id":"unece:FinancialAdjustment"},"rdfs:comment":""},{"@id":"unece:financialAdjustmentReasonCode","@type":["rdf:Property","owl:DatatypeProperty"],"rdfs:label":"financialAdjustmentReasonCode","schema:rangeIncludes":{"@id":"unece:FinancialAdjustmentReasonCodeList"},"schema:domainIncludes":{"@id":"unece:FinancialAdjustment"},"rdfs:comment":"A code specifying a reason for this financial adjustment."},{"@id":"unece:invoiceReferenceDocument","@type":["rdf:Property","owl:ObjectProperty"],"rdfs:label":"invoiceReferenceDocument","schema:rangeIncludes":{"@id":"unece:Document"},"schema:domainIncludes":{"@id":"unece:FinancialAdjustment"},"rdfs:comment":"Written, printed or electronic matter that is referenced."},{"@id":"unece:reason","@type":["rdf:Property","owl:DatatypeProperty"],"rdfs:label":"reason","schema:rangeIncludes":{"@id":"schema:Text"},"schema:domainIncludes":[{"@id":"unece:FinancialAdjustment"},{"@id":"unece:FinancingStatus"},{"@id":"unece:TradeAllowanceCharge"},{"@id":"unece:ValidationStatus"},{"@id":"unece:CancellationStatus"},{"@id":"unece:DocumentStatus"}],"rdfs:comment":"A reason, expressed as text, for this cancellation status."},{"@id":"unece:relatedTax","@type":["rdf:Property","owl:ObjectProperty"],"rdfs:label":"relatedTax","schema:rangeIncludes":{"@id":"unece:Tax"},"schema:domainIncludes":{"@id":"unece:FinancialAdjustment"},"rdfs:comment":"A trade tax related to this financial adjustment."},{"@id":"unece:appliedAllowanceChargeReasonCode","@type":["rdf:Property","owl:DatatypeProperty"],"rdfs:label":"appliedAllowanceChargeReasonCode","schema:rangeIncludes":{"@id":"schema:Text"},"schema:domainIncludes":{"@id":"unece:AppliedAllowanceCharge"},"rdfs:comment":"The code specifying the reason for this applied allowance charge."},{"@id":"unece:basisAmount","@type":["rdf:Property","owl:ObjectProperty"],"rdfs:label":"basisAmount","schema:rangeIncludes":{"@id":"unece:AmountType"},"schema:domainIncludes":[{"@id":"unece:AppliedAllowanceCharge"},{"@id":"unece:PaymentDiscountTerms"},{"@id":"unece:PaymentPenaltyTerms"},{"@id":"unece:AppliedTax"},{"@id":"unece:Tax"},{"@id":"unece:TradeAllowanceCharge"}],"rdfs:comment":""},{"@id":"unece:calculationPercent","@type":["rdf:Property","owl:DatatypeProperty"],"rdfs:label":"calculationPercent","schema:rangeIncludes":{"@id":"schema:Text"},"schema:domainIncludes":[{"@id":"unece:AppliedAllowanceCharge"},{"@id":"unece:PaymentDiscountTerms"},{"@id":"unece:PaymentPenaltyTerms"},{"@id":"unece:TradeAllowanceCharge"},{"@id":"unece:TradePrice"}],"rdfs:comment":"The calculation percentage for this trade price."},{"@id":"unece:categoryAppliedTax","@type":["rdf:Property","owl:ObjectProperty"],"rdfs:label":"categoryAppliedTax","schema:rangeIncludes":{"@id":"unece:AppliedTax"},"schema:domainIncludes":{"@id":"unece:AppliedAllowanceCharge"},"rdfs:comment":"The applied tax category of this applied allowance charge."},{"@id":"unece:chargeIndicator","@type":["rdf:Property","owl:DatatypeProperty"],"rdfs:label":"chargeIndicator","schema:rangeIncludes":{"@id":"schema:Boolean"},"schema:domainIncludes":[{"@id":"unece:AppliedAllowanceCharge"},{"@id":"unece:TradeAllowanceCharge"}],"rdfs:comment":"The indication of whether or not the applied allowance charge is a charge."},{"@id":"unece:description","@type":["rdf:Property","owl:DatatypeProperty"],"rdfs:label":"description","schema:rangeIncludes":{"@id":"schema:Text"},"schema:domainIncludes":[{"@id":"unece:AppliedAllowanceCharge"},{"@id":"unece:Cash"},{"@id":"unece:Cheque"},{"@id":"unece:DigitalMethod"},{"@id":"unece:FinancialCard"},{"@id":"unece:PaymentTerms"},{"@id":"unece:BreakdownStatement"},{"@id":"unece:HeaderBalanceOut"},{"@id":"unece:PaymentBalanceOut"},{"@id":"unece:Guarantee"},{"@id":"unece:RegisteredTax"},{"@id":"unece:RequestingParty"},{"@id":"unece:Tax"},{"@id":"unece:Voucher"},{"@id":"unece:TradeAllowanceCharge"},{"@id":"unece:TradePrice"},{"@id":"unece:Document"},{"@id":"unece:ExchangedDocument"},{"@id":"unece:BinaryFile"},{"@id":"unece:SpecifiedAction"},{"@id":"unece:Measurement"},{"@id":"unece:QuantityAnalysis"},{"@id":"unece:SpecifiedFault"},{"@id":"unece:Picture"},{"@id":"unece:UsageCondition"},{"@id":"unece:Location"},{"@id":"unece:CommunicationEvent"},{"@id":"unece:CustomerClass"},{"@id":"unece:InformationSource"},{"@id":"unece:GeographicalFeature"},{"@id":"unece:Communication"},{"@id":"unece:SpecifiedPeriod"},{"@id":"unece:WorkItemDimension"},{"@id":"unece:DocumentStatus"},{"@id":"unece:Project"},{"@id":"unece:SpecifiedNote"},{"@id":"unece:MetricCharacteristic"},{"@id":"unece:AvailablePeriod"},{"@id":"unece:DocumentCharacteristic"},{"@id":"unece:GeographicalObjectCharacteristic"},{"@id":"unece:IdentifiedFault"},{"@id":"unece:Membership"},{"@id":"unece:Schedule"},{"@id":"unece:SpatialDimension"},{"@id":"unece:SpecifiedFeature"},{"@id":"unece:SpecifiedLocation"},{"@id":"unece:SpecifiedParameter"},{"@id":"unece:Address"},{"@id":"unece:Event"}],"rdfs:comment":"A textual description for the type of transportation waste recovery disposal process."},{"@id":"unece:creditDateTime","@type":["rdf:Property","owl:DatatypeProperty"],"rdfs:label":"creditDateTime","schema:rangeIncludes":{"@id":"schema:DateTime"},"schema:domainIncludes":{"@id":"unece:Booking"},"rdfs:comment":"The credit date, time, date time, or other date time value of this financial booking."},{"@id":"unece:debitDateTime","@type":["rdf:Property","owl:DatatypeProperty"],"rdfs:label":"debitDateTime","schema:rangeIncludes":{"@id":"schema:DateTime"},"schema:domainIncludes":{"@id":"unece:Booking"},"rdfs:comment":"The debit date, time, date time, or other date time value of this financial booking."},{"@id":"unece:actualDiscountAmount","@type":["rdf:Property","owl:ObjectProperty"],"rdfs:label":"actualDiscountAmount","schema:rangeIncludes":{"@id":"unece:AmountType"},"schema:domainIncludes":{"@id":"unece:PaymentDiscountTerms"},"rdfs:comment":""},{"@id":"unece:basisDateTime","@type":["rdf:Property","owl:DatatypeProperty"],"rdfs:label":"basisDateTime","schema:rangeIncludes":{"@id":"schema:Text"},"schema:domainIncludes":[{"@id":"unece:PaymentDiscountTerms"},{"@id":"unece:PaymentPenaltyTerms"},{"@id":"unece:TradePrice"}],"rdfs:comment":"The date, time, date time, or other date time value used as the basis for this trade price."},{"@id":"unece:basisPeriodMeasure","@type":["rdf:Property","owl:ObjectProperty"],"rdfs:label":"basisPeriodMeasure","schema:rangeIncludes":{"@id":"unece:MeasureType"},"schema:domainIncludes":[{"@id":"unece:PaymentDiscountTerms"},{"@id":"unece:PaymentPenaltyTerms"}],"rdfs:comment":""},{"@id":"unece:actualPenaltyAmount","@type":["rdf:Property","owl:ObjectProperty"],"rdfs:label":"actualPenaltyAmount","schema:rangeIncludes":{"@id":"unece:AmountType"},"schema:domainIncludes":{"@id":"unece:PaymentPenaltyTerms"},"rdfs:comment":""},{"@id":"unece:additionalClearingSystemId","@type":["rdf:Property","owl:DatatypeProperty"],"rdfs:label":"additionalClearingSystemId","schema:rangeIncludes":{"@id":"schema:Text"},"schema:domainIncludes":{"@id":"unece:CreditorFinancialInstitution"},"rdfs:comment":"An additional clearing system identifier for this creditor financial institution."},{"@id":"unece:australianBSBId","@type":["rdf:Property","owl:DatatypeProperty"],"rdfs:label":"australianBSBId","schema:rangeIncludes":{"@id":"schema:Text"},"schema:domainIncludes":[{"@id":"unece:CreditorFinancialInstitution"},{"@id":"unece:DebtorFinancialInstitution"}],"rdfs:comment":"The unique Australian Bank State Branch (BSB) Code identifier as assigned by the Australian Payments Clearing Association (APCA) for this creditor financial institution."},{"@id":"unece:australianSNId","@type":["rdf:Property","owl:DatatypeProperty"],"rdfs:label":"australianSNId","schema:rangeIncludes":{"@id":"schema:Text"},"schema:domainIncludes":{"@id":"unece:CreditorFinancialInstitution"},"rdfs:comment":"The Australian Small Network (SN) identifier as assigned by the Australian Payments Clearing Association (APCA) for this creditor financial institution."},{"@id":"unece:austrianBankleitzahlId","@type":["rdf:Property","owl:DatatypeProperty"],"rdfs:label":"austrianBankleitzahlId","schema:rangeIncludes":{"@id":"schema:Text"},"schema:domainIncludes":[{"@id":"unece:CreditorFinancialInstitution"},{"@id":"unece:DebtorFinancialInstitution"}],"rdfs:comment":"The unique Austrian Bankleitzahl identifier for this creditor financial institution."},{"@id":"unece:bICId","@type":["rdf:Property","owl:DatatypeProperty"],"rdfs:label":"bICId","schema:rangeIncludes":{"@id":"schema:Text"},"schema:domainIncludes":[{"@id":"unece:CreditorFinancialInstitution"},{"@id":"unece:FinancialIdentity"},{"@id":"unece:DebtorFinancialInstitution"},{"@id":"unece:PaymentFinancialInstitution"}],"rdfs:comment":"The Bank Identifier Code (BIC) as defined by ISO 9362 (Banking telecommunication messages, Bank Identifier Codes) for this financial identity."},{"@id":"unece:cHIPSParticipantId","@type":["rdf:Property","owl:DatatypeProperty"],"rdfs:label":"cHIPSParticipantId","schema:rangeIncludes":{"@id":"schema:Text"},"schema:domainIncludes":[{"@id":"unece:CreditorFinancialInstitution"},{"@id":"unece:DebtorFinancialInstitution"}],"rdfs:comment":"The unique (United States) Clearing House Interbank Payment System (CHIPS) Participant Identifier (ID) as assigned by the New York Clearing House for this creditor financial institution."},{"@id":"unece:cHIPSUniversalId","@type":["rdf:Property","owl:DatatypeProperty"],"rdfs:label":"cHIPSUniversalId","schema:rangeIncludes":{"@id":"schema:Text"},"schema:domainIncludes":[{"@id":"unece:CreditorFinancialInstitution"},{"@id":"unece:FinancialIdentity"},{"@id":"unece:DebtorFinancialInstitution"}],"rdfs:comment":"The (United States) Clearing House Interbank Payments System (CHIPS) Universal Identification (UID) as assigned by the New York Clearing House for this financial identity."},{"@id":"unece:canadianPaymentsAssociationId","@type":["rdf:Property","owl:DatatypeProperty"],"rdfs:label":"canadianPaymentsAssociationId","schema:rangeIncludes":{"@id":"schema:Text"},"schema:domainIncludes":[{"@id":"unece:CreditorFinancialInstitution"},{"@id":"unece:DebtorFinancialInstitution"}],"rdfs:comment":"The unique Canadian Payments Association Routing Number identifier for this creditor financial institution."},{"@id":"unece:clearingSystemName","@type":["rdf:Property","owl:DatatypeProperty"],"rdfs:label":"clearingSystemName","schema:rangeIncludes":{"@id":"schema:Text"},"schema:domainIncludes":[{"@id":"unece:CreditorFinancialInstitution"},{"@id":"unece:DebtorFinancialInstitution"}],"rdfs:comment":"The clearing system name, expressed as text, for this creditor financial institution."},{"@id":"unece:fedwireRoutingNumberId","@type":["rdf:Property","owl:DatatypeProperty"],"rdfs:label":"fedwireRoutingNumberId","schema:rangeIncludes":{"@id":"schema:Text"},"schema:domainIncludes":[{"@id":"unece:CreditorFinancialInstitution"},{"@id":"unece:DebtorFinancialInstitution"}],"rdfs:comment":"The unique Fedwire Routing Number identifier as assigned by the American Bankers Association (ABA) for this creditor financial institution."},{"@id":"unece:germanBankleitzahlId","@type":["rdf:Property","owl:DatatypeProperty"],"rdfs:label":"germanBankleitzahlId","schema:rangeIncludes":{"@id":"schema:Text"},"schema:domainIncludes":[{"@id":"unece:CreditorFinancialInstitution"},{"@id":"unece:DebtorFinancialInstitution"}],"rdfs:comment":"The unique German Bankleitzahl identifier for this creditor financial institution."},{"@id":"unece:hellenicBankId","@type":["rdf:Property","owl:DatatypeProperty"],"rdfs:label":"hellenicBankId","schema:rangeIncludes":{"@id":"schema:Text"},"schema:domainIncludes":[{"@id":"unece:CreditorFinancialInstitution"},{"@id":"unece:DebtorFinancialInstitution"}],"rdfs:comment":"The unique Hellenic Bank Identification Code identifier for this creditor financial institution."},{"@id":"unece:hongKongBankId","@type":["rdf:Property","owl:DatatypeProperty"],"rdfs:label":"hongKongBankId","schema:rangeIncludes":{"@id":"schema:Text"},"schema:domainIncludes":[{"@id":"unece:CreditorFinancialInstitution"},{"@id":"unece:DebtorFinancialInstitution"}],"rdfs:comment":"The unique Hong Kong Bank Code identifier for this creditor financial institution."},{"@id":"unece:indianFinancialSystemId","@type":["rdf:Property","owl:DatatypeProperty"],"rdfs:label":"indianFinancialSystemId","schema:rangeIncludes":{"@id":"schema:Text"},"schema:domainIncludes":[{"@id":"unece:CreditorFinancialInstitution"},{"@id":"unece:DebtorFinancialInstitution"}],"rdfs:comment":"The unique Indian Financial System Code identifier for this creditor financial institution."},{"@id":"unece:irishNSCId","@type":["rdf:Property","owl:DatatypeProperty"],"rdfs:label":"irishNSCId","schema:rangeIncludes":{"@id":"schema:Text"},"schema:domainIncludes":[{"@id":"unece:CreditorFinancialInstitution"},{"@id":"unece:DebtorFinancialInstitution"}],"rdfs:comment":"The unique Irish National Sorting Code (NSC) identifier as assigned by the Irish Payments Services Organisation (IPSO) for this creditor financial institution."},{"@id":"unece:italianDomesticId","@type":["rdf:Property","owl:DatatypeProperty"],"rdfs:label":"italianDomesticId","schema:rangeIncludes":{"@id":"schema:Text"},"schema:domainIncludes":[{"@id":"unece:CreditorFinancialInstitution"},{"@id":"unece:DebtorFinancialInstitution"}],"rdfs:comment":"The unique Italian Domestic Identification Code identifier as assigned by the Associazione Bancaria Italiana (ABI) for this creditor financial institution."},{"@id":"unece:japanFinancialInstitutionCommonId","@type":["rdf:Property","owl:DatatypeProperty"],"rdfs:label":"japanFinancialInstitutionCommonId","schema:rangeIncludes":{"@id":"schema:Text"},"schema:domainIncludes":[{"@id":"unece:CreditorFinancialInstitution"},{"@id":"unece:DebtorFinancialInstitution"}],"rdfs:comment":"The Japan Financial Institution Common identifier as assigned by the Japanese Bankers Association for this creditor financial institution."},{"@id":"unece:locationAddress","@type":["rdf:Property","owl:ObjectProperty"],"rdfs:label":"locationAddress","schema:rangeIncludes":{"@id":"unece:FinancialInstitutionAddress"},"schema:domainIncludes":[{"@id":"unece:CreditorFinancialInstitution"},{"@id":"unece:DebtorFinancialInstitution"},{"@id":"unece:BranchFinancialInstitution"}],"rdfs:comment":"The location address for this branch of a financial institution."},{"@id":"unece:newZealandNCCId","@type":["rdf:Property","owl:DatatypeProperty"],"rdfs:label":"newZealandNCCId","schema:rangeIncludes":{"@id":"schema:Text"},"schema:domainIncludes":[{"@id":"unece:CreditorFinancialInstitution"},{"@id":"unece:DebtorFinancialInstitution"}],"rdfs:comment":"The unique New Zealand National Clearing Code (NCC) identifier as assigned by the New Zealand Bankers' Association (NZBA) for this creditor financial institution."},{"@id":"unece:polishNationalClearingId","@type":["rdf:Property","owl:DatatypeProperty"],"rdfs:label":"polishNationalClearingId","schema:rangeIncludes":{"@id":"schema:Text"},"schema:domainIncludes":[{"@id":"unece:CreditorFinancialInstitution"},{"@id":"unece:DebtorFinancialInstitution"}],"rdfs:comment":"The unique Polish National Clearing Code identifier for this creditor financial institution."},{"@id":"unece:portugueseNCCId","@type":["rdf:Property","owl:DatatypeProperty"],"rdfs:label":"portugueseNCCId","schema:rangeIncludes":{"@id":"schema:Text"},"schema:domainIncludes":[{"@id":"unece:CreditorFinancialInstitution"},{"@id":"unece:DebtorFinancialInstitution"}],"rdfs:comment":"The unique Portuguese National Clearing Code (NCC) identifier for this creditor financial institution."},{"@id":"unece:russianCentralBankId","@type":["rdf:Property","owl:DatatypeProperty"],"rdfs:label":"russianCentralBankId","schema:rangeIncludes":{"@id":"schema:Text"},"schema:domainIncludes":[{"@id":"unece:CreditorFinancialInstitution"},{"@id":"unece:DebtorFinancialInstitution"}],"rdfs:comment":"The unique Russian Central Bank Identification Code identifier for this creditor financial institution."},{"@id":"unece:sICId","@type":["rdf:Property","owl:DatatypeProperty"],"rdfs:label":"sICId","schema:rangeIncludes":{"@id":"schema:Text"},"schema:domainIncludes":[{"@id":"unece:CreditorFinancialInstitution"},{"@id":"unece:DebtorFinancialInstitution"}],"rdfs:comment":"The unique Swiss Interbank Clearing (SIC) Code identifier for this creditor financial institution."},{"@id":"unece:southAfricanNCCId","@type":["rdf:Property","owl:DatatypeProperty"],"rdfs:label":"southAfricanNCCId","schema:rangeIncludes":{"@id":"schema:Text"},"schema:domainIncludes":[{"@id":"unece:CreditorFinancialInstitution"},{"@id":"unece:DebtorFinancialInstitution"}],"rdfs:comment":"The unique South African National Clearing Code (NCC) identifier as assigned by the South African Bankers Services Company Ltd. (BankServ) for this creditor financial institution."},{"@id":"unece:spanishDomesticInterbankingId","@type":["rdf:Property","owl:DatatypeProperty"],"rdfs:label":"spanishDomesticInterbankingId","schema:rangeIncludes":{"@id":"schema:Text"},"schema:domainIncludes":[{"@id":"unece:CreditorFinancialInstitution"},{"@id":"unece:DebtorFinancialInstitution"}],"rdfs:comment":"The unique Spanish Domestic Interbanking Code identifier as assigned by the Centro de Cooperacion Interbancaria (CCI) for this creditor financial institution."},{"@id":"unece:specifiedProprietaryIdentity","@type":["rdf:Property","owl:ObjectProperty"],"rdfs:label":"specifiedProprietaryIdentity","schema:rangeIncludes":{"@id":"unece:ProprietaryIdentity"},"schema:domainIncludes":[{"@id":"unece:CreditorFinancialInstitution"},{"@id":"unece:RequestingParty"},{"@id":"unece:PersonIdentity"}],"rdfs:comment":"Proprietary information which uniquely identifies a person or organization."},{"@id":"unece:subDivisionFinancialInstitution","@type":["rdf:Property","owl:ObjectProperty"],"rdfs:label":"subDivisionFinancialInstitution","schema:rangeIncludes":{"@id":"unece:BranchFinancialInstitution"},"schema:domainIncludes":[{"@id":"unece:CreditorFinancialInstitution"},{"@id":"unece:DebtorFinancialInstitution"}],"rdfs:comment":"The branch financial institution for this creditor financial institution."},{"@id":"unece:swissBCId","@type":["rdf:Property","owl:DatatypeProperty"],"rdfs:label":"swissBCId","schema:rangeIncludes":{"@id":"schema:Text"},"schema:domainIncludes":[{"@id":"unece:CreditorFinancialInstitution"},{"@id":"unece:DebtorFinancialInstitution"}],"rdfs:comment":"The unique Swiss Bank Code (BC) identifier for this creditor financial institution."},{"@id":"unece:uKSortCodeId","@type":["rdf:Property","owl:DatatypeProperty"],"rdfs:label":"uKSortCodeId","schema:rangeIncludes":{"@id":"schema:Text"},"schema:domainIncludes":[{"@id":"unece:CreditorFinancialInstitution"},{"@id":"unece:DebtorFinancialInstitution"}],"rdfs:comment":"The unique United Kingdom (UK) Sort Code identifier as assigned by the UK Payment Association (APACS) for this creditor financial institution."},{"@id":"unece:additionalInformationIncludedNote","@type":["rdf:Property","owl:ObjectProperty"],"rdfs:label":"additionalInformationIncludedNote","schema:rangeIncludes":{"@id":"unece:Note"},"schema:domainIncludes":{"@id":"unece:FinancingRequestDocument"},"rdfs:comment":"A textual or coded description, such as a remark or additional information."},{"@id":"unece:agreementInformation","@type":["rdf:Property","owl:DatatypeProperty"],"rdfs:label":"agreementInformation","schema:rangeIncludes":{"@id":"schema:Text"},"schema:domainIncludes":{"@id":"unece:FinancingRequestDocument"},"rdfs:comment":"Agreement information, expressed as text, in this financing request document, such as a collection mandate."},{"@id":"unece:authorization","@type":["rdf:Property","owl:DatatypeProperty"],"rdfs:label":"authorization","schema:rangeIncludes":{"@id":"schema:Text"},"schema:domainIncludes":{"@id":"unece:FinancingRequestDocument"},"rdfs:comment":"An authorization, expressed as text, for this financing request document."},{"@id":"unece:cancellationReason","@type":["rdf:Property","owl:DatatypeProperty"],"rdfs:label":"cancellationReason","schema:rangeIncludes":{"@id":"schema:Text"},"schema:domainIncludes":{"@id":"unece:FinancingRequestDocument"},"rdfs:comment":"A cancellation reason, expressed as text, in this financing request document."},{"@id":"unece:contractualClause","@type":["rdf:Property","owl:ObjectProperty"],"rdfs:label":"contractualClause","schema:rangeIncludes":{"@id":"unece:Clause"},"schema:domainIncludes":[{"@id":"unece:FinancingRequestDocument"},{"@id":"unece:Document"},{"@id":"unece:ExchangedDocument"}],"rdfs:comment":"A distinct article or provision in a document, which requires compliance."},{"@id":"unece:copyIndicator","@type":["rdf:Property","owl:DatatypeProperty"],"rdfs:label":"copyIndicator","schema:rangeIncludes":{"@id":"schema:Boolean"},"schema:domainIncludes":[{"@id":"unece:FinancingRequestDocument"},{"@id":"unece:Document"},{"@id":"unece:ExchangedDocument"}],"rdfs:comment":"The indication of whether or not the referenced document is a copy."},{"@id":"unece:financingRequestDocumentCurrencyCode","@type":["rdf:Property","owl:DatatypeProperty"],"rdfs:label":"financingRequestDocumentCurrencyCode","schema:rangeIncludes":{"@id":"unece:CurrencyCodeList"},"schema:domainIncludes":{"@id":"unece:FinancingRequestDocument"},"rdfs:comment":"The code specifying the currency in this financing request document."},{"@id":"unece:firstAgentSpecifiedFinancialInstitution","@type":["rdf:Property","owl:ObjectProperty"],"rdfs:label":"firstAgentSpecifiedFinancialInstitution","schema:rangeIncludes":{"@id":"unece:CreditorFinancialInstitution"},"schema:domainIncludes":{"@id":"unece:FinancingRequestDocument"},"rdfs:comment":"The creditor financial institution specified as the first agent in this financing request document."},{"@id":"unece:groupId","@type":["rdf:Property","owl:DatatypeProperty"],"rdfs:label":"groupId","schema:rangeIncludes":{"@id":"schema:Text"},"schema:domainIncludes":{"@id":"unece:FinancingRequestDocument"},"rdfs:comment":"The group identifier in this financing request document."},{"@id":"unece:groupedTransactionSpecifiedQuantity","@type":["rdf:Property","owl:ObjectProperty"],"rdfs:label":"groupedTransactionSpecifiedQuantity","schema:rangeIncludes":{"@id":"unece:QuantityType"},"schema:domainIncludes":{"@id":"unece:FinancingRequestDocument"},"rdfs:comment":""},{"@id":"unece:groupedTransactionTotalAmount","@type":["rdf:Property","owl:ObjectProperty"],"rdfs:label":"groupedTransactionTotalAmount","schema:rangeIncludes":{"@id":"unece:AmountType"},"schema:domainIncludes":{"@id":"unece:FinancingRequestDocument"},"rdfs:comment":""},{"@id":"unece:intermediarySpecifiedFinancialInstitution","@type":["rdf:Property","owl:ObjectProperty"],"rdfs:label":"intermediarySpecifiedFinancialInstitution","schema:rangeIncludes":{"@id":"unece:CreditorFinancialInstitution"},"schema:domainIncludes":{"@id":"unece:FinancingRequestDocument"},"rdfs:comment":"The creditor financial institution specified as the intermediary in this financing request document."},{"@id":"unece:specifiedCancellationStatus","@type":["rdf:Property","owl:ObjectProperty"],"rdfs:label":"specifiedCancellationStatus","schema:rangeIncludes":{"@id":"unece:CancellationStatus"},"schema:domainIncludes":{"@id":"unece:FinancingRequestDocument"},"rdfs:comment":"Information relevant to a condition of a cancellation."},{"@id":"unece:specifiedRequestingParty","@type":["rdf:Property","owl:ObjectProperty"],"rdfs:label":"specifiedRequestingParty","schema:rangeIncludes":{"@id":"unece:RequestingParty"},"schema:domainIncludes":{"@id":"unece:FinancingRequestDocument"},"rdfs:comment":"The requesting party specified in this financing request document."},{"@id":"unece:specifiedValidationStatus","@type":["rdf:Property","owl:ObjectProperty"],"rdfs:label":"specifiedValidationStatus","schema:rangeIncludes":{"@id":"unece:ValidationStatus"},"schema:domainIncludes":{"@id":"unece:FinancingRequestDocument"},"rdfs:comment":"Information relevant to a condition of a validation."},{"@id":"unece:agentAssignedCustomerId","@type":["rdf:Property","owl:DatatypeProperty"],"rdfs:label":"agentAssignedCustomerId","schema:rangeIncludes":{"@id":"schema:Text"},"schema:domainIncludes":{"@id":"unece:FinancialIdentity"},"rdfs:comment":"The agent assigned customer identifier for this financial identity."},{"@id":"unece:bEIId","@type":["rdf:Property","owl:DatatypeProperty"],"rdfs:label":"bEIId","schema:rangeIncludes":{"@id":"schema:Text"},"schema:domainIncludes":[{"@id":"unece:FinancialIdentity"},{"@id":"unece:PaymentFinancialInstitution"},{"@id":"unece:RequestingParty"}],"rdfs:comment":"The Business Entity Identifier (BEI) as defined by ISO 9362 (Banking telecommunication messages, Bank Identifier Codes) for this financial identity."},{"@id":"unece:bankAssignedId","@type":["rdf:Property","owl:DatatypeProperty"],"rdfs:label":"bankAssignedId","schema:rangeIncludes":{"@id":"schema:Text"},"schema:domainIncludes":{"@id":"unece:FinancialIdentity"},"rdfs:comment":"The bank assigned identifier for this financial identity."},{"@id":"unece:iBEIId","@type":["rdf:Property","owl:DatatypeProperty"],"rdfs:label":"iBEIId","schema:rangeIncludes":{"@id":"schema:Text"},"schema:domainIncludes":{"@id":"unece:FinancialIdentity"},"rdfs:comment":"The International Business Entity Identifier (IBEI) for this financial identity."},{"@id":"unece:applicableFinancialCard","@type":["rdf:Property","owl:ObjectProperty"],"rdfs:label":"applicableFinancialCard","schema:rangeIncludes":{"@id":"unece:FinancialCard"},"schema:domainIncludes":{"@id":"unece:PaymentMeans"},"rdfs:comment":"A financial card applicable to this trade settlement payment means."},{"@id":"unece:creditorSpecifiedFinancialInstitution","@type":["rdf:Property","owl:ObjectProperty"],"rdfs:label":"creditorSpecifiedFinancialInstitution","schema:rangeIncludes":{"@id":"unece:PaymentFinancialInstitution"},"schema:domainIncludes":{"@id":"unece:PaymentMeans"},"rdfs:comment":"A creditor financial institution specified for this trade settlement payment means."},{"@id":"unece:debtorSpecifiedFinancialInstitution","@type":["rdf:Property","owl:ObjectProperty"],"rdfs:label":"debtorSpecifiedFinancialInstitution","schema:rangeIncludes":{"@id":"unece:PaymentFinancialInstitution"},"schema:domainIncludes":{"@id":"unece:PaymentMeans"},"rdfs:comment":"A debtor financial institution specified for this trade settlement payment means."},{"@id":"unece:identifiedCash","@type":["rdf:Property","owl:ObjectProperty"],"rdfs:label":"identifiedCash","schema:rangeIncludes":{"@id":"unece:Cash"},"schema:domainIncludes":{"@id":"unece:PaymentMeans"},"rdfs:comment":"A cash payment identified for this trade settlement payment means."},{"@id":"unece:identifiedCheque","@type":["rdf:Property","owl:ObjectProperty"],"rdfs:label":"identifiedCheque","schema:rangeIncludes":{"@id":"unece:Cheque"},"schema:domainIncludes":{"@id":"unece:PaymentMeans"},"rdfs:comment":"A cheque payment identified for this trade settlement payment means."},{"@id":"unece:identifiedDigitalMethod","@type":["rdf:Property","owl:ObjectProperty"],"rdfs:label":"identifiedDigitalMethod","schema:rangeIncludes":{"@id":"unece:DigitalMethod"},"schema:domainIncludes":{"@id":"unece:PaymentMeans"},"rdfs:comment":"A digital payment method identified for this trade settlement payment means."},{"@id":"unece:identifiedFinancialCard","@type":["rdf:Property","owl:ObjectProperty"],"rdfs:label":"identifiedFinancialCard","schema:rangeIncludes":{"@id":"unece:FinancialCard"},"schema:domainIncludes":{"@id":"unece:PaymentMeans"},"rdfs:comment":"A financial card identified for this trade settlement payment means."},{"@id":"unece:identifiedVoucher","@type":["rdf:Property","owl:ObjectProperty"],"rdfs:label":"identifiedVoucher","schema:rangeIncludes":{"@id":"unece:Voucher"},"schema:domainIncludes":{"@id":"unece:PaymentMeans"},"rdfs:comment":"An experience item voucher identified for this trade settlement payment means."},{"@id":"unece:information","@type":["rdf:Property","owl:DatatypeProperty"],"rdfs:label":"information","schema:rangeIncludes":{"@id":"schema:Text"},"schema:domainIncludes":[{"@id":"unece:PaymentMeans"},{"@id":"unece:TradePrice"},{"@id":"unece:Document"},{"@id":"unece:ExchangedDocument"},{"@id":"unece:SpecifiedMethod"},{"@id":"unece:DocumentStatus"},{"@id":"unece:Segment"},{"@id":"unece:Tolerance"},{"@id":"unece:Authentication"}],"rdfs:comment":"Information, expressed as text, concerning the transport of these dangerous goods."},{"@id":"unece:payeePartyFinancialAccount","@type":["rdf:Property","owl:ObjectProperty"],"rdfs:label":"payeePartyFinancialAccount","schema:rangeIncludes":{"@id":"unece:CreditorFinancialAccount"},"schema:domainIncludes":{"@id":"unece:PaymentMeans"},"rdfs:comment":"A creditor financial account of the payee party for this trade settlement payment means."},{"@id":"unece:payeeSpecifiedFinancialInstitution","@type":["rdf:Property","owl:ObjectProperty"],"rdfs:label":"payeeSpecifiedFinancialInstitution","schema:rangeIncludes":{"@id":"unece:CreditorFinancialInstitution"},"schema:domainIncludes":{"@id":"unece:PaymentMeans"},"rdfs:comment":"The creditor financial institution of the payee party specified for this trade settlement payment means."},{"@id":"unece:payerPartyFinancialAccount","@type":["rdf:Property","owl:ObjectProperty"],"rdfs:label":"payerPartyFinancialAccount","schema:rangeIncludes":{"@id":"unece:DebtorFinancialAccount"},"schema:domainIncludes":{"@id":"unece:PaymentMeans"},"rdfs:comment":"The debtor financial account of the payer party for this trade settlement payment means."},{"@id":"unece:payerSpecifiedFinancialInstitution","@type":["rdf:Property","owl:ObjectProperty"],"rdfs:label":"payerSpecifiedFinancialInstitution","schema:rangeIncludes":{"@id":"unece:DebtorFinancialInstitution"},"schema:domainIncludes":{"@id":"unece:PaymentMeans"},"rdfs:comment":"The debtor financial institution of the payer party specified for this trade settlement payment means."},{"@id":"unece:paymentGuaranteeMeansGuaranteeMethodCode","@type":["rdf:Property","owl:DatatypeProperty"],"rdfs:label":"paymentGuaranteeMeansGuaranteeMethodCode","schema:rangeIncludes":{"@id":"unece:PaymentGuaranteeMeansCodeList"},"schema:domainIncludes":{"@id":"unece:PaymentMeans"},"rdfs:comment":"The code specifying the method of guarantee for this trade settlement payment means."},{"@id":"unece:paymentMeansChannelPaymentChannelCode","@type":["rdf:Property","owl:DatatypeProperty"],"rdfs:label":"paymentMeansChannelPaymentChannelCode","schema:rangeIncludes":{"@id":"unece:PaymentMeansChannelCodeList"},"schema:domainIncludes":{"@id":"unece:PaymentMeans"},"rdfs:comment":"The code specifying the payment channel through which this trade settlement payment is to be processed (Reference United Nations Code List (UNCL) 4435)."},{"@id":"unece:paymentMeansTypeCode","@type":["rdf:Property","owl:DatatypeProperty"],"rdfs:label":"paymentMeansTypeCode","schema:rangeIncludes":{"@id":"unece:PaymentMeansCodeList"},"schema:domainIncludes":{"@id":"unece:PaymentMeans"},"rdfs:comment":"The code specifying the type of trade settlement payment means, such as cash or check."},{"@id":"unece:paymentMethodCode","@type":["rdf:Property","owl:DatatypeProperty"],"rdfs:label":"paymentMethodCode","schema:rangeIncludes":{"@id":"schema:Text"},"schema:domainIncludes":{"@id":"unece:PaymentMeans"},"rdfs:comment":"The code specifying the method by which a payment may be made for this trade settlement payment means."},{"@id":"unece:specifiedPaymentFinancialInstitution","@type":["rdf:Property","owl:ObjectProperty"],"rdfs:label":"specifiedPaymentFinancialInstitution","schema:rangeIncludes":{"@id":"unece:PaymentFinancialInstitution"},"schema:domainIncludes":{"@id":"unece:PaymentMeans"},"rdfs:comment":"A financial institution specified for this trade settlement payment means."},{"@id":"unece:tradeSettlementPaymentMeansId","@type":["rdf:Property","owl:DatatypeProperty"],"rdfs:label":"tradeSettlementPaymentMeansId","schema:rangeIncludes":{"@id":"schema:Text"},"schema:domainIncludes":{"@id":"unece:PaymentMeans"},"rdfs:comment":"An identifier for this trade settlement payment means."},{"@id":"unece:applicableIndicator","@type":["rdf:Property","owl:DatatypeProperty"],"rdfs:label":"applicableIndicator","schema:rangeIncludes":{"@id":"schema:Boolean"},"schema:domainIncludes":[{"@id":"unece:Cash"},{"@id":"unece:Cheque"},{"@id":"unece:DigitalMethod"},{"@id":"unece:FinancialCard"},{"@id":"unece:Voucher"}],"rdfs:comment":"The indication of whether or not this cash used for payment. is applicable."},{"@id":"unece:clearingRegion","@type":["rdf:Property","owl:DatatypeProperty"],"rdfs:label":"clearingRegion","schema:rangeIncludes":{"@id":"schema:Text"},"schema:domainIncludes":{"@id":"unece:Cheque"},"rdfs:comment":"The clearing region, expressed as text, for this payment cheque."},{"@id":"unece:deliveryMethod","@type":["rdf:Property","owl:DatatypeProperty"],"rdfs:label":"deliveryMethod","schema:rangeIncludes":{"@id":"schema:Text"},"schema:domainIncludes":{"@id":"unece:Cheque"},"rdfs:comment":"The delivery method, expressed as text, for this payment cheque."},{"@id":"unece:deliveryMethodCode","@type":["rdf:Property","owl:DatatypeProperty"],"rdfs:label":"deliveryMethodCode","schema:rangeIncludes":{"@id":"schema:Text"},"schema:domainIncludes":{"@id":"unece:Cheque"},"rdfs:comment":"The code specifying the delivery method for this payment cheque."},{"@id":"unece:instructionPriorityCode","@type":["rdf:Property","owl:DatatypeProperty"],"rdfs:label":"instructionPriorityCode","schema:rangeIncludes":{"@id":"schema:Text"},"schema:domainIncludes":{"@id":"unece:Cheque"},"rdfs:comment":"The code specifying the instruction priority for this payment cheque, such as the urgency or order of importance for the processing of the payment cheque."},{"@id":"unece:layoutDescription","@type":["rdf:Property","owl:DatatypeProperty"],"rdfs:label":"layoutDescription","schema:rangeIncludes":{"@id":"schema:Text"},"schema:domainIncludes":{"@id":"unece:Cheque"},"rdfs:comment":"The textual description of the layout for this payment cheque, such as a description of the company logo and digitized signature printed on the cheque."},{"@id":"unece:maturityDateTime","@type":["rdf:Property","owl:DatatypeProperty"],"rdfs:label":"maturityDateTime","schema:rangeIncludes":{"@id":"schema:Text"},"schema:domainIncludes":{"@id":"unece:Cheque"},"rdfs:comment":"The date, time, date time, or other date time value when this payment cheque reaches maturity."},{"@id":"unece:memoField","@type":["rdf:Property","owl:DatatypeProperty"],"rdfs:label":"memoField","schema:rangeIncludes":{"@id":"schema:Text"},"schema:domainIncludes":{"@id":"unece:Cheque"},"rdfs:comment":"The memo field, expressed as text, on this payment check."},{"@id":"unece:number","@type":["rdf:Property","owl:DatatypeProperty"],"rdfs:label":"number","schema:rangeIncludes":{"@id":"schema:Text"},"schema:domainIncludes":{"@id":"unece:Cheque"},"rdfs:comment":"The number, expressed as text, of this payment cheque."},{"@id":"unece:printLocation","@type":["rdf:Property","owl:DatatypeProperty"],"rdfs:label":"printLocation","schema:rangeIncludes":{"@id":"schema:Text"},"schema:domainIncludes":{"@id":"unece:Cheque"},"rdfs:comment":"The print location, expressed as text, for this payment cheque."},{"@id":"unece:cardholderName","@type":["rdf:Property","owl:DatatypeProperty"],"rdfs:label":"cardholderName","schema:rangeIncludes":{"@id":"schema:Text"},"schema:domainIncludes":[{"@id":"unece:DigitalMethod"},{"@id":"unece:FinancialCard"}],"rdfs:comment":"A cardholder's name, expressed as text, for this digital method used for payment."},{"@id":"unece:expiryDateTime","@type":["rdf:Property","owl:DatatypeProperty"],"rdfs:label":"expiryDateTime","schema:rangeIncludes":{"@id":"schema:Text"},"schema:domainIncludes":[{"@id":"unece:DigitalMethod"},{"@id":"unece:FinancialCard"},{"@id":"unece:TradePrice"}],"rdfs:comment":"An expiry date, time, date time or other date time value for this specified licence."},{"@id":"unece:issuingCompanyName","@type":["rdf:Property","owl:DatatypeProperty"],"rdfs:label":"issuingCompanyName","schema:rangeIncludes":{"@id":"schema:Text"},"schema:domainIncludes":[{"@id":"unece:DigitalMethod"},{"@id":"unece:FinancialCard"},{"@id":"unece:Voucher"}],"rdfs:comment":"A name, expressed as text, of the company issuing this experience item voucher."},{"@id":"unece:validFromDateTime","@type":["rdf:Property","owl:DatatypeProperty"],"rdfs:label":"validFromDateTime","schema:rangeIncludes":{"@id":"schema:Text"},"schema:domainIncludes":[{"@id":"unece:DigitalMethod"},{"@id":"unece:FinancialCard"}],"rdfs:comment":"The date from which this trade settlement financial card is valid."},{"@id":"unece:verificationNumeric","@type":["rdf:Property","owl:DatatypeProperty"],"rdfs:label":"verificationNumeric","schema:rangeIncludes":{"@id":"schema:Text"},"schema:domainIncludes":[{"@id":"unece:DigitalMethod"},{"@id":"unece:FinancialCard"}],"rdfs:comment":"The unique card verification number for security purposes to help verify the card user is in actual possession of this trade settlement financial card."},{"@id":"unece:creditAvailableAmount","@type":["rdf:Property","owl:ObjectProperty"],"rdfs:label":"creditAvailableAmount","schema:rangeIncludes":{"@id":"unece:AmountType"},"schema:domainIncludes":{"@id":"unece:FinancialCard"},"rdfs:comment":""},{"@id":"unece:creditLimitAmount","@type":["rdf:Property","owl:ObjectProperty"],"rdfs:label":"creditLimitAmount","schema:rangeIncludes":{"@id":"unece:AmountType"},"schema:domainIncludes":{"@id":"unece:FinancialCard"},"rdfs:comment":""},{"@id":"unece:expiryDate","@type":["rdf:Property","owl:DatatypeProperty"],"rdfs:label":"expiryDate","schema:rangeIncludes":{"@id":"schema:Text"},"schema:domainIncludes":{"@id":"unece:FinancialCard"},"rdfs:comment":"The date of expiry up to which this trade settlement financial card is valid."},{"@id":"unece:interestRatePercent","@type":["rdf:Property","owl:DatatypeProperty"],"rdfs:label":"interestRatePercent","schema:rangeIncludes":{"@id":"schema:Text"},"schema:domainIncludes":{"@id":"unece:FinancialCard"},"rdfs:comment":"The interest rate expressed as a percentage for this trade settlement financial card."},{"@id":"unece:microchipIndicator","@type":["rdf:Property","owl:DatatypeProperty"],"rdfs:label":"microchipIndicator","schema:rangeIncludes":{"@id":"schema:Boolean"},"schema:domainIncludes":{"@id":"unece:FinancialCard"},"rdfs:comment":"The indication of whether or not this trade settlement financial card has a microchip."},{"@id":"unece:applicablePaymentDiscountTerms","@type":["rdf:Property","owl:ObjectProperty"],"rdfs:label":"applicablePaymentDiscountTerms","schema:rangeIncludes":{"@id":"unece:PaymentDiscountTerms"},"schema:domainIncludes":{"@id":"unece:PaymentTerms"},"rdfs:comment":"Trade payment discount terms applicable to these trade payment terms."},{"@id":"unece:applicablePaymentPenaltyTerms","@type":["rdf:Property","owl:ObjectProperty"],"rdfs:label":"applicablePaymentPenaltyTerms","schema:rangeIncludes":{"@id":"unece:PaymentPenaltyTerms"},"schema:domainIncludes":{"@id":"unece:PaymentTerms"},"rdfs:comment":"Trade payment penalty terms applicable to these trade payment terms."},{"@id":"unece:billStartDateTime","@type":["rdf:Property","owl:DatatypeProperty"],"rdfs:label":"billStartDateTime","schema:rangeIncludes":{"@id":"schema:Text"},"schema:domainIncludes":{"@id":"unece:PaymentTerms"},"rdfs:comment":"The date, time, date time, or other date time value of the bill start specified by these trade payment terms."},{"@id":"unece:instructionCode","@type":["rdf:Property","owl:DatatypeProperty"],"rdfs:label":"instructionCode","schema:rangeIncludes":{"@id":"schema:Text"},"schema:domainIncludes":{"@id":"unece:PaymentTerms"},"rdfs:comment":"A code specifying an instruction for these trade payment terms."},{"@id":"unece:partialPaymentAmount","@type":["rdf:Property","owl:ObjectProperty"],"rdfs:label":"partialPaymentAmount","schema:rangeIncludes":{"@id":"unece:AmountType"},"schema:domainIncludes":{"@id":"unece:PaymentTerms"},"rdfs:comment":""},{"@id":"unece:partialPaymentPercent","@type":["rdf:Property","owl:DatatypeProperty"],"rdfs:label":"partialPaymentPercent","schema:rangeIncludes":{"@id":"schema:Text"},"schema:domainIncludes":{"@id":"unece:PaymentTerms"},"rdfs:comment":"A partial payment, expressed as a percent, in these trade payment terms."},{"@id":"unece:paymentTermsEventTimeReferenceFromEventCode","@type":["rdf:Property","owl:DatatypeProperty"],"rdfs:label":"paymentTermsEventTimeReferenceFromEventCode","schema:rangeIncludes":{"@id":"unece:PaymentTermsEventTimeReferenceCodeList"},"schema:domainIncludes":{"@id":"unece:PaymentTerms"},"rdfs:comment":"The code specifying the event from which these trade payment terms are offered for a length of time."},{"@id":"unece:paymentTermsId","@type":["rdf:Property","owl:DatatypeProperty"],"rdfs:label":"paymentTermsId","schema:rangeIncludes":{"@id":"unece:PaymentTermsId"},"schema:domainIncludes":{"@id":"unece:PaymentTerms"},"rdfs:comment":"The unique identifier of these trade payment terms."},{"@id":"unece:paymentTermsTypeCode","@type":["rdf:Property","owl:DatatypeProperty"],"rdfs:label":"paymentTermsTypeCode","schema:rangeIncludes":{"@id":"unece:PaymentTermsTypeCodeList"},"schema:domainIncludes":{"@id":"unece:PaymentTerms"},"rdfs:comment":"A code specifying the type of trade payment terms."},{"@id":"unece:settlementPeriodMeasure","@type":["rdf:Property","owl:ObjectProperty"],"rdfs:label":"settlementPeriodMeasure","schema:rangeIncludes":{"@id":"unece:MeasureType"},"schema:domainIncludes":{"@id":"unece:PaymentTerms"},"rdfs:comment":""},{"@id":"unece:tradePaymentTermsDirectDebitMandateId","@type":["rdf:Property","owl:DatatypeProperty"],"rdfs:label":"tradePaymentTermsDirectDebitMandateId","schema:rangeIncludes":{"@id":"schema:Text"},"schema:domainIncludes":{"@id":"unece:PaymentTerms"},"rdfs:comment":"An identifier of a direct debit mandate in these trade payment terms."},{"@id":"unece:tradePaymentTermsInstructionTypeCode","@type":["rdf:Property","owl:DatatypeProperty"],"rdfs:label":"tradePaymentTermsInstructionTypeCode","schema:rangeIncludes":{"@id":"schema:Text"},"schema:domainIncludes":{"@id":"unece:PaymentTerms"},"rdfs:comment":"A code specifying a type of instruction for these trade payment terms."},{"@id":"unece:tradePaymentTermsPaymentMeansId","@type":["rdf:Property","owl:DatatypeProperty"],"rdfs:label":"tradePaymentTermsPaymentMeansId","schema:rangeIncludes":{"@id":"schema:Text"},"schema:domainIncludes":{"@id":"unece:PaymentTerms"},"rdfs:comment":"An identifier of a payment means in these trade payment terms."},{"@id":"unece:appliedTaxTypeCode","@type":["rdf:Property","owl:DatatypeProperty"],"rdfs:label":"appliedTaxTypeCode","schema:rangeIncludes":{"@id":"schema:Text"},"schema:domainIncludes":{"@id":"unece:AppliedTax"},"rdfs:comment":"The code specifying the applied tax type such as VAT."},{"@id":"unece:calculatedAmount","@type":["rdf:Property","owl:ObjectProperty"],"rdfs:label":"calculatedAmount","schema:rangeIncludes":{"@id":"unece:AmountType"},"schema:domainIncludes":[{"@id":"unece:AppliedTax"},{"@id":"unece:HeaderBalanceOut"},{"@id":"unece:PaymentBalanceOut"},{"@id":"unece:Tax"}],"rdfs:comment":""},{"@id":"unece:calculatedRate","@type":["rdf:Property","owl:DatatypeProperty"],"rdfs:label":"calculatedRate","schema:rangeIncludes":{"@id":"schema:Text"},"schema:domainIncludes":[{"@id":"unece:AppliedTax"},{"@id":"unece:Tax"}],"rdfs:comment":"The rate used to calculate the amount of this trade related tax, levy or duty."},{"@id":"unece:taxPointDate","@type":["rdf:Property","owl:DatatypeProperty"],"rdfs:label":"taxPointDate","schema:rangeIncludes":{"@id":"schema:Text"},"schema:domainIncludes":[{"@id":"unece:AppliedTax"},{"@id":"unece:Tax"}],"rdfs:comment":"The date of the tax point when taxes, such as VAT, are to be applied."},{"@id":"unece:branchName","@type":["rdf:Property","owl:DatatypeProperty"],"rdfs:label":"branchName","schema:rangeIncludes":{"@id":"schema:Text"},"schema:domainIncludes":{"@id":"unece:PaymentFinancialInstitution"},"rdfs:comment":"A branch name, expressed as text, for this payment financial institution."},{"@id":"unece:branchNameId","@type":["rdf:Property","owl:DatatypeProperty"],"rdfs:label":"branchNameId","schema:rangeIncludes":{"@id":"schema:Text"},"schema:domainIncludes":{"@id":"unece:PaymentFinancialInstitution"},"rdfs:comment":"The identifier of the branch name for this payment financial institution."},{"@id":"unece:gLNId","@type":["rdf:Property","owl:DatatypeProperty"],"rdfs:label":"gLNId","schema:rangeIncludes":{"@id":"schema:Text"},"schema:domainIncludes":{"@id":"unece:PaymentFinancialInstitution"},"rdfs:comment":"A Global Location Number (GLN) identifier for this trade party."},{"@id":"unece:nameId","@type":["rdf:Property","owl:DatatypeProperty"],"rdfs:label":"nameId","schema:rangeIncludes":{"@id":"schema:Text"},"schema:domainIncludes":{"@id":"unece:PaymentFinancialInstitution"},"rdfs:comment":"The identifier of the name for this payment financial institution."},{"@id":"unece:roleCode","@type":["rdf:Property","owl:DatatypeProperty"],"rdfs:label":"roleCode","schema:rangeIncludes":{"@id":"schema:Text"},"schema:domainIncludes":[{"@id":"unece:PaymentFinancialInstitution"},{"@id":"unece:CooperatingOrganization"}],"rdfs:comment":"The code specifying the role for this cooperating organization."},{"@id":"unece:specifiedCommunication","@type":["rdf:Property","owl:ObjectProperty"],"rdfs:label":"specifiedCommunication","schema:rangeIncludes":{"@id":"unece:Communication"},"schema:domainIncludes":{"@id":"unece:PaymentFinancialInstitution"},"rdfs:comment":"The exchange of thoughts, messages, or information, as universally exchanged by speech, signals, writing, or behaviour between persons and/or organizations."},{"@id":"unece:specifiedPaymentFinancialAccount","@type":["rdf:Property","owl:ObjectProperty"],"rdfs:label":"specifiedPaymentFinancialAccount","schema:rangeIncludes":{"@id":"unece:PaymentFinancialAccount"},"schema:domainIncludes":{"@id":"unece:PaymentFinancialInstitution"},"rdfs:comment":"A payment financial account specified for this payment financial institution."},{"@id":"unece:binaryFile","@type":["rdf:Property","owl:ObjectProperty"],"rdfs:label":"binaryFile","schema:rangeIncludes":{"@id":"unece:BinaryFile"},"schema:domainIncludes":[{"@id":"unece:BreakdownStatement"},{"@id":"unece:BasicWorkItem"},{"@id":"unece:GroupedWorkItem"}],"rdfs:comment":"A specified computer file or program stored in a binary format."},{"@id":"unece:changedStatus","@type":["rdf:Property","owl:ObjectProperty"],"rdfs:label":"changedStatus","schema:rangeIncludes":{"@id":"unece:RecordedStatus"},"schema:domainIncludes":[{"@id":"unece:BreakdownStatement"},{"@id":"unece:BasicWorkItem"},{"@id":"unece:GroupedWorkItem"},{"@id":"unece:QuantityAnalysis"}],"rdfs:comment":"Recorded information relevant to a condition or a position of an object."},{"@id":"unece:comment","@type":["rdf:Property","owl:DatatypeProperty"],"rdfs:label":"comment","schema:rangeIncludes":{"@id":"schema:Text"},"schema:domainIncludes":[{"@id":"unece:BreakdownStatement"},{"@id":"unece:BasicWorkItem"},{"@id":"unece:GroupedWorkItem"}],"rdfs:comment":"A comment, expressed as text for this MDH illness."},{"@id":"unece:contractualLanguageCode","@type":["rdf:Property","owl:DatatypeProperty"],"rdfs:label":"contractualLanguageCode","schema:rangeIncludes":{"@id":"schema:Text"},"schema:domainIncludes":[{"@id":"unece:BreakdownStatement"},{"@id":"unece:BasicWorkItem"},{"@id":"unece:GroupedWorkItem"},{"@id":"unece:ComplexDescription"},{"@id":"unece:QuantityAnalysis"},{"@id":"unece:WorkItemDimension"},{"@id":"unece:Response"},{"@id":"unece:SpecificationQuery"}],"rdfs:comment":"The code specifying the contractual language for this basic work item."},{"@id":"unece:creationBinaryFile","@type":["rdf:Property","owl:ObjectProperty"],"rdfs:label":"creationBinaryFile","schema:rangeIncludes":{"@id":"unece:BinaryFile"},"schema:domainIncludes":{"@id":"unece:BreakdownStatement"},"rdfs:comment":"A specified computer file or program stored in a binary format."},{"@id":"unece:defaultCurrencyCode","@type":["rdf:Property","owl:DatatypeProperty"],"rdfs:label":"defaultCurrencyCode","schema:rangeIncludes":{"@id":"unece:CurrencyCodeList"},"schema:domainIncludes":{"@id":"unece:BreakdownStatement"},"rdfs:comment":"The code specifying the default currency for this valuation breakdown statement."},{"@id":"unece:defaultLanguageCode","@type":["rdf:Property","owl:DatatypeProperty"],"rdfs:label":"defaultLanguageCode","schema:rangeIncludes":{"@id":"schema:Text"},"schema:domainIncludes":{"@id":"unece:BreakdownStatement"},"rdfs:comment":"The code specifying the default language for this valuation breakdown statement."},{"@id":"unece:itemBasicWorkItem","@type":["rdf:Property","owl:ObjectProperty"],"rdfs:label":"itemBasicWorkItem","schema:rangeIncludes":{"@id":"unece:BasicWorkItem"},"schema:domainIncludes":[{"@id":"unece:BreakdownStatement"},{"@id":"unece:BasicWorkItem"},{"@id":"unece:GroupedWorkItem"}],"rdfs:comment":"A basic work item in this basic work item."},{"@id":"unece:itemGroupedWorkItem","@type":["rdf:Property","owl:ObjectProperty"],"rdfs:label":"itemGroupedWorkItem","schema:rangeIncludes":{"@id":"unece:GroupedWorkItem"},"schema:domainIncludes":[{"@id":"unece:BreakdownStatement"},{"@id":"unece:GroupedWorkItem"}],"rdfs:comment":"A grouped work item in this valuation breakdown statement."},{"@id":"unece:measurementMethodId","@type":["rdf:Property","owl:DatatypeProperty"],"rdfs:label":"measurementMethodId","schema:rangeIncludes":{"@id":"schema:Text"},"schema:domainIncludes":{"@id":"unece:BreakdownStatement"},"rdfs:comment":"A unique identifier of a method of measurement for this valuation breakdown statement."},{"@id":"unece:priceListId","@type":["rdf:Property","owl:DatatypeProperty"],"rdfs:label":"priceListId","schema:rangeIncludes":{"@id":"schema:Text"},"schema:domainIncludes":{"@id":"unece:BreakdownStatement"},"rdfs:comment":"The identifier of a price list for this valuation breakdown statement."},{"@id":"unece:readerBinaryFile","@type":["rdf:Property","owl:ObjectProperty"],"rdfs:label":"readerBinaryFile","schema:rangeIncludes":{"@id":"unece:BinaryFile"},"schema:domainIncludes":{"@id":"unece:BreakdownStatement"},"rdfs:comment":"A specified computer file or program stored in a binary format."},{"@id":"unece:requestedActionCode","@type":["rdf:Property","owl:DatatypeProperty"],"rdfs:label":"requestedActionCode","schema:rangeIncludes":{"@id":"schema:Text"},"schema:domainIncludes":[{"@id":"unece:BreakdownStatement"},{"@id":"unece:BasicWorkItem"},{"@id":"unece:GroupedWorkItem"},{"@id":"unece:DocumentStatus"}],"rdfs:comment":"A code specifying a requested action for this basic work item."},{"@id":"unece:totalPrice","@type":["rdf:Property","owl:ObjectProperty"],"rdfs:label":"totalPrice","schema:rangeIncludes":{"@id":"unece:CalculatedPrice"},"schema:domainIncludes":[{"@id":"unece:BreakdownStatement"},{"@id":"unece:BasicWorkItem"},{"@id":"unece:GroupedWorkItem"}],"rdfs:comment":"A total calculated price for this basic work item."},{"@id":"unece:breakdownBalanceOut","@type":["rdf:Property","owl:ObjectProperty"],"rdfs:label":"breakdownBalanceOut","schema:rangeIncludes":{"@id":"unece:HeaderBalanceOut"},"schema:domainIncludes":{"@id":"unece:HeaderBalanceOut"},"rdfs:comment":"A balance out breakdown of this header balance out."},{"@id":"unece:occurrenceDateTime","@type":["rdf:Property","owl:DatatypeProperty"],"rdfs:label":"occurrenceDateTime","schema:rangeIncludes":{"@id":"schema:Text"},"schema:domainIncludes":[{"@id":"unece:HeaderBalanceOut"},{"@id":"unece:PaymentBalanceOut"},{"@id":"unece:CommunicationEvent"},{"@id":"unece:Schedule"}],"rdfs:comment":"A date, time, date time, or other date time of an occurrence in this supply chain schedule."},{"@id":"unece:reasonCode","@type":["rdf:Property","owl:DatatypeProperty"],"rdfs:label":"reasonCode","schema:rangeIncludes":{"@id":"schema:Text"},"schema:domainIncludes":[{"@id":"unece:HeaderBalanceOut"},{"@id":"unece:PaymentBalanceOut"},{"@id":"unece:TradePrice"},{"@id":"unece:ValidationStatus"},{"@id":"unece:Error"},{"@id":"unece:CommunicationEvent"},{"@id":"unece:CancellationStatus"}],"rdfs:comment":"A code specifying a reason for the declared error."},{"@id":"unece:reasonDescription","@type":["rdf:Property","owl:DatatypeProperty"],"rdfs:label":"reasonDescription","schema:rangeIncludes":{"@id":"schema:Text"},"schema:domainIncludes":[{"@id":"unece:HeaderBalanceOut"},{"@id":"unece:PaymentBalanceOut"}],"rdfs:comment":"A textual description of the reason for this header balance out."},{"@id":"unece:buildingNumber","@type":["rdf:Property","owl:DatatypeProperty"],"rdfs:label":"buildingNumber","schema:rangeIncludes":{"@id":"schema:Text"},"schema:domainIncludes":[{"@id":"unece:FinancialInstitutionAddress"},{"@id":"unece:Address"}],"rdfs:comment":"The building number, expressed as text, in this trade address."},{"@id":"unece:cityId","@type":["rdf:Property","owl:DatatypeProperty"],"rdfs:label":"cityId","schema:rangeIncludes":{"@id":"schema:Text"},"schema:domainIncludes":[{"@id":"unece:FinancialInstitutionAddress"},{"@id":"unece:Address"}],"rdfs:comment":"The identifier of the city for this trade address, such as United Nations Location Code (UNLOCODE)."},{"@id":"unece:cityName","@type":["rdf:Property","owl:DatatypeProperty"],"rdfs:label":"cityName","schema:rangeIncludes":{"@id":"schema:Text"},"schema:domainIncludes":[{"@id":"unece:FinancialInstitutionAddress"},{"@id":"unece:BirthAddress"},{"@id":"unece:Address"}],"rdfs:comment":"The name, expressed as text, of the city, town or village of this birth address."},{"@id":"unece:countryId","@type":["rdf:Property","owl:DatatypeProperty"],"rdfs:label":"countryId","schema:rangeIncludes":{"@id":"schema:Text"},"schema:domainIncludes":[{"@id":"unece:FinancialInstitutionAddress"},{"@id":"unece:Country"},{"@id":"unece:LegalRegistration"}],"rdfs:comment":"A unique country identifier for this location party."},{"@id":"unece:countryName","@type":["rdf:Property","owl:DatatypeProperty"],"rdfs:label":"countryName","schema:rangeIncludes":{"@id":"schema:Text"},"schema:domainIncludes":[{"@id":"unece:FinancialInstitutionAddress"},{"@id":"unece:Location"},{"@id":"unece:Address"}],"rdfs:comment":"A name, expressed as text, of the country for this trade address."},{"@id":"unece:countrySubDivisionId","@type":["rdf:Property","owl:DatatypeProperty"],"rdfs:label":"countrySubDivisionId","schema:rangeIncludes":{"@id":"schema:Text"},"schema:domainIncludes":[{"@id":"unece:FinancialInstitutionAddress"},{"@id":"unece:Location"},{"@id":"unece:Address"}],"rdfs:comment":"A unique identifier of the country sub-division for this trade address."},{"@id":"unece:countrySubDivisionName","@type":["rdf:Property","owl:DatatypeProperty"],"rdfs:label":"countrySubDivisionName","schema:rangeIncludes":{"@id":"schema:Text"},"schema:domainIncludes":[{"@id":"unece:FinancialInstitutionAddress"},{"@id":"unece:BirthAddress"},{"@id":"unece:Address"}],"rdfs:comment":"A name, expressed as text, of the sub-division of a country for this trade address."},{"@id":"unece:departmentName","@type":["rdf:Property","owl:DatatypeProperty"],"rdfs:label":"departmentName","schema:rangeIncludes":{"@id":"schema:Text"},"schema:domainIncludes":[{"@id":"unece:FinancialInstitutionAddress"},{"@id":"unece:Address"}],"rdfs:comment":"The name, expressed as text, of a department for this trade address."},{"@id":"unece:financialInstitutionAddressTypeCode","@type":["rdf:Property","owl:DatatypeProperty"],"rdfs:label":"financialInstitutionAddressTypeCode","schema:rangeIncludes":{"@id":"schema:Text"},"schema:domainIncludes":{"@id":"unece:FinancialInstitutionAddress"},"rdfs:comment":"The code specifying the type of financial institution address."},{"@id":"unece:lineFive","@type":["rdf:Property","owl:DatatypeProperty"],"rdfs:label":"lineFive","schema:rangeIncludes":{"@id":"schema:Text"},"schema:domainIncludes":[{"@id":"unece:FinancialInstitutionAddress"},{"@id":"unece:Address"}],"rdfs:comment":"The fifth free form line, expressed as text, of this financial institution address."},{"@id":"unece:lineFour","@type":["rdf:Property","owl:DatatypeProperty"],"rdfs:label":"lineFour","schema:rangeIncludes":{"@id":"schema:Text"},"schema:domainIncludes":[{"@id":"unece:FinancialInstitutionAddress"},{"@id":"unece:Address"}],"rdfs:comment":"The fourth free form line, expressed as text, of this financial institution address."},{"@id":"unece:lineOne","@type":["rdf:Property","owl:DatatypeProperty"],"rdfs:label":"lineOne","schema:rangeIncludes":{"@id":"schema:Text"},"schema:domainIncludes":[{"@id":"unece:FinancialInstitutionAddress"},{"@id":"unece:Address"}],"rdfs:comment":"The first free form line, expressed as text, of this financial institution address."},{"@id":"unece:lineThree","@type":["rdf:Property","owl:DatatypeProperty"],"rdfs:label":"lineThree","schema:rangeIncludes":{"@id":"schema:Text"},"schema:domainIncludes":[{"@id":"unece:FinancialInstitutionAddress"},{"@id":"unece:Address"}],"rdfs:comment":"The third free form line, expressed as text, of this financial institution address."},{"@id":"unece:lineTwo","@type":["rdf:Property","owl:DatatypeProperty"],"rdfs:label":"lineTwo","schema:rangeIncludes":{"@id":"schema:Text"},"schema:domainIncludes":[{"@id":"unece:FinancialInstitutionAddress"},{"@id":"unece:Address"}],"rdfs:comment":"The second free form line, expressed as text, of this financial institution address."},{"@id":"unece:postOfficeBox","@type":["rdf:Property","owl:DatatypeProperty"],"rdfs:label":"postOfficeBox","schema:rangeIncludes":{"@id":"schema:Text"},"schema:domainIncludes":[{"@id":"unece:FinancialInstitutionAddress"},{"@id":"unece:Address"}],"rdfs:comment":"The post office box, expressed as text, for this financial institution address."},{"@id":"unece:postcodeCode","@type":["rdf:Property","owl:DatatypeProperty"],"rdfs:label":"postcodeCode","schema:rangeIncludes":{"@id":"schema:Text"},"schema:domainIncludes":[{"@id":"unece:FinancialInstitutionAddress"},{"@id":"unece:Address"}],"rdfs:comment":"A code specifying the postcode of this trade address."},{"@id":"unece:streetName","@type":["rdf:Property","owl:DatatypeProperty"],"rdfs:label":"streetName","schema:rangeIncludes":{"@id":"schema:Text"},"schema:domainIncludes":[{"@id":"unece:FinancialInstitutionAddress"},{"@id":"unece:Address"}],"rdfs:comment":"A name, expressed as text, of a street or thoroughfare for this trade address."},{"@id":"unece:condition","@type":["rdf:Property","owl:DatatypeProperty"],"rdfs:label":"condition","schema:rangeIncludes":{"@id":"schema:Text"},"schema:domainIncludes":[{"@id":"unece:Guarantee"},{"@id":"unece:DocumentStatus"}],"rdfs:comment":"A condition or status, expressed as text, for this process characteristic."},{"@id":"unece:effectiveDelimitedPeriod","@type":["rdf:Property","owl:ObjectProperty"],"rdfs:label":"effectiveDelimitedPeriod","schema:rangeIncludes":{"@id":"unece:DelimitedPeriod"},"schema:domainIncludes":{"@id":"unece:Guarantee"},"rdfs:comment":"A period of time from a start date time onwards up to an end date time."},{"@id":"unece:liabilityAmount","@type":["rdf:Property","owl:ObjectProperty"],"rdfs:label":"liabilityAmount","schema:rangeIncludes":{"@id":"unece:AmountType"},"schema:domainIncludes":{"@id":"unece:Guarantee"},"rdfs:comment":""},{"@id":"unece:customsDutyIndicator","@type":["rdf:Property","owl:DatatypeProperty"],"rdfs:label":"customsDutyIndicator","schema:rangeIncludes":{"@id":"schema:Boolean"},"schema:domainIncludes":[{"@id":"unece:RegisteredTax"},{"@id":"unece:Tax"}],"rdfs:comment":"The indication of whether or not this registered tax is a customs duty."},{"@id":"unece:exemptionReason","@type":["rdf:Property","owl:DatatypeProperty"],"rdfs:label":"exemptionReason","schema:rangeIncludes":{"@id":"schema:Text"},"schema:domainIncludes":[{"@id":"unece:RegisteredTax"},{"@id":"unece:Tax"}],"rdfs:comment":"A reason, expressed as text, for exemption from this registered tax."},{"@id":"unece:exemptionReasonCode","@type":["rdf:Property","owl:DatatypeProperty"],"rdfs:label":"exemptionReasonCode","schema:rangeIncludes":{"@id":"schema:Text"},"schema:domainIncludes":{"@id":"unece:RegisteredTax"},"rdfs:comment":"The code specifying the exemption reason for this registered tax."},{"@id":"unece:jurisdiction","@type":["rdf:Property","owl:DatatypeProperty"],"rdfs:label":"jurisdiction","schema:rangeIncludes":{"@id":"schema:Text"},"schema:domainIncludes":[{"@id":"unece:RegisteredTax"},{"@id":"unece:Tax"}],"rdfs:comment":"A jurisdiction, expressed as text, for this registered tax."},{"@id":"unece:registeredTaxTypeCode","@type":["rdf:Property","owl:DatatypeProperty"],"rdfs:label":"registeredTaxTypeCode","schema:rangeIncludes":{"@id":"schema:Text"},"schema:domainIncludes":{"@id":"unece:RegisteredTax"},"rdfs:comment":"The code specifying the type of registered tax."},{"@id":"unece:paidAmount","@type":["rdf:Property","owl:ObjectProperty"],"rdfs:label":"paidAmount","schema:rangeIncludes":{"@id":"unece:AmountType"},"schema:domainIncludes":[{"@id":"unece:InstalmentPayment"},{"@id":"unece:AdvancePayment"}],"rdfs:comment":""},{"@id":"unece:sequenceId","@type":["rdf:Property","owl:DatatypeProperty"],"rdfs:label":"sequenceId","schema:rangeIncludes":{"@id":"schema:Text"},"schema:domainIncludes":{"@id":"unece:InstalmentPayment"},"rdfs:comment":"The sequence identifier for this instalment payment."},{"@id":"unece:specifiedFinancingRequestResultDocument","@type":["rdf:Property","owl:ObjectProperty"],"rdfs:label":"specifiedFinancingRequestResultDocument","schema:rangeIncludes":{"@id":"unece:FinancingRequestResultDocument"},"schema:domainIncludes":{"@id":"unece:InstalmentPayment"},"rdfs:comment":"The financing request result document specified for this instalment payment."},{"@id":"unece:financedRatePercent","@type":["rdf:Property","owl:DatatypeProperty"],"rdfs:label":"financedRatePercent","schema:rangeIncludes":{"@id":"schema:Text"},"schema:domainIncludes":{"@id":"unece:FinancingRequestResultDocument"},"rdfs:comment":"The financed rate, expressed as a percentage, in this financing request result document."},{"@id":"unece:specifiedFinancingStatus","@type":["rdf:Property","owl:ObjectProperty"],"rdfs:label":"specifiedFinancingStatus","schema:rangeIncludes":{"@id":"unece:FinancingStatus"},"schema:domainIncludes":{"@id":"unece:FinancingRequestResultDocument"},"rdfs:comment":"The financing status specified in this financing request result document."},{"@id":"unece:financingStatusConditionCode","@type":["rdf:Property","owl:DatatypeProperty"],"rdfs:label":"financingStatusConditionCode","schema:rangeIncludes":{"@id":"unece:FinancingStatusCodeList"},"schema:domainIncludes":{"@id":"unece:FinancingStatus"},"rdfs:comment":"The code specifying the condition of this financing status."},{"@id":"unece:financingStatusReasonCode","@type":["rdf:Property","owl:DatatypeProperty"],"rdfs:label":"financingStatusReasonCode","schema:rangeIncludes":{"@id":"unece:FinancingStatusReasonCodeList"},"schema:domainIncludes":{"@id":"unece:FinancingStatus"},"rdfs:comment":"The code specifying the reason for this financing status."},{"@id":"unece:reasonInformation","@type":["rdf:Property","owl:DatatypeProperty"],"rdfs:label":"reasonInformation","schema:rangeIncludes":{"@id":"schema:Text"},"schema:domainIncludes":[{"@id":"unece:FinancingStatus"},{"@id":"unece:CancellationStatus"},{"@id":"unece:DocumentStatus"}],"rdfs:comment":"Information, expressed as text, related to the reason for this cancellation status."},{"@id":"unece:includedTax","@type":["rdf:Property","owl:ObjectProperty"],"rdfs:label":"includedTax","schema:rangeIncludes":{"@id":"unece:Tax"},"schema:domainIncludes":[{"@id":"unece:AdvancePayment"},{"@id":"unece:TradePrice"}],"rdfs:comment":"A tax included in this advance payment."},{"@id":"unece:receivedDateTime","@type":["rdf:Property","owl:DatatypeProperty"],"rdfs:label":"receivedDateTime","schema:rangeIncludes":{"@id":"schema:DateTime"},"schema:domainIncludes":{"@id":"unece:AdvancePayment"},"rdfs:comment":"The date, time, date time, or other date time value when information related to this transport event was received, from the perspective of the receiver."},{"@id":"unece:specifiedInstalmentPayment","@type":["rdf:Property","owl:ObjectProperty"],"rdfs:label":"specifiedInstalmentPayment","schema:rangeIncludes":{"@id":"unece:InstalmentPayment"},"schema:domainIncludes":{"@id":"unece:InstalmentPlan"},"rdfs:comment":"An instalment payment specified for this instalment plan."},{"@id":"unece:accessRightsTypeAccessRightsCode","@type":["rdf:Property","owl:DatatypeProperty"],"rdfs:label":"accessRightsTypeAccessRightsCode","schema:rangeIncludes":{"@id":"unece:AccessRightsTypeCodeList"},"schema:domainIncludes":{"@id":"unece:RequestingParty"},"rdfs:comment":"The code specifying the access rights, such as unlimited, restricted, prohibited, for this requesting party."},{"@id":"unece:languageCode","@type":["rdf:Property","owl:DatatypeProperty"],"rdfs:label":"languageCode","schema:rangeIncludes":{"@id":"schema:Text"},"schema:domainIncludes":{"@id":"unece:RequestingParty"},"rdfs:comment":"A code specifying a language for this requesting party."},{"@id":"unece:partyTypeCode","@type":["rdf:Property","owl:DatatypeProperty"],"rdfs:label":"partyTypeCode","schema:rangeIncludes":{"@id":"unece:PartyTypeCodeList"},"schema:domainIncludes":{"@id":"unece:RequestingParty"},"rdfs:comment":"A code specifying the type of TT party."},{"@id":"unece:actualComplexDescription","@type":["rdf:Property","owl:ObjectProperty"],"rdfs:label":"actualComplexDescription","schema:rangeIncludes":{"@id":"unece:ComplexDescription"},"schema:domainIncludes":[{"@id":"unece:BasicWorkItem"},{"@id":"unece:GroupedWorkItem"}],"rdfs:comment":"An aggregation of descriptive information consisting of different but related characteristics that together constitute a work item complex description."},{"@id":"unece:alternativeClassificationCode","@type":["rdf:Property","owl:DatatypeProperty"],"rdfs:label":"alternativeClassificationCode","schema:rangeIncludes":{"@id":"schema:Text"},"schema:domainIncludes":[{"@id":"unece:BasicWorkItem"},{"@id":"unece:GroupedWorkItem"},{"@id":"unece:QuantityAnalysis"}],"rdfs:comment":"A code specifying an alternative classification for this basic work item."},{"@id":"unece:index","@type":["rdf:Property","owl:DatatypeProperty"],"rdfs:label":"index","schema:rangeIncludes":{"@id":"schema:Text"},"schema:domainIncludes":[{"@id":"unece:BasicWorkItem"},{"@id":"unece:GroupedWorkItem"}],"rdfs:comment":"The index, expressed as text, to be used for this basic work item."},{"@id":"unece:priceListItemId","@type":["rdf:Property","owl:DatatypeProperty"],"rdfs:label":"priceListItemId","schema:rangeIncludes":{"@id":"schema:Text"},"schema:domainIncludes":[{"@id":"unece:BasicWorkItem"},{"@id":"unece:GroupedWorkItem"}],"rdfs:comment":"The identifier of a price list item for this grouped work item."},{"@id":"unece:primaryClassificationCode","@type":["rdf:Property","owl:DatatypeProperty"],"rdfs:label":"primaryClassificationCode","schema:rangeIncludes":{"@id":"schema:Text"},"schema:domainIncludes":[{"@id":"unece:BasicWorkItem"},{"@id":"unece:GroupedWorkItem"},{"@id":"unece:QuantityAnalysis"}],"rdfs:comment":"A code specifying a primary classification value for this work item quantity analysis."},{"@id":"unece:referenceId","@type":["rdf:Property","owl:DatatypeProperty"],"rdfs:label":"referenceId","schema:rangeIncludes":{"@id":"schema:Text"},"schema:domainIncludes":{"@id":"unece:BasicWorkItem"},"rdfs:comment":"The unique identifier of another work item referenced by this basic work item."},{"@id":"unece:totalQuantity","@type":["rdf:Property","owl:ObjectProperty"],"rdfs:label":"totalQuantity","schema:rangeIncludes":{"@id":"unece:QuantityType"},"schema:domainIncludes":[{"@id":"unece:BasicWorkItem"},{"@id":"unece:GroupedWorkItem"}],"rdfs:comment":""},{"@id":"unece:totalQuantityAnalysis","@type":["rdf:Property","owl:ObjectProperty"],"rdfs:label":"totalQuantityAnalysis","schema:rangeIncludes":{"@id":"unece:QuantityAnalysis"},"schema:domainIncludes":{"@id":"unece:BasicWorkItem"},"rdfs:comment":"The quantity analysis for this work item."},{"@id":"unece:totalQuantityClassificationCode","@type":["rdf:Property","owl:DatatypeProperty"],"rdfs:label":"totalQuantityClassificationCode","schema:rangeIncludes":{"@id":"schema:Text"},"schema:domainIncludes":{"@id":"unece:BasicWorkItem"},"rdfs:comment":"The code specifying the classification of the total quantity for this basic work item."},{"@id":"unece:unitPrice","@type":["rdf:Property","owl:ObjectProperty"],"rdfs:label":"unitPrice","schema:rangeIncludes":{"@id":"unece:CalculatedPrice"},"schema:domainIncludes":{"@id":"unece:BasicWorkItem"},"rdfs:comment":"A unit calculated price for this basic work item."},{"@id":"unece:calculatedPriceTypeCode","@type":["rdf:Property","owl:DatatypeProperty"],"rdfs:label":"calculatedPriceTypeCode","schema:rangeIncludes":{"@id":"schema:Text"},"schema:domainIncludes":{"@id":"unece:CalculatedPrice"},"rdfs:comment":"A code specifying the type of calculated price."},{"@id":"unece:chargeAmount","@type":["rdf:Property","owl:ObjectProperty"],"rdfs:label":"chargeAmount","schema:rangeIncludes":{"@id":"unece:AmountType"},"schema:domainIncludes":[{"@id":"unece:CalculatedPrice"},{"@id":"unece:TradePrice"},{"@id":"unece:ReferencePrice"}],"rdfs:comment":""},{"@id":"unece:relatedAllowanceCharge","@type":["rdf:Property","owl:ObjectProperty"],"rdfs:label":"relatedAllowanceCharge","schema:rangeIncludes":{"@id":"unece:AppliedAllowanceCharge"},"schema:domainIncludes":{"@id":"unece:CalculatedPrice"},"rdfs:comment":"Applied allowance charge information related to this calculated price."},{"@id":"unece:allowanceChargeBasisAmount","@type":["rdf:Property","owl:ObjectProperty"],"rdfs:label":"allowanceChargeBasisAmount","schema:rangeIncludes":{"@id":"unece:AmountType"},"schema:domainIncludes":{"@id":"unece:Tax"},"rdfs:comment":""},{"@id":"unece:applicablePercent","@type":["rdf:Property","owl:DatatypeProperty"],"rdfs:label":"applicablePercent","schema:rangeIncludes":{"@id":"schema:Text"},"schema:domainIncludes":{"@id":"unece:Tax"},"rdfs:comment":"The percent of trade tax applicable, such as to an object or an activity."},{"@id":"unece:basisQuantity","@type":["rdf:Property","owl:ObjectProperty"],"rdfs:label":"basisQuantity","schema:rangeIncludes":{"@id":"unece:QuantityType"},"schema:domainIncludes":[{"@id":"unece:Tax"},{"@id":"unece:TradeAllowanceCharge"},{"@id":"unece:TradePrice"},{"@id":"unece:ReferencePrice"}],"rdfs:comment":""},{"@id":"unece:buyerDeductibleTaxSpecifiedAccountingAccount","@type":["rdf:Property","owl:ObjectProperty"],"rdfs:label":"buyerDeductibleTaxSpecifiedAccountingAccount","schema:rangeIncludes":{"@id":"unece:AccountingAccount"},"schema:domainIncludes":{"@id":"unece:Tax"},"rdfs:comment":"The buyer deductible tax specified accounting account for this trade related tax, levy or duty."},{"@id":"unece:buyerNonDeductibleTaxSpecifiedAccountingAccount","@type":["rdf:Property","owl:ObjectProperty"],"rdfs:label":"buyerNonDeductibleTaxSpecifiedAccountingAccount","schema:rangeIncludes":{"@id":"unece:AccountingAccount"},"schema:domainIncludes":{"@id":"unece:Tax"},"rdfs:comment":"The buyer non-deductible tax specified accounting account for this trade related tax, levy or duty."},{"@id":"unece:buyerRepayableTaxSpecifiedAccountingAccount","@type":["rdf:Property","owl:ObjectProperty"],"rdfs:label":"buyerRepayableTaxSpecifiedAccountingAccount","schema:rangeIncludes":{"@id":"unece:AccountingAccount"},"schema:domainIncludes":{"@id":"unece:Tax"},"rdfs:comment":"The buyer repayable tax specified accounting account for this trade related tax, levy or duty."},{"@id":"unece:calculationMethodCode","@type":["rdf:Property","owl:DatatypeProperty"],"rdfs:label":"calculationMethodCode","schema:rangeIncludes":{"@id":"schema:Text"},"schema:domainIncludes":{"@id":"unece:Tax"},"rdfs:comment":"The code specifying the method by which this trade related tax, levy or duty is calculated, such as codes for \"tax calculated after line total summation\", \"tax calculated before line total summation\", \"tax back calculated based on grand total\"."},{"@id":"unece:calculationSequenceNumeric","@type":["rdf:Property","owl:DatatypeProperty"],"rdfs:label":"calculationSequenceNumeric","schema:rangeIncludes":{"@id":"schema:Text"},"schema:domainIncludes":{"@id":"unece:Tax"},"rdfs:comment":"A numeric expression of the sequence in which this trade related tax is to be or has been applied when multiple taxes are applicable per calculation, such as first \"Value Added Tax (VAT)\", second \"Transfer\"."},{"@id":"unece:categoryName","@type":["rdf:Property","owl:DatatypeProperty"],"rdfs:label":"categoryName","schema:rangeIncludes":{"@id":"schema:Text"},"schema:domainIncludes":[{"@id":"unece:Tax"},{"@id":"unece:CustomerClass"}],"rdfs:comment":"A category name, expressed as text, of this specified customer class."},{"@id":"unece:customsDutyRegimeTypeCode","@type":["rdf:Property","owl:DatatypeProperty"],"rdfs:label":"customsDutyRegimeTypeCode","schema:rangeIncludes":{"@id":"unece:CustomsDutyRegimeTypeCodeList"},"schema:domainIncludes":{"@id":"unece:Tax"},"rdfs:comment":"The code specifying a type of regime applicable to the assessment or calculation of this trade related tax, levy or duty, such as a preferential duty rate."},{"@id":"unece:customsProcedureGuaranteeCode","@type":["rdf:Property","owl:DatatypeProperty"],"rdfs:label":"customsProcedureGuaranteeCode","schema:rangeIncludes":{"@id":"unece:CustomsProcedureGuaranteeCodeList"},"schema:domainIncludes":{"@id":"unece:Tax"},"rdfs:comment":"The code specifying an undertaking given in cash, bond or as a written guarantee to ensure that an obligation will be fulfilled for this cross-border regulatory procedure."},{"@id":"unece:deductionAmount","@type":["rdf:Property","owl:ObjectProperty"],"rdfs:label":"deductionAmount","schema:rangeIncludes":{"@id":"unece:AmountType"},"schema:domainIncludes":{"@id":"unece:Tax"},"rdfs:comment":""},{"@id":"unece:exemptionAuthorizationId","@type":["rdf:Property","owl:DatatypeProperty"],"rdfs:label":"exemptionAuthorizationId","schema:rangeIncludes":{"@id":"schema:Text"},"schema:domainIncludes":{"@id":"unece:Tax"},"rdfs:comment":"The unique identifier of the exemption authorization for this trade tax."},{"@id":"unece:exemptionIndicator","@type":["rdf:Property","owl:DatatypeProperty"],"rdfs:label":"exemptionIndicator","schema:rangeIncludes":{"@id":"schema:Boolean"},"schema:domainIncludes":{"@id":"unece:Tax"},"rdfs:comment":"The indication of whether or not there is an exemption from this trade tax."},{"@id":"unece:grandTotalAmount","@type":["rdf:Property","owl:ObjectProperty"],"rdfs:label":"grandTotalAmount","schema:rangeIncludes":{"@id":"unece:AmountType"},"schema:domainIncludes":[{"@id":"unece:Tax"},{"@id":"unece:TradeSettlementPaymentMonetarySummation"}],"rdfs:comment":""},{"@id":"unece:guarantee","@type":["rdf:Property","owl:DatatypeProperty"],"rdfs:label":"guarantee","schema:rangeIncludes":{"@id":"schema:Text"},"schema:domainIncludes":{"@id":"unece:Tax"},"rdfs:comment":"The undertaking, expressed as text, given in cash, bond or as a written guarantee to ensure that an obligation will be fulfilled for this cross-border regulatory procedure."},{"@id":"unece:informationAmount","@type":["rdf:Property","owl:ObjectProperty"],"rdfs:label":"informationAmount","schema:rangeIncludes":{"@id":"unece:AmountType"},"schema:domainIncludes":{"@id":"unece:Tax"},"rdfs:comment":""},{"@id":"unece:lineTotalBasisAmount","@type":["rdf:Property","owl:ObjectProperty"],"rdfs:label":"lineTotalBasisAmount","schema:rangeIncludes":{"@id":"unece:AmountType"},"schema:domainIncludes":{"@id":"unece:Tax"},"rdfs:comment":""},{"@id":"unece:localTaxSystemId","@type":["rdf:Property","owl:DatatypeProperty"],"rdfs:label":"localTaxSystemId","schema:rangeIncludes":{"@id":"schema:Text"},"schema:domainIncludes":{"@id":"unece:Tax"},"rdfs:comment":"The identifier of the local tax system for this trade tax."},{"@id":"unece:paymentId","@type":["rdf:Property","owl:DatatypeProperty"],"rdfs:label":"paymentId","schema:rangeIncludes":{"@id":"schema:Text"},"schema:domainIncludes":{"@id":"unece:Tax"},"rdfs:comment":"The unique identifier of the payment of this trade related tax, levy or duty."},{"@id":"unece:placeApplicableLocation","@type":["rdf:Property","owl:ObjectProperty"],"rdfs:label":"placeApplicableLocation","schema:rangeIncludes":{"@id":"unece:Location"},"schema:domainIncludes":{"@id":"unece:Tax"},"rdfs:comment":"A reference to a physical location or place."},{"@id":"unece:rateApplicablePercent","@type":["rdf:Property","owl:DatatypeProperty"],"rdfs:label":"rateApplicablePercent","schema:rangeIncludes":{"@id":"schema:Text"},"schema:domainIncludes":{"@id":"unece:Tax"},"rdfs:comment":"The applicable rate, expressed as a percentage, for this trade tax, levy or duty."},{"@id":"unece:rateCode","@type":["rdf:Property","owl:DatatypeProperty"],"rdfs:label":"rateCode","schema:rangeIncludes":{"@id":"schema:Text"},"schema:domainIncludes":{"@id":"unece:Tax"},"rdfs:comment":"The code specifying the rate for this trade related tax, levy or duty."},{"@id":"unece:selfAssessedBasisAmount","@type":["rdf:Property","owl:ObjectProperty"],"rdfs:label":"selfAssessedBasisAmount","schema:rangeIncludes":{"@id":"unece:AmountType"},"schema:domainIncludes":{"@id":"unece:Tax"},"rdfs:comment":""},{"@id":"unece:selfAssessedBasisQuantity","@type":["rdf:Property","owl:ObjectProperty"],"rdfs:label":"selfAssessedBasisQuantity","schema:rangeIncludes":{"@id":"unece:QuantityType"},"schema:domainIncludes":{"@id":"unece:Tax"},"rdfs:comment":""},{"@id":"unece:selfAssessedCalculatedAmount","@type":["rdf:Property","owl:ObjectProperty"],"rdfs:label":"selfAssessedCalculatedAmount","schema:rangeIncludes":{"@id":"unece:AmountType"},"schema:domainIncludes":{"@id":"unece:Tax"},"rdfs:comment":""},{"@id":"unece:sellerPayableTaxSpecifiedAccountingAccount","@type":["rdf:Property","owl:ObjectProperty"],"rdfs:label":"sellerPayableTaxSpecifiedAccountingAccount","schema:rangeIncludes":{"@id":"unece:AccountingAccount"},"schema:domainIncludes":{"@id":"unece:Tax"},"rdfs:comment":"The seller payable tax specified accounting account for this trade related tax, levy or duty."},{"@id":"unece:sellerRefundableTaxSpecifiedAccountingAccount","@type":["rdf:Property","owl:ObjectProperty"],"rdfs:label":"sellerRefundableTaxSpecifiedAccountingAccount","schema:rangeIncludes":{"@id":"unece:AccountingAccount"},"schema:domainIncludes":{"@id":"unece:Tax"},"rdfs:comment":"The seller refundable tax specified accounting account for this trade related tax, levy or duty."},{"@id":"unece:serviceSupplyCountry","@type":["rdf:Property","owl:ObjectProperty"],"rdfs:label":"serviceSupplyCountry","schema:rangeIncludes":{"@id":"unece:Country"},"schema:domainIncludes":{"@id":"unece:Tax"},"rdfs:comment":"The area of land that belongs to a nation together with its properties, such as population, political organization, etc., used or referenced for trade purposes."},{"@id":"unece:specifiedAccountingAccount","@type":["rdf:Property","owl:ObjectProperty"],"rdfs:label":"specifiedAccountingAccount","schema:rangeIncludes":{"@id":"unece:AccountingAccount"},"schema:domainIncludes":{"@id":"unece:Tax"},"rdfs:comment":"A specified accounting account for this trade related tax, levy or duty."},{"@id":"unece:tariffDeductionQuantity","@type":["rdf:Property","owl:ObjectProperty"],"rdfs:label":"tariffDeductionQuantity","schema:rangeIncludes":{"@id":"unece:QuantityType"},"schema:domainIncludes":{"@id":"unece:Tax"},"rdfs:comment":""},{"@id":"unece:taxBasisAllowanceRate","@type":["rdf:Property","owl:DatatypeProperty"],"rdfs:label":"taxBasisAllowanceRate","schema:rangeIncludes":{"@id":"schema:Text"},"schema:domainIncludes":{"@id":"unece:Tax"},"rdfs:comment":"The rate of the tax basis allowance (deduction or discount) used to calculate the trade related tax, levy or duty."},{"@id":"unece:taxCategoryCode","@type":["rdf:Property","owl:DatatypeProperty"],"rdfs:label":"taxCategoryCode","schema:rangeIncludes":{"@id":"unece:TaxCategoryCodeList"},"schema:domainIncludes":{"@id":"unece:Tax"},"rdfs:comment":"The code specifying the category to which this trade related tax, levy or duty applies, such as codes for \"Exempt from Tax\", \"Standard Rate\", \"Free Export Item - Tax Not Charged\" [Reference United Nations Code List (UNCL) 5305]."},{"@id":"unece:taxExemptionAuthorityId","@type":["rdf:Property","owl:DatatypeProperty"],"rdfs:label":"taxExemptionAuthorityId","schema:rangeIncludes":{"@id":"schema:Text"},"schema:domainIncludes":{"@id":"unece:Tax"},"rdfs:comment":"The unique tax exemption authority identifier for this trade tax."},{"@id":"unece:taxExemptionReasonExemptionReasonCode","@type":["rdf:Property","owl:DatatypeProperty"],"rdfs:label":"taxExemptionReasonExemptionReasonCode","schema:rangeIncludes":{"@id":"unece:TaxExemptionReasonCodeList"},"schema:domainIncludes":{"@id":"unece:Tax"},"rdfs:comment":"A code specifying a reason for exemption from this trade related tax, levy or duty."},{"@id":"unece:taxType","@type":["rdf:Property","owl:DatatypeProperty"],"rdfs:label":"taxType","schema:rangeIncludes":{"@id":"schema:Text"},"schema:domainIncludes":{"@id":"unece:Tax"},"rdfs:comment":"The type, expressed as text, of this trade related tax, levy or duty."},{"@id":"unece:taxTypeCode","@type":["rdf:Property","owl:DatatypeProperty"],"rdfs:label":"taxTypeCode","schema:rangeIncludes":{"@id":"unece:TaxTypeCodeList"},"schema:domainIncludes":{"@id":"unece:Tax"},"rdfs:comment":"The code specifying the type of trade related tax, levy or duty, such as a code for a Value Added Tax (VAT) [Reference United Nations Code List (UNCL) 5153]."},{"@id":"unece:timeReferenceDueDateTypeCode","@type":["rdf:Property","owl:DatatypeProperty"],"rdfs:label":"timeReferenceDueDateTypeCode","schema:rangeIncludes":{"@id":"unece:TimeReferenceCodeList"},"schema:domainIncludes":{"@id":"unece:Tax"},"rdfs:comment":"The code specifying a type of due date for this trade tax."},{"@id":"unece:tradeTaxCurrencyCode","@type":["rdf:Property","owl:DatatypeProperty"],"rdfs:label":"tradeTaxCurrencyCode","schema:rangeIncludes":{"@id":"unece:CurrencyCodeList"},"schema:domainIncludes":{"@id":"unece:Tax"},"rdfs:comment":"The code specifying the currency for this trade related tax, levy or duty [UNCL 6345]."},{"@id":"unece:tradeTaxPaymentMethodCode","@type":["rdf:Property","owl:DatatypeProperty"],"rdfs:label":"tradeTaxPaymentMethodCode","schema:rangeIncludes":{"@id":"unece:PaymentMethodCodeList"},"schema:domainIncludes":{"@id":"unece:Tax"},"rdfs:comment":"The code specifying the payment method for this trade related tax, levy or duty."},{"@id":"unece:unitBasisAmount","@type":["rdf:Property","owl:ObjectProperty"],"rdfs:label":"unitBasisAmount","schema:rangeIncludes":{"@id":"unece:AmountType"},"schema:domainIncludes":[{"@id":"unece:Tax"},{"@id":"unece:TradeAllowanceCharge"}],"rdfs:comment":""},{"@id":"unece:associatedDocument","@type":["rdf:Property","owl:ObjectProperty"],"rdfs:label":"associatedDocument","schema:rangeIncludes":{"@id":"unece:Document"},"schema:domainIncludes":[{"@id":"unece:CurrencyExchange"},{"@id":"unece:TradePrice"}],"rdfs:comment":"Written, printed or electronic matter that is referenced."},{"@id":"unece:conversionRate","@type":["rdf:Property","owl:DatatypeProperty"],"rdfs:label":"conversionRate","schema:rangeIncludes":{"@id":"schema:Text"},"schema:domainIncludes":{"@id":"unece:CurrencyExchange"},"rdfs:comment":"The rate factor used for conversion from the source currency to the target currency for trade purposes."},{"@id":"unece:conversionRateDateTime","@type":["rdf:Property","owl:DatatypeProperty"],"rdfs:label":"conversionRateDateTime","schema:rangeIncludes":{"@id":"schema:Text"},"schema:domainIncludes":{"@id":"unece:CurrencyExchange"},"rdfs:comment":"The date, time, date time or other date time value of the conversion rate for this trade related currency exchange."},{"@id":"unece:currencySourceCurrencyCode","@type":["rdf:Property","owl:DatatypeProperty"],"rdfs:label":"currencySourceCurrencyCode","schema:rangeIncludes":{"@id":"unece:CurrencyCodeList"},"schema:domainIncludes":{"@id":"unece:CurrencyExchange"},"rdfs:comment":"The code specifying the source currency of a trade related currency conversion."},{"@id":"unece:currencyTargetCurrencyCode","@type":["rdf:Property","owl:DatatypeProperty"],"rdfs:label":"currencyTargetCurrencyCode","schema:rangeIncludes":{"@id":"unece:CurrencyCodeList"},"schema:domainIncludes":{"@id":"unece:CurrencyExchange"},"rdfs:comment":"The code specifying the target currency of a trade related currency conversion."},{"@id":"unece:sourceUnitBasisNumeric","@type":["rdf:Property","owl:DatatypeProperty"],"rdfs:label":"sourceUnitBasisNumeric","schema:rangeIncludes":{"@id":"schema:Text"},"schema:domainIncludes":{"@id":"unece:CurrencyExchange"},"rdfs:comment":"The numeric unit basis of the source currency used in this trade related currency exchange rate calculation."},{"@id":"unece:targetUnitBaseNumeric","@type":["rdf:Property","owl:DatatypeProperty"],"rdfs:label":"targetUnitBaseNumeric","schema:rangeIncludes":{"@id":"schema:Text"},"schema:domainIncludes":{"@id":"unece:CurrencyExchange"},"rdfs:comment":"The numeric unit basis of the target currency used in this trade related currency exchange rate calculation."},{"@id":"unece:tradeCurrencyExchangeMarketId","@type":["rdf:Property","owl:DatatypeProperty"],"rdfs:label":"tradeCurrencyExchangeMarketId","schema:rangeIncludes":{"@id":"schema:Text"},"schema:domainIncludes":{"@id":"unece:CurrencyExchange"},"rdfs:comment":"The unique identifier of the currency exchange market from which the exchange rate is taken for trade purposes."},{"@id":"unece:faceAmount","@type":["rdf:Property","owl:ObjectProperty"],"rdfs:label":"faceAmount","schema:rangeIncludes":{"@id":"unece:AmountType"},"schema:domainIncludes":{"@id":"unece:Voucher"},"rdfs:comment":""},{"@id":"unece:issueDateTime","@type":["rdf:Property","owl:DatatypeProperty"],"rdfs:label":"issueDateTime","schema:rangeIncludes":{"@id":"schema:Text"},"schema:domainIncludes":[{"@id":"unece:Voucher"},{"@id":"unece:Document"},{"@id":"unece:ExchangedDocument"},{"@id":"unece:Error"},{"@id":"unece:Version"}],"rdfs:comment":"An issue date, time, date time or other date time value for this declared error."},{"@id":"unece:adjustedBalanceOutAmount","@type":["rdf:Property","owl:ObjectProperty"],"rdfs:label":"adjustedBalanceOutAmount","schema:rangeIncludes":{"@id":"unece:AmountType"},"schema:domainIncludes":{"@id":"unece:TradeSettlementPaymentMonetarySummation"},"rdfs:comment":""},{"@id":"unece:applicablePaymentBalanceOut","@type":["rdf:Property","owl:ObjectProperty"],"rdfs:label":"applicablePaymentBalanceOut","schema:rangeIncludes":{"@id":"unece:PaymentBalanceOut"},"schema:domainIncludes":{"@id":"unece:TradeSettlementPaymentMonetarySummation"},"rdfs:comment":"A balance out applicable to this trade settlement payment monetary summation."},{"@id":"unece:balanceOutAmount","@type":["rdf:Property","owl:ObjectProperty"],"rdfs:label":"balanceOutAmount","schema:rangeIncludes":{"@id":"unece:AmountType"},"schema:domainIncludes":{"@id":"unece:TradeSettlementPaymentMonetarySummation"},"rdfs:comment":""},{"@id":"unece:equivalentTransferTotalAmount","@type":["rdf:Property","owl:ObjectProperty"],"rdfs:label":"equivalentTransferTotalAmount","schema:rangeIncludes":{"@id":"unece:AmountType"},"schema:domainIncludes":{"@id":"unece:TradeSettlementPaymentMonetarySummation"},"rdfs:comment":""},{"@id":"unece:includingTaxesLineTotalAmount","@type":["rdf:Property","owl:ObjectProperty"],"rdfs:label":"includingTaxesLineTotalAmount","schema:rangeIncludes":{"@id":"unece:AmountType"},"schema:domainIncludes":{"@id":"unece:TradeSettlementPaymentMonetarySummation"},"rdfs:comment":""},{"@id":"unece:netLineTotalAmount","@type":["rdf:Property","owl:ObjectProperty"],"rdfs:label":"netLineTotalAmount","schema:rangeIncludes":{"@id":"unece:AmountType"},"schema:domainIncludes":{"@id":"unece:TradeSettlementPaymentMonetarySummation"},"rdfs:comment":""},{"@id":"unece:paymentTotalAmount","@type":["rdf:Property","owl:ObjectProperty"],"rdfs:label":"paymentTotalAmount","schema:rangeIncludes":{"@id":"unece:AmountType"},"schema:domainIncludes":{"@id":"unece:TradeSettlementPaymentMonetarySummation"},"rdfs:comment":""},{"@id":"unece:taxTotalAmount","@type":["rdf:Property","owl:ObjectProperty"],"rdfs:label":"taxTotalAmount","schema:rangeIncludes":{"@id":"unece:AmountType"},"schema:domainIncludes":{"@id":"unece:TradeSettlementPaymentMonetarySummation"},"rdfs:comment":""},{"@id":"unece:actualCurrencyExchange","@type":["rdf:Property","owl:ObjectProperty"],"rdfs:label":"actualCurrencyExchange","schema:rangeIncludes":{"@id":"unece:CurrencyExchange"},"schema:domainIncludes":{"@id":"unece:TradeAllowanceCharge"},"rdfs:comment":"The actual trade currency exchange for this trade allowance charge."},{"@id":"unece:allowanceChargeIdTypeCode","@type":["rdf:Property","owl:DatatypeProperty"],"rdfs:label":"allowanceChargeIdTypeCode","schema:rangeIncludes":{"@id":"unece:AllowanceChargeIdCodeList"},"schema:domainIncludes":{"@id":"unece:TradeAllowanceCharge"},"rdfs:comment":"The code specifying the type of this trade allowance charge."},{"@id":"unece:allowanceChargeReasonCode","@type":["rdf:Property","owl:DatatypeProperty"],"rdfs:label":"allowanceChargeReasonCode","schema:rangeIncludes":{"@id":"unece:AllowanceChargeReasonCodeList"},"schema:domainIncludes":{"@id":"unece:TradeAllowanceCharge"},"rdfs:comment":"The code specifying the reason for this trade allowance charge."},{"@id":"unece:categoryTradeTax","@type":["rdf:Property","owl:ObjectProperty"],"rdfs:label":"categoryTradeTax","schema:rangeIncludes":{"@id":"unece:Tax"},"schema:domainIncludes":{"@id":"unece:TradeAllowanceCharge"},"rdfs:comment":"A tax category of this trade allowance charge."},{"@id":"unece:prepaidIndicator","@type":["rdf:Property","owl:DatatypeProperty"],"rdfs:label":"prepaidIndicator","schema:rangeIncludes":{"@id":"schema:Boolean"},"schema:domainIncludes":{"@id":"unece:TradeAllowanceCharge"},"rdfs:comment":"The indication of whether or not this trade allowance charge is prepaid."},{"@id":"unece:sequenceNumeric","@type":["rdf:Property","owl:DatatypeProperty"],"rdfs:label":"sequenceNumeric","schema:rangeIncludes":{"@id":"schema:Text"},"schema:domainIncludes":[{"@id":"unece:TradeAllowanceCharge"},{"@id":"unece:SpecifiedPeriod"},{"@id":"unece:DocumentStatus"}],"rdfs:comment":"A sequence number for these specified personal effects."},{"@id":"unece:applicableCustomerClass","@type":["rdf:Property","owl:ObjectProperty"],"rdfs:label":"applicableCustomerClass","schema:rangeIncludes":{"@id":"unece:CustomerClass"},"schema:domainIncludes":{"@id":"unece:TradePrice"},"rdfs:comment":"The conditions and requirements of the type of person who may use or purchase a product or service."},{"@id":"unece:applicableSpecifiedNote","@type":["rdf:Property","owl:ObjectProperty"],"rdfs:label":"applicableSpecifiedNote","schema:rangeIncludes":{"@id":"unece:SpecifiedNote"},"schema:domainIncludes":{"@id":"unece:TradePrice"},"rdfs:comment":"A specified textual or coded description, such as a remark or additional information."},{"@id":"unece:appliedAllowanceCharge","@type":["rdf:Property","owl:ObjectProperty"],"rdfs:label":"appliedAllowanceCharge","schema:rangeIncludes":{"@id":"unece:TradeAllowanceCharge"},"schema:domainIncludes":{"@id":"unece:TradePrice"},"rdfs:comment":"An allowance or charge applied to the trade price."},{"@id":"unece:bracketTypeCode","@type":["rdf:Property","owl:DatatypeProperty"],"rdfs:label":"bracketTypeCode","schema:rangeIncludes":{"@id":"schema:Text"},"schema:domainIncludes":{"@id":"unece:TradePrice"},"rdfs:comment":"The code specifying the type of bracket for this trade price."},{"@id":"unece:cancellationPercent","@type":["rdf:Property","owl:DatatypeProperty"],"rdfs:label":"cancellationPercent","schema:rangeIncludes":{"@id":"schema:Text"},"schema:domainIncludes":{"@id":"unece:TradePrice"},"rdfs:comment":"The cancellation percentage for this trade price."},{"@id":"unece:categoryTypeCode","@type":["rdf:Property","owl:DatatypeProperty"],"rdfs:label":"categoryTypeCode","schema:rangeIncludes":{"@id":"schema:Text"},"schema:domainIncludes":{"@id":"unece:TradePrice"},"rdfs:comment":"The code specifying the type of category, such as refund or service charge, for this trade price."},{"@id":"unece:changeReason","@type":["rdf:Property","owl:DatatypeProperty"],"rdfs:label":"changeReason","schema:rangeIncludes":{"@id":"schema:Text"},"schema:domainIncludes":{"@id":"unece:TradePrice"},"rdfs:comment":"A reason, expressed as text, for a change of this trade price."},{"@id":"unece:customerServicePointQuantity","@type":["rdf:Property","owl:ObjectProperty"],"rdfs:label":"customerServicePointQuantity","schema:rangeIncludes":{"@id":"unece:QuantityType"},"schema:domainIncludes":{"@id":"unece:TradePrice"},"rdfs:comment":""},{"@id":"unece:dayQuantity","@type":["rdf:Property","owl:ObjectProperty"],"rdfs:label":"dayQuantity","schema:rangeIncludes":{"@id":"unece:QuantityType"},"schema:domainIncludes":[{"@id":"unece:TradePrice"},{"@id":"unece:SpecifiedPeriod"}],"rdfs:comment":""},{"@id":"unece:deliveryLocation","@type":["rdf:Property","owl:ObjectProperty"],"rdfs:label":"deliveryLocation","schema:rangeIncludes":{"@id":"unece:Location"},"schema:domainIncludes":{"@id":"unece:TradePrice"},"rdfs:comment":"A reference to a physical location or place."},{"@id":"unece:determinationCode","@type":["rdf:Property","owl:DatatypeProperty"],"rdfs:label":"determinationCode","schema:rangeIncludes":{"@id":"schema:Text"},"schema:domainIncludes":{"@id":"unece:TradePrice"},"rdfs:comment":"The code specifying the determination of this trade price."},{"@id":"unece:grandTotalChargeAmount","@type":["rdf:Property","owl:ObjectProperty"],"rdfs:label":"grandTotalChargeAmount","schema:rangeIncludes":{"@id":"unece:AmountType"},"schema:domainIncludes":{"@id":"unece:TradePrice"},"rdfs:comment":""},{"@id":"unece:maximumQuantity","@type":["rdf:Property","owl:ObjectProperty"],"rdfs:label":"maximumQuantity","schema:rangeIncludes":{"@id":"unece:QuantityType"},"schema:domainIncludes":{"@id":"unece:TradePrice"},"rdfs:comment":""},{"@id":"unece:minimumQuantity","@type":["rdf:Property","owl:ObjectProperty"],"rdfs:label":"minimumQuantity","schema:rangeIncludes":{"@id":"unece:QuantityType"},"schema:domainIncludes":{"@id":"unece:TradePrice"},"rdfs:comment":""},{"@id":"unece:multipleReasonIndicator","@type":["rdf:Property","owl:DatatypeProperty"],"rdfs:label":"multipleReasonIndicator","schema:rangeIncludes":{"@id":"schema:Boolean"},"schema:domainIncludes":{"@id":"unece:TradePrice"},"rdfs:comment":"The indication of whether or not multiple reasons affect this trade price."},{"@id":"unece:netPriceIndicator","@type":["rdf:Property","owl:DatatypeProperty"],"rdfs:label":"netPriceIndicator","schema:rangeIncludes":{"@id":"schema:Boolean"},"schema:domainIncludes":[{"@id":"unece:TradePrice"},{"@id":"unece:ReferencePrice"}],"rdfs:comment":"An indication of whether or not the reference price is a net price."},{"@id":"unece:operationalApplicablePeriod","@type":["rdf:Property","owl:ObjectProperty"],"rdfs:label":"operationalApplicablePeriod","schema:rangeIncludes":{"@id":"unece:SpecifiedPeriod"},"schema:domainIncludes":{"@id":"unece:TradePrice"},"rdfs:comment":"A specified period of time."},{"@id":"unece:orderUnitConversionFactorNumeric","@type":["rdf:Property","owl:DatatypeProperty"],"rdfs:label":"orderUnitConversionFactorNumeric","schema:rangeIncludes":{"@id":"schema:Text"},"schema:domainIncludes":{"@id":"unece:TradePrice"},"rdfs:comment":"The value used as the factor to convert the order unit into the price unit for this trade price."},{"@id":"unece:priceType","@type":["rdf:Property","owl:DatatypeProperty"],"rdfs:label":"priceType","schema:rangeIncludes":{"@id":"schema:Text"},"schema:domainIncludes":{"@id":"unece:TradePrice"},"rdfs:comment":"A type, expressed as text, for this trade price."},{"@id":"unece:priceTypeCode","@type":["rdf:Property","owl:DatatypeProperty"],"rdfs:label":"priceTypeCode","schema:rangeIncludes":{"@id":"unece:PriceTypeCodeList"},"schema:domainIncludes":{"@id":"unece:TradePrice"},"rdfs:comment":"The code specifying the type of trade price."},{"@id":"unece:seasonalApplicablePeriod","@type":["rdf:Property","owl:ObjectProperty"],"rdfs:label":"seasonalApplicablePeriod","schema:rangeIncludes":{"@id":"unece:SpecifiedPeriod"},"schema:domainIncludes":{"@id":"unece:TradePrice"},"rdfs:comment":"A specified period of time."},{"@id":"unece:seasonalRankCode","@type":["rdf:Property","owl:DatatypeProperty"],"rdfs:label":"seasonalRankCode","schema:rangeIncludes":{"@id":"schema:Text"},"schema:domainIncludes":{"@id":"unece:TradePrice"},"rdfs:comment":"The code specifying the seasonal rank of this trade price."},{"@id":"unece:specifiedPaymentTradeSettlement","@type":["rdf:Property","owl:ObjectProperty"],"rdfs:label":"specifiedPaymentTradeSettlement","schema:rangeIncludes":{"@id":"unece:PaymentTradeSettlement"},"schema:domainIncludes":{"@id":"unece:TradePrice"},"rdfs:comment":"A payment trade settlement specified for this trade price."},{"@id":"unece:totalChargeAmount","@type":["rdf:Property","owl:ObjectProperty"],"rdfs:label":"totalChargeAmount","schema:rangeIncludes":{"@id":"unece:AmountType"},"schema:domainIncludes":{"@id":"unece:TradePrice"},"rdfs:comment":""},{"@id":"unece:tradeComparisonPrice","@type":["rdf:Property","owl:ObjectProperty"],"rdfs:label":"tradeComparisonPrice","schema:rangeIncludes":{"@id":"unece:ReferencePrice"},"schema:domainIncludes":{"@id":"unece:TradePrice"},"rdfs:comment":"A price that provides a trade comparison with this trade price."},{"@id":"unece:unitAmount","@type":["rdf:Property","owl:ObjectProperty"],"rdfs:label":"unitAmount","schema:rangeIncludes":{"@id":"unece:AmountType"},"schema:domainIncludes":{"@id":"unece:TradePrice"},"rdfs:comment":""},{"@id":"unece:validityPeriod","@type":["rdf:Property","owl:ObjectProperty"],"rdfs:label":"validityPeriod","schema:rangeIncludes":{"@id":"unece:SpecifiedPeriod"},"schema:domainIncludes":[{"@id":"unece:TradePrice"},{"@id":"unece:Document"},{"@id":"unece:BinaryFile"},{"@id":"unece:DocumentStatus"}],"rdfs:comment":"A specified period of time."},{"@id":"unece:comparisonMethodCode","@type":["rdf:Property","owl:DatatypeProperty"],"rdfs:label":"comparisonMethodCode","schema:rangeIncludes":{"@id":"schema:Text"},"schema:domainIncludes":{"@id":"unece:ReferencePrice"},"rdfs:comment":"The code specifying the comparison method for this reference price."},{"@id":"unece:addedAdjustmentAmount","@type":["rdf:Property","owl:ObjectProperty"],"rdfs:label":"addedAdjustmentAmount","schema:rangeIncludes":{"@id":"unece:AmountType"},"schema:domainIncludes":{"@id":"unece:CustomsValuation"},"rdfs:comment":""},{"@id":"unece:addedAdjustmentPercent","@type":["rdf:Property","owl:DatatypeProperty"],"rdfs:label":"addedAdjustmentPercent","schema:rangeIncludes":{"@id":"schema:Text"},"schema:domainIncludes":{"@id":"unece:CustomsValuation"},"rdfs:comment":"The adjustment added, expressed as a percentage, for this cross-border customs valuation."},{"@id":"unece:applicableCurrencyExchange","@type":["rdf:Property","owl:ObjectProperty"],"rdfs:label":"applicableCurrencyExchange","schema:rangeIncludes":{"@id":"unece:CurrencyExchange"},"schema:domainIncludes":{"@id":"unece:CustomsValuation"},"rdfs:comment":"A currency exchange applicable to this supply chain consignment."},{"@id":"unece:buyerSellerRelationshipIndicator","@type":["rdf:Property","owl:DatatypeProperty"],"rdfs:label":"buyerSellerRelationshipIndicator","schema:rangeIncludes":{"@id":"schema:Boolean"},"schema:domainIncludes":{"@id":"unece:CustomsValuation"},"rdfs:comment":"The indication of whether or not there is a relationship between the buyer and the seller, such as a financial relationship, for this cross-border customs valuation."},{"@id":"unece:buyerSellerRelationshipPriceInfluenceIndicator","@type":["rdf:Property","owl:DatatypeProperty"],"rdfs:label":"buyerSellerRelationshipPriceInfluenceIndicator","schema:rangeIncludes":{"@id":"schema:Boolean"},"schema:domainIncludes":{"@id":"unece:CustomsValuation"},"rdfs:comment":"The indication of whether or not the buyer seller relationship influences the price of the goods for this cross-border customs valuation."},{"@id":"unece:chargeApportionMethodCode","@type":["rdf:Property","owl:DatatypeProperty"],"rdfs:label":"chargeApportionMethodCode","schema:rangeIncludes":{"@id":"schema:Text"},"schema:domainIncludes":{"@id":"unece:CustomsValuation"},"rdfs:comment":"The code specifying the method of the apportion of charges for this cross-border customs valuation."},{"@id":"unece:deductedAdjustmentAmount","@type":["rdf:Property","owl:ObjectProperty"],"rdfs:label":"deductedAdjustmentAmount","schema:rangeIncludes":{"@id":"unece:AmountType"},"schema:domainIncludes":{"@id":"unece:CustomsValuation"},"rdfs:comment":""},{"@id":"unece:deductedAdjustmentPercent","@type":["rdf:Property","owl:DatatypeProperty"],"rdfs:label":"deductedAdjustmentPercent","schema:rangeIncludes":{"@id":"schema:Text"},"schema:domainIncludes":{"@id":"unece:CustomsValuation"},"rdfs:comment":"The adjustment deducted, expressed as a percentage, for this cross-border customs valuation."},{"@id":"unece:methodCode","@type":["rdf:Property","owl:DatatypeProperty"],"rdfs:label":"methodCode","schema:rangeIncludes":{"@id":"schema:Text"},"schema:domainIncludes":[{"@id":"unece:CustomsValuation"},{"@id":"unece:Pairing"}],"rdfs:comment":"The code specifying the method by which this cross-border customs valuation is determined."},{"@id":"unece:otherChargeAmount","@type":["rdf:Property","owl:ObjectProperty"],"rdfs:label":"otherChargeAmount","schema:rangeIncludes":{"@id":"unece:AmountType"},"schema:domainIncludes":{"@id":"unece:CustomsValuation"},"rdfs:comment":""},{"@id":"unece:royaltyLicenseFeeIndicator","@type":["rdf:Property","owl:DatatypeProperty"],"rdfs:label":"royaltyLicenseFeeIndicator","schema:rangeIncludes":{"@id":"schema:Boolean"},"schema:domainIncludes":{"@id":"unece:CustomsValuation"},"rdfs:comment":"The indication of whether or not there is a royalty or licence fee related to the goods for this cross-border customs valuation."},{"@id":"unece:salePriceConditionIndicator","@type":["rdf:Property","owl:DatatypeProperty"],"rdfs:label":"salePriceConditionIndicator","schema:rangeIncludes":{"@id":"schema:Boolean"},"schema:domainIncludes":{"@id":"unece:CustomsValuation"},"rdfs:comment":"The indication of whether or not there is a condition imposed on the sale price of the goods for this cross-border customs valuation."},{"@id":"unece:saleRestriction","@type":["rdf:Property","owl:DatatypeProperty"],"rdfs:label":"saleRestriction","schema:rangeIncludes":{"@id":"schema:Text"},"schema:domainIncludes":{"@id":"unece:CustomsValuation"},"rdfs:comment":"A restriction, expressed as text, imposed on the sale of the goods for this cross-border customs valuation."},{"@id":"unece:saleRestrictionIndicator","@type":["rdf:Property","owl:DatatypeProperty"],"rdfs:label":"saleRestrictionIndicator","schema:rangeIncludes":{"@id":"schema:Boolean"},"schema:domainIncludes":{"@id":"unece:CustomsValuation"},"rdfs:comment":"The indication of whether or not there is any restriction imposed on the sale of the goods for this cross-border customs valuation."},{"@id":"unece:wTOAdditionCode","@type":["rdf:Property","owl:DatatypeProperty"],"rdfs:label":"wTOAdditionCode","schema:rangeIncludes":{"@id":"schema:Text"},"schema:domainIncludes":{"@id":"unece:CustomsValuation"},"rdfs:comment":"The code specifying any additions necessary under the World Trade Organization (WTO) Valuation Agreement used for the assessment of this cross-border customs valuation."},{"@id":"unece:abstract","@type":["rdf:Property","owl:DatatypeProperty"],"rdfs:label":"abstract","schema:rangeIncludes":{"@id":"schema:Text"},"schema:domainIncludes":{"@id":"unece:ComplexDescription"},"rdfs:comment":"A textual abstract of the content of the work item complex description."},{"@id":"unece:content","@type":["rdf:Property","owl:DatatypeProperty"],"rdfs:label":"content","schema:rangeIncludes":{"@id":"schema:Text"},"schema:domainIncludes":[{"@id":"unece:ComplexDescription"},{"@id":"unece:InformationSource"},{"@id":"unece:Note"},{"@id":"unece:Response"},{"@id":"unece:SpecialQuery"},{"@id":"unece:SpecifiedNote"},{"@id":"unece:Clause"},{"@id":"unece:SpecificationQuery"}],"rdfs:comment":"A content, expressed as text, of this note."},{"@id":"unece:requestingQuery","@type":["rdf:Property","owl:ObjectProperty"],"rdfs:label":"requestingQuery","schema:rangeIncludes":{"@id":"unece:SpecificationQuery"},"schema:domainIncludes":{"@id":"unece:ComplexDescription"},"rdfs:comment":"A requesting specification query for this work item complex description."},{"@id":"unece:respondingResponse","@type":["rdf:Property","owl:ObjectProperty"],"rdfs:label":"respondingResponse","schema:rangeIncludes":{"@id":"unece:Response"},"schema:domainIncludes":{"@id":"unece:ComplexDescription"},"rdfs:comment":"A responding specification response for this work item complex description."},{"@id":"unece:subsetComplexDescription","@type":["rdf:Property","owl:ObjectProperty"],"rdfs:label":"subsetComplexDescription","schema:rangeIncludes":{"@id":"unece:ComplexDescription"},"schema:domainIncludes":{"@id":"unece:ComplexDescription"},"rdfs:comment":"The complex description subset for this work item complex description."},{"@id":"unece:acceptablePeriod","@type":["rdf:Property","owl:ObjectProperty"],"rdfs:label":"acceptablePeriod","schema:rangeIncludes":{"@id":"unece:SpecifiedPeriod"},"schema:domainIncludes":{"@id":"unece:Document"},"rdfs:comment":"The specified period within which this referenced document may be accepted."},{"@id":"unece:acceptanceDateTime","@type":["rdf:Property","owl:DatatypeProperty"],"rdfs:label":"acceptanceDateTime","schema:rangeIncludes":{"@id":"schema:Text"},"schema:domainIncludes":[{"@id":"unece:Document"},{"@id":"unece:ExchangedDocument"}],"rdfs:comment":"The date, time, date time, or other date time value for the acceptance of this exchanged document."},{"@id":"unece:attachedBinaryFile","@type":["rdf:Property","owl:ObjectProperty"],"rdfs:label":"attachedBinaryFile","schema:rangeIncludes":{"@id":"unece:BinaryFile"},"schema:domainIncludes":[{"@id":"unece:Document"},{"@id":"unece:ExchangedDocument"},{"@id":"unece:Picture"}],"rdfs:comment":"A binary file attached for this sustainability inspection."},{"@id":"unece:attachmentBinaryObject","@type":["rdf:Property","owl:DatatypeProperty"],"rdfs:label":"attachmentBinaryObject","schema:rangeIncludes":{"@id":"schema:Text"},"schema:domainIncludes":{"@id":"unece:Document"},"rdfs:comment":"A binary object that is attached or otherwise appended to this referenced document."},{"@id":"unece:authenticatedOriginalIndicator","@type":["rdf:Property","owl:DatatypeProperty"],"rdfs:label":"authenticatedOriginalIndicator","schema:rangeIncludes":{"@id":"schema:Boolean"},"schema:domainIncludes":{"@id":"unece:Document"},"rdfs:comment":"The indication of whether or not this referenced document is an authenticated original."},{"@id":"unece:categoryCode","@type":["rdf:Property","owl:DatatypeProperty"],"rdfs:label":"categoryCode","schema:rangeIncludes":{"@id":"schema:Text"},"schema:domainIncludes":[{"@id":"unece:Document"},{"@id":"unece:ExchangedDocument"},{"@id":"unece:SpecifiedFault"},{"@id":"unece:Object"},{"@id":"unece:CustomerClass"},{"@id":"unece:InformationSource"},{"@id":"unece:Authentication"}],"rdfs:comment":"A code specifying a category for this cross-border regulatory procedure, such as the appendices of the CITES Convention."},{"@id":"unece:documentLanguageId","@type":["rdf:Property","owl:DatatypeProperty"],"rdfs:label":"documentLanguageId","schema:rangeIncludes":{"@id":"unece:LanguageId"},"schema:domainIncludes":{"@id":"unece:Document"},"rdfs:comment":"An identifier for a language used in this referenced document."},{"@id":"unece:documentStatusCode","@type":["rdf:Property","owl:DatatypeProperty"],"rdfs:label":"documentStatusCode","schema:rangeIncludes":{"@id":"unece:DocumentStatusCodeList"},"schema:domainIncludes":[{"@id":"unece:Document"},{"@id":"unece:ExchangedDocument"}],"rdfs:comment":"The code specifying the status for this referenced document."},{"@id":"unece:documentType","@type":["rdf:Property","owl:DatatypeProperty"],"rdfs:label":"documentType","schema:rangeIncludes":{"@id":"schema:Text"},"schema:domainIncludes":{"@id":"unece:Document"},"rdfs:comment":"A type, expressed as text, for this referenced document."},{"@id":"unece:documentTypeCode","@type":["rdf:Property","owl:DatatypeProperty"],"rdfs:label":"documentTypeCode","schema:rangeIncludes":{"@id":"unece:DocumentCodeList"},"schema:domainIncludes":[{"@id":"unece:Document"},{"@id":"unece:ExchangedDocument"}],"rdfs:comment":"A code specifying a type of acknowledgement document."},{"@id":"unece:effectiveSpecifiedPeriod","@type":["rdf:Property","owl:ObjectProperty"],"rdfs:label":"effectiveSpecifiedPeriod","schema:rangeIncludes":{"@id":"unece:SpecifiedPeriod"},"schema:domainIncludes":[{"@id":"unece:Document"},{"@id":"unece:ExchangedDocument"}],"rdfs:comment":"The period within which this document line is effective."},{"@id":"unece:electronicPresentationIndicator","@type":["rdf:Property","owl:DatatypeProperty"],"rdfs:label":"electronicPresentationIndicator","schema:rangeIncludes":{"@id":"schema:Boolean"},"schema:domainIncludes":[{"@id":"unece:Document"},{"@id":"unece:ExchangedDocument"}],"rdfs:comment":"The indication of whether or not this exchanged document is presented in an electronic format."},{"@id":"unece:globalId","@type":["rdf:Property","owl:DatatypeProperty"],"rdfs:label":"globalId","schema:rangeIncludes":{"@id":"schema:Text"},"schema:domainIncludes":[{"@id":"unece:Document"},{"@id":"unece:ExchangedDocument"},{"@id":"unece:Location"}],"rdfs:comment":"A global identifier for this supply chain consignment item."},{"@id":"unece:includedAmount","@type":["rdf:Property","owl:ObjectProperty"],"rdfs:label":"includedAmount","schema:rangeIncludes":{"@id":"unece:AmountType"},"schema:domainIncludes":{"@id":"unece:Document"},"rdfs:comment":"A monetary value included in this referenced document."},{"@id":"unece:includedNote","@type":["rdf:Property","owl:ObjectProperty"],"rdfs:label":"includedNote","schema:rangeIncludes":{"@id":"unece:Note"},"schema:domainIncludes":[{"@id":"unece:Document"},{"@id":"unece:ExchangedDocument"},{"@id":"unece:DocumentStatus"}],"rdfs:comment":"A note included for this document status."},{"@id":"unece:issueLocation","@type":["rdf:Property","owl:ObjectProperty"],"rdfs:label":"issueLocation","schema:rangeIncludes":{"@id":"unece:Location"},"schema:domainIncludes":[{"@id":"unece:Document"},{"@id":"unece:ExchangedDocument"},{"@id":"unece:Authentication"}],"rdfs:comment":"The issue location for this document authentication."},{"@id":"unece:issuerAssignedId","@type":["rdf:Property","owl:DatatypeProperty"],"rdfs:label":"issuerAssignedId","schema:rangeIncludes":{"@id":"schema:Text"},"schema:domainIncludes":{"@id":"unece:Document"},"rdfs:comment":"The unique issuer assigned identifier for this referenced document."},{"@id":"unece:issuerParty","@type":["rdf:Property","owl:ObjectProperty"],"rdfs:label":"issuerParty","schema:rangeIncludes":{"@id":"unece:Party"},"schema:domainIncludes":[{"@id":"unece:Document"},{"@id":"unece:ExchangedDocument"}],"rdfs:comment":"A party that issues this specified declaration."},{"@id":"unece:issuerSpecifiedInstructions","@type":["rdf:Property","owl:ObjectProperty"],"rdfs:label":"issuerSpecifiedInstructions","schema:rangeIncludes":{"@id":"unece:DocumentHandlingInstructions"},"schema:domainIncludes":{"@id":"unece:Document"},"rdfs:comment":"Handling instructions specified by the issuer for this referenced document."},{"@id":"unece:lineId","@type":["rdf:Property","owl:DatatypeProperty"],"rdfs:label":"lineId","schema:rangeIncludes":{"@id":"schema:Text"},"schema:domainIncludes":{"@id":"unece:Document"},"rdfs:comment":"The unique identifier of a line in this referenced document."},{"@id":"unece:lodgementLocation","@type":["rdf:Property","owl:ObjectProperty"],"rdfs:label":"lodgementLocation","schema:rangeIncludes":{"@id":"unece:Location"},"schema:domainIncludes":[{"@id":"unece:Document"},{"@id":"unece:ExchangedDocument"}],"rdfs:comment":"The location where this exchanged document has been lodged."},{"@id":"unece:pageId","@type":["rdf:Property","owl:DatatypeProperty"],"rdfs:label":"pageId","schema:rangeIncludes":{"@id":"schema:Text"},"schema:domainIncludes":{"@id":"unece:Document"},"rdfs:comment":"The identifier of the page for this referenced document."},{"@id":"unece:previousRevisionId","@type":["rdf:Property","owl:DatatypeProperty"],"rdfs:label":"previousRevisionId","schema:rangeIncludes":{"@id":"schema:Text"},"schema:domainIncludes":[{"@id":"unece:Document"},{"@id":"unece:ExchangedDocument"}],"rdfs:comment":"An identifier for a previous revision of this referenced document."},{"@id":"unece:processCondition","@type":["rdf:Property","owl:DatatypeProperty"],"rdfs:label":"processCondition","schema:rangeIncludes":{"@id":"schema:Text"},"schema:domainIncludes":[{"@id":"unece:Document"},{"@id":"unece:DocumentStatus"}],"rdfs:comment":"A process condition, expressed as text, for this acknowledgement document."},{"@id":"unece:processConditionCode","@type":["rdf:Property","owl:DatatypeProperty"],"rdfs:label":"processConditionCode","schema:rangeIncludes":{"@id":"schema:Text"},"schema:domainIncludes":[{"@id":"unece:Document"},{"@id":"unece:DocumentStatus"}],"rdfs:comment":"The code specifying the process condition for this acknowledgement document."},{"@id":"unece:recipientTradeParty","@type":["rdf:Property","owl:ObjectProperty"],"rdfs:label":"recipientTradeParty","schema:rangeIncludes":{"@id":"unece:Party"},"schema:domainIncludes":[{"@id":"unece:Document"},{"@id":"unece:ExchangedDocument"}],"rdfs:comment":"A trade party that receives this exchanged document."},{"@id":"unece:referenceDateTime","@type":["rdf:Property","owl:DatatypeProperty"],"rdfs:label":"referenceDateTime","schema:rangeIncludes":{"@id":"schema:Text"},"schema:domainIncludes":[{"@id":"unece:Document"},{"@id":"unece:DocumentStatus"}],"rdfs:comment":"The reference date or date time for this referenced document."},{"@id":"unece:referenceRelationshipTypeCode","@type":["rdf:Property","owl:DatatypeProperty"],"rdfs:label":"referenceRelationshipTypeCode","schema:rangeIncludes":{"@id":"unece:ReferenceCodeList"},"schema:domainIncludes":{"@id":"unece:Document"},"rdfs:comment":"The code specifying the type of relationship between this referenced document and another artefact, such as a replacement of an original document."},{"@id":"unece:referenceTypeCode","@type":["rdf:Property","owl:DatatypeProperty"],"rdfs:label":"referenceTypeCode","schema:rangeIncludes":{"@id":"unece:ReferenceCodeList"},"schema:domainIncludes":[{"@id":"unece:Document"},{"@id":"unece:Location"}],"rdfs:comment":"The code specifying the reference type of this referenced document."},{"@id":"unece:remarks","@type":["rdf:Property","owl:DatatypeProperty"],"rdfs:label":"remarks","schema:rangeIncludes":{"@id":"schema:Text"},"schema:domainIncludes":[{"@id":"unece:Document"},{"@id":"unece:ExchangedDocument"}],"rdfs:comment":"A remark, expressed as text, regarding this exchanged document."},{"@id":"unece:revisionId","@type":["rdf:Property","owl:DatatypeProperty"],"rdfs:label":"revisionId","schema:rangeIncludes":{"@id":"schema:Text"},"schema:domainIncludes":[{"@id":"unece:Document"},{"@id":"unece:ExchangedDocument"}],"rdfs:comment":"A unique identifier for a revision of this referenced document."},{"@id":"unece:sectionName","@type":["rdf:Property","owl:DatatypeProperty"],"rdfs:label":"sectionName","schema:rangeIncludes":{"@id":"schema:Text"},"schema:domainIncludes":{"@id":"unece:Document"},"rdfs:comment":"A section name, expressed as text, for this referenced document."},{"@id":"unece:senderTradeParty","@type":["rdf:Property","owl:ObjectProperty"],"rdfs:label":"senderTradeParty","schema:rangeIncludes":{"@id":"unece:Party"},"schema:domainIncludes":[{"@id":"unece:Document"},{"@id":"unece:ExchangedDocument"}],"rdfs:comment":"The party that sends this exchanged document."},{"@id":"unece:signatoryAuthentication","@type":["rdf:Property","owl:ObjectProperty"],"rdfs:label":"signatoryAuthentication","schema:rangeIncludes":{"@id":"unece:Authentication"},"schema:domainIncludes":[{"@id":"unece:Document"},{"@id":"unece:ExchangedDocument"}],"rdfs:comment":"A signatory authentication for this referenced document."},{"@id":"unece:specifiedDocumentStatus","@type":["rdf:Property","owl:ObjectProperty"],"rdfs:label":"specifiedDocumentStatus","schema:rangeIncludes":{"@id":"unece:DocumentStatus"},"schema:domainIncludes":{"@id":"unece:Document"},"rdfs:comment":"Status information specified for this referenced document."},{"@id":"unece:status","@type":["rdf:Property","owl:DatatypeProperty"],"rdfs:label":"status","schema:rangeIncludes":{"@id":"schema:Text"},"schema:domainIncludes":{"@id":"unece:Document"},"rdfs:comment":"A status, expressed as text, for this acknowledgement document."},{"@id":"unece:subordinateLineId","@type":["rdf:Property","owl:DatatypeProperty"],"rdfs:label":"subordinateLineId","schema:rangeIncludes":{"@id":"schema:Text"},"schema:domainIncludes":{"@id":"unece:Document"},"rdfs:comment":"An identifier of a subordinate line of this document line."},{"@id":"unece:subtypeCode","@type":["rdf:Property","owl:DatatypeProperty"],"rdfs:label":"subtypeCode","schema:rangeIncludes":{"@id":"schema:Text"},"schema:domainIncludes":[{"@id":"unece:Document"},{"@id":"unece:ExchangedDocument"}],"rdfs:comment":"A code specifying a subtype of this referenced document."},{"@id":"unece:totalIssueCountNumeric","@type":["rdf:Property","owl:DatatypeProperty"],"rdfs:label":"totalIssueCountNumeric","schema:rangeIncludes":{"@id":"schema:Text"},"schema:domainIncludes":{"@id":"unece:Document"},"rdfs:comment":"The total issue count for this referenced document."},{"@id":"unece:uRIId","@type":["rdf:Property","owl:DatatypeProperty"],"rdfs:label":"uRIId","schema:rangeIncludes":{"@id":"schema:Text"},"schema:domainIncludes":[{"@id":"unece:Document"},{"@id":"unece:BinaryFile"},{"@id":"unece:Picture"},{"@id":"unece:Communication"}],"rdfs:comment":"A Uniform Resource Identifier (URI) for this specified certification."},{"@id":"unece:versionId","@type":["rdf:Property","owl:DatatypeProperty"],"rdfs:label":"versionId","schema:rangeIncludes":{"@id":"schema:Text"},"schema:domainIncludes":[{"@id":"unece:Document"},{"@id":"unece:ExchangedDocument"},{"@id":"unece:BinaryFile"},{"@id":"unece:SpecialQuery"}],"rdfs:comment":"The identifier for the version of this exchanged declaration."},{"@id":"unece:agentParty","@type":["rdf:Property","owl:ObjectProperty"],"rdfs:label":"agentParty","schema:rangeIncludes":{"@id":"unece:Party"},"schema:domainIncludes":{"@id":"unece:ExchangedDocument"},"rdfs:comment":"A party representing another party for this exchanged document."},{"@id":"unece:amendmentPurpose","@type":["rdf:Property","owl:DatatypeProperty"],"rdfs:label":"amendmentPurpose","schema:rangeIncludes":{"@id":"schema:Text"},"schema:domainIncludes":{"@id":"unece:ExchangedDocument"},"rdfs:comment":"An amendment purpose, expressed in text, for this exchanged document."},{"@id":"unece:approverSignatoryAuthentication","@type":["rdf:Property","owl:ObjectProperty"],"rdfs:label":"approverSignatoryAuthentication","schema:rangeIncludes":{"@id":"unece:Authentication"},"schema:domainIncludes":{"@id":"unece:ExchangedDocument"},"rdfs:comment":"The approver signature that authenticates this exchanged document."},{"@id":"unece:buyerSignatoryAuthentication","@type":["rdf:Property","owl:ObjectProperty"],"rdfs:label":"buyerSignatoryAuthentication","schema:rangeIncludes":{"@id":"unece:Authentication"},"schema:domainIncludes":{"@id":"unece:ExchangedDocument"},"rdfs:comment":"The buyer signature that authenticates this exchanged document."},{"@id":"unece:cancellationDateTime","@type":["rdf:Property","owl:DatatypeProperty"],"rdfs:label":"cancellationDateTime","schema:rangeIncludes":{"@id":"schema:Text"},"schema:domainIncludes":{"@id":"unece:ExchangedDocument"},"rdfs:comment":"The date, time, date time, or other date time value of a cancellation of the exchanged document."},{"@id":"unece:controlRequirementIndicator","@type":["rdf:Property","owl:DatatypeProperty"],"rdfs:label":"controlRequirementIndicator","schema:rangeIncludes":{"@id":"schema:Boolean"},"schema:domainIncludes":{"@id":"unece:ExchangedDocument"},"rdfs:comment":"The indication of whether or not a control is required for this cross-border regulatory procedure."},{"@id":"unece:copyIssuedQuantity","@type":["rdf:Property","owl:ObjectProperty"],"rdfs:label":"copyIssuedQuantity","schema:rangeIncludes":{"@id":"unece:QuantityType"},"schema:domainIncludes":{"@id":"unece:ExchangedDocument"},"rdfs:comment":"The number of copies issued of this exchanged document."},{"@id":"unece:copyRequiredQuantity","@type":["rdf:Property","owl:ObjectProperty"],"rdfs:label":"copyRequiredQuantity","schema:rangeIncludes":{"@id":"unece:QuantityType"},"schema:domainIncludes":{"@id":"unece:ExchangedDocument"},"rdfs:comment":"The number of copies required of this exchanged document."},{"@id":"unece:customsId","@type":["rdf:Property","owl:DatatypeProperty"],"rdfs:label":"customsId","schema:rangeIncludes":{"@id":"schema:Text"},"schema:domainIncludes":{"@id":"unece:ExchangedDocument"},"rdfs:comment":"A unique identifier, for customs purposes, for this consignment."},{"@id":"unece:exchangedDocumentAmendmentPurposeCode","@type":["rdf:Property","owl:DatatypeProperty"],"rdfs:label":"exchangedDocumentAmendmentPurposeCode","schema:rangeIncludes":{"@id":"schema:Text"},"schema:domainIncludes":{"@id":"unece:ExchangedDocument"},"rdfs:comment":"A code specifying a purpose of an amendment to this exchanged document."},{"@id":"unece:exchangedDocumentResponseTypeCode","@type":["rdf:Property","owl:DatatypeProperty"],"rdfs:label":"exchangedDocumentResponseTypeCode","schema:rangeIncludes":{"@id":"unece:ResponseTypeCodeList"},"schema:domainIncludes":{"@id":"unece:ExchangedDocument"},"rdfs:comment":"A code specifying a type of response requested for this exchanged document."},{"@id":"unece:firstSignatoryAuthentication","@type":["rdf:Property","owl:ObjectProperty"],"rdfs:label":"firstSignatoryAuthentication","schema:rangeIncludes":{"@id":"unece:Authentication"},"schema:domainIncludes":{"@id":"unece:ExchangedDocument"},"rdfs:comment":"The first or primary signature that authenticates this exchanged document."},{"@id":"unece:firstVersionIssueDateTime","@type":["rdf:Property","owl:DatatypeProperty"],"rdfs:label":"firstVersionIssueDateTime","schema:rangeIncludes":{"@id":"schema:Text"},"schema:domainIncludes":{"@id":"unece:ExchangedDocument"},"rdfs:comment":"The date, time, date time or other date time value when the first version of this exchanged document was issued."},{"@id":"unece:fourthSignatoryAuthentication","@type":["rdf:Property","owl:ObjectProperty"],"rdfs:label":"fourthSignatoryAuthentication","schema:rangeIncludes":{"@id":"unece:Authentication"},"schema:domainIncludes":{"@id":"unece:ExchangedDocument"},"rdfs:comment":"The fourth signature, also known as the third counter signature, that has been authenticated on this exchanged document indicating where appropriate the authentication party."},{"@id":"unece:languageId","@type":["rdf:Property","owl:DatatypeProperty"],"rdfs:label":"languageId","schema:rangeIncludes":{"@id":"schema:Text"},"schema:domainIncludes":{"@id":"unece:ExchangedDocument"},"rdfs:comment":"A unique identifier for a language used in this exchanged document."},{"@id":"unece:lineCountNumeric","@type":["rdf:Property","owl:DatatypeProperty"],"rdfs:label":"lineCountNumeric","schema:rangeIncludes":{"@id":"schema:Text"},"schema:domainIncludes":{"@id":"unece:ExchangedDocument"},"rdfs:comment":"The count of the number of lines in this exchanged document."},{"@id":"unece:lineItemQuantity","@type":["rdf:Property","owl:ObjectProperty"],"rdfs:label":"lineItemQuantity","schema:rangeIncludes":{"@id":"unece:QuantityType"},"schema:domainIncludes":{"@id":"unece:ExchangedDocument"},"rdfs:comment":"The number of line items for this supply chain trade transaction."},{"@id":"unece:messageFunctionPurposeCode","@type":["rdf:Property","owl:DatatypeProperty"],"rdfs:label":"messageFunctionPurposeCode","schema:rangeIncludes":{"@id":"unece:MessageFunctionCodeList"},"schema:domainIncludes":{"@id":"unece:ExchangedDocument"},"rdfs:comment":"A code specifying the purpose of this exchanged document, such as request or reminder."},{"@id":"unece:offsetProcessingStatus","@type":["rdf:Property","owl:DatatypeProperty"],"rdfs:label":"offsetProcessingStatus","schema:rangeIncludes":{"@id":"schema:Text"},"schema:domainIncludes":{"@id":"unece:ExchangedDocument"},"rdfs:comment":"A status of an offset processing, expressed as text, for this exchanged document, such as the process offsetted by this document."},{"@id":"unece:originalIssuedQuantity","@type":["rdf:Property","owl:ObjectProperty"],"rdfs:label":"originalIssuedQuantity","schema:rangeIncludes":{"@id":"unece:QuantityType"},"schema:domainIncludes":{"@id":"unece:ExchangedDocument"},"rdfs:comment":"The number of originals issued of this exchanged document."},{"@id":"unece:originalRequiredQuantity","@type":["rdf:Property","owl:ObjectProperty"],"rdfs:label":"originalRequiredQuantity","schema:rangeIncludes":{"@id":"unece:QuantityType"},"schema:domainIncludes":{"@id":"unece:ExchangedDocument"},"rdfs:comment":"The number of originals required of this exchanged document."},{"@id":"unece:purpose","@type":["rdf:Property","owl:DatatypeProperty"],"rdfs:label":"purpose","schema:rangeIncludes":{"@id":"schema:Text"},"schema:domainIncludes":{"@id":"unece:ExchangedDocument"},"rdfs:comment":"The purpose, expressed as text, of this exchanged document."},{"@id":"unece:recipientAssignedId","@type":["rdf:Property","owl:DatatypeProperty"],"rdfs:label":"recipientAssignedId","schema:rangeIncludes":{"@id":"schema:Text"},"schema:domainIncludes":{"@id":"unece:ExchangedDocument"},"rdfs:comment":"A unique recipient assigned identifier for this exchanged document."},{"@id":"unece:referenceDocument","@type":["rdf:Property","owl:ObjectProperty"],"rdfs:label":"referenceDocument","schema:rangeIncludes":{"@id":"unece:Document"},"schema:domainIncludes":{"@id":"unece:ExchangedDocument"},"rdfs:comment":"A document referenced by this acknowledgement document."},{"@id":"unece:rejectionResponseDateTime","@type":["rdf:Property","owl:DatatypeProperty"],"rdfs:label":"rejectionResponseDateTime","schema:rangeIncludes":{"@id":"schema:Text"},"schema:domainIncludes":{"@id":"unece:ExchangedDocument"},"rdfs:comment":"A date, time, date time, or other date time value of a rejection response of the exchanged document."},{"@id":"unece:responseDateTime","@type":["rdf:Property","owl:DatatypeProperty"],"rdfs:label":"responseDateTime","schema:rangeIncludes":{"@id":"schema:Text"},"schema:domainIncludes":[{"@id":"unece:ExchangedDocument"},{"@id":"unece:SpecialQuery"}],"rdfs:comment":"A date, time, date time, or other date time value of a response of the exchanged document."},{"@id":"unece:responseReasonCode","@type":["rdf:Property","owl:DatatypeProperty"],"rdfs:label":"responseReasonCode","schema:rangeIncludes":{"@id":"schema:Text"},"schema:domainIncludes":{"@id":"unece:ExchangedDocument"},"rdfs:comment":"A code specifying a response reason for this exchanged document."},{"@id":"unece:revisionDateTime","@type":["rdf:Property","owl:DatatypeProperty"],"rdfs:label":"revisionDateTime","schema:rangeIncludes":{"@id":"schema:Text"},"schema:domainIncludes":{"@id":"unece:ExchangedDocument"},"rdfs:comment":"The date, time, date time or other date time value for the revision of this exchanged document."},{"@id":"unece:secondSignatoryAuthentication","@type":["rdf:Property","owl:ObjectProperty"],"rdfs:label":"secondSignatoryAuthentication","schema:rangeIncludes":{"@id":"unece:Authentication"},"schema:domainIncludes":{"@id":"unece:ExchangedDocument"},"rdfs:comment":"The second signature, also known as the first counter signature, that has been authenticated on this exchanged document indicating where appropriate the authentication party."},{"@id":"unece:senderAssignedId","@type":["rdf:Property","owl:DatatypeProperty"],"rdfs:label":"senderAssignedId","schema:rangeIncludes":{"@id":"schema:Text"},"schema:domainIncludes":{"@id":"unece:ExchangedDocument"},"rdfs:comment":"A unique sender assigned identifier for this exchanged document."},{"@id":"unece:submissionDateTime","@type":["rdf:Property","owl:DatatypeProperty"],"rdfs:label":"submissionDateTime","schema:rangeIncludes":{"@id":"schema:Text"},"schema:domainIncludes":{"@id":"unece:ExchangedDocument"},"rdfs:comment":"The date, time, date time or other date time value for the formal submission of this exchanged document to a receiver by a sender."},{"@id":"unece:thirdSignatoryAuthentication","@type":["rdf:Property","owl:ObjectProperty"],"rdfs:label":"thirdSignatoryAuthentication","schema:rangeIncludes":{"@id":"unece:Authentication"},"schema:domainIncludes":{"@id":"unece:ExchangedDocument"},"rdfs:comment":"The third signature, also known as the second counter signature, that has been authenticated on this exchanged document indicating where appropriate the authentication party."},{"@id":"unece:traderAssignedId","@type":["rdf:Property","owl:DatatypeProperty"],"rdfs:label":"traderAssignedId","schema:rangeIncludes":{"@id":"schema:Text"},"schema:domainIncludes":{"@id":"unece:ExchangedDocument"},"rdfs:comment":"A unique trader assigned identifier for this exchanged document."},{"@id":"unece:urgency","@type":["rdf:Property","owl:DatatypeProperty"],"rdfs:label":"urgency","schema:rangeIncludes":{"@id":"schema:Text"},"schema:domainIncludes":{"@id":"unece:ExchangedDocument"},"rdfs:comment":"An urgency, expressed as text, of this exchanged document."},{"@id":"unece:urgencyCode","@type":["rdf:Property","owl:DatatypeProperty"],"rdfs:label":"urgencyCode","schema:rangeIncludes":{"@id":"schema:Text"},"schema:domainIncludes":{"@id":"unece:ExchangedDocument"},"rdfs:comment":"The code specifying the urgency for this exchanged document."},{"@id":"unece:access","@type":["rdf:Property","owl:DatatypeProperty"],"rdfs:label":"access","schema:rangeIncludes":{"@id":"schema:Text"},"schema:domainIncludes":{"@id":"unece:BinaryFile"},"rdfs:comment":"Access information, expressed as text, for this specified binary file, such as security and download parameters."},{"@id":"unece:accessAvailabilityPeriod","@type":["rdf:Property","owl:ObjectProperty"],"rdfs:label":"accessAvailabilityPeriod","schema:rangeIncludes":{"@id":"unece:SpecifiedPeriod"},"schema:domainIncludes":{"@id":"unece:BinaryFile"},"rdfs:comment":"The specified period when access to this binary file is available."},{"@id":"unece:authorName","@type":["rdf:Property","owl:DatatypeProperty"],"rdfs:label":"authorName","schema:rangeIncludes":{"@id":"schema:Text"},"schema:domainIncludes":{"@id":"unece:BinaryFile"},"rdfs:comment":"A name of an author, expressed as text, of this specified binary file."},{"@id":"unece:characterSetCode","@type":["rdf:Property","owl:DatatypeProperty"],"rdfs:label":"characterSetCode","schema:rangeIncludes":{"@id":"schema:Text"},"schema:domainIncludes":{"@id":"unece:BinaryFile"},"rdfs:comment":"The code specifying the character set for this specified binary file."},{"@id":"unece:encodingCode","@type":["rdf:Property","owl:DatatypeProperty"],"rdfs:label":"encodingCode","schema:rangeIncludes":{"@id":"schema:Text"},"schema:domainIncludes":{"@id":"unece:BinaryFile"},"rdfs:comment":"The code specifying the encoding of this specified binary file."},{"@id":"unece:fileName","@type":["rdf:Property","owl:DatatypeProperty"],"rdfs:label":"fileName","schema:rangeIncludes":{"@id":"schema:Text"},"schema:domainIncludes":{"@id":"unece:BinaryFile"},"rdfs:comment":"The file name, expressed as text, of this specified binary file."},{"@id":"unece:includedBinaryObject","@type":["rdf:Property","owl:DatatypeProperty"],"rdfs:label":"includedBinaryObject","schema:rangeIncludes":{"@id":"schema:Text"},"schema:domainIncludes":{"@id":"unece:BinaryFile"},"rdfs:comment":"A binary object included in this specified binary file."},{"@id":"unece:mIMECode","@type":["rdf:Property","owl:DatatypeProperty"],"rdfs:label":"mIMECode","schema:rangeIncludes":{"@id":"unece:MimeCodeList"},"schema:domainIncludes":{"@id":"unece:BinaryFile"},"rdfs:comment":"The code specifying the Multipurpose Internet Mail Extensions (MIME) type for this specified binary file."},{"@id":"unece:sizeMeasure","@type":["rdf:Property","owl:ObjectProperty"],"rdfs:label":"sizeMeasure","schema:rangeIncludes":{"@id":"unece:MeasureType"},"schema:domainIncludes":{"@id":"unece:BinaryFile"},"rdfs:comment":"The measure of the size of this specified binary file."},{"@id":"unece:title","@type":["rdf:Property","owl:DatatypeProperty"],"rdfs:label":"title","schema:rangeIncludes":{"@id":"schema:Text"},"schema:domainIncludes":{"@id":"unece:BinaryFile"},"rdfs:comment":"A title, expressed as text, for this specified binary file."},{"@id":"unece:acquisitionDateTime","@type":["rdf:Property","owl:DatatypeProperty"],"rdfs:label":"acquisitionDateTime","schema:rangeIncludes":{"@id":"schema:Text"},"schema:domainIncludes":{"@id":"unece:GeographicalCoordinate"},"rdfs:comment":"The date, time, date time or other date time value of the acquisition of this geographical coordinate."},{"@id":"unece:alternativeSourceSystemId","@type":["rdf:Property","owl:DatatypeProperty"],"rdfs:label":"alternativeSourceSystemId","schema:rangeIncludes":{"@id":"schema:Text"},"schema:domainIncludes":{"@id":"unece:GeographicalCoordinate"},"rdfs:comment":"An alternative source system identifier for this geographical coordinate."},{"@id":"unece:altimetricSystemId","@type":["rdf:Property","owl:DatatypeProperty"],"rdfs:label":"altimetricSystemId","schema:rangeIncludes":{"@id":"schema:Text"},"schema:domainIncludes":{"@id":"unece:GeographicalCoordinate"},"rdfs:comment":"The unique identifier of the system used for measuring the altitude."},{"@id":"unece:altitudeMeasure","@type":["rdf:Property","owl:ObjectProperty"],"rdfs:label":"altitudeMeasure","schema:rangeIncludes":{"@id":"unece:MeasureType"},"schema:domainIncludes":{"@id":"unece:GeographicalCoordinate"},"rdfs:comment":"The measure of the altitude that reflects the vertical elevation of an object above a surface for this geographical coordinate (Reference ISO 6709)."},{"@id":"unece:latitudeDirectionIndicator","@type":["rdf:Property","owl:DatatypeProperty"],"rdfs:label":"latitudeDirectionIndicator","schema:rangeIncludes":{"@id":"schema:Boolean"},"schema:domainIncludes":{"@id":"unece:GeographicalCoordinate"},"rdfs:comment":"The indication of whether the latitude compass direction from the Equator meridian to the meridian of a specific place is North (+) or South (-)  (Reference ISO 6709)."},{"@id":"unece:latitudeMeasure","@type":["rdf:Property","owl:ObjectProperty"],"rdfs:label":"latitudeMeasure","schema:rangeIncludes":{"@id":"unece:MeasureType"},"schema:domainIncludes":{"@id":"unece:GeographicalCoordinate"},"rdfs:comment":"The measure of the latitude as an angular distance north or south from the Equator meridian to the meridian of a specific place for this geographical coordinate (Reference ISO 6709)."},{"@id":"unece:longitudeDirectionIndicator","@type":["rdf:Property","owl:DatatypeProperty"],"rdfs:label":"longitudeDirectionIndicator","schema:rangeIncludes":{"@id":"schema:Boolean"},"schema:domainIncludes":{"@id":"unece:GeographicalCoordinate"},"rdfs:comment":"The indication of whether the longitude as a compass direction from the Greenwich meridian to the meridian of a specific place is East (+) or West (-) for this geographical coordinate (Reference ISO 6709)."},{"@id":"unece:longitudeMeasure","@type":["rdf:Property","owl:ObjectProperty"],"rdfs:label":"longitudeMeasure","schema:rangeIncludes":{"@id":"unece:MeasureType"},"schema:domainIncludes":{"@id":"unece:GeographicalCoordinate"},"rdfs:comment":"The measure of the longitude as an angular distance east or west from the Greenwich meridian to the meridian of a specific place (Reference ISO 6709)."},{"@id":"unece:systemId","@type":["rdf:Property","owl:DatatypeProperty"],"rdfs:label":"systemId","schema:rangeIncludes":{"@id":"schema:Text"},"schema:domainIncludes":{"@id":"unece:GeographicalCoordinate"},"rdfs:comment":"The unique identifier of the classification system for this product classification."},{"@id":"unece:timeZone","@type":["rdf:Property","owl:DatatypeProperty"],"rdfs:label":"timeZone","schema:rangeIncludes":{"@id":"schema:Text"},"schema:domainIncludes":{"@id":"unece:GeographicalCoordinate"},"rdfs:comment":"The time zone, expressed as text, for this geographical coordinate."},{"@id":"unece:timeZoneCode","@type":["rdf:Property","owl:DatatypeProperty"],"rdfs:label":"timeZoneCode","schema:rangeIncludes":{"@id":"schema:Text"},"schema:domainIncludes":{"@id":"unece:GeographicalCoordinate"},"rdfs:comment":"The code specifying the time zone of this geographical coordinate."},{"@id":"unece:timeZoneDateTime","@type":["rdf:Property","owl:DatatypeProperty"],"rdfs:label":"timeZoneDateTime","schema:rangeIncludes":{"@id":"schema:DateTime"},"schema:domainIncludes":{"@id":"unece:GeographicalCoordinate"},"rdfs:comment":"The date, time, date time, or other date time value for the time zone of this geographical coordinate."},{"@id":"unece:usedCoordinateReferenceSystem","@type":["rdf:Property","owl:ObjectProperty"],"rdfs:label":"usedCoordinateReferenceSystem","schema:rangeIncludes":{"@id":"unece:CoordinateReferenceSystem"},"schema:domainIncludes":[{"@id":"unece:GeographicalCoordinate"},{"@id":"unece:GeographicalFeature"}],"rdfs:comment":"The CS (Coordinate System) engineering coordinate reference system used for this geographical coordinate."},{"@id":"unece:usedCoordinateSourceSystem","@type":["rdf:Property","owl:ObjectProperty"],"rdfs:label":"usedCoordinateSourceSystem","schema:rangeIncludes":{"@id":"unece:CoordinateSourceSystem"},"schema:domainIncludes":[{"@id":"unece:GeographicalCoordinate"},{"@id":"unece:GeographicalFeature"}],"rdfs:comment":"The geographical coordinate source system used for this geographical coordinate."},{"@id":"unece:actionType","@type":["rdf:Property","owl:DatatypeProperty"],"rdfs:label":"actionType","schema:rangeIncludes":{"@id":"schema:Text"},"schema:domainIncludes":{"@id":"unece:SpecifiedAction"},"rdfs:comment":"A type, expressed as text, for this corrective action."},{"@id":"unece:activityAuthorizedParty","@type":["rdf:Property","owl:ObjectProperty"],"rdfs:label":"activityAuthorizedParty","schema:rangeIncludes":{"@id":"unece:Party"},"schema:domainIncludes":{"@id":"unece:CountrySubDivision"},"rdfs:comment":"A party that is authorized to perform an activity in this trade country sub-division."},{"@id":"unece:hierarchicalLevelCode","@type":["rdf:Property","owl:DatatypeProperty"],"rdfs:label":"hierarchicalLevelCode","schema:rangeIncludes":{"@id":"schema:Text"},"schema:domainIncludes":{"@id":"unece:CountrySubDivision"},"rdfs:comment":"The code specifying the hierarchical level of this trade country sub-division."},{"@id":"unece:locationFunctionTypeCode","@type":["rdf:Property","owl:DatatypeProperty"],"rdfs:label":"locationFunctionTypeCode","schema:rangeIncludes":{"@id":"unece:LocationFunctionCodeList"},"schema:domainIncludes":[{"@id":"unece:CountrySubDivision"},{"@id":"unece:SubordinateLocation"},{"@id":"unece:SubordinateSubordinateLocation"}],"rdfs:comment":"A code specifying the type of this logistics related location."},{"@id":"unece:subordinateCountrySubDivision","@type":["rdf:Property","owl:ObjectProperty"],"rdfs:label":"subordinateCountrySubDivision","schema:rangeIncludes":{"@id":"unece:CountrySubDivision"},"schema:domainIncludes":[{"@id":"unece:CountrySubDivision"},{"@id":"unece:Country"}],"rdfs:comment":"A subordinate country sub-division within this trade country sub-division."},{"@id":"unece:superordinateCountrySubDivision","@type":["rdf:Property","owl:ObjectProperty"],"rdfs:label":"superordinateCountrySubDivision","schema:rangeIncludes":{"@id":"unece:CountrySubDivision"},"schema:domainIncludes":{"@id":"unece:CountrySubDivision"},"rdfs:comment":"A superordinate country sub-division for this trade country sub-division."},{"@id":"unece:activityLevelMeasure","@type":["rdf:Property","owl:ObjectProperty"],"rdfs:label":"activityLevelMeasure","schema:rangeIncludes":{"@id":"unece:MeasureType"},"schema:domainIncludes":{"@id":"unece:RadioactiveIsotope"},"rdfs:comment":"A measure of the activity level of this specified radioactive isotope."},{"@id":"unece:note","@type":["rdf:Property","owl:DatatypeProperty"],"rdfs:label":"note","schema:rangeIncludes":{"@id":"schema:Text"},"schema:domainIncludes":{"@id":"unece:RadioactiveIsotope"},"rdfs:comment":"A note, expressed as text, for this specified radioactive isotope."},{"@id":"unece:specifiedRadionuclide","@type":["rdf:Property","owl:ObjectProperty"],"rdfs:label":"specifiedRadionuclide","schema:rangeIncludes":{"@id":"unece:Radionuclide"},"schema:domainIncludes":{"@id":"unece:RadioactiveIsotope"},"rdfs:comment":"The radionuclide details specified for this radioactive isotope."},{"@id":"unece:actualMeasure","@type":["rdf:Property","owl:ObjectProperty"],"rdfs:label":"actualMeasure","schema:rangeIncludes":{"@id":"unece:MeasureType"},"schema:domainIncludes":{"@id":"unece:Measurement"},"rdfs:comment":"An actual measure for this measurement."},{"@id":"unece:comparisonOperatorCode","@type":["rdf:Property","owl:DatatypeProperty"],"rdfs:label":"comparisonOperatorCode","schema:rangeIncludes":{"@id":"schema:Text"},"schema:domainIncludes":{"@id":"unece:Measurement"},"rdfs:comment":"A code specifying the operator, such as, less than, greater than or equal to, for comparing two actual measures."},{"@id":"unece:conditionMeasure","@type":["rdf:Property","owl:ObjectProperty"],"rdfs:label":"conditionMeasure","schema:rangeIncludes":{"@id":"unece:MeasureType"},"schema:domainIncludes":{"@id":"unece:Measurement"},"rdfs:comment":"A measure of a condition for this measurement."},{"@id":"unece:method","@type":["rdf:Property","owl:DatatypeProperty"],"rdfs:label":"method","schema:rangeIncludes":{"@id":"schema:Text"},"schema:domainIncludes":{"@id":"unece:Measurement"},"rdfs:comment":"A measurement method expressed as text."},{"@id":"unece:actualQuantityDimension","@type":["rdf:Property","owl:ObjectProperty"],"rdfs:label":"actualQuantityDimension","schema:rangeIncludes":{"@id":"unece:WorkItemDimension"},"schema:domainIncludes":{"@id":"unece:QuantityAnalysis"},"rdfs:comment":"A work item dimension of the actual quantity in this work item quantity analysis."},{"@id":"unece:actualQuantityPercent","@type":["rdf:Property","owl:DatatypeProperty"],"rdfs:label":"actualQuantityPercent","schema:rangeIncludes":{"@id":"schema:Text"},"schema:domainIncludes":{"@id":"unece:QuantityAnalysis"},"rdfs:comment":"The percentage of a total quantity that the actual quantity of this work item quantity analysis represents."},{"@id":"unece:breakdownQuantityAnalysis","@type":["rdf:Property","owl:ObjectProperty"],"rdfs:label":"breakdownQuantityAnalysis","schema:rangeIncludes":{"@id":"unece:QuantityAnalysis"},"schema:domainIncludes":{"@id":"unece:QuantityAnalysis"},"rdfs:comment":"A quantity analysis breakdown of this work item quantity analysis."},{"@id":"unece:actualSpecifiedPercent","@type":["rdf:Property","owl:DatatypeProperty"],"rdfs:label":"actualSpecifiedPercent","schema:rangeIncludes":{"@id":"schema:Text"},"schema:domainIncludes":{"@id":"unece:SpecifiedFault"},"rdfs:comment":"The actual percentage of this specified fault."},{"@id":"unece:actualSpecifiedQuantity","@type":["rdf:Property","owl:ObjectProperty"],"rdfs:label":"actualSpecifiedQuantity","schema:rangeIncludes":{"@id":"unece:QuantityType"},"schema:domainIncludes":{"@id":"unece:SpecifiedFault"},"rdfs:comment":"The actual total quantity of this specified fault."},{"@id":"unece:classificationCode","@type":["rdf:Property","owl:DatatypeProperty"],"rdfs:label":"classificationCode","schema:rangeIncludes":{"@id":"schema:Text"},"schema:domainIncludes":{"@id":"unece:SpecifiedFault"},"rdfs:comment":"A code specifying a classification for this field crop."},{"@id":"unece:estimatedSpecifiedPercent","@type":["rdf:Property","owl:DatatypeProperty"],"rdfs:label":"estimatedSpecifiedPercent","schema:rangeIncludes":{"@id":"schema:Text"},"schema:domainIncludes":{"@id":"unece:SpecifiedFault"},"rdfs:comment":"The estimated percentage of this specified fault."},{"@id":"unece:faultType","@type":["rdf:Property","owl:DatatypeProperty"],"rdfs:label":"faultType","schema:rangeIncludes":{"@id":"schema:Text"},"schema:domainIncludes":{"@id":"unece:SpecifiedFault"},"rdfs:comment":"A type, expressed as text, of this specified fault."},{"@id":"unece:operationalApplicableTolerance","@type":["rdf:Property","owl:ObjectProperty"],"rdfs:label":"operationalApplicableTolerance","schema:rangeIncludes":{"@id":"unece:Tolerance"},"schema:domainIncludes":{"@id":"unece:SpecifiedFault"},"rdfs:comment":"An applicable operational tolerance of this specified fault."},{"@id":"unece:areaIncluded","@type":["rdf:Property","owl:DatatypeProperty"],"rdfs:label":"areaIncluded","schema:rangeIncludes":{"@id":"schema:Text"},"schema:domainIncludes":{"@id":"unece:Picture"},"rdfs:comment":"The area or location, expressed as text, that is included in this photographic picture."},{"@id":"unece:copyrightOwnerName","@type":["rdf:Property","owl:DatatypeProperty"],"rdfs:label":"copyrightOwnerName","schema:rangeIncludes":{"@id":"schema:Text"},"schema:domainIncludes":{"@id":"unece:Picture"},"rdfs:comment":"The name of the copyright owner, expressed as text, for this photographic picture."},{"@id":"unece:digitalImageBinaryObject","@type":["rdf:Property","owl:DatatypeProperty"],"rdfs:label":"digitalImageBinaryObject","schema:rangeIncludes":{"@id":"schema:Text"},"schema:domainIncludes":{"@id":"unece:Picture"},"rdfs:comment":"Binary object data that is the actual digital image for this photographic picture."},{"@id":"unece:intendedUse","@type":["rdf:Property","owl:DatatypeProperty"],"rdfs:label":"intendedUse","schema:rangeIncludes":{"@id":"schema:Text"},"schema:domainIncludes":{"@id":"unece:Picture"},"rdfs:comment":"An intended use, expressed as text, for this photographic picture."},{"@id":"unece:intendedUseCode","@type":["rdf:Property","owl:DatatypeProperty"],"rdfs:label":"intendedUseCode","schema:rangeIncludes":{"@id":"schema:Text"},"schema:domainIncludes":{"@id":"unece:Picture"},"rdfs:comment":"The code specifying the intended use of this photographic picture."},{"@id":"unece:linearDimension","@type":["rdf:Property","owl:ObjectProperty"],"rdfs:label":"linearDimension","schema:rangeIncludes":{"@id":"unece:SpatialDimension"},"schema:domainIncludes":{"@id":"unece:Picture"},"rdfs:comment":"A linear dimension or a set of linear dimensions of this logistics packaging."},{"@id":"unece:pictureType","@type":["rdf:Property","owl:DatatypeProperty"],"rdfs:label":"pictureType","schema:rangeIncludes":{"@id":"schema:Text"},"schema:domainIncludes":{"@id":"unece:Picture"},"rdfs:comment":"The type, expressed as text, of this photographic picture."},{"@id":"unece:reference","@type":["rdf:Property","owl:DatatypeProperty"],"rdfs:label":"reference","schema:rangeIncludes":{"@id":"schema:Text"},"schema:domainIncludes":{"@id":"unece:Picture"},"rdfs:comment":"A reference, expressed as text, for this header trade agreement."},{"@id":"unece:renderingInformation","@type":["rdf:Property","owl:DatatypeProperty"],"rdfs:label":"renderingInformation","schema:rangeIncludes":{"@id":"schema:Text"},"schema:domainIncludes":{"@id":"unece:Picture"},"rdfs:comment":"Rendering information, expressed as text, for this photographic picture."},{"@id":"unece:resolutionTypeCode","@type":["rdf:Property","owl:DatatypeProperty"],"rdfs:label":"resolutionTypeCode","schema:rangeIncludes":{"@id":"schema:Text"},"schema:domainIncludes":{"@id":"unece:Picture"},"rdfs:comment":"The code specifying the type of resolution for this photographic picture."},{"@id":"unece:resolutionValueNumeric","@type":["rdf:Property","owl:DatatypeProperty"],"rdfs:label":"resolutionValueNumeric","schema:rangeIncludes":{"@id":"schema:Text"},"schema:domainIncludes":{"@id":"unece:Picture"},"rdfs:comment":"The value, expressed as a number, for the resolution of this photographic picture."},{"@id":"unece:specifiedNote","@type":["rdf:Property","owl:ObjectProperty"],"rdfs:label":"specifiedNote","schema:rangeIncludes":{"@id":"unece:Note"},"schema:domainIncludes":{"@id":"unece:Picture"},"rdfs:comment":"A note specified for this photographic picture."},{"@id":"unece:subject","@type":["rdf:Property","owl:DatatypeProperty"],"rdfs:label":"subject","schema:rangeIncludes":{"@id":"schema:Text"},"schema:domainIncludes":[{"@id":"unece:Picture"},{"@id":"unece:Note"},{"@id":"unece:SpecialQuery"},{"@id":"unece:SpecifiedNote"}],"rdfs:comment":"A subject, expressed as text, of this specified note."},{"@id":"unece:takenDateTime","@type":["rdf:Property","owl:DatatypeProperty"],"rdfs:label":"takenDateTime","schema:rangeIncludes":{"@id":"schema:Text"},"schema:domainIncludes":{"@id":"unece:Picture"},"rdfs:comment":"The date, time, date time, or other date value of when this photographic picture was created."},{"@id":"unece:titleName","@type":["rdf:Property","owl:DatatypeProperty"],"rdfs:label":"titleName","schema:rangeIncludes":{"@id":"schema:Text"},"schema:domainIncludes":{"@id":"unece:Picture"},"rdfs:comment":"The name, expressed as text, of the title for this photographic picture."},{"@id":"unece:additionalReason","@type":["rdf:Property","owl:DatatypeProperty"],"rdfs:label":"additionalReason","schema:rangeIncludes":{"@id":"schema:Text"},"schema:domainIncludes":{"@id":"unece:ValidationStatus"},"rdfs:comment":"Information, expressed as text, related to the reason for this validation status."},{"@id":"unece:validationDocumentStatusConditionCode","@type":["rdf:Property","owl:DatatypeProperty"],"rdfs:label":"validationDocumentStatusConditionCode","schema:rangeIncludes":{"@id":"unece:ValidationDocumentStatusCodeList"},"schema:domainIncludes":{"@id":"unece:ValidationStatus"},"rdfs:comment":"The code specifying the condition of this validation status."},{"@id":"unece:ageLimitation","@type":["rdf:Property","owl:DatatypeProperty"],"rdfs:label":"ageLimitation","schema:rangeIncludes":{"@id":"schema:Text"},"schema:domainIncludes":{"@id":"unece:UsageCondition"},"rdfs:comment":"An age limitation, expressed as text, for this specified usage condition."},{"@id":"unece:appropriateClothing","@type":["rdf:Property","owl:DatatypeProperty"],"rdfs:label":"appropriateClothing","schema:rangeIncludes":{"@id":"schema:Text"},"schema:domainIncludes":{"@id":"unece:UsageCondition"},"rdfs:comment":"Appropriate clothing, expressed as text, for this specified usage condition."},{"@id":"unece:duration","@type":["rdf:Property","owl:DatatypeProperty"],"rdfs:label":"duration","schema:rangeIncludes":{"@id":"schema:Text"},"schema:domainIncludes":[{"@id":"unece:UsageCondition"},{"@id":"unece:SpecifiedPeriod"}],"rdfs:comment":"A duration, expressed as text, for this specified period."},{"@id":"unece:genderLimitation","@type":["rdf:Property","owl:DatatypeProperty"],"rdfs:label":"genderLimitation","schema:rangeIncludes":{"@id":"schema:Text"},"schema:domainIncludes":{"@id":"unece:UsageCondition"},"rdfs:comment":"A gender limitation, expressed as text, for this specified usage condition."},{"@id":"unece:occupancy","@type":["rdf:Property","owl:DatatypeProperty"],"rdfs:label":"occupancy","schema:rangeIncludes":{"@id":"schema:Text"},"schema:domainIncludes":{"@id":"unece:UsageCondition"},"rdfs:comment":"Occupancy, expressed as text, for this specified usage condition."},{"@id":"unece:requiringParty","@type":["rdf:Property","owl:ObjectProperty"],"rdfs:label":"requiringParty","schema:rangeIncludes":{"@id":"unece:Party"},"schema:domainIncludes":{"@id":"unece:UsageCondition"},"rdfs:comment":"A party requiring this specified usage condition."},{"@id":"unece:alienRegistrationId","@type":["rdf:Property","owl:DatatypeProperty"],"rdfs:label":"alienRegistrationId","schema:rangeIncludes":{"@id":"schema:Text"},"schema:domainIncludes":{"@id":"unece:PersonIdentity"},"rdfs:comment":"The alien registration identifier for this person."},{"@id":"unece:driversLicenceId","@type":["rdf:Property","owl:DatatypeProperty"],"rdfs:label":"driversLicenceId","schema:rangeIncludes":{"@id":"schema:Text"},"schema:domainIncludes":{"@id":"unece:PersonIdentity"},"rdfs:comment":"The drivers licence identifier for this person."},{"@id":"unece:identityCardId","@type":["rdf:Property","owl:DatatypeProperty"],"rdfs:label":"identityCardId","schema:rangeIncludes":{"@id":"schema:Text"},"schema:domainIncludes":{"@id":"unece:PersonIdentity"},"rdfs:comment":"The identity card identifier for this person."},{"@id":"unece:passportId","@type":["rdf:Property","owl:DatatypeProperty"],"rdfs:label":"passportId","schema:rangeIncludes":{"@id":"schema:Text"},"schema:domainIncludes":{"@id":"unece:PersonIdentity"},"rdfs:comment":"The identifier of the passport of this guest."},{"@id":"unece:socialSecurityId","@type":["rdf:Property","owl:DatatypeProperty"],"rdfs:label":"socialSecurityId","schema:rangeIncludes":{"@id":"schema:Text"},"schema:domainIncludes":{"@id":"unece:PersonIdentity"},"rdfs:comment":"The social security identifier for this person."},{"@id":"unece:applicableParameter","@type":["rdf:Property","owl:ObjectProperty"],"rdfs:label":"applicableParameter","schema:rangeIncludes":{"@id":"unece:SpecifiedParameter"},"schema:domainIncludes":{"@id":"unece:SpecifiedMethod"},"rdfs:comment":"A parameter applicable to this specified method."},{"@id":"unece:certificationId","@type":["rdf:Property","owl:DatatypeProperty"],"rdfs:label":"certificationId","schema:rangeIncludes":{"@id":"schema:Text"},"schema:domainIncludes":{"@id":"unece:SpecifiedMethod"},"rdfs:comment":"A certification identifier of this specified method."},{"@id":"unece:certificationTypeCode","@type":["rdf:Property","owl:DatatypeProperty"],"rdfs:label":"certificationTypeCode","schema:rangeIncludes":{"@id":"schema:Text"},"schema:domainIncludes":{"@id":"unece:SpecifiedMethod"},"rdfs:comment":"The code specifying the certification type of this method."},{"@id":"unece:externalReference","@type":["rdf:Property","owl:DatatypeProperty"],"rdfs:label":"externalReference","schema:rangeIncludes":{"@id":"schema:Text"},"schema:domainIncludes":{"@id":"unece:SpecifiedMethod"},"rdfs:comment":"An external reference, expressed as text, for this specified method."},{"@id":"unece:localTypeCode","@type":["rdf:Property","owl:DatatypeProperty"],"rdfs:label":"localTypeCode","schema:rangeIncludes":{"@id":"schema:Text"},"schema:domainIncludes":{"@id":"unece:SpecifiedMethod"},"rdfs:comment":"The code specifying the local type for this method."},{"@id":"unece:measurementCode","@type":["rdf:Property","owl:DatatypeProperty"],"rdfs:label":"measurementCode","schema:rangeIncludes":{"@id":"schema:Text"},"schema:domainIncludes":{"@id":"unece:SpecifiedMethod"},"rdfs:comment":"The code specifying the measurement for this method."},{"@id":"unece:obligatoryTypeCode","@type":["rdf:Property","owl:DatatypeProperty"],"rdfs:label":"obligatoryTypeCode","schema:rangeIncludes":{"@id":"schema:Text"},"schema:domainIncludes":{"@id":"unece:SpecifiedMethod"},"rdfs:comment":"The code specifying the obligatory type for this method."},{"@id":"unece:standardTypeCode","@type":["rdf:Property","owl:DatatypeProperty"],"rdfs:label":"standardTypeCode","schema:rangeIncludes":{"@id":"schema:Text"},"schema:domainIncludes":{"@id":"unece:SpecifiedMethod"},"rdfs:comment":"The code specifying the standard type for this method."},{"@id":"unece:usedTechnologyCode","@type":["rdf:Property","owl:DatatypeProperty"],"rdfs:label":"usedTechnologyCode","schema:rangeIncludes":{"@id":"schema:Text"},"schema:domainIncludes":{"@id":"unece:SpecifiedMethod"},"rdfs:comment":"The code specifying the technology used by this method."},{"@id":"unece:applicableRadioactiveIsotope","@type":["rdf:Property","owl:ObjectProperty"],"rdfs:label":"applicableRadioactiveIsotope","schema:rangeIncludes":{"@id":"unece:RadioactiveIsotope"},"schema:domainIncludes":{"@id":"unece:RadioactiveMaterial"},"rdfs:comment":"An isotope applicable to this radioactive material."},{"@id":"unece:compositionDescription","@type":["rdf:Property","owl:DatatypeProperty"],"rdfs:label":"compositionDescription","schema:rangeIncludes":{"@id":"schema:Text"},"schema:domainIncludes":{"@id":"unece:RadioactiveMaterial"},"rdfs:comment":"The textual description of the composition of this radioactive material."},{"@id":"unece:criticalitySafetyIndexNumeric","@type":["rdf:Property","owl:DatatypeProperty"],"rdfs:label":"criticalitySafetyIndexNumeric","schema:rangeIncludes":{"@id":"schema:Text"},"schema:domainIncludes":{"@id":"unece:RadioactiveMaterial"},"rdfs:comment":"The criticality safety index number of this radioactive material."},{"@id":"unece:fissileCriticalitySafetyIndexNumeric","@type":["rdf:Property","owl:DatatypeProperty"],"rdfs:label":"fissileCriticalitySafetyIndexNumeric","schema:rangeIncludes":{"@id":"schema:Text"},"schema:domainIncludes":{"@id":"unece:RadioactiveMaterial"},"rdfs:comment":"The number (rounded up to the next tenth) assigned to and placed on the label of a fissile radioactive material package, to designate the degree of control of accumulation of packages, overpacks or freight containers containing fissile material during transportation."},{"@id":"unece:fissileExceptionIndicator","@type":["rdf:Property","owl:DatatypeProperty"],"rdfs:label":"fissileExceptionIndicator","schema:rangeIncludes":{"@id":"schema:Boolean"},"schema:domainIncludes":{"@id":"unece:RadioactiveMaterial"},"rdfs:comment":"The indication of whether or not this radioactive material is a fissile exception."},{"@id":"unece:lowDispersibleInformation","@type":["rdf:Property","owl:DatatypeProperty"],"rdfs:label":"lowDispersibleInformation","schema:rangeIncludes":{"@id":"schema:Text"},"schema:domainIncludes":{"@id":"unece:RadioactiveMaterial"},"rdfs:comment":"Information, expressed as text, describing the low dispersion properties of this radioactive material."},{"@id":"unece:radioactivePackageTransportIndexCode","@type":["rdf:Property","owl:DatatypeProperty"],"rdfs:label":"radioactivePackageTransportIndexCode","schema:rangeIncludes":{"@id":"schema:Text"},"schema:domainIncludes":{"@id":"unece:RadioactiveMaterial"},"rdfs:comment":"A code specifying a package transport index for this radioactive material."},{"@id":"unece:radionuclideName","@type":["rdf:Property","owl:DatatypeProperty"],"rdfs:label":"radionuclideName","schema:rangeIncludes":{"@id":"schema:Text"},"schema:domainIncludes":{"@id":"unece:RadioactiveMaterial"},"rdfs:comment":"The name of the radionuclide, expressed as text, of this radioactive material."},{"@id":"unece:specialFormInformation","@type":["rdf:Property","owl:DatatypeProperty"],"rdfs:label":"specialFormInformation","schema:rangeIncludes":{"@id":"schema:Text"},"schema:domainIncludes":{"@id":"unece:RadioactiveMaterial"},"rdfs:comment":"Information, expressed as text, describing the special form for this radioactive material."},{"@id":"unece:transportIndexNumeric","@type":["rdf:Property","owl:DatatypeProperty"],"rdfs:label":"transportIndexNumeric","schema:rangeIncludes":{"@id":"schema:Text"},"schema:domainIncludes":{"@id":"unece:RadioactiveMaterial"},"rdfs:comment":"The transport index number of this radioactive material."},{"@id":"unece:associatedGeographicalFeature","@type":["rdf:Property","owl:ObjectProperty"],"rdfs:label":"associatedGeographicalFeature","schema:rangeIncludes":{"@id":"unece:GeographicalFeature"},"schema:domainIncludes":[{"@id":"unece:Location"},{"@id":"unece:CommunicationEvent"}],"rdfs:comment":"A geographical feature associated with this communication event."},{"@id":"unece:locationCountryId","@type":["rdf:Property","owl:DatatypeProperty"],"rdfs:label":"locationCountryId","schema:rangeIncludes":{"@id":"unece:CountryId"},"schema:domainIncludes":{"@id":"unece:Location"},"rdfs:comment":"The identifier of the country for this referenced location."},{"@id":"unece:locationTypeCode","@type":["rdf:Property","owl:DatatypeProperty"],"rdfs:label":"locationTypeCode","schema:rangeIncludes":{"@id":"schema:Text"},"schema:domainIncludes":{"@id":"unece:Location"},"rdfs:comment":"The code specifying the type of referenced location."},{"@id":"unece:postalAddress","@type":["rdf:Property","owl:ObjectProperty"],"rdfs:label":"postalAddress","schema:rangeIncludes":{"@id":"unece:Address"},"schema:domainIncludes":[{"@id":"unece:Location"},{"@id":"unece:LegalOrganization"}],"rdfs:comment":"A postal address for this legally set up organization."},{"@id":"unece:specifiedSupplyChainEvent","@type":["rdf:Property","owl:ObjectProperty"],"rdfs:label":"specifiedSupplyChainEvent","schema:rangeIncludes":{"@id":"unece:Event"},"schema:domainIncludes":{"@id":"unece:Location"},"rdfs:comment":"A supply chain event specified for this product batch."},{"@id":"unece:specifiedTradeParty","@type":["rdf:Property","owl:ObjectProperty"],"rdfs:label":"specifiedTradeParty","schema:rangeIncludes":{"@id":"unece:Party"},"schema:domainIncludes":{"@id":"unece:Location"},"rdfs:comment":"A party specified for this experience event."},{"@id":"unece:uTCOffsetNumeric","@type":["rdf:Property","owl:DatatypeProperty"],"rdfs:label":"uTCOffsetNumeric","schema:rangeIncludes":{"@id":"schema:Text"},"schema:domainIncludes":{"@id":"unece:Location"},"rdfs:comment":"The UTC (Universal Time Coordinate) time offset value for this referenced location."},{"@id":"unece:applicationSpecifiedParameter","@type":["rdf:Property","owl:ObjectProperty"],"rdfs:label":"applicationSpecifiedParameter","schema:rangeIncludes":{"@id":"unece:DocumentContextParameter"},"schema:domainIncludes":{"@id":"unece:ExchangedDocumentContext"},"rdfs:comment":"An application context parameter specified for this exchanged document context."},{"@id":"unece:bIMSpecifiedParameter","@type":["rdf:Property","owl:ObjectProperty"],"rdfs:label":"bIMSpecifiedParameter","schema:rangeIncludes":{"@id":"unece:DocumentContextParameter"},"schema:domainIncludes":{"@id":"unece:ExchangedDocumentContext"},"rdfs:comment":"A Business Information Master (BIM) context parameter specified for this exchanged document context."},{"@id":"unece:businessProcessSpecifiedParameter","@type":["rdf:Property","owl:ObjectProperty"],"rdfs:label":"businessProcessSpecifiedParameter","schema:rangeIncludes":{"@id":"unece:DocumentContextParameter"},"schema:domainIncludes":{"@id":"unece:ExchangedDocumentContext"},"rdfs:comment":"A business process context parameter specified for this exchanged document context."},{"@id":"unece:guidelineSpecifiedParameter","@type":["rdf:Property","owl:ObjectProperty"],"rdfs:label":"guidelineSpecifiedParameter","schema:rangeIncludes":{"@id":"unece:DocumentContextParameter"},"schema:domainIncludes":{"@id":"unece:ExchangedDocumentContext"},"rdfs:comment":"A guideline context parameter specified for this exchanged document context."},{"@id":"unece:messageStandardSpecifiedParameter","@type":["rdf:Property","owl:ObjectProperty"],"rdfs:label":"messageStandardSpecifiedParameter","schema:rangeIncludes":{"@id":"unece:DocumentContextParameter"},"schema:domainIncludes":{"@id":"unece:ExchangedDocumentContext"},"rdfs:comment":"The message standard document context parameter specified for this exchanged document context."},{"@id":"unece:processingTransactionDateTime","@type":["rdf:Property","owl:DatatypeProperty"],"rdfs:label":"processingTransactionDateTime","schema:rangeIncludes":{"@id":"schema:Text"},"schema:domainIncludes":{"@id":"unece:ExchangedDocumentContext"},"rdfs:comment":"The date, time, date time, or other date time value of the processing of a transaction for this exchanged document context."},{"@id":"unece:scenarioSpecifiedParameter","@type":["rdf:Property","owl:ObjectProperty"],"rdfs:label":"scenarioSpecifiedParameter","schema:rangeIncludes":{"@id":"unece:DocumentContextParameter"},"schema:domainIncludes":{"@id":"unece:ExchangedDocumentContext"},"rdfs:comment":"A scenario context parameter specified for this exchanged document context."},{"@id":"unece:specifiedTransactionId","@type":["rdf:Property","owl:DatatypeProperty"],"rdfs:label":"specifiedTransactionId","schema:rangeIncludes":{"@id":"schema:Text"},"schema:domainIncludes":{"@id":"unece:ExchangedDocumentContext"},"rdfs:comment":"The identifier of a specified transaction in this exchanged document context."},{"@id":"unece:subsetSpecifiedParameter","@type":["rdf:Property","owl:ObjectProperty"],"rdfs:label":"subsetSpecifiedParameter","schema:rangeIncludes":{"@id":"unece:DocumentContextParameter"},"schema:domainIncludes":{"@id":"unece:ExchangedDocumentContext"},"rdfs:comment":"A subset context parameter specified for this exchanged document context."},{"@id":"unece:testIndicator","@type":["rdf:Property","owl:DatatypeProperty"],"rdfs:label":"testIndicator","schema:rangeIncludes":{"@id":"schema:Boolean"},"schema:domainIncludes":{"@id":"unece:ExchangedDocumentContext"},"rdfs:comment":"The indication of whether or not this XHE document is a test ."},{"@id":"unece:userSpecifiedParameter","@type":["rdf:Property","owl:ObjectProperty"],"rdfs:label":"userSpecifiedParameter","schema:rangeIncludes":{"@id":"unece:DocumentContextParameter"},"schema:domainIncludes":{"@id":"unece:ExchangedDocumentContext"},"rdfs:comment":"A user specified document context parameter specified for this exchanged document context."},{"@id":"unece:associatedDirectPositionList","@type":["rdf:Property","owl:ObjectProperty"],"rdfs:label":"associatedDirectPositionList","schema:rangeIncludes":{"@id":"unece:DirectPositionList"},"schema:domainIncludes":[{"@id":"unece:GeographicalLine"},{"@id":"unece:GeographicalMultiCurve"},{"@id":"unece:GeographicalMultiPoint"},{"@id":"unece:GeographicalPoint"}],"rdfs:comment":"The direct position list associated with this geographical line."},{"@id":"unece:associatedGeographicalObjectCharacteristic","@type":["rdf:Property","owl:ObjectProperty"],"rdfs:label":"associatedGeographicalObjectCharacteristic","schema:rangeIncludes":{"@id":"unece:GeographicalObjectCharacteristic"},"schema:domainIncludes":[{"@id":"unece:GeographicalLine"},{"@id":"unece:GeographicalMultiCurve"},{"@id":"unece:GeographicalMultiPoint"},{"@id":"unece:GeographicalPoint"},{"@id":"unece:Circle"},{"@id":"unece:GeographicalGrid"},{"@id":"unece:GeographicalMultiSurface"},{"@id":"unece:GeographicalSurface"},{"@id":"unece:LinearRing"},{"@id":"unece:Polygon"}],"rdfs:comment":"The geographical object characteristic associated with this geographical grid."},{"@id":"unece:associatedLocation","@type":["rdf:Property","owl:ObjectProperty"],"rdfs:label":"associatedLocation","schema:rangeIncludes":{"@id":"unece:Location"},"schema:domainIncludes":[{"@id":"unece:GeographicalLine"},{"@id":"unece:GeographicalPoint"},{"@id":"unece:Circle"},{"@id":"unece:GeographicalGrid"},{"@id":"unece:Polygon"}],"rdfs:comment":"A logistics location associated with this specified circle."},{"@id":"unece:memberGeographicalLine","@type":["rdf:Property","owl:ObjectProperty"],"rdfs:label":"memberGeographicalLine","schema:rangeIncludes":{"@id":"unece:GeographicalLine"},"schema:domainIncludes":{"@id":"unece:GeographicalMultiCurve"},"rdfs:comment":"A geographical line member of this geographical multi-curve."},{"@id":"unece:memberGeographicalPoint","@type":["rdf:Property","owl:ObjectProperty"],"rdfs:label":"memberGeographicalPoint","schema:rangeIncludes":{"@id":"unece:GeographicalPoint"},"schema:domainIncludes":{"@id":"unece:GeographicalMultiPoint"},"rdfs:comment":"A geographical point member of this geographical multi-point feature."},{"@id":"unece:associatedEvent","@type":["rdf:Property","owl:ObjectProperty"],"rdfs:label":"associatedEvent","schema:rangeIncludes":{"@id":"unece:Event"},"schema:domainIncludes":{"@id":"unece:Error"},"rdfs:comment":"A corrective event associated with this declared error."},{"@id":"unece:occurrenceLogisticsLocation","@type":["rdf:Property","owl:ObjectProperty"],"rdfs:label":"occurrenceLogisticsLocation","schema:rangeIncludes":{"@id":"unece:Location"},"schema:domainIncludes":{"@id":"unece:CommunicationEvent"},"rdfs:comment":"A logistics location where this supply chain event occurs."},{"@id":"unece:operationalResponsibleParty","@type":["rdf:Property","owl:ObjectProperty"],"rdfs:label":"operationalResponsibleParty","schema:rangeIncludes":{"@id":"unece:Party"},"schema:domainIncludes":{"@id":"unece:CommunicationEvent"},"rdfs:comment":"The operational responsible party for this communication event."},{"@id":"unece:unitQuantity","@type":["rdf:Property","owl:ObjectProperty"],"rdfs:label":"unitQuantity","schema:rangeIncludes":{"@id":"unece:QuantityType"},"schema:domainIncludes":[{"@id":"unece:CommunicationEvent"},{"@id":"unece:EventElement"}],"rdfs:comment":"A number of units for this supply chain event."},{"@id":"unece:valueMeasure","@type":["rdf:Property","owl:ObjectProperty"],"rdfs:label":"valueMeasure","schema:rangeIncludes":{"@id":"unece:MeasureType"},"schema:domainIncludes":[{"@id":"unece:CommunicationEvent"},{"@id":"unece:WorkItemDimension"},{"@id":"unece:MetricCharacteristic"},{"@id":"unece:DocumentCharacteristic"},{"@id":"unece:SpatialDimension"},{"@id":"unece:SpecifiedParameter"}],"rdfs:comment":"A measure of a value for this document characteristic."},{"@id":"unece:centreGeographicalPoint","@type":["rdf:Property","owl:ObjectProperty"],"rdfs:label":"centreGeographicalPoint","schema:rangeIncludes":{"@id":"unece:GeographicalPoint"},"schema:domainIncludes":{"@id":"unece:Circle"},"rdfs:comment":"The geographical point which defines the centre of this specified circle."},{"@id":"unece:radiusMeasure","@type":["rdf:Property","owl:ObjectProperty"],"rdfs:label":"radiusMeasure","schema:rangeIncludes":{"@id":"unece:MeasureType"},"schema:domainIncludes":{"@id":"unece:Circle"},"rdfs:comment":"The measure of the radius for this specified circle."},{"@id":"unece:axisName","@type":["rdf:Property","owl:DatatypeProperty"],"rdfs:label":"axisName","schema:rangeIncludes":{"@id":"schema:Text"},"schema:domainIncludes":{"@id":"unece:GeographicalGrid"},"rdfs:comment":"An axis name, expressed as text, for this geographical grid."},{"@id":"unece:cell","@type":["rdf:Property","owl:DatatypeProperty"],"rdfs:label":"cell","schema:rangeIncludes":{"@id":"schema:Text"},"schema:domainIncludes":{"@id":"unece:GeographicalGrid"},"rdfs:comment":"The cell value, expressed as text, for this geographical grid."},{"@id":"unece:dimensionNumeric","@type":["rdf:Property","owl:DatatypeProperty"],"rdfs:label":"dimensionNumeric","schema:rangeIncludes":{"@id":"schema:Text"},"schema:domainIncludes":{"@id":"unece:GeographicalGrid"},"rdfs:comment":"The dimension, expressed as a number, of this geographical grid."},{"@id":"unece:highLimit","@type":["rdf:Property","owl:DatatypeProperty"],"rdfs:label":"highLimit","schema:rangeIncludes":{"@id":"schema:Text"},"schema:domainIncludes":{"@id":"unece:GeographicalGrid"},"rdfs:comment":"The tuple of elements, expressed as text, indicating the high limit of this geographical grid specifying the diagonally opposing corner of each axis."},{"@id":"unece:lowLimit","@type":["rdf:Property","owl:DatatypeProperty"],"rdfs:label":"lowLimit","schema:rangeIncludes":{"@id":"schema:Text"},"schema:domainIncludes":{"@id":"unece:GeographicalGrid"},"rdfs:comment":"The tuple of elements, expressed as text, indicating the low limit of this geographical grid specifying the offset of each axis."},{"@id":"unece:offsetVectorNumeric","@type":["rdf:Property","owl:DatatypeProperty"],"rdfs:label":"offsetVectorNumeric","schema:rangeIncludes":{"@id":"schema:Text"},"schema:domainIncludes":{"@id":"unece:GeographicalGrid"},"rdfs:comment":"The offset vector, expressed as a number, which indicates the offset of cells along each axis for this geographical grid."},{"@id":"unece:originAssociatedDirectPositionList","@type":["rdf:Property","owl:ObjectProperty"],"rdfs:label":"originAssociatedDirectPositionList","schema:rangeIncludes":{"@id":"unece:DirectPositionList"},"schema:domainIncludes":{"@id":"unece:GeographicalGrid"},"rdfs:comment":"The direct position list associated with the origin of this geographical grid."},{"@id":"unece:includedPolygon","@type":["rdf:Property","owl:ObjectProperty"],"rdfs:label":"includedPolygon","schema:rangeIncludes":{"@id":"unece:Polygon"},"schema:domainIncludes":[{"@id":"unece:GeographicalMultiSurface"},{"@id":"unece:GeographicalSurface"},{"@id":"unece:GeographicalFeature"}],"rdfs:comment":"A polygon included in this geographical multi-surface."},{"@id":"unece:coordinate","@type":["rdf:Property","owl:DatatypeProperty"],"rdfs:label":"coordinate","schema:rangeIncludes":{"@id":"schema:Text"},"schema:domainIncludes":[{"@id":"unece:LinearRing"},{"@id":"unece:DirectPositionList"}],"rdfs:comment":"A coordinate, expressed as text, for this specified linear ring."},{"@id":"unece:coordinateDirectPosition","@type":["rdf:Property","owl:ObjectProperty"],"rdfs:label":"coordinateDirectPosition","schema:rangeIncludes":{"@id":"unece:DirectPosition"},"schema:domainIncludes":{"@id":"unece:LinearRing"},"rdfs:comment":"The specified direct position of a coordinate for this linear ring."},{"@id":"unece:exteriorLinearRing","@type":["rdf:Property","owl:ObjectProperty"],"rdfs:label":"exteriorLinearRing","schema:rangeIncludes":{"@id":"unece:LinearRing"},"schema:domainIncludes":{"@id":"unece:Polygon"},"rdfs:comment":"The exterior linear specified ring for this polygon."},{"@id":"unece:interiorLinearRing","@type":["rdf:Property","owl:ObjectProperty"],"rdfs:label":"interiorLinearRing","schema:rangeIncludes":{"@id":"unece:LinearRing"},"schema:domainIncludes":{"@id":"unece:Polygon"},"rdfs:comment":"An interior linear ring specified for this polygon."},{"@id":"unece:authorizedRegistration","@type":["rdf:Property","owl:ObjectProperty"],"rdfs:label":"authorizedRegistration","schema:rangeIncludes":{"@id":"unece:LegalRegistration"},"schema:domainIncludes":{"@id":"unece:LegalOrganization"},"rdfs:comment":"A legal registration authorized for this legally set up organization."},{"@id":"unece:businessTypeCode","@type":["rdf:Property","owl:DatatypeProperty"],"rdfs:label":"businessTypeCode","schema:rangeIncludes":{"@id":"schema:Text"},"schema:domainIncludes":{"@id":"unece:LegalOrganization"},"rdfs:comment":"A code specifying the type of business of this legally set up organization."},{"@id":"unece:establishedDateTime","@type":["rdf:Property","owl:DatatypeProperty"],"rdfs:label":"establishedDateTime","schema:rangeIncludes":{"@id":"schema:Text"},"schema:domainIncludes":{"@id":"unece:LegalOrganization"},"rdfs:comment":"The date, time, date time, or other date time value when this legally set up organization was established."},{"@id":"unece:legalClassificationCode","@type":["rdf:Property","owl:DatatypeProperty"],"rdfs:label":"legalClassificationCode","schema:rangeIncludes":{"@id":"schema:Text"},"schema:domainIncludes":{"@id":"unece:LegalOrganization"},"rdfs:comment":"The code specifying the legal classification of this organization, such as Incorporated (Inc), Limited Liability Corporation (LLC) or non-profit."},{"@id":"unece:tradingBusinessName","@type":["rdf:Property","owl:DatatypeProperty"],"rdfs:label":"tradingBusinessName","schema:rangeIncludes":{"@id":"schema:Text"},"schema:domainIncludes":{"@id":"unece:LegalOrganization"},"rdfs:comment":"The trading business name, expressed as text, of this legally set up organization."},{"@id":"unece:axisLabelList","@type":["rdf:Property","owl:DatatypeProperty"],"rdfs:label":"axisLabelList","schema:rangeIncludes":{"@id":"schema:Text"},"schema:domainIncludes":[{"@id":"unece:DirectPosition"},{"@id":"unece:DirectPositionList"}],"rdfs:comment":"An ordered list of axis labels, expressed as text, for this specified direct position list."},{"@id":"unece:coordinateReferenceDimension","@type":["rdf:Property","owl:DatatypeProperty"],"rdfs:label":"coordinateReferenceDimension","schema:rangeIncludes":{"@id":"schema:Text"},"schema:domainIncludes":[{"@id":"unece:DirectPosition"},{"@id":"unece:DirectPositionList"}],"rdfs:comment":"A coordinate reference dimension, expressed as text, for this specified direct position list."},{"@id":"unece:countNumeric","@type":["rdf:Property","owl:DatatypeProperty"],"rdfs:label":"countNumeric","schema:rangeIncludes":{"@id":"schema:Text"},"schema:domainIncludes":[{"@id":"unece:DirectPosition"},{"@id":"unece:DirectPositionList"}],"rdfs:comment":"A count for this specified direct position list."},{"@id":"unece:uOMLabelList","@type":["rdf:Property","owl:DatatypeProperty"],"rdfs:label":"uOMLabelList","schema:rangeIncludes":{"@id":"schema:Text"},"schema:domainIncludes":[{"@id":"unece:DirectPosition"},{"@id":"unece:DirectPositionList"}],"rdfs:comment":"An ordered list of Unit Of Measure (UOM) labels, expressed as text, for this specified direct position list."},{"@id":"unece:birthAddressCountryId","@type":["rdf:Property","owl:DatatypeProperty"],"rdfs:label":"birthAddressCountryId","schema:rangeIncludes":{"@id":"unece:CountryId"},"schema:domainIncludes":{"@id":"unece:BirthAddress"},"rdfs:comment":"The identifier of a country for this birth address."},{"@id":"unece:cancellationDocumentStatusConditionCode","@type":["rdf:Property","owl:DatatypeProperty"],"rdfs:label":"cancellationDocumentStatusConditionCode","schema:rangeIncludes":{"@id":"schema:Text"},"schema:domainIncludes":{"@id":"unece:CancellationStatus"},"rdfs:comment":"The code specifying the condition of this cancellation status."},{"@id":"unece:category","@type":["rdf:Property","owl:DatatypeProperty"],"rdfs:label":"category","schema:rangeIncludes":{"@id":"schema:Text"},"schema:domainIncludes":{"@id":"unece:Object"},"rdfs:comment":"A category, expressed as text, for this specified object."},{"@id":"unece:objectType","@type":["rdf:Property","owl:DatatypeProperty"],"rdfs:label":"objectType","schema:rangeIncludes":{"@id":"schema:Text"},"schema:domainIncludes":{"@id":"unece:Object"},"rdfs:comment":"A type, expressed as text, for this specified object."},{"@id":"unece:remark","@type":["rdf:Property","owl:DatatypeProperty"],"rdfs:label":"remark","schema:rangeIncludes":{"@id":"schema:Text"},"schema:domainIncludes":{"@id":"unece:Object"},"rdfs:comment":"A remark, expressed as text, for this cross-border regulatory procedure."},{"@id":"unece:genderCode","@type":["rdf:Property","owl:DatatypeProperty"],"rdfs:label":"genderCode","schema:rangeIncludes":{"@id":"schema:Text"},"schema:domainIncludes":[{"@id":"unece:CustomerClass"},{"@id":"unece:Person"}],"rdfs:comment":"A code specifying the gender of this transport person."},{"@id":"unece:lowerAgeLimitNumeric","@type":["rdf:Property","owl:DatatypeProperty"],"rdfs:label":"lowerAgeLimitNumeric","schema:rangeIncludes":{"@id":"schema:Text"},"schema:domainIncludes":{"@id":"unece:CustomerClass"},"rdfs:comment":"The value, expressed as a number of years, for the lower age limit for the category of this specified customer class."},{"@id":"unece:mealServiceCategoryCode","@type":["rdf:Property","owl:DatatypeProperty"],"rdfs:label":"mealServiceCategoryCode","schema:rangeIncludes":{"@id":"schema:Text"},"schema:domainIncludes":{"@id":"unece:CustomerClass"},"rdfs:comment":"The code specifying the meal service category for this specified customer class."},{"@id":"unece:specialBeddingServiceOfferedIndicator","@type":["rdf:Property","owl:DatatypeProperty"],"rdfs:label":"specialBeddingServiceOfferedIndicator","schema:rangeIncludes":{"@id":"schema:Boolean"},"schema:domainIncludes":{"@id":"unece:CustomerClass"},"rdfs:comment":"The indication of whether or not special bedding service is offered for this specified customer class."},{"@id":"unece:upperAgeLimitNumeric","@type":["rdf:Property","owl:DatatypeProperty"],"rdfs:label":"upperAgeLimitNumeric","schema:rangeIncludes":{"@id":"schema:Text"},"schema:domainIncludes":{"@id":"unece:CustomerClass"},"rdfs:comment":"The value, expressed as a number of years, for the upper age limit for the category of this specified customer class."},{"@id":"unece:securityInformation","@type":["rdf:Property","owl:DatatypeProperty"],"rdfs:label":"securityInformation","schema:rangeIncludes":{"@id":"schema:Text"},"schema:domainIncludes":{"@id":"unece:InformationSource"},"rdfs:comment":"Security information, expressed as text, of this specified information source."},{"@id":"unece:websiteURIId","@type":["rdf:Property","owl:DatatypeProperty"],"rdfs:label":"websiteURIId","schema:rangeIncludes":{"@id":"schema:Text"},"schema:domainIncludes":[{"@id":"unece:InformationSource"},{"@id":"unece:Communication"}],"rdfs:comment":"A website Uniform Resource Identifier (URI) for this specified marketplace."},{"@id":"unece:changedDateTime","@type":["rdf:Property","owl:DatatypeProperty"],"rdfs:label":"changedDateTime","schema:rangeIncludes":{"@id":"schema:Text"},"schema:domainIncludes":{"@id":"unece:RecordedStatus"},"rdfs:comment":"The date, time, date time, or other date time value when this recorded status changed."},{"@id":"unece:changerName","@type":["rdf:Property","owl:DatatypeProperty"],"rdfs:label":"changerName","schema:rangeIncludes":{"@id":"schema:Text"},"schema:domainIncludes":{"@id":"unece:RecordedStatus"},"rdfs:comment":"The name of the person or system, expressed as text, that changed this recorded status."},{"@id":"unece:recordedStatusConditionCode","@type":["rdf:Property","owl:DatatypeProperty"],"rdfs:label":"recordedStatusConditionCode","schema:rangeIncludes":{"@id":"schema:Text"},"schema:domainIncludes":{"@id":"unece:RecordedStatus"},"rdfs:comment":"The code specifying the condition for this recorded status."},{"@id":"unece:collectionIndicator","@type":["rdf:Property","owl:DatatypeProperty"],"rdfs:label":"collectionIndicator","schema:rangeIncludes":{"@id":"schema:Boolean"},"schema:domainIncludes":{"@id":"unece:GeographicalFeature"},"rdfs:comment":"The indication of whether or not this specified geographical feature is a collection of features."},{"@id":"unece:coordinateReferenceSystemId","@type":["rdf:Property","owl:DatatypeProperty"],"rdfs:label":"coordinateReferenceSystemId","schema:rangeIncludes":{"@id":"schema:Text"},"schema:domainIncludes":{"@id":"unece:GeographicalFeature"},"rdfs:comment":"The identifier of the coordinate reference system for this geographical feature."},{"@id":"unece:includedCircle","@type":["rdf:Property","owl:ObjectProperty"],"rdfs:label":"includedCircle","schema:rangeIncludes":{"@id":"unece:Circle"},"schema:domainIncludes":{"@id":"unece:GeographicalFeature"},"rdfs:comment":"A circle included in this specified geographical feature."},{"@id":"unece:includedGeographicalGrid","@type":["rdf:Property","owl:ObjectProperty"],"rdfs:label":"includedGeographicalGrid","schema:rangeIncludes":{"@id":"unece:GeographicalGrid"},"schema:domainIncludes":{"@id":"unece:GeographicalFeature"},"rdfs:comment":"The geographical grid included in this geographical feature."},{"@id":"unece:includedGeographicalLine","@type":["rdf:Property","owl:ObjectProperty"],"rdfs:label":"includedGeographicalLine","schema:rangeIncludes":{"@id":"unece:GeographicalLine"},"schema:domainIncludes":{"@id":"unece:GeographicalFeature"},"rdfs:comment":"The geographical line included in this geographical feature."},{"@id":"unece:includedGeographicalMultiCurve","@type":["rdf:Property","owl:ObjectProperty"],"rdfs:label":"includedGeographicalMultiCurve","schema:rangeIncludes":{"@id":"unece:GeographicalMultiCurve"},"schema:domainIncludes":{"@id":"unece:GeographicalFeature"},"rdfs:comment":"The geographical multi-curve included in this geographical feature."},{"@id":"unece:includedGeographicalMultiPoint","@type":["rdf:Property","owl:ObjectProperty"],"rdfs:label":"includedGeographicalMultiPoint","schema:rangeIncludes":{"@id":"unece:GeographicalMultiPoint"},"schema:domainIncludes":{"@id":"unece:GeographicalFeature"},"rdfs:comment":"The geographical multi-point included in this geographical feature."},{"@id":"unece:includedGeographicalMultiSurface","@type":["rdf:Property","owl:ObjectProperty"],"rdfs:label":"includedGeographicalMultiSurface","schema:rangeIncludes":{"@id":"unece:GeographicalMultiSurface"},"schema:domainIncludes":{"@id":"unece:GeographicalFeature"},"rdfs:comment":"The geographical multi-surface included in this geographical feature."},{"@id":"unece:includedGeographicalPoint","@type":["rdf:Property","owl:ObjectProperty"],"rdfs:label":"includedGeographicalPoint","schema:rangeIncludes":{"@id":"unece:GeographicalPoint"},"schema:domainIncludes":{"@id":"unece:GeographicalFeature"},"rdfs:comment":"The geographical point included in this geographical feature."},{"@id":"unece:includedGeographicalSurface","@type":["rdf:Property","owl:ObjectProperty"],"rdfs:label":"includedGeographicalSurface","schema:rangeIncludes":{"@id":"unece:GeographicalSurface"},"schema:domainIncludes":{"@id":"unece:GeographicalFeature"},"rdfs:comment":"The geographical surface included in this geographical feature."},{"@id":"unece:communicationChannelCode","@type":["rdf:Property","owl:DatatypeProperty"],"rdfs:label":"communicationChannelCode","schema:rangeIncludes":{"@id":"unece:CommunicationChannelCodeList"},"schema:domainIncludes":{"@id":"unece:Communication"},"rdfs:comment":"The code specifying the channel or manner in which a universal communication can be made, such as telephone or email."},{"@id":"unece:completeNumber","@type":["rdf:Property","owl:DatatypeProperty"],"rdfs:label":"completeNumber","schema:rangeIncludes":{"@id":"schema:Text"},"schema:domainIncludes":{"@id":"unece:Communication"},"rdfs:comment":"The text string of characters that make up the complete number for this universal communication."},{"@id":"unece:emailURIId","@type":["rdf:Property","owl:DatatypeProperty"],"rdfs:label":"emailURIId","schema:rangeIncludes":{"@id":"schema:Text"},"schema:domainIncludes":{"@id":"unece:Communication"},"rdfs:comment":"The Uniform Resource Identifier (URI) of the email for this universal communication."},{"@id":"unece:invalidIndicator","@type":["rdf:Property","owl:DatatypeProperty"],"rdfs:label":"invalidIndicator","schema:rangeIncludes":{"@id":"schema:Boolean"},"schema:domainIncludes":[{"@id":"unece:Communication"},{"@id":"unece:Address"}],"rdfs:comment":"The indication of whether or not this trade address is invalid."},{"@id":"unece:completeDateTime","@type":["rdf:Property","owl:DatatypeProperty"],"rdfs:label":"completeDateTime","schema:rangeIncludes":{"@id":"schema:Text"},"schema:domainIncludes":{"@id":"unece:SpecifiedPeriod"},"rdfs:comment":"The date, time, date time or other date time value for a complete specified period of time expressed as a specific month, a specific week, etc."},{"@id":"unece:continuousIndicator","@type":["rdf:Property","owl:DatatypeProperty"],"rdfs:label":"continuousIndicator","schema:rangeIncludes":{"@id":"schema:Boolean"},"schema:domainIncludes":{"@id":"unece:SpecifiedPeriod"},"rdfs:comment":"The indication of whether or not this specified period is continuous."},{"@id":"unece:durationMeasure","@type":["rdf:Property","owl:ObjectProperty"],"rdfs:label":"durationMeasure","schema:rangeIncludes":{"@id":"unece:MeasureType"},"schema:domainIncludes":[{"@id":"unece:SpecifiedPeriod"},{"@id":"unece:DelimitedPeriod"}],"rdfs:comment":"A measure of the length of time for this specified time period such as hours, days, weeks, months, years."},{"@id":"unece:endDateTime","@type":["rdf:Property","owl:DatatypeProperty"],"rdfs:label":"endDateTime","schema:rangeIncludes":{"@id":"schema:Text"},"schema:domainIncludes":[{"@id":"unece:SpecifiedPeriod"},{"@id":"unece:AvailablePeriod"},{"@id":"unece:Membership"},{"@id":"unece:DelimitedPeriod"}],"rdfs:comment":"The date, time, date time or other date time value for the end of this available period of time."},{"@id":"unece:endDayOfWeekCode","@type":["rdf:Property","owl:DatatypeProperty"],"rdfs:label":"endDayOfWeekCode","schema:rangeIncludes":{"@id":"schema:Text"},"schema:domainIncludes":{"@id":"unece:SpecifiedPeriod"},"rdfs:comment":"The code specifying the end day of the week for this specified period."},{"@id":"unece:inclusiveIndicator","@type":["rdf:Property","owl:DatatypeProperty"],"rdfs:label":"inclusiveIndicator","schema:rangeIncludes":{"@id":"schema:Boolean"},"schema:domainIncludes":{"@id":"unece:SpecifiedPeriod"},"rdfs:comment":"The indication of whether or not the start and end dates are included in this specified period."},{"@id":"unece:maximumDurationMeasure","@type":["rdf:Property","owl:ObjectProperty"],"rdfs:label":"maximumDurationMeasure","schema:rangeIncludes":{"@id":"unece:DurationUnitMeasureType"},"schema:domainIncludes":{"@id":"unece:SpecifiedPeriod"},"rdfs:comment":"The measure of the maximum length of time for this specified period, such as hours, days, weeks, months, years."},{"@id":"unece:minimumDurationMeasure","@type":["rdf:Property","owl:ObjectProperty"],"rdfs:label":"minimumDurationMeasure","schema:rangeIncludes":{"@id":"unece:DurationUnitMeasureType"},"schema:domainIncludes":{"@id":"unece:SpecifiedPeriod"},"rdfs:comment":"The measure of the minimum length of time for this specified period, such as hours, days, weeks, months, years."},{"@id":"unece:nightQuantity","@type":["rdf:Property","owl:ObjectProperty"],"rdfs:label":"nightQuantity","schema:rangeIncludes":{"@id":"unece:QuantityType"},"schema:domainIncludes":{"@id":"unece:SpecifiedPeriod"},"rdfs:comment":"The number of nights in this specified period."},{"@id":"unece:openIndicator","@type":["rdf:Property","owl:DatatypeProperty"],"rdfs:label":"openIndicator","schema:rangeIncludes":{"@id":"schema:Boolean"},"schema:domainIncludes":{"@id":"unece:SpecifiedPeriod"},"rdfs:comment":"The indication of whether or not an entity is open during this specified period."},{"@id":"unece:purposeCode","@type":["rdf:Property","owl:DatatypeProperty"],"rdfs:label":"purposeCode","schema:rangeIncludes":{"@id":"schema:Text"},"schema:domainIncludes":{"@id":"unece:SpecifiedPeriod"},"rdfs:comment":"A code specifying a purpose for this field crop."},{"@id":"unece:seasonCode","@type":["rdf:Property","owl:DatatypeProperty"],"rdfs:label":"seasonCode","schema:rangeIncludes":{"@id":"schema:Text"},"schema:domainIncludes":{"@id":"unece:SpecifiedPeriod"},"rdfs:comment":"A code specifying a season for this trade product."},{"@id":"unece:startDateFlexibilityCode","@type":["rdf:Property","owl:DatatypeProperty"],"rdfs:label":"startDateFlexibilityCode","schema:rangeIncludes":{"@id":"schema:Text"},"schema:domainIncludes":{"@id":"unece:SpecifiedPeriod"},"rdfs:comment":"The code specifying the flexibility of the start date of this specified period."},{"@id":"unece:startDateTime","@type":["rdf:Property","owl:DatatypeProperty"],"rdfs:label":"startDateTime","schema:rangeIncludes":{"@id":"schema:Text"},"schema:domainIncludes":[{"@id":"unece:SpecifiedPeriod"},{"@id":"unece:AvailablePeriod"},{"@id":"unece:Membership"},{"@id":"unece:DelimitedPeriod"}],"rdfs:comment":"The date, time, date time or other date time value for the start of this available period of time."},{"@id":"unece:startDayOfWeekCode","@type":["rdf:Property","owl:DatatypeProperty"],"rdfs:label":"startDayOfWeekCode","schema:rangeIncludes":{"@id":"schema:Text"},"schema:domainIncludes":{"@id":"unece:SpecifiedPeriod"},"rdfs:comment":"The code specifying the start day of the week for this specified period."},{"@id":"unece:componentDimension","@type":["rdf:Property","owl:ObjectProperty"],"rdfs:label":"componentDimension","schema:rangeIncludes":{"@id":"unece:WorkItemDimension"},"schema:domainIncludes":{"@id":"unece:WorkItemDimension"},"rdfs:comment":"A work item component dimension for this work item dimension."},{"@id":"unece:workItemDimensionTypeCode","@type":["rdf:Property","owl:DatatypeProperty"],"rdfs:label":"workItemDimensionTypeCode","schema:rangeIncludes":{"@id":"schema:Text"},"schema:domainIncludes":{"@id":"unece:WorkItemDimension"},"rdfs:comment":"The code specifying the type of this work item dimension."},{"@id":"unece:documentStatusConditionCode","@type":["rdf:Property","owl:DatatypeProperty"],"rdfs:label":"documentStatusConditionCode","schema:rangeIncludes":{"@id":"unece:DocumentStatusCodeList"},"schema:domainIncludes":{"@id":"unece:DocumentStatus"},"rdfs:comment":"The code specifying the condition of this document status."},{"@id":"unece:documentStatusReasonCode","@type":["rdf:Property","owl:DatatypeProperty"],"rdfs:label":"documentStatusReasonCode","schema:rangeIncludes":{"@id":"schema:Text"},"schema:domainIncludes":{"@id":"unece:DocumentStatus"},"rdfs:comment":"A code specifying a reason for this document status."},{"@id":"unece:invalidInformation","@type":["rdf:Property","owl:DatatypeProperty"],"rdfs:label":"invalidInformation","schema:rangeIncludes":{"@id":"schema:Text"},"schema:domainIncludes":{"@id":"unece:DocumentStatus"},"rdfs:comment":"The invalid information, expressed as text, for this document status."},{"@id":"unece:reasonClassification","@type":["rdf:Property","owl:DatatypeProperty"],"rdfs:label":"reasonClassification","schema:rangeIncludes":{"@id":"schema:Text"},"schema:domainIncludes":{"@id":"unece:DocumentStatus"},"rdfs:comment":"A reason classification, expressed as text, for this document status."},{"@id":"unece:reasonClassificationCode","@type":["rdf:Property","owl:DatatypeProperty"],"rdfs:label":"reasonClassificationCode","schema:rangeIncludes":{"@id":"schema:Text"},"schema:domainIncludes":{"@id":"unece:DocumentStatus"},"rdfs:comment":"The code specifying the reason classification for this document status."},{"@id":"unece:reasonInformationCode","@type":["rdf:Property","owl:DatatypeProperty"],"rdfs:label":"reasonInformationCode","schema:rangeIncludes":{"@id":"schema:Text"},"schema:domainIncludes":{"@id":"unece:DocumentStatus"},"rdfs:comment":"The code specifying the reason for the information for this document status."},{"@id":"unece:requestedAction","@type":["rdf:Property","owl:DatatypeProperty"],"rdfs:label":"requestedAction","schema:rangeIncludes":{"@id":"schema:Text"},"schema:domainIncludes":{"@id":"unece:DocumentStatus"},"rdfs:comment":"A requested action, expressed as text, for this document status."},{"@id":"unece:specifiedDocumentCharacteristic","@type":["rdf:Property","owl:ObjectProperty"],"rdfs:label":"specifiedDocumentCharacteristic","schema:rangeIncludes":{"@id":"unece:DocumentCharacteristic"},"schema:domainIncludes":{"@id":"unece:DocumentStatus"},"rdfs:comment":"A document characteristic specified for this document status."},{"@id":"unece:validInformation","@type":["rdf:Property","owl:DatatypeProperty"],"rdfs:label":"validInformation","schema:rangeIncludes":{"@id":"schema:Text"},"schema:domainIncludes":{"@id":"unece:DocumentStatus"},"rdfs:comment":"The valid information, expressed as text, for this document status."},{"@id":"unece:constraintIndicator","@type":["rdf:Property","owl:DatatypeProperty"],"rdfs:label":"constraintIndicator","schema:rangeIncludes":{"@id":"schema:Boolean"},"schema:domainIncludes":{"@id":"unece:Project"},"rdfs:comment":"The indication of whether or not the project is constrained by an authority such as the World Trade Organization (WTO) for this procuring project."},{"@id":"unece:netBudgetAmount","@type":["rdf:Property","owl:ObjectProperty"],"rdfs:label":"netBudgetAmount","schema:rangeIncludes":{"@id":"unece:AmountType"},"schema:domainIncludes":{"@id":"unece:Project"},"rdfs:comment":"The monetary value of the net budget for this procuring project."},{"@id":"unece:subWorksTypeCode","@type":["rdf:Property","owl:DatatypeProperty"],"rdfs:label":"subWorksTypeCode","schema:rangeIncludes":{"@id":"schema:Text"},"schema:domainIncludes":{"@id":"unece:Project"},"rdfs:comment":"A code specifying the type of sub works, such as land surveying or information technology consulting, for this procuring project."},{"@id":"unece:totalBudgetAmount","@type":["rdf:Property","owl:ObjectProperty"],"rdfs:label":"totalBudgetAmount","schema:rangeIncludes":{"@id":"unece:AmountType"},"schema:domainIncludes":{"@id":"unece:Project"},"rdfs:comment":"The monetary value of the total budget which includes net amount, taxes, and material and instalment costs for this procuring project."},{"@id":"unece:worksTypeCode","@type":["rdf:Property","owl:DatatypeProperty"],"rdfs:label":"worksTypeCode","schema:rangeIncludes":{"@id":"schema:Text"},"schema:domainIncludes":{"@id":"unece:Project"},"rdfs:comment":"A code specifying the type of work, such as surveying or consulting, for this procuring project."},{"@id":"unece:contentCode","@type":["rdf:Property","owl:DatatypeProperty"],"rdfs:label":"contentCode","schema:rangeIncludes":{"@id":"schema:Text"},"schema:domainIncludes":{"@id":"unece:Note"},"rdfs:comment":"A code specifying the content of this note."},{"@id":"unece:noteSubjectCode","@type":["rdf:Property","owl:DatatypeProperty"],"rdfs:label":"noteSubjectCode","schema:rangeIncludes":{"@id":"schema:Text"},"schema:domainIncludes":{"@id":"unece:Note"},"rdfs:comment":"A code specifying the subject of this note."},{"@id":"unece:queryId","@type":["rdf:Property","owl:DatatypeProperty"],"rdfs:label":"queryId","schema:rangeIncludes":{"@id":"schema:Text"},"schema:domainIncludes":{"@id":"unece:Response"},"rdfs:comment":"The unique identifier for the query to which this response refers."},{"@id":"unece:responseTypeCode","@type":["rdf:Property","owl:DatatypeProperty"],"rdfs:label":"responseTypeCode","schema:rangeIncludes":{"@id":"unece:ResponseTypeCodeList"},"schema:domainIncludes":{"@id":"unece:Response"},"rdfs:comment":"The code specifying the type of this specification response."},{"@id":"unece:latestResponseDateTime","@type":["rdf:Property","owl:DatatypeProperty"],"rdfs:label":"latestResponseDateTime","schema:rangeIncludes":{"@id":"schema:DateTime"},"schema:domainIncludes":{"@id":"unece:SpecialQuery"},"rdfs:comment":"The date, time, date time, or other date time value for the latest response to this special query."},{"@id":"unece:responseStatusCode","@type":["rdf:Property","owl:DatatypeProperty"],"rdfs:label":"responseStatusCode","schema:rangeIncludes":{"@id":"schema:Text"},"schema:domainIncludes":{"@id":"unece:SpecialQuery"},"rdfs:comment":"The code specifying the response status for this special query."},{"@id":"unece:submittedDateTime","@type":["rdf:Property","owl:DatatypeProperty"],"rdfs:label":"submittedDateTime","schema:rangeIncludes":{"@id":"schema:DateTime"},"schema:domainIncludes":{"@id":"unece:SpecialQuery"},"rdfs:comment":"The date, time, date time, or other date time value when this special query was submitted."},{"@id":"unece:submittingPersonName","@type":["rdf:Property","owl:DatatypeProperty"],"rdfs:label":"submittingPersonName","schema:rangeIncludes":{"@id":"schema:Text"},"schema:domainIncludes":{"@id":"unece:SpecialQuery"},"rdfs:comment":"The name, expressed as text, of the person submitting this special query."},{"@id":"unece:subjectCode","@type":["rdf:Property","owl:DatatypeProperty"],"rdfs:label":"subjectCode","schema:rangeIncludes":{"@id":"schema:Text"},"schema:domainIncludes":{"@id":"unece:SpecifiedNote"},"rdfs:comment":"The code specifying the subject of this specified note."},{"@id":"unece:contentTypeCode","@type":["rdf:Property","owl:DatatypeProperty"],"rdfs:label":"contentTypeCode","schema:rangeIncludes":{"@id":"schema:Text"},"schema:domainIncludes":{"@id":"unece:MetricCharacteristic"},"rdfs:comment":"A code specifying the content type of this product characteristic."},{"@id":"unece:value","@type":["rdf:Property","owl:DatatypeProperty"],"rdfs:label":"value","schema:rangeIncludes":{"@id":"schema:Text"},"schema:domainIncludes":[{"@id":"unece:MetricCharacteristic"},{"@id":"unece:DocumentCharacteristic"},{"@id":"unece:SpecifiedParameter"},{"@id":"unece:Range"},{"@id":"unece:DocumentContextParameter"}],"rdfs:comment":"A value, expressed as text, for this document characteristic."},{"@id":"unece:valueAmount","@type":["rdf:Property","owl:ObjectProperty"],"rdfs:label":"valueAmount","schema:rangeIncludes":{"@id":"unece:AmountType"},"schema:domainIncludes":[{"@id":"unece:MetricCharacteristic"},{"@id":"unece:DocumentCharacteristic"}],"rdfs:comment":"A value, expressed as a monetary value, for this document characteristic."},{"@id":"unece:valueCode","@type":["rdf:Property","owl:DatatypeProperty"],"rdfs:label":"valueCode","schema:rangeIncludes":{"@id":"schema:Text"},"schema:domainIncludes":[{"@id":"unece:MetricCharacteristic"},{"@id":"unece:DocumentCharacteristic"},{"@id":"unece:Range"}],"rdfs:comment":"A code specifying a value for this specified range."},{"@id":"unece:valueDateTime","@type":["rdf:Property","owl:DatatypeProperty"],"rdfs:label":"valueDateTime","schema:rangeIncludes":{"@id":"schema:Text"},"schema:domainIncludes":[{"@id":"unece:MetricCharacteristic"},{"@id":"unece:DocumentCharacteristic"}],"rdfs:comment":"A date, time, date time or other date time value for this document characteristic."},{"@id":"unece:valueIndicator","@type":["rdf:Property","owl:DatatypeProperty"],"rdfs:label":"valueIndicator","schema:rangeIncludes":{"@id":"schema:Boolean"},"schema:domainIncludes":{"@id":"unece:MetricCharacteristic"},"rdfs:comment":"The value for this metric characteristic expressed as an indicator."},{"@id":"unece:valueMethod","@type":["rdf:Property","owl:ObjectProperty"],"rdfs:label":"valueMethod","schema:rangeIncludes":{"@id":"unece:SpecifiedMethod"},"schema:domainIncludes":{"@id":"unece:MetricCharacteristic"},"rdfs:comment":"A method specified for a value of this metric characteristic."},{"@id":"unece:valueNumeric","@type":["rdf:Property","owl:DatatypeProperty"],"rdfs:label":"valueNumeric","schema:rangeIncludes":{"@id":"schema:Text"},"schema:domainIncludes":[{"@id":"unece:MetricCharacteristic"},{"@id":"unece:DocumentCharacteristic"}],"rdfs:comment":"A value, expressed as a number, for this document characteristic."},{"@id":"unece:valueParameter","@type":["rdf:Property","owl:ObjectProperty"],"rdfs:label":"valueParameter","schema:rangeIncludes":{"@id":"unece:SpecifiedParameter"},"schema:domainIncludes":{"@id":"unece:MetricCharacteristic"},"rdfs:comment":"A parameter specified for a value for this metric characteristic."},{"@id":"unece:valueQuantity","@type":["rdf:Property","owl:ObjectProperty"],"rdfs:label":"valueQuantity","schema:rangeIncludes":{"@id":"unece:QuantityType"},"schema:domainIncludes":[{"@id":"unece:MetricCharacteristic"},{"@id":"unece:DocumentCharacteristic"}],"rdfs:comment":"A value, expressed as a quantity, for this document characteristic."},{"@id":"unece:valueRange","@type":["rdf:Property","owl:ObjectProperty"],"rdfs:label":"valueRange","schema:rangeIncludes":{"@id":"unece:Range"},"schema:domainIncludes":{"@id":"unece:MetricCharacteristic"},"rdfs:comment":"A range specified for a value of this metric characteristic."},{"@id":"unece:valueTolerance","@type":["rdf:Property","owl:ObjectProperty"],"rdfs:label":"valueTolerance","schema:rangeIncludes":{"@id":"unece:Tolerance"},"schema:domainIncludes":[{"@id":"unece:MetricCharacteristic"},{"@id":"unece:SpecifiedParameter"}],"rdfs:comment":"A tolerance specified for a value of this metric characteristic."},{"@id":"unece:lastRegisteredYearDateTime","@type":["rdf:Property","owl:DatatypeProperty"],"rdfs:label":"lastRegisteredYearDateTime","schema:rangeIncludes":{"@id":"schema:Text"},"schema:domainIncludes":{"@id":"unece:LegalRegistration"},"rdfs:comment":"The last registered year of this government registration."},{"@id":"unece:location","@type":["rdf:Property","owl:DatatypeProperty"],"rdfs:label":"location","schema:rangeIncludes":{"@id":"schema:Text"},"schema:domainIncludes":{"@id":"unece:DocumentCharacteristic"},"rdfs:comment":"A location, expressed as text, for this MDH sanitary measure."},{"@id":"unece:valueAdjustmentDirectionCode","@type":["rdf:Property","owl:DatatypeProperty"],"rdfs:label":"valueAdjustmentDirectionCode","schema:rangeIncludes":{"@id":"schema:Text"},"schema:domainIncludes":{"@id":"unece:DocumentCharacteristic"},"rdfs:comment":"The code specifying the adjustment direction for value of this document characteristic."},{"@id":"unece:valueChangedIndicator","@type":["rdf:Property","owl:DatatypeProperty"],"rdfs:label":"valueChangedIndicator","schema:rangeIncludes":{"@id":"schema:Boolean"},"schema:domainIncludes":{"@id":"unece:DocumentCharacteristic"},"rdfs:comment":"The indication of whether or not the value of this document characteristic is changed."},{"@id":"unece:valuePercent","@type":["rdf:Property","owl:DatatypeProperty"],"rdfs:label":"valuePercent","schema:rangeIncludes":{"@id":"schema:Text"},"schema:domainIncludes":{"@id":"unece:DocumentCharacteristic"},"rdfs:comment":"A value, expressed as a percentage, for this document characteristic."},{"@id":"unece:descriptionReference","@type":["rdf:Property","owl:DatatypeProperty"],"rdfs:label":"descriptionReference","schema:rangeIncludes":{"@id":"schema:Text"},"schema:domainIncludes":{"@id":"unece:GeographicalObjectCharacteristic"},"rdfs:comment":"The description reference, expressed as text, for this geographical object characteristic."},{"@id":"unece:geometryCollectionIndicator","@type":["rdf:Property","owl:DatatypeProperty"],"rdfs:label":"geometryCollectionIndicator","schema:rangeIncludes":{"@id":"schema:Boolean"},"schema:domainIncludes":{"@id":"unece:GeographicalObjectCharacteristic"},"rdfs:comment":"The indication of whether or not this geographical object can be characterized as a geometry collection."},{"@id":"unece:physicalIndicator","@type":["rdf:Property","owl:DatatypeProperty"],"rdfs:label":"physicalIndicator","schema:rangeIncludes":{"@id":"schema:Boolean"},"schema:domainIncludes":{"@id":"unece:GeographicalObjectCharacteristic"},"rdfs:comment":"The indication of whether or not this geographical object can be characterized as physical."},{"@id":"unece:relevantGeometryType","@type":["rdf:Property","owl:DatatypeProperty"],"rdfs:label":"relevantGeometryType","schema:rangeIncludes":{"@id":"schema:Text"},"schema:domainIncludes":{"@id":"unece:GeographicalObjectCharacteristic"},"rdfs:comment":"The type of geometry, expressed as text, relevant for this geographical object characteristic."},{"@id":"unece:shapeType","@type":["rdf:Property","owl:DatatypeProperty"],"rdfs:label":"shapeType","schema:rangeIncludes":{"@id":"schema:Text"},"schema:domainIncludes":{"@id":"unece:GeographicalObjectCharacteristic"},"rdfs:comment":"The type of shape, expressed as text, such as a semi-circle, for this geographical object characteristic."},{"@id":"unece:identificationCode","@type":["rdf:Property","owl:DatatypeProperty"],"rdfs:label":"identificationCode","schema:rangeIncludes":{"@id":"schema:Text"},"schema:domainIncludes":{"@id":"unece:IdentifiedFault"},"rdfs:comment":"A code specifying an identified fault."},{"@id":"unece:dimensionTypeCode","@type":["rdf:Property","owl:DatatypeProperty"],"rdfs:label":"dimensionTypeCode","schema:rangeIncludes":{"@id":"unece:DimensionTypeCodeList"},"schema:domainIncludes":{"@id":"unece:SpatialDimension"},"rdfs:comment":"The code specifying the type of spatial dimension, such as thickness, area, or volume."},{"@id":"unece:heightMeasure","@type":["rdf:Property","owl:ObjectProperty"],"rdfs:label":"heightMeasure","schema:rangeIncludes":{"@id":"unece:MeasureType"},"schema:domainIncludes":{"@id":"unece:SpatialDimension"},"rdfs:comment":"The measure of the height component of this spatial dimension."},{"@id":"unece:lengthMeasure","@type":["rdf:Property","owl:ObjectProperty"],"rdfs:label":"lengthMeasure","schema:rangeIncludes":{"@id":"unece:MeasureType"},"schema:domainIncludes":{"@id":"unece:SpatialDimension"},"rdfs:comment":"The measure of the length component of this spatial dimension."},{"@id":"unece:linearUnitDiameterMeasure","@type":["rdf:Property","owl:ObjectProperty"],"rdfs:label":"linearUnitDiameterMeasure","schema:rangeIncludes":{"@id":"unece:LinearUnitMeasureType"},"schema:domainIncludes":{"@id":"unece:SpatialDimension"},"rdfs:comment":"The measure of the diameter component for this spatial dimension."},{"@id":"unece:widthMeasure","@type":["rdf:Property","owl:ObjectProperty"],"rdfs:label":"widthMeasure","schema:rangeIncludes":{"@id":"unece:MeasureType"},"schema:domainIncludes":{"@id":"unece:SpatialDimension"},"rdfs:comment":"The measure of the width component of this spatial dimension."},{"@id":"unece:keywordMarketingPhrase","@type":["rdf:Property","owl:DatatypeProperty"],"rdfs:label":"keywordMarketingPhrase","schema:rangeIncludes":{"@id":"schema:Text"},"schema:domainIncludes":{"@id":"unece:SpecifiedFeature"},"rdfs:comment":"A keyword marketing phrase, expressed as text, for this feature."},{"@id":"unece:marketingPhrase","@type":["rdf:Property","owl:DatatypeProperty"],"rdfs:label":"marketingPhrase","schema:rangeIncludes":{"@id":"schema:Text"},"schema:domainIncludes":{"@id":"unece:SpecifiedFeature"},"rdfs:comment":"A catch phrase, expressed as text, for marketing of this trade product feature."},{"@id":"unece:objective","@type":["rdf:Property","owl:DatatypeProperty"],"rdfs:label":"objective","schema:rangeIncludes":{"@id":"schema:Text"},"schema:domainIncludes":{"@id":"unece:SpecifiedFeature"},"rdfs:comment":"An objective, expressed as text, for this experience product."},{"@id":"unece:usageCode","@type":["rdf:Property","owl:DatatypeProperty"],"rdfs:label":"usageCode","schema:rangeIncludes":{"@id":"schema:Text"},"schema:domainIncludes":{"@id":"unece:SpecifiedFeature"},"rdfs:comment":"The code specifying the usage for this specified feature."},{"@id":"unece:directions","@type":["rdf:Property","owl:DatatypeProperty"],"rdfs:label":"directions","schema:rangeIncludes":{"@id":"schema:Text"},"schema:domainIncludes":{"@id":"unece:SpecifiedLocation"},"rdfs:comment":"Directions, expressed as text, for this specified location."},{"@id":"unece:geopoliticalRegionCode","@type":["rdf:Property","owl:DatatypeProperty"],"rdfs:label":"geopoliticalRegionCode","schema:rangeIncludes":{"@id":"schema:Text"},"schema:domainIncludes":{"@id":"unece:SpecifiedLocation"},"rdfs:comment":"The code specifying the geopolitical region for this specified location."},{"@id":"unece:geopoliticalRegionName","@type":["rdf:Property","owl:DatatypeProperty"],"rdfs:label":"geopoliticalRegionName","schema:rangeIncludes":{"@id":"schema:Text"},"schema:domainIncludes":{"@id":"unece:SpecifiedLocation"},"rdfs:comment":"The name, expressed as text, of the geopolitical region for this specified location."},{"@id":"unece:mapURIId","@type":["rdf:Property","owl:DatatypeProperty"],"rdfs:label":"mapURIId","schema:rangeIncludes":{"@id":"schema:Text"},"schema:domainIncludes":{"@id":"unece:SpecifiedLocation"},"rdfs:comment":"The Uniform Resource Identifier (URI) of the map of this specified route."},{"@id":"unece:specifiedLocationTypeCode","@type":["rdf:Property","owl:DatatypeProperty"],"rdfs:label":"specifiedLocationTypeCode","schema:rangeIncludes":{"@id":"schema:Text"},"schema:domainIncludes":{"@id":"unece:SpecifiedLocation"},"rdfs:comment":"The code specifying the type of this specified location."},{"@id":"unece:specifiedTradeAddress","@type":["rdf:Property","owl:ObjectProperty"],"rdfs:label":"specifiedTradeAddress","schema:rangeIncludes":{"@id":"unece:Address"},"schema:domainIncludes":{"@id":"unece:SpecifiedLocation"},"rdfs:comment":"A address specified for this location."},{"@id":"unece:parameterType","@type":["rdf:Property","owl:DatatypeProperty"],"rdfs:label":"parameterType","schema:rangeIncludes":{"@id":"schema:Text"},"schema:domainIncludes":{"@id":"unece:SpecifiedParameter"},"rdfs:comment":"A type, expressed as text, for this observation objective parameter."},{"@id":"unece:statusValueMeasure","@type":["rdf:Property","owl:ObjectProperty"],"rdfs:label":"statusValueMeasure","schema:rangeIncludes":{"@id":"unece:MeasureType"},"schema:domainIncludes":{"@id":"unece:SpecifiedParameter"},"rdfs:comment":"A measure of a value of the status for this specified parameter."},{"@id":"unece:valueAllowedIndicator","@type":["rdf:Property","owl:DatatypeProperty"],"rdfs:label":"valueAllowedIndicator","schema:rangeIncludes":{"@id":"schema:Boolean"},"schema:domainIncludes":{"@id":"unece:SpecifiedParameter"},"rdfs:comment":"The indication of whether or not the value for this specified parameter is allowed."},{"@id":"unece:endId","@type":["rdf:Property","owl:DatatypeProperty"],"rdfs:label":"endId","schema:rangeIncludes":{"@id":"schema:Text"},"schema:domainIncludes":{"@id":"unece:Range"},"rdfs:comment":"The identifier of the end of this specified range."},{"@id":"unece:maximumValueMeasure","@type":["rdf:Property","owl:ObjectProperty"],"rdfs:label":"maximumValueMeasure","schema:rangeIncludes":{"@id":"unece:MeasureType"},"schema:domainIncludes":[{"@id":"unece:Range"},{"@id":"unece:SpecifiedTemperature"}],"rdfs:comment":"A measure of a maximum value for this sustainability characteristic."},{"@id":"unece:minimumValueMeasure","@type":["rdf:Property","owl:ObjectProperty"],"rdfs:label":"minimumValueMeasure","schema:rangeIncludes":{"@id":"unece:MeasureType"},"schema:domainIncludes":[{"@id":"unece:Range"},{"@id":"unece:SpecifiedTemperature"}],"rdfs:comment":"A measure of a minimum value for this sustainability characteristic."},{"@id":"unece:startId","@type":["rdf:Property","owl:DatatypeProperty"],"rdfs:label":"startId","schema:rangeIncludes":{"@id":"schema:Text"},"schema:domainIncludes":{"@id":"unece:Range"},"rdfs:comment":"The identifier of the start of this specified range."},{"@id":"unece:totalItemQuantity","@type":["rdf:Property","owl:ObjectProperty"],"rdfs:label":"totalItemQuantity","schema:rangeIncludes":{"@id":"unece:QuantityType"},"schema:domainIncludes":{"@id":"unece:Range"},"rdfs:comment":"The total number of items in this specified range."},{"@id":"unece:valueBaseSystemCode","@type":["rdf:Property","owl:DatatypeProperty"],"rdfs:label":"valueBaseSystemCode","schema:rangeIncludes":{"@id":"schema:Text"},"schema:domainIncludes":{"@id":"unece:Range"},"rdfs:comment":"The code specifying the value base system, such as Arabic numerals, for this specified range."},{"@id":"unece:identificationType","@type":["rdf:Property","owl:DatatypeProperty"],"rdfs:label":"identificationType","schema:rangeIncludes":{"@id":"schema:Text"},"schema:domainIncludes":{"@id":"unece:ProprietaryIdentity"},"rdfs:comment":"An identifier type, expressed as text, for this proprietary identity."},{"@id":"unece:level","@type":["rdf:Property","owl:DatatypeProperty"],"rdfs:label":"level","schema:rangeIncludes":{"@id":"schema:Text"},"schema:domainIncludes":{"@id":"unece:CoordinateReferenceSystem"},"rdfs:comment":"The level, expressed as text, of this CS engineering coordinate reference system."},{"@id":"unece:specifiedPeriod","@type":["rdf:Property","owl:ObjectProperty"],"rdfs:label":"specifiedPeriod","schema:rangeIncludes":{"@id":"unece:DelimitedPeriod"},"schema:domainIncludes":{"@id":"unece:CoordinateReferenceSystem"},"rdfs:comment":"A delimited period specified for this CS engineering coordinate reference system."},{"@id":"unece:subordinateCoordinateReferenceSystem","@type":["rdf:Property","owl:ObjectProperty"],"rdfs:label":"subordinateCoordinateReferenceSystem","schema:rangeIncludes":{"@id":"unece:CoordinateReferenceSystem"},"schema:domainIncludes":{"@id":"unece:CoordinateReferenceSystem"},"rdfs:comment":"A CS engineering coordinate reference system subordinate to this CS engineering coordinate reference system."},{"@id":"unece:signalSourceAvailableQuantity","@type":["rdf:Property","owl:ObjectProperty"],"rdfs:label":"signalSourceAvailableQuantity","schema:rangeIncludes":{"@id":"unece:QuantityType"},"schema:domainIncludes":{"@id":"unece:CoordinateSourceSystem"},"rdfs:comment":"The quantity of signal source available for this geographical coordinate source system."},{"@id":"unece:sourceTypeCode","@type":["rdf:Property","owl:DatatypeProperty"],"rdfs:label":"sourceTypeCode","schema:rangeIncludes":{"@id":"schema:Text"},"schema:domainIncludes":{"@id":"unece:CoordinateSourceSystem"},"rdfs:comment":"The code specifying a type of source for this geographical coordinate source system."},{"@id":"unece:toleranceMeasure","@type":["rdf:Property","owl:ObjectProperty"],"rdfs:label":"toleranceMeasure","schema:rangeIncludes":{"@id":"unece:MeasureType"},"schema:domainIncludes":{"@id":"unece:CoordinateSourceSystem"},"rdfs:comment":"The measure of the tolerance of this calibrated measurement."},{"@id":"unece:usedSignalSourceQuantity","@type":["rdf:Property","owl:ObjectProperty"],"rdfs:label":"usedSignalSourceQuantity","schema:rangeIncludes":{"@id":"unece:QuantityType"},"schema:domainIncludes":{"@id":"unece:CoordinateSourceSystem"},"rdfs:comment":"The quantity of the used signal source of this geographical coordinate source system."},{"@id":"unece:specifiedVersion","@type":["rdf:Property","owl:ObjectProperty"],"rdfs:label":"specifiedVersion","schema:rangeIncludes":{"@id":"unece:Version"},"schema:domainIncludes":{"@id":"unece:DocumentContextParameter"},"rdfs:comment":"The document version specified for this document context parameter."},{"@id":"unece:includedCountry","@type":["rdf:Property","owl:ObjectProperty"],"rdfs:label":"includedCountry","schema:rangeIncludes":{"@id":"unece:Country"},"schema:domainIncludes":{"@id":"unece:GeopoliticalRegion"},"rdfs:comment":"A country included in this trade geopolitical region."},{"@id":"unece:maximumSpecifiedCharacteristic","@type":["rdf:Property","owl:ObjectProperty"],"rdfs:label":"maximumSpecifiedCharacteristic","schema:rangeIncludes":{"@id":"unece:MetricCharacteristic"},"schema:domainIncludes":{"@id":"unece:Issue"},"rdfs:comment":"The maximum metric characteristic specified for this target issue."},{"@id":"unece:minimumSpecifiedCharacteristic","@type":["rdf:Property","owl:ObjectProperty"],"rdfs:label":"minimumSpecifiedCharacteristic","schema:rangeIncludes":{"@id":"unece:MetricCharacteristic"},"schema:domainIncludes":{"@id":"unece:Issue"},"rdfs:comment":"The minimum metric characteristic specified for this target issue."},{"@id":"unece:specifiedMetricCharacteristic","@type":["rdf:Property","owl:ObjectProperty"],"rdfs:label":"specifiedMetricCharacteristic","schema:rangeIncludes":{"@id":"unece:MetricCharacteristic"},"schema:domainIncludes":{"@id":"unece:Issue"},"rdfs:comment":"The metric characteristic specified for this target issue."},{"@id":"unece:lowDispersibleStatusIndicator","@type":["rdf:Property","owl:DatatypeProperty"],"rdfs:label":"lowDispersibleStatusIndicator","schema:rangeIncludes":{"@id":"schema:Boolean"},"schema:domainIncludes":{"@id":"unece:Radionuclide"},"rdfs:comment":"The indication of whether or not this radioactive radionuclide has a low dispersible status."},{"@id":"unece:specialFormIndicator","@type":["rdf:Property","owl:DatatypeProperty"],"rdfs:label":"specialFormIndicator","schema:rangeIncludes":{"@id":"schema:Boolean"},"schema:domainIncludes":{"@id":"unece:Radionuclide"},"rdfs:comment":"The indication of whether or not this radioactive radionuclide has a special form."},{"@id":"unece:includedSegment","@type":["rdf:Property","owl:ObjectProperty"],"rdfs:label":"includedSegment","schema:rangeIncludes":{"@id":"unece:Segment"},"schema:domainIncludes":{"@id":"unece:Section"},"rdfs:comment":"A segment included in this label section."},{"@id":"unece:patternCode","@type":["rdf:Property","owl:DatatypeProperty"],"rdfs:label":"patternCode","schema:rangeIncludes":{"@id":"schema:Text"},"schema:domainIncludes":{"@id":"unece:Section"},"rdfs:comment":"The code specifying the pattern of this label section."},{"@id":"unece:imageBinaryObject","@type":["rdf:Property","owl:DatatypeProperty"],"rdfs:label":"imageBinaryObject","schema:rangeIncludes":{"@id":"schema:Text"},"schema:domainIncludes":{"@id":"unece:Segment"},"rdfs:comment":"The image, expressed as a binary object, for this section segment."},{"@id":"unece:physicalGeographicalCoordinate","@type":["rdf:Property","owl:ObjectProperty"],"rdfs:label":"physicalGeographicalCoordinate","schema:rangeIncludes":{"@id":"unece:GeographicalCoordinate"},"schema:domainIncludes":[{"@id":"unece:SubordinateLocation"},{"@id":"unece:SubordinateSubordinateLocation"}],"rdfs:comment":"Geographical coordinate information for this logistics related location."},{"@id":"unece:subordinateSubordinateSubordinateLocation","@type":["rdf:Property","owl:ObjectProperty"],"rdfs:label":"subordinateSubordinateSubordinateLocation","schema:rangeIncludes":{"@id":"unece:SubordinateSubordinateLocation"},"schema:domainIncludes":{"@id":"unece:SubordinateLocation"},"rdfs:comment":"The location subordinate to this subordinate location."},{"@id":"unece:previousStatusCode","@type":["rdf:Property","owl:DatatypeProperty"],"rdfs:label":"previousStatusCode","schema:rangeIncludes":{"@id":"unece:WorkflowStatusCodeList"},"schema:domainIncludes":{"@id":"unece:WorkflowObject"},"rdfs:comment":"The code specifying the previous status of this trade workflow object."},{"@id":"unece:workflowStatusCode","@type":["rdf:Property","owl:DatatypeProperty"],"rdfs:label":"workflowStatusCode","schema:rangeIncludes":{"@id":"unece:WorkflowStatusCodeList"},"schema:domainIncludes":{"@id":"unece:WorkflowObject"},"rdfs:comment":"The code specifying the status of this trade workflow object."},{"@id":"unece:languageName","@type":["rdf:Property","owl:DatatypeProperty"],"rdfs:label":"languageName","schema:rangeIncludes":{"@id":"schema:Text"},"schema:domainIncludes":{"@id":"unece:LanguageProficiency"},"rdfs:comment":"A name, expressed as text, of the language for which this language proficiency is defined."},{"@id":"unece:personalLanguageProficiencyLanguageCode","@type":["rdf:Property","owl:DatatypeProperty"],"rdfs:label":"personalLanguageProficiencyLanguageCode","schema:rangeIncludes":{"@id":"unece:LanguageCodeList"},"schema:domainIncludes":{"@id":"unece:LanguageProficiency"},"rdfs:comment":"The code specifying the language for this personal language proficiency."},{"@id":"unece:personalLanguageProficiencyLanguageId","@type":["rdf:Property","owl:DatatypeProperty"],"rdfs:label":"personalLanguageProficiencyLanguageId","schema:rangeIncludes":{"@id":"unece:LanguageId"},"schema:domainIncludes":{"@id":"unece:LanguageProficiency"},"rdfs:comment":"The identifier of the language for which this personal language proficiency is defined."},{"@id":"unece:readingLevelCode","@type":["rdf:Property","owl:DatatypeProperty"],"rdfs:label":"readingLevelCode","schema:rangeIncludes":{"@id":"schema:Text"},"schema:domainIncludes":{"@id":"unece:LanguageProficiency"},"rdfs:comment":"The code specifying the personal reading proficiency level in this language."},{"@id":"unece:speakingLevelCode","@type":["rdf:Property","owl:DatatypeProperty"],"rdfs:label":"speakingLevelCode","schema:rangeIncludes":{"@id":"schema:Text"},"schema:domainIncludes":{"@id":"unece:LanguageProficiency"},"rdfs:comment":"The code specifying the personal speaking proficiency level in this language."},{"@id":"unece:writingLevelCode","@type":["rdf:Property","owl:DatatypeProperty"],"rdfs:label":"writingLevelCode","schema:rangeIncludes":{"@id":"schema:Text"},"schema:domainIncludes":{"@id":"unece:LanguageProficiency"},"rdfs:comment":"The code specifying the personal writing proficiency level in this language."},{"@id":"unece:locationCode","@type":["rdf:Property","owl:DatatypeProperty"],"rdfs:label":"locationCode","schema:rangeIncludes":{"@id":"schema:Text"},"schema:domainIncludes":{"@id":"unece:SecurityTag"},"rdfs:comment":"The code specifying the location of this product security tag."},{"@id":"unece:matchingEvent","@type":["rdf:Property","owl:ObjectProperty"],"rdfs:label":"matchingEvent","schema:rangeIncludes":{"@id":"unece:CommunicationEvent"},"schema:domainIncludes":{"@id":"unece:Pairing"},"rdfs:comment":"A matching event for this communication pairing."},{"@id":"unece:pairedIndicator","@type":["rdf:Property","owl:DatatypeProperty"],"rdfs:label":"pairedIndicator","schema:rangeIncludes":{"@id":"schema:Boolean"},"schema:domainIncludes":{"@id":"unece:Pairing"},"rdfs:comment":"The indication of whether or not the entity is paired in this communication pairing."},{"@id":"unece:targetEntityId","@type":["rdf:Property","owl:DatatypeProperty"],"rdfs:label":"targetEntityId","schema:rangeIncludes":{"@id":"schema:Text"},"schema:domainIncludes":{"@id":"unece:Pairing"},"rdfs:comment":"The identifier of the target entity for this communication pairing."},{"@id":"unece:temperatureUnitValueMeasure","@type":["rdf:Property","owl:ObjectProperty"],"rdfs:label":"temperatureUnitValueMeasure","schema:rangeIncludes":{"@id":"unece:TemperatureUnitMeasureType"},"schema:domainIncludes":{"@id":"unece:SpecifiedTemperature"},"rdfs:comment":"The measure of the value of this specified temperature, such as a temperature value of ten degrees Celsius."},{"@id":"unece:usedInformationSource","@type":["rdf:Property","owl:ObjectProperty"],"rdfs:label":"usedInformationSource","schema:rangeIncludes":{"@id":"unece:InformationSource"},"schema:domainIncludes":{"@id":"unece:CooperatingOrganization"},"rdfs:comment":"A specified cooperative information source used for or from this cooperating organization."},{"@id":"unece:objectClassId","@type":["rdf:Property","owl:DatatypeProperty"],"rdfs:label":"objectClassId","schema:rangeIncludes":{"@id":"schema:Text"},"schema:domainIncludes":{"@id":"unece:EventElement"},"rdfs:comment":"The identifier of the object class for this TT event element."},{"@id":"unece:procedure","@type":["rdf:Property","owl:DatatypeProperty"],"rdfs:label":"procedure","schema:rangeIncludes":{"@id":"schema:Text"},"schema:domainIncludes":{"@id":"unece:DocumentHandlingInstructions"},"rdfs:comment":"A procedure, expressed as text, for a set of inspection instructions."},{"@id":"unece:requirementIndicator","@type":["rdf:Property","owl:DatatypeProperty"],"rdfs:label":"requirementIndicator","schema:rangeIncludes":{"@id":"schema:Boolean"},"schema:domainIncludes":{"@id":"unece:DocumentHandlingInstructions"},"rdfs:comment":"The indication of whether or not a requirement exists for these document handling instructions."},{"@id":"unece:MeasureTypeValue","@type":["rdf:Property","owl:DatatypeProperty"],"rdfs:label":"MeasureTypeValue","schema:rangeIncludes":{"@id":"schema:Float"},"schema:domainIncludes":{"@id":"unece:MeasureType"},"rdfs:comment":"The numeric value."},{"@id":"unece:MeasureTypeCode","@type":["rdf:Property","owl:DatatypeProperty"],"rdfs:label":"MeasureTypeCode","schema:rangeIncludes":{"@id":"unece:MeasureCode"},"schema:domainIncludes":{"@id":"unece:MeasureType"},"rdfs:comment":"The unit code."},{"@id":"unece:TemperatureUnitMeasureTypeValue","@type":["rdf:Property","owl:DatatypeProperty"],"rdfs:label":"TemperatureUnitMeasureTypeValue","schema:rangeIncludes":{"@id":"schema:Float"},"schema:domainIncludes":{"@id":"unece:TemperatureUnitMeasureType"},"rdfs:comment":"The numeric value."},{"@id":"unece:TemperatureUnitMeasureTypeCode","@type":["rdf:Property","owl:DatatypeProperty"],"rdfs:label":"TemperatureUnitMeasureTypeCode","schema:rangeIncludes":{"@id":"unece:TemperatureUnitMeasureCode"},"schema:domainIncludes":{"@id":"unece:TemperatureUnitMeasureType"},"rdfs:comment":"The unit code."},{"@id":"unece:QuantityTypeValue","@type":["rdf:Property","owl:DatatypeProperty"],"rdfs:label":"QuantityTypeValue","schema:rangeIncludes":{"@id":"schema:Float"},"schema:domainIncludes":{"@id":"unece:QuantityType"},"rdfs:comment":"The numeric value."},{"@id":"unece:QuantityTypeCode","@type":["rdf:Property","owl:DatatypeProperty"],"rdfs:label":"QuantityTypeCode","schema:rangeIncludes":{"@id":"unece:QuantityCode"},"schema:domainIncludes":{"@id":"unece:QuantityType"},"rdfs:comment":"The unit code."},{"@id":"unece:AmountTypeValue","@type":["rdf:Property","owl:DatatypeProperty"],"rdfs:label":"AmountTypeValue","schema:rangeIncludes":{"@id":"schema:Float"},"schema:domainIncludes":{"@id":"unece:AmountType"},"rdfs:comment":"A number of monetary units."},{"@id":"unece:AmountTypeCurrency","@type":["rdf:Property","owl:DatatypeProperty"],"rdfs:label":"AmountTypeCurrency","schema:rangeIncludes":{"@id":"unece:AmountCurrency"},"schema:domainIncludes":{"@id":"unece:AmountType"},"rdfs:comment":"An amount currency code."},{"@id":"unece:DurationUnitMeasureTypeValue","@type":["rdf:Property","owl:DatatypeProperty"],"rdfs:label":"DurationUnitMeasureTypeValue","schema:rangeIncludes":{"@id":"schema:Float"},"schema:domainIncludes":{"@id":"unece:DurationUnitMeasureType"},"rdfs:comment":"The numeric value."},{"@id":"unece:DurationUnitMeasureTypeCode","@type":["rdf:Property","owl:DatatypeProperty"],"rdfs:label":"DurationUnitMeasureTypeCode","schema:rangeIncludes":{"@id":"unece:DurationUnitMeasureCode"},"schema:domainIncludes":{"@id":"unece:DurationUnitMeasureType"},"rdfs:comment":"The unit code."},{"@id":"unece:marginValueNumeric","@type":["rdf:Property","owl:DatatypeProperty"],"rdfs:label":"marginValueNumeric","schema:rangeIncludes":{"@id":"schema:Text"},"schema:domainIncludes":{"@id":"unece:Tolerance"},"rdfs:comment":"The margin numeric value of this specified tolerance."},{"@id":"unece:marginValuePercent","@type":["rdf:Property","owl:DatatypeProperty"],"rdfs:label":"marginValuePercent","schema:rangeIncludes":{"@id":"schema:Text"},"schema:domainIncludes":{"@id":"unece:Tolerance"},"rdfs:comment":"The margin percentage value of this specified tolerance."},{"@id":"unece:minusValuePercent","@type":["rdf:Property","owl:DatatypeProperty"],"rdfs:label":"minusValuePercent","schema:rangeIncludes":{"@id":"schema:Text"},"schema:domainIncludes":{"@id":"unece:Tolerance"},"rdfs:comment":"The minus percentage value of this specified tolerance."},{"@id":"unece:minusValueQuantity","@type":["rdf:Property","owl:ObjectProperty"],"rdfs:label":"minusValueQuantity","schema:rangeIncludes":{"@id":"unece:QuantityType"},"schema:domainIncludes":{"@id":"unece:Tolerance"},"rdfs:comment":"The minus quantity value of this specified tolerance."},{"@id":"unece:surplusValuePercent","@type":["rdf:Property","owl:DatatypeProperty"],"rdfs:label":"surplusValuePercent","schema:rangeIncludes":{"@id":"schema:Text"},"schema:domainIncludes":{"@id":"unece:Tolerance"},"rdfs:comment":"The surplus percentage value of this specified tolerance."},{"@id":"unece:surplusValueQuantity","@type":["rdf:Property","owl:ObjectProperty"],"rdfs:label":"surplusValueQuantity","schema:rangeIncludes":{"@id":"unece:QuantityType"},"schema:domainIncludes":{"@id":"unece:Tolerance"},"rdfs:comment":"The surplus quantity value of this specified tolerance."},{"@id":"unece:LinearUnitMeasureTypeValue","@type":["rdf:Property","owl:DatatypeProperty"],"rdfs:label":"LinearUnitMeasureTypeValue","schema:rangeIncludes":{"@id":"schema:Float"},"schema:domainIncludes":{"@id":"unece:LinearUnitMeasureType"},"rdfs:comment":"The numeric value."},{"@id":"unece:LinearUnitMeasureTypeCode","@type":["rdf:Property","owl:DatatypeProperty"],"rdfs:label":"LinearUnitMeasureTypeCode","schema:rangeIncludes":{"@id":"unece:LinearUnitMeasureCode"},"schema:domainIncludes":{"@id":"unece:LinearUnitMeasureType"},"rdfs:comment":"The unit code."},{"@id":"unece:governmentActionTypeCode","@type":["rdf:Property","owl:DatatypeProperty"],"rdfs:label":"governmentActionTypeCode","schema:rangeIncludes":{"@id":"unece:GovernmentActionCodeList"},"schema:domainIncludes":{"@id":"unece:Authentication"},"rdfs:comment":"The code specifying the type of document authentication."},{"@id":"unece:includedClause","@type":["rdf:Property","owl:ObjectProperty"],"rdfs:label":"includedClause","schema:rangeIncludes":{"@id":"unece:Clause"},"schema:domainIncludes":{"@id":"unece:Authentication"},"rdfs:comment":"A document clause included in this document authentication."},{"@id":"unece:locationProviderParty","@type":["rdf:Property","owl:ObjectProperty"],"rdfs:label":"locationProviderParty","schema:rangeIncludes":{"@id":"unece:Party"},"schema:domainIncludes":{"@id":"unece:Authentication"},"rdfs:comment":"The trade party providing the location for this document authentication."},{"@id":"unece:providerParty","@type":["rdf:Property","owl:ObjectProperty"],"rdfs:label":"providerParty","schema:rangeIncludes":{"@id":"unece:Party"},"schema:domainIncludes":{"@id":"unece:Authentication"},"rdfs:comment":"The provider party for this monitoring IOT device."},{"@id":"unece:representationTypeCode","@type":["rdf:Property","owl:DatatypeProperty"],"rdfs:label":"representationTypeCode","schema:rangeIncludes":{"@id":"schema:Text"},"schema:domainIncludes":{"@id":"unece:Authentication"},"rdfs:comment":"The code specifying the type of representation of this document authentication, such as direct or indirect."},{"@id":"unece:signatory","@type":["rdf:Property","owl:DatatypeProperty"],"rdfs:label":"signatory","schema:rangeIncludes":{"@id":"schema:Text"},"schema:domainIncludes":{"@id":"unece:Authentication"},"rdfs:comment":"The signatory, expressed as text, for this document authentication."},{"@id":"unece:signatoryImageBinaryObject","@type":["rdf:Property","owl:DatatypeProperty"],"rdfs:label":"signatoryImageBinaryObject","schema:rangeIncludes":{"@id":"schema:Text"},"schema:domainIncludes":{"@id":"unece:Authentication"},"rdfs:comment":"The signatory image, expressed as a binary object, for this document authentication."},{"@id":"unece:statement","@type":["rdf:Property","owl:DatatypeProperty"],"rdfs:label":"statement","schema:rangeIncludes":{"@id":"schema:Text"},"schema:domainIncludes":{"@id":"unece:Authentication"},"rdfs:comment":"A statement, expressed as text, for this specified inspection result."},{"@id":"unece:statementCode","@type":["rdf:Property","owl:DatatypeProperty"],"rdfs:label":"statementCode","schema:rangeIncludes":{"@id":"schema:Text"},"schema:domainIncludes":{"@id":"unece:Authentication"},"rdfs:comment":"The code specifying the statement for this document authentication."},{"@id":"unece:associatedMeasurement","@type":["rdf:Property","owl:ObjectProperty"],"rdfs:label":"associatedMeasurement","schema:rangeIncludes":{"@id":"unece:Measurement"},"schema:domainIncludes":{"@id":"unece:Clause"},"rdfs:comment":"A measurement associated with this document clause."},{"@id":"unece:associatedPeriod","@type":["rdf:Property","owl:ObjectProperty"],"rdfs:label":"associatedPeriod","schema:rangeIncludes":{"@id":"unece:SpecifiedPeriod"},"schema:domainIncludes":{"@id":"unece:Clause"},"rdfs:comment":"A period of time associated with this document clause."},{"@id":"unece:uRLId","@type":["rdf:Property","owl:DatatypeProperty"],"rdfs:label":"uRLId","schema:rangeIncludes":{"@id":"schema:Text"},"schema:domainIncludes":{"@id":"unece:Clause"},"rdfs:comment":"The Uniform Resource Locator (URL) for this document clause."},{"@id":"unece:additionalStreetName","@type":["rdf:Property","owl:DatatypeProperty"],"rdfs:label":"additionalStreetName","schema:rangeIncludes":{"@id":"schema:Text"},"schema:domainIncludes":{"@id":"unece:Address"},"rdfs:comment":"The additional name of a street, expressed as text, for this trade address."},{"@id":"unece:addressTypeCode","@type":["rdf:Property","owl:DatatypeProperty"],"rdfs:label":"addressTypeCode","schema:rangeIncludes":{"@id":"unece:AddressTypeCodeList"},"schema:domainIncludes":{"@id":"unece:Address"},"rdfs:comment":"A code specifying the type of this trade address, such as business address or home address."},{"@id":"unece:attentionOf","@type":["rdf:Property","owl:DatatypeProperty"],"rdfs:label":"attentionOf","schema:rangeIncludes":{"@id":"schema:Text"},"schema:domainIncludes":{"@id":"unece:Address"},"rdfs:comment":"The name, expressed as text, of a person or department in the organization to whom incoming mail is marked with words such as 'for the attention of' or 'FAO' or 'ATTN' for this trade address."},{"@id":"unece:buildingName","@type":["rdf:Property","owl:DatatypeProperty"],"rdfs:label":"buildingName","schema:rangeIncludes":{"@id":"schema:Text"},"schema:domainIncludes":{"@id":"unece:Address"},"rdfs:comment":"The name, expressed as text, of a building, a house or other structure on a street at this trade address."},{"@id":"unece:careOf","@type":["rdf:Property","owl:DatatypeProperty"],"rdfs:label":"careOf","schema:rangeIncludes":{"@id":"schema:Text"},"schema:domainIncludes":{"@id":"unece:Address"},"rdfs:comment":"The name, expressed as text, of a person or organization at this trade address to whom incoming mail is marked with words such as 'care of' or 'C/O'."},{"@id":"unece:citySubDivisionName","@type":["rdf:Property","owl:DatatypeProperty"],"rdfs:label":"citySubDivisionName","schema:rangeIncludes":{"@id":"schema:Text"},"schema:domainIncludes":{"@id":"unece:Address"},"rdfs:comment":"A name, expressed as text, of a sub-division of a city for this trade address, for example a district or borough."},{"@id":"unece:freeForm","@type":["rdf:Property","owl:DatatypeProperty"],"rdfs:label":"freeForm","schema:rangeIncludes":{"@id":"schema:Text"},"schema:domainIncludes":{"@id":"unece:Address"},"rdfs:comment":"A free form representation, expressed as text, of this trade address."},{"@id":"unece:geoCoordinateIdentificationGeographicalCoordinate","@type":["rdf:Property","owl:ObjectProperty"],"rdfs:label":"geoCoordinateIdentificationGeographicalCoordinate","schema:rangeIncludes":{"@id":"unece:GeographicalCoordinate"},"schema:domainIncludes":{"@id":"unece:Address"},"rdfs:comment":"An identification of a set of geographical coordinates for this trade address."},{"@id":"unece:actualOccurrenceDateTime","@type":["rdf:Property","owl:DatatypeProperty"],"rdfs:label":"actualOccurrenceDateTime","schema:rangeIncludes":{"@id":"schema:Text"},"schema:domainIncludes":{"@id":"unece:Event"},"rdfs:comment":"The date, time, date time or other date time value of the actual arrival related to this transport event."},{"@id":"unece:actualOccurrencePeriod","@type":["rdf:Property","owl:ObjectProperty"],"rdfs:label":"actualOccurrencePeriod","schema:rangeIncludes":{"@id":"unece:SpecifiedPeriod"},"schema:domainIncludes":{"@id":"unece:Event"},"rdfs:comment":"The actual period of time during which this transport event occurred."},{"@id":"unece:estimatedOccurrenceDateTime","@type":["rdf:Property","owl:DatatypeProperty"],"rdfs:label":"estimatedOccurrenceDateTime","schema:rangeIncludes":{"@id":"schema:Text"},"schema:domainIncludes":{"@id":"unece:Event"},"rdfs:comment":"The estimated date, time, date time, or other date time value of the occurrence of this transport event."},{"@id":"unece:occurrencePeriod","@type":["rdf:Property","owl:ObjectProperty"],"rdfs:label":"occurrencePeriod","schema:rangeIncludes":{"@id":"unece:SpecifiedPeriod"},"schema:domainIncludes":{"@id":"unece:Event"},"rdfs:comment":"The specified period of laycan time during which this transport event occurs."},{"@id":"unece:scheduledOccurrenceDateTime","@type":["rdf:Property","owl:DatatypeProperty"],"rdfs:label":"scheduledOccurrenceDateTime","schema:rangeIncludes":{"@id":"schema:Text"},"schema:domainIncludes":{"@id":"unece:Event"},"rdfs:comment":"A pilot boarding place, expressed as text, for this transport event."},{"@id":"unece:scheduledOccurrencePeriod","@type":["rdf:Property","owl:ObjectProperty"],"rdfs:label":"scheduledOccurrencePeriod","schema:rangeIncludes":{"@id":"unece:SpecifiedPeriod"},"schema:domainIncludes":{"@id":"unece:Event"},"rdfs:comment":"The scheduled period of time specified for the occurrence of this transport event."},{"@id":"unece:WeightUnitMeasureTypeValue","@type":["rdf:Property","owl:DatatypeProperty"],"rdfs:label":"WeightUnitMeasureTypeValue","schema:rangeIncludes":{"@id":"schema:Float"},"schema:domainIncludes":{"@id":"unece:WeightUnitMeasureType"},"rdfs:comment":"The numeric value."},{"@id":"unece:WeightUnitMeasureTypeCode","@type":["rdf:Property","owl:DatatypeProperty"],"rdfs:label":"WeightUnitMeasureTypeCode","schema:rangeIncludes":{"@id":"unece:WeightUnitMeasureCode"},"schema:domainIncludes":{"@id":"unece:WeightUnitMeasureType"},"rdfs:comment":"The unit code."},{"@id":"unece:UnitMeasureTypeValue","@type":["rdf:Property","owl:DatatypeProperty"],"rdfs:label":"UnitMeasureTypeValue","schema:rangeIncludes":{"@id":"schema:Float"},"schema:domainIncludes":{"@id":"unece:UnitMeasureType"},"rdfs:comment":"The numeric value."},{"@id":"unece:UnitMeasureTypeCode","@type":["rdf:Property","owl:DatatypeProperty"],"rdfs:label":"UnitMeasureTypeCode","schema:rangeIncludes":{"@id":"unece:UnitMeasureCode"},"schema:domainIncludes":{"@id":"unece:UnitMeasureType"},"rdfs:comment":"The unit code."},{"@id":"unece:VolumeUnitMeasureTypeValue","@type":["rdf:Property","owl:DatatypeProperty"],"rdfs:label":"VolumeUnitMeasureTypeValue","schema:rangeIncludes":{"@id":"schema:Float"},"schema:domainIncludes":{"@id":"unece:VolumeUnitMeasureType"},"rdfs:comment":"The numeric value."},{"@id":"unece:VolumeUnitMeasureTypeCode","@type":["rdf:Property","owl:DatatypeProperty"],"rdfs:label":"VolumeUnitMeasureTypeCode","schema:rangeIncludes":{"@id":"unece:VolumeUnitMeasureCode"},"schema:domainIncludes":{"@id":"unece:VolumeUnitMeasureType"},"rdfs:comment":"The unit code."},{"@id":"unece:AirFlowUnitMeasureTypeValue","@type":["rdf:Property","owl:DatatypeProperty"],"rdfs:label":"AirFlowUnitMeasureTypeValue","schema:rangeIncludes":{"@id":"schema:Float"},"schema:domainIncludes":{"@id":"unece:AirFlowUnitMeasureType"},"rdfs:comment":"The numeric value."},{"@id":"unece:AirFlowUnitMeasureTypeCode","@type":["rdf:Property","owl:DatatypeProperty"],"rdfs:label":"AirFlowUnitMeasureTypeCode","schema:rangeIncludes":{"@id":"unece:AirFlowUnitMeasureCode"},"schema:domainIncludes":{"@id":"unece:AirFlowUnitMeasureType"},"rdfs:comment":"The unit code."},{"@id":"unece:birthCountryId","@type":["rdf:Property","owl:DatatypeProperty"],"rdfs:label":"birthCountryId","schema:rangeIncludes":{"@id":"schema:Text"},"schema:domainIncludes":{"@id":"unece:Person"},"rdfs:comment":"The identifier of the birth country of this transport person."},{"@id":"unece:birthDateTime","@type":["rdf:Property","owl:DatatypeProperty"],"rdfs:label":"birthDateTime","schema:rangeIncludes":{"@id":"schema:Text"},"schema:domainIncludes":{"@id":"unece:Person"},"rdfs:comment":"The birth date for this individual TT animal."},{"@id":"unece:birthplaceName","@type":["rdf:Property","owl:DatatypeProperty"],"rdfs:label":"birthplaceName","schema:rangeIncludes":{"@id":"schema:Text"},"schema:domainIncludes":{"@id":"unece:Person"},"rdfs:comment":"The name, expressed as text, of the place where this transport person was born."},{"@id":"unece:emailURICommunication","@type":["rdf:Property","owl:ObjectProperty"],"rdfs:label":"emailURICommunication","schema:rangeIncludes":{"@id":"unece:Communication"},"schema:domainIncludes":[{"@id":"unece:Person"},{"@id":"unece:Contact"}],"rdfs:comment":"A code specifying a category for this cross-border regulatory procedure, such as the appendices of the CITES Convention."},{"@id":"unece:familyName","@type":["rdf:Property","owl:DatatypeProperty"],"rdfs:label":"familyName","schema:rangeIncludes":{"@id":"schema:Text"},"schema:domainIncludes":{"@id":"unece:Person"},"rdfs:comment":"A date, time, date time, or other date time value that this person embarked upon a means of transport."},{"@id":"unece:givenName","@type":["rdf:Property","owl:DatatypeProperty"],"rdfs:label":"givenName","schema:rangeIncludes":{"@id":"schema:Text"},"schema:domainIncludes":{"@id":"unece:Person"},"rdfs:comment":"A given name, expressed as text, for this transport person."},{"@id":"unece:landlineTelephoneCommunication","@type":["rdf:Property","owl:ObjectProperty"],"rdfs:label":"landlineTelephoneCommunication","schema:rangeIncludes":{"@id":"unece:Communication"},"schema:domainIncludes":{"@id":"unece:Person"},"rdfs:comment":"The indication of whether or not this transport person is in transit."},{"@id":"unece:mobileTelephoneCommunication","@type":["rdf:Property","owl:ObjectProperty"],"rdfs:label":"mobileTelephoneCommunication","schema:rangeIncludes":{"@id":"unece:Communication"},"schema:domainIncludes":{"@id":"unece:Person"},"rdfs:comment":"Mobile telephone communication information for this transport person."},{"@id":"unece:nationalityCountry","@type":["rdf:Property","owl:ObjectProperty"],"rdfs:label":"nationalityCountry","schema:rangeIncludes":{"@id":"unece:Country"},"schema:domainIncludes":{"@id":"unece:Person"},"rdfs:comment":"A country that constitutes a nationality by origin, birth, or naturalization for this transport person."},{"@id":"unece:contactPersonTitleCode","@type":["rdf:Property","owl:DatatypeProperty"],"rdfs:label":"contactPersonTitleCode","schema:rangeIncludes":{"@id":"unece:TitleCodeList"},"schema:domainIncludes":{"@id":"unece:Contact"},"rdfs:comment":"The code specifying the title of this contact person, such as Ms., Doctor, Mister."},{"@id":"unece:countryResidenceCountryId","@type":["rdf:Property","owl:DatatypeProperty"],"rdfs:label":"countryResidenceCountryId","schema:rangeIncludes":{"@id":"unece:CountryId"},"schema:domainIncludes":{"@id":"unece:Contact"},"rdfs:comment":"The identifier of the residence country of this contact person."},{"@id":"unece:faxCommunication","@type":["rdf:Property","owl:ObjectProperty"],"rdfs:label":"faxCommunication","schema:rangeIncludes":{"@id":"unece:Communication"},"schema:domainIncludes":{"@id":"unece:Contact"},"rdfs:comment":"Facsimile communication information for this contact person."},{"@id":"unece:instantMessagingCommunication","@type":["rdf:Property","owl:ObjectProperty"],"rdfs:label":"instantMessagingCommunication","schema:rangeIncludes":{"@id":"unece:Communication"},"schema:domainIncludes":{"@id":"unece:Contact"},"rdfs:comment":"An instant messaging communication for this contact person."},{"@id":"unece:role","@type":["rdf:Property","owl:DatatypeProperty"],"rdfs:label":"role","schema:rangeIncludes":{"@id":"schema:Text"},"schema:domainIncludes":{"@id":"unece:Contact"},"rdfs:comment":"A role, expressed as text, for this contact person."},{"@id":"unece:specifiedBirthAddress","@type":["rdf:Property","owl:ObjectProperty"],"rdfs:label":"specifiedBirthAddress","schema:rangeIncludes":{"@id":"unece:BirthAddress"},"schema:domainIncludes":{"@id":"unece:Contact"},"rdfs:comment":"The birth address specified for this contact person."},{"@id":"unece:specifiedEmployerIdentity","@type":["rdf:Property","owl:ObjectProperty"],"rdfs:label":"specifiedEmployerIdentity","schema:rangeIncludes":{"@id":"unece:EmployerIdentity"},"schema:domainIncludes":{"@id":"unece:Contact"},"rdfs:comment":"An employer identity specified for this contact person."},{"@id":"unece:specifiedPersonIdentity","@type":["rdf:Property","owl:ObjectProperty"],"rdfs:label":"specifiedPersonIdentity","schema:rangeIncludes":{"@id":"unece:PersonIdentity"},"schema:domainIncludes":{"@id":"unece:Contact"},"rdfs:comment":"The person identity specified for this contact person."},{"@id":"unece:telephoneCommunication","@type":["rdf:Property","owl:ObjectProperty"],"rdfs:label":"telephoneCommunication","schema:rangeIncludes":{"@id":"unece:Communication"},"schema:domainIncludes":{"@id":"unece:Contact"},"rdfs:comment":"A telephone communication for this trade party."},{"@id":"unece:websiteURICommunication","@type":["rdf:Property","owl:ObjectProperty"],"rdfs:label":"websiteURICommunication","schema:rangeIncludes":{"@id":"unece:Communication"},"schema:domainIncludes":{"@id":"unece:Contact"},"rdfs:comment":"A website Uniform Resource Identifier (URI) communication for this contact person."}]}